# baseURI: http://topbraid.org/teamworktests
# imports: http://datashapes.org/dash
# imports: http://topbraid.org/teamwork.spin
# prefix: teamworktests

@prefix owl: <http://www.w3.org/2002/07/owl#> .
@prefix rdf: <http://www.w3.org/1999/02/22-rdf-syntax-ns#> .
@prefix rdfs: <http://www.w3.org/2000/01/rdf-schema#> .
@prefix sh: <http://www.w3.org/ns/shacl#> .
@prefix teamworktests: <http://topbraid.org/teamworktests#> .
@prefix xsd: <http://www.w3.org/2001/XMLSchema#> .

<http://topbraid.org/teamwork#TestEnvironment>
  rdf:type rdfs:Class ;
  rdf:type sh:Shape ;
  rdfs:comment "The class of teamwork-related test environments. These are based on TriG files containing the master and TCH graphs as well as the users graph." ;
  rdfs:label "Teamwork test environment" ;
  rdfs:subClassOf <http://datashapes.org/dash#TestEnvironment> ;
.
<http://topbraid.org/teamwork#declarePrefix>
  rdf:type rdf:Property ;
  rdfs:comment "Used to remember prefix declarations local to a graph within that graph." ;
  rdfs:domain owl:Ontology ;
  rdfs:label "declare prefix" ;
  rdfs:range sh:PrefixDeclaration ;
.
<http://topbraid.org/teamwork#testEnvironmentPath>
  rdf:type rdf:Property ;
  rdfs:comment "The path of an environment's TriG file, relative to the workspace root." ;
  rdfs:domain <http://topbraid.org/teamwork#TestEnvironment> ;
  rdfs:label "test environment path" ;
  rdfs:range xsd:string ;
.
<http://topbraid.org/teamworktests>
  rdf:type owl:Ontology ;
  owl:imports <http://datashapes.org/dash> ;
  owl:imports <http://topbraid.org/teamwork.spin> ;
  owl:versionInfo "Created with TopBraid Composer" ;
.
