# baseURI: http://uispin.org/svg
# imports: http://uispin.org/css
# imports: http://uispin.org/ui
# prefix: svg

@prefix owl: <http://www.w3.org/2002/07/owl#> .
@prefix rdf: <http://www.w3.org/1999/02/22-rdf-syntax-ns#> .
@prefix rdfs: <http://www.w3.org/2000/01/rdf-schema#> .
@prefix spin: <http://spinrdf.org/spin#> .
@prefix spl: <http://spinrdf.org/spl#> .
@prefix svg: <http://uispin.org/svg#> .
@prefix ui: <http://uispin.org/ui#> .
@prefix xlink: <http://www.w3.org/1999/xlink#> .
@prefix xsd: <http://www.w3.org/2001/XMLSchema#> .

<http://uispin.org/css#audio-level>
  a ui:StyleProperty ;
  rdfs:label "audio-level" ;
  rdfs:subPropertyOf <http://uispin.org/css#properties> ;
.
<http://uispin.org/css#buffered-rendering>
  a ui:StyleProperty ;
  rdfs:label "buffered-rendering" ;
  rdfs:subPropertyOf <http://uispin.org/css#properties> ;
.
<http://uispin.org/css#color>
  rdfs:label "color" ;
.
<http://uispin.org/css#color-rendering>
  a ui:StyleProperty ;
  rdfs:label "color-rendering" ;
  rdfs:subPropertyOf <http://uispin.org/css#properties> ;
.
<http://uispin.org/css#display-align>
  a ui:StyleProperty ;
  rdfs:label "display-align" ;
  rdfs:subPropertyOf <http://uispin.org/css#properties> ;
.
<http://uispin.org/css#fill>
  a ui:StyleProperty ;
  rdfs:label "fill" ;
  rdfs:subPropertyOf <http://uispin.org/css#properties> ;
.
<http://uispin.org/css#fill-opacity>
  a ui:StyleProperty ;
  rdfs:label "fill-opacity" ;
  rdfs:subPropertyOf <http://uispin.org/css#properties> ;
.
<http://uispin.org/css#fill-rule>
  a ui:StyleProperty ;
  rdfs:label "fill-rule" ;
  rdfs:subPropertyOf <http://uispin.org/css#properties> ;
.
<http://uispin.org/css#image-rendering>
  a ui:StyleProperty ;
  rdfs:label "image-rendering" ;
  rdfs:subPropertyOf <http://uispin.org/css#properties> ;
.
<http://uispin.org/css#line-increment>
  a ui:StyleProperty ;
  rdfs:label "line-increment" ;
  rdfs:subPropertyOf <http://uispin.org/css#properties> ;
.
<http://uispin.org/css#opacity>
  a ui:StyleProperty ;
  rdfs:label "opacity" ;
  rdfs:subPropertyOf <http://uispin.org/css#properties> ;
.
<http://uispin.org/css#pointer-events>
  a ui:StyleProperty ;
  rdfs:label "pointer-events" ;
  rdfs:subPropertyOf <http://uispin.org/css#properties> ;
.
<http://uispin.org/css#shape-rendering>
  a ui:StyleProperty ;
  rdfs:label "shape-rendering" ;
  rdfs:subPropertyOf <http://uispin.org/css#properties> ;
.
<http://uispin.org/css#solid-color>
  a ui:StyleProperty ;
  rdfs:label "solid-color" ;
  rdfs:subPropertyOf <http://uispin.org/css#properties> ;
.
<http://uispin.org/css#solid-opacity>
  a ui:StyleProperty ;
  rdfs:label "solid-opacity" ;
  rdfs:subPropertyOf <http://uispin.org/css#properties> ;
.
<http://uispin.org/css#stop-color>
  a ui:StyleProperty ;
  rdfs:label "stop-color" ;
  rdfs:subPropertyOf <http://uispin.org/css#properties> ;
.
<http://uispin.org/css#stop-opacity>
  a ui:StyleProperty ;
  rdfs:label "stop-opacity" ;
  rdfs:subPropertyOf <http://uispin.org/css#properties> ;
.
<http://uispin.org/css#stroke>
  a ui:StyleProperty ;
  rdfs:label "stroke" ;
  rdfs:subPropertyOf <http://uispin.org/css#properties> ;
.
<http://uispin.org/css#stroke-dasharray>
  a ui:StyleProperty ;
  rdfs:label "stroke-dasharray" ;
  rdfs:subPropertyOf <http://uispin.org/css#properties> ;
.
<http://uispin.org/css#stroke-dashoffset>
  a ui:StyleProperty ;
  rdfs:label "stroke-dashoffset" ;
  rdfs:subPropertyOf <http://uispin.org/css#properties> ;
.
<http://uispin.org/css#stroke-linecap>
  a ui:StyleProperty ;
  rdfs:label "stroke-linecap" ;
  rdfs:subPropertyOf <http://uispin.org/css#properties> ;
.
<http://uispin.org/css#stroke-linejoin>
  a ui:StyleProperty ;
  rdfs:label "stroke-linejoin" ;
  rdfs:subPropertyOf <http://uispin.org/css#properties> ;
.
<http://uispin.org/css#stroke-miterlimit>
  a ui:StyleProperty ;
  rdfs:label "stroke-miterlimit" ;
  rdfs:subPropertyOf <http://uispin.org/css#properties> ;
.
<http://uispin.org/css#stroke-opacity>
  a ui:StyleProperty ;
  rdfs:label "stroke-opacity" ;
  rdfs:subPropertyOf <http://uispin.org/css#properties> ;
.
<http://uispin.org/css#stroke-width>
  a ui:StyleProperty ;
  rdfs:label "stroke-width" ;
  rdfs:subPropertyOf <http://uispin.org/css#properties> ;
.
<http://uispin.org/css#text-anchor>
  a ui:StyleProperty ;
  rdfs:label "text-anchor" ;
  rdfs:subPropertyOf <http://uispin.org/css#properties> ;
.
<http://uispin.org/css#text-rendering>
  a ui:StyleProperty ;
  rdfs:label "text-rendering" ;
  rdfs:subPropertyOf <http://uispin.org/css#properties> ;
.
<http://uispin.org/css#vector-effect>
  a ui:StyleProperty ;
  rdfs:label "vector-effect" ;
  rdfs:subPropertyOf <http://uispin.org/css#properties> ;
.
<http://uispin.org/css#viewport-fill>
  a ui:StyleProperty ;
  rdfs:label "viewport-fill" ;
  rdfs:subPropertyOf <http://uispin.org/css#properties> ;
.
<http://uispin.org/css#viewport-fill-opacity>
  a ui:StyleProperty ;
  rdfs:label "viewport-fill-opacity" ;
  rdfs:subPropertyOf <http://uispin.org/css#properties> ;
.
<http://uispin.org/svg>
  a owl:Ontology ;
  rdfs:comment "A vocabulary to represent Scalable Vector Graphics (SVG) in UISPIN RDF documents. This version supports SVG Tiny 1.2." ;
  owl:imports <http://uispin.org/css> ;
  owl:imports <http://uispin.org/ui> ;
.
svg:A
  a ui:NodeClass ;
  rdfs:comment "SVG provides an 'a' element, analogous to HTML's 'a' element, to indicate links (also known as hyperlinks or Web links)" ;
  rdfs:label "A" ;
  rdfs:seeAlso <http://www.w3.org/TR/SVGTiny12/linking.html#AElement> ;
  rdfs:subClassOf svg:ContainerElements ;
.
svg:Animate
  a ui:NodeClass ;
  rdfs:comment "The 'animate' element is used to animate a single attribute or property over time." ;
  rdfs:label "Animate" ;
  rdfs:seeAlso <http://www.w3.org/TR/SVGTiny12/animate.html#AnimateElement> ;
  rdfs:subClassOf svg:AnimationElements ;
.
svg:AnimateColor
  a ui:NodeClass ;
  rdfs:comment "The 'animateColor' element specifies a color transition over time." ;
  rdfs:label "Animate color" ;
  rdfs:seeAlso <http://www.w3.org/TR/SVGTiny12/animate.html#AnimateColorElement> ;
  rdfs:subClassOf svg:AnimationElements ;
.
svg:AnimateMotion
  a ui:NodeClass ;
  rdfs:comment "The 'animateMotion' element causes its target element to move along a motion path." ;
  rdfs:label "Animate motion" ;
  rdfs:seeAlso <http://www.w3.org/TR/SVGTiny12/animate.html#AnimateMotionElement> ;
  rdfs:subClassOf svg:AnimationElements ;
.
svg:AnimateTransform
  a ui:NodeClass ;
  rdfs:comment "The 'animateTransform' element animates a transformation attribute on a target element, thereby allowing animations to control translation, scaling, rotation and/or skewing." ;
  rdfs:label "Animate transform" ;
  rdfs:seeAlso <http://www.w3.org/TR/SVGTiny12/animate.html#AnimateTransformElement> ;
  rdfs:subClassOf svg:AnimationElements ;
.
svg:Animation
  a ui:NodeClass ;
  rdfs:comment "The 'animation' elements specifies an SVG document providing synchronized animated vector graphics." ;
  rdfs:label "Animation" ;
  rdfs:seeAlso <http://www.w3.org/TR/SVGTiny12/multimedia.html#AnimationElement> ;
  rdfs:subClassOf svg:GraphicsElements ;
.
svg:AnimationElements
  a ui:NodeClass ;
  ui:abstract true ;
  rdfs:comment "Abstract superclass of the various SVG animation elements." ;
  rdfs:label "Animation element" ;
  rdfs:subClassOf svg:Elements ;
.
svg:Attribute
  a rdfs:Class ;
  rdfs:label "Attribute" ;
  rdfs:subClassOf rdf:Property ;
.
svg:Audio
  a ui:NodeClass ;
  rdfs:comment "The 'audio' element specifies an audio file which is to be rendered to provide synchronized audio." ;
  rdfs:label "Audio" ;
  rdfs:seeAlso <http://www.w3.org/TR/SVGTiny12/multimedia.html#AudioElement> ;
  rdfs:subClassOf svg:MultimediaElements ;
.
svg:Circle
  a ui:NodeClass ;
  spin:constraint [
      a spl:Argument ;
      spl:predicate svg:cx ;
      rdfs:comment "The x-axis coordinate of the center of the circle. The lacuna value is '0'." ;
    ] ;
  spin:constraint [
      a spl:Argument ;
      spl:predicate svg:cy ;
      rdfs:comment "The y-axis coordinate of the center of the circle. The lacuna value is '0'." ;
    ] ;
  spin:constraint [
      a spl:Argument ;
      spl:predicate svg:r ;
      rdfs:comment "The radius of the circle. A negative value is unsupported. A value of zero disables rendering of the element. The lacuna value is '0'." ;
    ] ;
  rdfs:comment "The 'circle' element defines a circle based on a center point and a radius." ;
  rdfs:label "Circle" ;
  rdfs:seeAlso <http://www.w3.org/TR/SVGTiny12/shapes.html#CircleElement> ;
  rdfs:subClassOf svg:GraphicsElements ;
.
svg:ContainerElements
  a ui:NodeClass ;
  ui:abstract true ;
  rdfs:comment "Abstract base class of the various SVG container elements." ;
  rdfs:label "Container elements" ;
  rdfs:subClassOf svg:Elements ;
.
svg:Defs
  a ui:NodeClass ;
  rdfs:comment "The 'defs' element is a container element for referenced elements." ;
  rdfs:label "Defs" ;
  rdfs:seeAlso <http://www.w3.org/TR/SVGTiny12/struct.html#DefsElement> ;
  rdfs:subClassOf svg:StructuralElements ;
.
svg:Desc
  a ui:NodeClass ;
  rdfs:label "Desc" ;
  rdfs:seeAlso <http://www.w3.org/TR/SVGTiny12/struct.html#TitleAndDescriptionElements> ;
  rdfs:subClassOf svg:DescriptiveElements ;
.
svg:DescriptiveElements
  a ui:NodeClass ;
  ui:abstract true ;
  rdfs:comment "Abstract base class of descriptive SVG elements." ;
  rdfs:label "Descriptive elements" ;
  rdfs:subClassOf svg:Elements ;
.
svg:Discard
  a ui:NodeClass ;
  rdfs:comment "The 'discard' element allows authors to specify the time at which particular elements are to be discarded, thereby reducing the resources required by an SVG user agent." ;
  rdfs:label "Discard" ;
  rdfs:seeAlso <http://www.w3.org/TR/SVGTiny12/struct.html#DiscardElement> ;
  rdfs:subClassOf svg:AnimationElements ;
.
svg:Elements
  a ui:NodeClass ;
  spin:constraint [
      a spl:Argument ;
      spl:predicate svg:class ;
      rdfs:comment "Assigns one or more class names to an element." ;
    ] ;
  spin:constraint [
      a spl:Argument ;
      spl:predicate svg:content ;
      rdfs:comment "The 'content' attribute provides a plain text value that may be suitable for humans, or may be machine-readable, or both, depending on the context." ;
    ] ;
  spin:constraint [
      a spl:Argument ;
      spl:predicate svg:id ;
      rdfs:comment "This attribute specifies a unique identifier for the element. Because of wider use and compatibility with legacy content and existing user agents (including authoring tools), it is recommended that content intended for use in a Web browser environment use 'id' instead of 'xml:id'." ;
    ] ;
  ui:abstract true ;
  rdfs:comment "Abstract base class of all SVG elements. Defines common attributes such as id and class." ;
  rdfs:label "SVG Elements" ;
  rdfs:subClassOf ui:Element ;
.
svg:Ellipse
  a ui:NodeClass ;
  spin:constraint [
      a spl:Argument ;
      spl:predicate svg:cx ;
      rdfs:comment "The x-axis coordinate of the center of the ellipse. The lacuna value is '0'." ;
    ] ;
  spin:constraint [
      a spl:Argument ;
      spl:predicate svg:cy ;
      rdfs:comment "The y-axis coordinate of the center of the ellipse. The lacuna value is '0'." ;
    ] ;
  spin:constraint [
      a spl:Argument ;
      spl:predicate svg:rx ;
      rdfs:comment "The x-axis radius of the ellipse. A negative value is unsupported. A value of zero disables rendering of the element. The lacuna value is '0'." ;
    ] ;
  spin:constraint [
      a spl:Argument ;
      spl:predicate svg:ry ;
      rdfs:comment "The y-axis radius of the ellipse. A negative value is unsupported. A value of zero disables rendering of the element. The lacuna value is '0'." ;
    ] ;
  rdfs:comment "The 'ellipse' element defines an ellipse which is axis-aligned with the current user coordinate system based on a center point and two radii." ;
  rdfs:label "Ellipse" ;
  rdfs:seeAlso <http://www.w3.org/TR/SVGTiny12/shapes.html#EllipseElement> ;
  rdfs:subClassOf svg:GraphicsElements ;
.
svg:Font
  a ui:NodeClass ;
  rdfs:comment "The 'font' element defines an SVG font." ;
  rdfs:label "Font" ;
  rdfs:seeAlso <http://www.w3.org/TR/SVGTiny12/fonts.html#FontElement> ;
  rdfs:subClassOf svg:FontElements ;
.
svg:Font-face
  a ui:NodeClass ;
  rdfs:comment "The 'font-face' element is an XML structure which corresponds directly to the @font-face facility in CSS2. It can be used to describe the characteristics of any font, SVG font or otherwise." ;
  rdfs:label "Font-face" ;
  rdfs:seeAlso <http://www.w3.org/TR/SVGTiny12/fonts.html#FontFaceElement> ;
  rdfs:subClassOf svg:FontElements ;
.
svg:Font-face-src
  a ui:NodeClass ;
  rdfs:comment "The 'font-face-src' element, together with the 'font-face-uri' elements described further down correspond to the 'src' descriptor within an @font-face rule." ;
  rdfs:label "Font-face-src" ;
  rdfs:seeAlso <http://www.w3.org/TR/SVGTiny12/fonts.html#FontFaceSrcElement> ;
  rdfs:subClassOf svg:FontElements ;
.
svg:Font-face-uri
  a ui:NodeClass ;
  rdfs:comment "The 'font-face-uri' element is used within a 'font-face-src' element to reference a font defined inside or outside of the current SVG document." ;
  rdfs:label "Font-face-uri" ;
  rdfs:seeAlso <http://www.w3.org/TR/SVGTiny12/fonts.html#FontFaceUriElement> ;
  rdfs:subClassOf svg:FontElements ;
.
svg:FontElements
  a ui:NodeClass ;
  ui:abstract true ;
  rdfs:comment "Abstract base class of SVG font elements." ;
  rdfs:label "Font elements" ;
  rdfs:subClassOf svg:Elements ;
.
svg:ForeignObject
  a ui:NodeClass ;
  rdfs:comment "The 'foreignObject' element is an extensibility point which allows user agents to offer graphical rendering features beyond those which are defined within this specification." ;
  rdfs:label "Foreign object" ;
  rdfs:seeAlso <http://www.w3.org/TR/SVGTiny12/extend.html#ForeignObjectElement> ;
  rdfs:subClassOf svg:StructuralElements ;
.
svg:G
  a ui:NodeClass ;
  rdfs:comment "The 'g' element is a container element for grouping together related graphics elements." ;
  rdfs:label "G" ;
  rdfs:seeAlso <http://www.w3.org/TR/SVGTiny12/struct.html#GElement> ;
  rdfs:subClassOf svg:ContainerElements ;
.
svg:Glyph
  a ui:NodeClass ;
  rdfs:comment "The 'glyph' element defines the graphics for a given glyph." ;
  rdfs:label "Glyph" ;
  rdfs:seeAlso <http://www.w3.org/TR/SVGTiny12/fonts.html#GlyphElement> ;
  rdfs:subClassOf svg:FontElements ;
.
svg:GraphicsElements
  a ui:NodeClass ;
  ui:abstract true ;
  rdfs:label "Graphics elements" ;
  rdfs:subClassOf svg:Elements ;
.
svg:Handler
  a ui:NodeClass ;
  rdfs:comment "The 'handler' element is similar to the 'script' element: its contents, either included inline or referenced, is code that is to be executed by a scripting engine used by user agent." ;
  rdfs:label "Handler" ;
  rdfs:seeAlso <http://www.w3.org/TR/SVGTiny12/script.html#HandlerElement> ;
  rdfs:subClassOf svg:ScriptingElements ;
.
svg:Hkern
  a ui:NodeClass ;
  rdfs:comment "The 'hkern' element defines kerning pairs for horizontally-oriented pairs of glyphs." ;
  rdfs:label "Hkern" ;
  rdfs:seeAlso <http://www.w3.org/TR/SVGTiny12/fonts.html#KernElements> ;
  rdfs:subClassOf svg:FontElements ;
.
svg:Image
  a ui:NodeClass ;
  spin:constraint [
      a spl:Argument ;
      spl:predicate svg:height ;
      rdfs:comment "The height of the rectangular region." ;
    ] ;
  spin:constraint [
      a spl:Argument ;
      spl:predicate svg:preserveAspectRatio ;
      rdfs:comment "See http://www.w3.org/TR/SVGTiny12/coords.html#PreserveAspectRatioAttribute" ;
    ] ;
  spin:constraint [
      a spl:Argument ;
      spl:predicate svg:type ;
      rdfs:comment "A hint about the expected Internet Media Type of the raster image. Implementations may choose to not fetch images of formats that they do not support. Note that if an Internet Media type returned by the server, the server metadata is authoritative over the type attribute. See Metadata hints in specifications in the Authoritative Metadata TAG finding ([MIME-RESPECT], section 5). To ensure that a user agent only downloads media in formats that it supports, thus optimizing download time and bandwidth usage, authors are encouraged to use 'requiredFormats', instead of 'type'." ;
    ] ;
  spin:constraint [
      a spl:Argument ;
      spl:predicate svg:width ;
      rdfs:comment "The width of the rectangular region." ;
    ] ;
  spin:constraint [
      a spl:Argument ;
      spl:predicate svg:x ;
      rdfs:comment "The x-axis coordinate of one corner of the rectangular region." ;
    ] ;
  spin:constraint [
      a spl:Argument ;
      spl:predicate svg:y ;
      rdfs:comment "The y-axis coordinate of one corner of the rectangular region." ;
    ] ;
  spin:constraint [
      a spl:Argument ;
      spl:predicate xlink:href ;
      rdfs:comment "An IRI reference to the image. An invalid IRI reference is an unsupported value. An empty attribute value (xlink:href=\"\") disables rendering of the element. The lacuna value is the empty string." ;
    ] ;
  rdfs:comment "The 'image' element indicates that the contents of an image are to be rendered into a given rectangle within the current user coordinate system." ;
  rdfs:label "Image" ;
  rdfs:seeAlso <http://www.w3.org/TR/SVGTiny12/struct.html#ImageElement> ;
  rdfs:subClassOf svg:GraphicsElements ;
.
svg:Line
  a ui:NodeClass ;
  spin:constraint [
      a spl:Argument ;
      spl:predicate svg:x1 ;
      rdfs:comment "The x-axis coordinate of the start of the line. The lacuna value is '0'." ;
    ] ;
  spin:constraint [
      a spl:Argument ;
      spl:predicate svg:x2 ;
      rdfs:comment "The x-axis coordinate of the end of the line. The lacuna value is '0'." ;
    ] ;
  spin:constraint [
      a spl:Argument ;
      spl:predicate svg:y1 ;
      rdfs:comment "The y-axis coordinate of the start of the line. The lacuna value is '0'." ;
    ] ;
  spin:constraint [
      a spl:Argument ;
      spl:predicate svg:y2 ;
      rdfs:comment "The y-axis coordinate of the end of the line. The lacuna value is '0'." ;
    ] ;
  rdfs:comment "The 'line' element defines a line segment that starts at one point and ends at another." ;
  rdfs:label "Line" ;
  rdfs:seeAlso <http://www.w3.org/TR/SVGTiny12/shapes.html#LineElement> ;
  rdfs:subClassOf svg:GraphicsElements ;
.
svg:LinearGradient
  a ui:NodeClass ;
  rdfs:comment "Linear gradients are defined by a 'linearGradient' element." ;
  rdfs:label "Linear gradient" ;
  rdfs:seeAlso <http://www.w3.org/TR/SVGTiny12/painting.html#LinearGradientElement> ;
  rdfs:subClassOf svg:PaintingElements ;
.
svg:Listener
  a ui:NodeClass ;
  rdfs:comment "The 'listener' element from XML Events [XML-EVENTS] must be supported." ;
  rdfs:label "Listener" ;
  rdfs:seeAlso <http://www.w3.org/TR/SVGTiny12/script.html#ListenerElement> ;
  rdfs:subClassOf svg:ScriptingElements ;
.
svg:Metadata
  a ui:NodeClass ;
  rdfs:comment "Metadata which is included with SVG content should be specified within 'metadata' elements." ;
  rdfs:label "Metadata" ;
  rdfs:seeAlso <http://www.w3.org/TR/SVGTiny12/metadata.html#MetadataElement> ;
  rdfs:subClassOf svg:DescriptiveElements ;
.
svg:Missing-glyph
  a ui:NodeClass ;
  rdfs:comment "The 'missing-glyph' element defines a graphic to use if there is an attempt to draw a glyph from a given font and the given glyph has not been defined." ;
  rdfs:label "Missing-glyph" ;
  rdfs:seeAlso <http://www.w3.org/TR/SVGTiny12/fonts.html#MissingGlyphElement> ;
  rdfs:subClassOf svg:FontElements ;
.
svg:Mpath
  a ui:NodeClass ;
  rdfs:comment "The 'mpath' element is used to reference an existing 'path' element for use as a motion animation path." ;
  rdfs:label "Mpath" ;
  rdfs:seeAlso <http://www.w3.org/TR/SVGTiny12/animate.html#MpathElement> ;
  rdfs:subClassOf svg:AnimationElements ;
.
svg:MultimediaElements
  a ui:NodeClass ;
  ui:abstract true ;
  rdfs:comment "Abstract base class of SVG multimedia elements." ;
  rdfs:label "Multimedia elements" ;
  rdfs:subClassOf svg:Elements ;
.
svg:PaintingElements
  a ui:NodeClass ;
  ui:abstract true ;
  rdfs:comment "Abstract base class of SVG painting elements." ;
  rdfs:label "Painting elements" ;
  rdfs:subClassOf svg:Elements ;
.
svg:Path
  a ui:NodeClass ;
  spin:constraint [
      a spl:Argument ;
      spl:predicate svg:d ;
      rdfs:comment "The definition of the outline of a shape. See Path data. An empty attribute value (d=\"\") disables rendering of the element. The lacuna value is the empty string." ;
    ] ;
  spin:constraint [
      a spl:Argument ;
      spl:predicate svg:pathLength ;
      rdfs:comment "The authoring length of the path, in user units. This value is used to calibrate the user agent's own distance-along-a-path calculations with that of the author. The user agent shall scale all distance-along-a-path computations by the ratio of 'pathLength' to the user agent's own computed value for total path length. 'pathLength' potentially affects calculations for motion animation and various stroke operations." ;
    ] ;
  rdfs:comment "Paths represent the outline of a shape which can be filled or stroked." ;
  rdfs:label "Path" ;
  rdfs:seeAlso <http://www.w3.org/TR/SVGTiny12/paths.html#PathElement> ;
  rdfs:subClassOf svg:GraphicsElements ;
.
svg:Polygon
  a ui:NodeClass ;
  rdfs:comment "The 'polygon' element defines a closed shape consisting of a set of connected straight line segments." ;
  rdfs:label "Polygon" ;
  rdfs:seeAlso <http://www.w3.org/TR/SVGTiny12/shapes.html#PolygonElement> ;
  rdfs:subClassOf svg:GraphicsElements ;
.
svg:Polyline
  a ui:NodeClass ;
  rdfs:comment "The 'polyline' element defines a set of connected straight line segments." ;
  rdfs:label "Polyline" ;
  rdfs:seeAlso <http://www.w3.org/TR/SVGTiny12/shapes.html#PolylineElement> ;
  rdfs:subClassOf svg:GraphicsElements ;
.
svg:Prefetch
  a ui:NodeClass ;
  rdfs:comment "SVG Tiny 1.2 adds functionality to allow content developers to suggest prefetching content from the server before it is needed to improve the rendering performance of the document." ;
  rdfs:label "Prefetch" ;
  rdfs:seeAlso <http://www.w3.org/TR/SVGTiny12/struct.html#PrefetchElement> ;
  rdfs:subClassOf svg:StructuralElements ;
.
svg:RadialGradient
  a ui:NodeClass ;
  rdfs:comment "Radial gradients are defined by a 'radialGradient' element." ;
  rdfs:label "Radial gradient" ;
  rdfs:seeAlso <http://www.w3.org/TR/SVGTiny12/painting.html#RadialGradientElement> ;
  rdfs:subClassOf svg:PaintingElements ;
.
svg:Rect
  a ui:NodeClass ;
  spin:constraint [
      a spl:Argument ;
      spl:predicate svg:height ;
      rdfs:comment "The height of the rectangle. A negative value is unsupported. A value of zero disables rendering of the element. The lacuna value is '0'." ;
    ] ;
  spin:constraint [
      a spl:Argument ;
      spl:predicate svg:rx ;
      rdfs:comment "For rounded rectangles, the x-axis radius of the ellipse used to round off the corners of the rectangle. A negative value is unsupported. See the notes below about what happens if the attribute is not specified." ;
    ] ;
  spin:constraint [
      a spl:Argument ;
      spl:predicate svg:ry ;
      rdfs:comment "For rounded rectangles, the y-axis radius of the ellipse used to round off the corners of the rectangle. A negative value is unsupported. See the notes below about what happens if the attribute is not specified." ;
    ] ;
  spin:constraint [
      a spl:Argument ;
      spl:predicate svg:width ;
      rdfs:comment "The width of the rectangle. A negative value is unsupported. A value of zero disables rendering of the element. The lacuna value is '0'." ;
    ] ;
  spin:constraint [
      a spl:Argument ;
      spl:predicate svg:x ;
      rdfs:comment "The x-axis coordinate of the side of the rectangle which has the smaller x-axis coordinate value in the current user coordinate system. The lacuna value is '0'." ;
    ] ;
  spin:constraint [
      a spl:Argument ;
      spl:predicate svg:y ;
      rdfs:comment "The y-axis coordinate of the side of the rectangle which has the smaller y-axis coordinate value in the current user coordinate system. The lacuna value is '0'." ;
    ] ;
  rdfs:comment "The 'rect' element defines a rectangle which is axis-aligned with the current user coordinate system." ;
  rdfs:label "Rect" ;
  rdfs:seeAlso <http://www.w3.org/TR/SVGTiny12/shapes.html#RectElement> ;
  rdfs:subClassOf svg:GraphicsElements ;
.
svg:Script
  a ui:NodeClass ;
  rdfs:comment "A 'script' element may either contain or point to executable content (e.g., ECMAScript or Java JAR file)." ;
  rdfs:label "Script" ;
  rdfs:seeAlso <http://www.w3.org/TR/SVGTiny12/script.html#ScriptElement> ;
  rdfs:subClassOf svg:ScriptingElements ;
.
svg:ScriptingElements
  a ui:NodeClass ;
  ui:abstract true ;
  rdfs:comment "Abstract base class of SVG scripting elements." ;
  rdfs:label "Scripting elements" ;
  rdfs:subClassOf svg:Elements ;
.
svg:Set
  a ui:NodeClass ;
  rdfs:comment "The 'set' element provides a simple means of just setting the value of an attribute for a specified duration." ;
  rdfs:label "Set" ;
  rdfs:seeAlso <http://www.w3.org/TR/SVGTiny12/animate.html#SetElement> ;
  rdfs:subClassOf svg:AnimationElements ;
.
svg:SolidColor
  a ui:NodeClass ;
  rdfs:comment "The 'solidColor' element is a paint server that provides a single color with opacity." ;
  rdfs:label "Solid color" ;
  rdfs:seeAlso <http://www.w3.org/TR/SVGTiny12/painting.html#SolidColorElement> ;
  rdfs:subClassOf svg:PaintingElements ;
.
svg:Stop
  a ui:NodeClass ;
  rdfs:comment "The ramp of colors to use on a gradient is defined by the 'stop' elements that are child elements to either the 'linearGradient' element or the 'radialGradient' element." ;
  rdfs:label "Stop" ;
  rdfs:seeAlso <http://www.w3.org/TR/SVGTiny12/painting.html#StopElement> ;
  rdfs:subClassOf svg:PaintingElements ;
.
svg:StructuralElements
  a ui:NodeClass ;
  ui:abstract true ;
  rdfs:comment "Abstract base class of the SCG structural elements." ;
  rdfs:label "Structural elements" ;
  rdfs:subClassOf svg:Elements ;
.
svg:Svg
  a ui:NodeClass ;
  spin:constraint [
      a spl:Argument ;
      spl:predicate svg:baseProfile ;
      rdfs:comment "Describes the minimum SVG language profile that the author believes is necessary to correctly render the content. See rules for baseProfile processing for further instructions." ;
    ] ;
  spin:constraint [
      a spl:Argument ;
      spl:predicate svg:contentScriptType ;
      rdfs:comment "Identifies the default scripting language for the given document. This attribute sets the default scripting language for all the instances of script in the document fragment. This language must be used for all scripts that do not specify their own scripting language. The <content-type> value specifies a media type, per Multipart Internet Mail Extensions: (MIME) Part Two: Media Types [RFC2046]. The lacuna value is \"application/ecmascript\"." ;
    ] ;
  spin:constraint [
      a spl:Argument ;
      spl:predicate svg:height ;
      rdfs:comment "The intrinsic height of the SVG document fragment." ;
    ] ;
  spin:constraint [
      a spl:Argument ;
      spl:predicate svg:playbackOrder ;
      rdfs:comment "Indicates whether it is possible to seek backwards in the document. In earlier versions of SVG there was no need to put restrictions on the direction of seeking but with the newly introduced facilities for long-running documents (e.g. the 'discard' element) there is sometimes a need to restrict this." ;
    ] ;
  spin:constraint [
      a spl:Argument ;
      spl:predicate svg:preserveAspectRatio ;
      rdfs:comment "See http://www.w3.org/TR/SVGTiny12/coords.html#PreserveAspectRatioAttribute" ;
    ] ;
  spin:constraint [
      a spl:Argument ;
      spl:predicate svg:snapshotTime ;
      rdfs:comment "Indicates a moment in time which is most relevant for a still-image of the animated SVG content. This time may be used as a hint to the SVG user agent for rendering a still-image of an animated SVG document, such as a preview. A value of 'none' means that no 'snapshotTime' is available. See example 05_22 for an example of using the 'snapshotTime' attribute." ;
    ] ;
  spin:constraint [
      a spl:Argument ;
      spl:predicate svg:timelineBegin ;
      rdfs:comment "Controls the initialization of the timeline for the document." ;
    ] ;
  spin:constraint [
      a spl:Argument ;
      spl:predicate svg:version ;
      rdfs:comment "Indicates the SVG language version to which this document fragment conforms." ;
    ] ;
  spin:constraint [
      a spl:Argument ;
      spl:predicate svg:width ;
      rdfs:comment "The intrinsic width of the SVG document fragment. Together with the 'height', 'viewBox' and 'preserveAspectRatio' attributes it defines the intrinsic aspect ratio and (unless both width and height are percentages) the intrinsic size of the svg element. See The initial viewport." ;
    ] ;
  spin:constraint [
      a spl:Argument ;
      spl:predicate svg:zoomAndPan ;
      rdfs:comment "See http://www.w3.org/TR/SVGTiny12/interact.html#ZoomAndPanAttribute" ;
    ] ;
  rdfs:comment "An SVG document fragment consists of any number of SVG elements contained within an 'svg' element, including the 'svg' element." ;
  rdfs:label "SVG" ;
  rdfs:seeAlso <http://www.w3.org/TR/SVGTiny12/struct.html#SVGElement> ;
  rdfs:subClassOf svg:StructuralElements ;
.
svg:Switch
  a ui:NodeClass ;
  rdfs:comment "The 'switch' element is a container element that can be used to select one of its child elements to process based on their conditional processing attributes." ;
  rdfs:label "Switch" ;
  rdfs:seeAlso <http://www.w3.org/TR/SVGTiny12/struct.html#SwitchElement> ;
  rdfs:subClassOf svg:StructuralElements ;
.
svg:Tbreak
  a ui:NodeClass ;
  rdfs:comment "The 'tbreak' element is an empty element that forcibly breaks the current line of text, even if the current line of text is empty (i.e. multiple consecutive 'tbreak' elements each cause a line break.)" ;
  rdfs:label "Tbreak" ;
  rdfs:seeAlso <http://www.w3.org/TR/SVGTiny12/text.html#tbreakElement> ;
  rdfs:subClassOf svg:TextElements ;
.
svg:Text
  a ui:NodeClass ;
  spin:constraint [
      a spl:Argument ;
      spl:predicate svg:editable ;
      rdfs:comment "This attribute indicates whether the text can be edited. See the definition of the 'editable' attribute." ;
    ] ;
  spin:constraint [
      a spl:Argument ;
      spl:predicate svg:rotate ;
      rdfs:comment "This attribute indicates the supplemental rotation about the alignment-point that must be applied to the glyphs corresponding to characters within this element according to the following rules:" ;
    ] ;
  spin:constraint [
      a spl:Argument ;
      spl:predicate svg:x ;
      rdfs:comment "If a single <coordinate> is provided, then the value represents the new absolute X coordinate for the current text position for rendering the glyphs that correspond to the first character within this element or any of its descendants." ;
    ] ;
  spin:constraint [
      a spl:Argument ;
      spl:predicate svg:y ;
      rdfs:comment "The corresponding list of absolute Y coordinates for the glyphs corresponding to the characters within this element. The processing rules for the 'y' attribute parallel the processing rules for the 'x' attribute." ;
    ] ;
  spin:constraint [
      a spl:Argument ;
      spl:predicate ui:text ;
      rdfs:comment "The text string." ;
    ] ;
  rdfs:comment "The 'text' element defines a graphics element consisting of text." ;
  rdfs:label "Text" ;
  rdfs:seeAlso <http://www.w3.org/TR/SVGTiny12/text.html#TextElement> ;
  rdfs:subClassOf svg:TextElements ;
.
svg:TextArea
  a ui:NodeClass ;
  rdfs:comment "The 'textArea' element allows simplistic wrapping of text content within a given region." ;
  rdfs:label "Text area" ;
  rdfs:seeAlso <http://www.w3.org/TR/SVGTiny12/text.html#TextAreaElement> ;
  rdfs:subClassOf svg:TextElements ;
.
svg:TextElements
  a ui:NodeClass ;
  ui:abstract true ;
  rdfs:comment "Abstract base class of the SVG text elements." ;
  rdfs:label "Text elements" ;
  rdfs:subClassOf svg:Elements ;
.
svg:Title
  a ui:NodeClass ;
  rdfs:comment "Each container element or graphics element in an SVG document may contain one or more of each of the 'title' and 'desc' descriptive elements, which together comprise a sort of heading and summary of the containing element." ;
  rdfs:label "Title" ;
  rdfs:seeAlso <http://www.w3.org/TR/SVGTiny12/struct.html#TitleAndDescriptionElements> ;
  rdfs:subClassOf svg:DescriptiveElements ;
.
svg:Tspan
  a ui:NodeClass ;
  rdfs:comment "Within a text content block element, graphic and font properties can be adjusted by including a 'tspan' element." ;
  rdfs:label "Tspan" ;
  rdfs:seeAlso <http://www.w3.org/TR/SVGTiny12/text.html#TSpanElement> ;
  rdfs:subClassOf svg:TextElements ;
.
svg:Use
  a ui:NodeClass ;
  rdfs:comment "Any 'g' or graphics element is potentially a template object that can be re-used (i.e. \"instantiated\") in the SVG document via a 'use' element, thus creating an instance tree." ;
  rdfs:label "Use" ;
  rdfs:seeAlso <http://www.w3.org/TR/SVGTiny12/struct.html#UseElement> ;
  rdfs:subClassOf svg:StructuralElements ;
.
svg:Video
  a ui:NodeClass ;
  rdfs:comment "The 'video' element specifies a video file which is to be rendered to provide synchronized video." ;
  rdfs:label "Video" ;
  rdfs:seeAlso <http://www.w3.org/TR/SVGTiny12/multimedia.html#VideoElement> ;
  rdfs:subClassOf svg:MultimediaElements ;
.
svg:about
  a svg:Attribute ;
  rdfs:label "about" ;
  rdfs:subPropertyOf svg:attributes ;
.
svg:accent-height
  a svg:Attribute ;
  rdfs:label "accent-height" ;
  rdfs:subPropertyOf svg:attributes ;
.
svg:accumulate
  a svg:Attribute ;
  rdfs:label "accumulate" ;
  rdfs:subPropertyOf svg:attributes ;
.
svg:additive
  a svg:Attribute ;
  rdfs:label "additive" ;
  rdfs:subPropertyOf svg:attributes ;
.
svg:alphabetic
  a svg:Attribute ;
  rdfs:label "alphabetic" ;
  rdfs:subPropertyOf svg:attributes ;
.
svg:arabic-form
  a svg:Attribute ;
  rdfs:label "arabic-form" ;
  rdfs:subPropertyOf svg:attributes ;
.
svg:ascent
  a svg:Attribute ;
  rdfs:label "ascent" ;
  rdfs:subPropertyOf svg:attributes ;
.
svg:attributeName
  a svg:Attribute ;
  rdfs:label "attribute name" ;
  rdfs:subPropertyOf svg:attributes ;
.
svg:attributeType
  a svg:Attribute ;
  rdfs:label "attribute type" ;
  rdfs:subPropertyOf svg:attributes ;
.
svg:attributes
  a svg:Attribute ;
  rdfs:comment "Abstract base property to group all SVG attributes." ;
  rdfs:label "attributes" ;
.
svg:bandwidth
  a svg:Attribute ;
  rdfs:label "bandwidth" ;
  rdfs:subPropertyOf svg:attributes ;
.
svg:baseProfile
  a svg:Attribute ;
  rdfs:label "base profile" ;
  rdfs:subPropertyOf svg:attributes ;
.
svg:bbox
  a svg:Attribute ;
  rdfs:label "bbox" ;
  rdfs:subPropertyOf svg:attributes ;
.
svg:begin
  a svg:Attribute ;
  rdfs:label "begin" ;
  rdfs:subPropertyOf svg:attributes ;
.
svg:by
  a svg:Attribute ;
  rdfs:label "by" ;
  rdfs:subPropertyOf svg:attributes ;
.
svg:calcMode
  a svg:Attribute ;
  rdfs:label "calc mode" ;
  rdfs:subPropertyOf svg:attributes ;
.
svg:cap-height
  a svg:Attribute ;
  rdfs:label "cap-height" ;
  rdfs:subPropertyOf svg:attributes ;
.
svg:class
  a svg:Attribute ;
  rdfs:label "class" ;
  rdfs:subPropertyOf svg:attributes ;
.
svg:content
  a svg:Attribute ;
  rdfs:label "content" ;
  rdfs:subPropertyOf svg:attributes ;
.
svg:contentScriptType
  a svg:Attribute ;
  rdfs:label "content script type" ;
  rdfs:subPropertyOf svg:attributes ;
.
svg:cx
  a svg:Attribute ;
  rdfs:label "cx" ;
  rdfs:subPropertyOf svg:attributes ;
.
svg:cy
  a svg:Attribute ;
  rdfs:label "cy" ;
  rdfs:subPropertyOf svg:attributes ;
.
svg:d
  a svg:Attribute ;
  rdfs:label "d" ;
  rdfs:subPropertyOf svg:attributes ;
.
svg:datatype
  a svg:Attribute ;
  rdfs:label "datatype" ;
  rdfs:subPropertyOf svg:attributes ;
.
svg:defaultAction
  a svg:Attribute ;
  rdfs:label "default action" ;
  rdfs:subPropertyOf svg:attributes ;
.
svg:descent
  a svg:Attribute ;
  rdfs:label "descent" ;
  rdfs:subPropertyOf svg:attributes ;
.
svg:dur
  a svg:Attribute ;
  rdfs:label "dur" ;
  rdfs:subPropertyOf svg:attributes ;
.
svg:editable
  a svg:Attribute ;
  rdfs:label "editable" ;
  rdfs:subPropertyOf svg:attributes ;
.
svg:end
  a svg:Attribute ;
  rdfs:label "end" ;
  rdfs:subPropertyOf svg:attributes ;
.
svg:externalResourcesRequired
  a svg:Attribute ;
  rdfs:label "external resources required" ;
  rdfs:subPropertyOf svg:attributes ;
.
svg:focusHighlight
  a svg:Attribute ;
  rdfs:label "focus highlight" ;
  rdfs:subPropertyOf svg:attributes ;
.
svg:focusable
  a svg:Attribute ;
  rdfs:label "focusable" ;
  rdfs:subPropertyOf svg:attributes ;
.
svg:font-stretch
  a svg:Attribute ;
  rdfs:label "font-stretch" ;
  rdfs:subPropertyOf svg:attributes ;
.
svg:fontFamily
  a svg:Attribute ;
  rdfs:label "font family" ;
  rdfs:subPropertyOf svg:attributes ;
.
svg:from
  a svg:Attribute ;
  rdfs:label "from" ;
  rdfs:subPropertyOf svg:attributes ;
.
svg:g1
  a svg:Attribute ;
  rdfs:label "g1" ;
  rdfs:subPropertyOf svg:attributes ;
.
svg:g2
  a svg:Attribute ;
  rdfs:label "g2" ;
  rdfs:subPropertyOf svg:attributes ;
.
svg:glyph-name
  a svg:Attribute ;
  rdfs:label "glyph-name" ;
  rdfs:subPropertyOf svg:attributes ;
.
svg:gradientUnits
  a svg:Attribute ;
  rdfs:label "gradient units" ;
  rdfs:subPropertyOf svg:attributes ;
.
svg:handler
  a svg:Attribute ;
  rdfs:label "handler" ;
  rdfs:subPropertyOf svg:attributes ;
.
svg:hanging
  a svg:Attribute ;
  rdfs:label "hanging" ;
  rdfs:subPropertyOf svg:attributes ;
.
svg:height
  a svg:Attribute ;
  rdfs:label "height" ;
  rdfs:subPropertyOf svg:attributes ;
.
svg:horiz-adv-x
  a svg:Attribute ;
  rdfs:label "horiz-adv-x" ;
  rdfs:subPropertyOf svg:attributes ;
.
svg:horiz-origin-x
  a svg:Attribute ;
  rdfs:label "horiz-origin-x" ;
  rdfs:subPropertyOf svg:attributes ;
.
svg:id
  a svg:Attribute ;
  rdfs:label "id" ;
  rdfs:range xsd:string ;
  rdfs:subPropertyOf svg:attributes ;
.
svg:ideographic
  a svg:Attribute ;
  rdfs:label "ideographic" ;
  rdfs:subPropertyOf svg:attributes ;
.
svg:initialVisibility
  a svg:Attribute ;
  rdfs:label "initial visibility" ;
  rdfs:subPropertyOf svg:attributes ;
.
svg:k
  a svg:Attribute ;
  rdfs:label "k" ;
  rdfs:subPropertyOf svg:attributes ;
.
svg:keyPoints
  a svg:Attribute ;
  rdfs:label "key points" ;
  rdfs:subPropertyOf svg:attributes ;
.
svg:keySplines
  a svg:Attribute ;
  rdfs:label "key splines" ;
  rdfs:subPropertyOf svg:attributes ;
.
svg:keyTimes
  a svg:Attribute ;
  rdfs:label "key times" ;
  rdfs:subPropertyOf svg:attributes ;
.
svg:lang
  a svg:Attribute ;
  rdfs:label "lang" ;
  rdfs:subPropertyOf svg:attributes ;
.
svg:mathematical
  a svg:Attribute ;
  rdfs:label "mathematical" ;
  rdfs:subPropertyOf svg:attributes ;
.
svg:max
  a svg:Attribute ;
  rdfs:label "max" ;
  rdfs:subPropertyOf svg:attributes ;
.
svg:mediaCharacterEncoding
  a svg:Attribute ;
  rdfs:label "media character encoding" ;
  rdfs:subPropertyOf svg:attributes ;
.
svg:mediaContentEncodings
  a svg:Attribute ;
  rdfs:label "media content encodings" ;
  rdfs:subPropertyOf svg:attributes ;
.
svg:mediaSize
  a svg:Attribute ;
  rdfs:label "media size" ;
  rdfs:subPropertyOf svg:attributes ;
.
svg:mediaTime
  a svg:Attribute ;
  rdfs:label "media time" ;
  rdfs:subPropertyOf svg:attributes ;
.
svg:min
  a svg:Attribute ;
  rdfs:label "min" ;
  rdfs:subPropertyOf svg:attributes ;
.
svg:nav-down
  a svg:Attribute ;
  rdfs:label "nav-down" ;
  rdfs:subPropertyOf svg:attributes ;
.
svg:nav-down-left
  a svg:Attribute ;
  rdfs:label "nav-down-left" ;
  rdfs:subPropertyOf svg:attributes ;
.
svg:nav-down-right
  a svg:Attribute ;
  rdfs:label "nav-down-right" ;
  rdfs:subPropertyOf svg:attributes ;
.
svg:nav-left
  a svg:Attribute ;
  rdfs:label "nav-left" ;
  rdfs:subPropertyOf svg:attributes ;
.
svg:nav-next
  a svg:Attribute ;
  rdfs:label "nav-next" ;
  rdfs:subPropertyOf svg:attributes ;
.
svg:nav-prev
  a svg:Attribute ;
  rdfs:label "nav-prev" ;
  rdfs:subPropertyOf svg:attributes ;
.
svg:nav-right
  a svg:Attribute ;
  rdfs:label "nav-right" ;
  rdfs:subPropertyOf svg:attributes ;
.
svg:nav-up
  a svg:Attribute ;
  rdfs:label "nav-up" ;
  rdfs:subPropertyOf svg:attributes ;
.
svg:nav-up-left
  a svg:Attribute ;
  rdfs:label "nav-up-left" ;
  rdfs:subPropertyOf svg:attributes ;
.
svg:nav-up-right
  a svg:Attribute ;
  rdfs:label "nav-up-right" ;
  rdfs:subPropertyOf svg:attributes ;
.
svg:observer
  a svg:Attribute ;
  rdfs:label "observer" ;
  rdfs:subPropertyOf svg:attributes ;
.
svg:offset
  a svg:Attribute ;
  rdfs:label "offset" ;
  rdfs:subPropertyOf svg:attributes ;
.
svg:origin
  a svg:Attribute ;
  rdfs:label "origin" ;
  rdfs:subPropertyOf svg:attributes ;
.
svg:overlay
  a svg:Attribute ;
  rdfs:label "overlay" ;
  rdfs:subPropertyOf svg:attributes ;
.
svg:overline-position
  a svg:Attribute ;
  rdfs:label "overline-position" ;
  rdfs:subPropertyOf svg:attributes ;
.
svg:overline-thickness
  a svg:Attribute ;
  rdfs:label "overline-thickness" ;
  rdfs:subPropertyOf svg:attributes ;
.
svg:panose-1
  a svg:Attribute ;
  rdfs:label "panose-1" ;
  rdfs:subPropertyOf svg:attributes ;
.
svg:path
  a svg:Attribute ;
  rdfs:label "path" ;
  rdfs:subPropertyOf svg:attributes ;
.
svg:pathLength
  a svg:Attribute ;
  rdfs:label "path length" ;
  rdfs:subPropertyOf svg:attributes ;
.
svg:phase
  a svg:Attribute ;
  rdfs:label "phase" ;
  rdfs:subPropertyOf svg:attributes ;
.
svg:playbackOrder
  a svg:Attribute ;
  rdfs:label "playback order" ;
  rdfs:subPropertyOf svg:attributes ;
.
svg:points
  a svg:Attribute ;
  rdfs:label "points" ;
  rdfs:subPropertyOf svg:attributes ;
.
svg:preserveAspectRatio
  a svg:Attribute ;
  rdfs:label "preserve aspect ratio" ;
  rdfs:subPropertyOf svg:attributes ;
.
svg:propagate
  a svg:Attribute ;
  rdfs:label "propagate" ;
  rdfs:subPropertyOf svg:attributes ;
.
svg:property
  a svg:Attribute ;
  rdfs:label "property" ;
  rdfs:subPropertyOf svg:attributes ;
.
svg:r
  a svg:Attribute ;
  rdfs:label "r" ;
  rdfs:subPropertyOf svg:attributes ;
.
svg:rel
  a svg:Attribute ;
  rdfs:label "rel" ;
  rdfs:subPropertyOf svg:attributes ;
.
svg:repeatCount
  a svg:Attribute ;
  rdfs:label "repeat count" ;
  rdfs:subPropertyOf svg:attributes ;
.
svg:repeatDur
  a svg:Attribute ;
  rdfs:label "repeat dur" ;
  rdfs:subPropertyOf svg:attributes ;
.
svg:requiredExtensions
  a svg:Attribute ;
  rdfs:label "required extensions" ;
  rdfs:subPropertyOf svg:attributes ;
.
svg:requiredFeatures
  a svg:Attribute ;
  rdfs:label "required features" ;
  rdfs:subPropertyOf svg:attributes ;
.
svg:requiredFonts
  a svg:Attribute ;
  rdfs:label "required fonts" ;
  rdfs:subPropertyOf svg:attributes ;
.
svg:requiredFormats
  a svg:Attribute ;
  rdfs:label "required formats" ;
  rdfs:subPropertyOf svg:attributes ;
.
svg:resource
  a svg:Attribute ;
  rdfs:label "resource" ;
  rdfs:subPropertyOf svg:attributes ;
.
svg:restart
  a svg:Attribute ;
  rdfs:label "restart" ;
  rdfs:subPropertyOf svg:attributes ;
.
svg:rev
  a svg:Attribute ;
  rdfs:label "rev" ;
  rdfs:subPropertyOf svg:attributes ;
.
svg:role
  a svg:Attribute ;
  rdfs:label "role" ;
  rdfs:subPropertyOf svg:attributes ;
.
svg:rotate
  a svg:Attribute ;
  rdfs:label "rotate" ;
  rdfs:subPropertyOf svg:attributes ;
.
svg:rx
  a svg:Attribute ;
  rdfs:label "rx" ;
  rdfs:subPropertyOf svg:attributes ;
.
svg:ry
  a svg:Attribute ;
  rdfs:label "ry" ;
  rdfs:subPropertyOf svg:attributes ;
.
svg:slope
  a svg:Attribute ;
  rdfs:label "slope" ;
  rdfs:subPropertyOf svg:attributes ;
.
svg:snapshotTime
  a svg:Attribute ;
  rdfs:label "snapshot time" ;
  rdfs:subPropertyOf svg:attributes ;
.
svg:stemh
  a svg:Attribute ;
  rdfs:label "stemh" ;
  rdfs:subPropertyOf svg:attributes ;
.
svg:stemv
  a svg:Attribute ;
  rdfs:label "stemv" ;
  rdfs:subPropertyOf svg:attributes ;
.
svg:strikethrough-position
  a svg:Attribute ;
  rdfs:label "strikethrough-position" ;
  rdfs:subPropertyOf svg:attributes ;
.
svg:strikethrough-thickness
  a svg:Attribute ;
  rdfs:label "strikethrough-thickness" ;
  rdfs:subPropertyOf svg:attributes ;
.
svg:syncBehavior
  a svg:Attribute ;
  rdfs:label "sync behavior" ;
  rdfs:subPropertyOf svg:attributes ;
.
svg:syncBehaviorDefault
  a svg:Attribute ;
  rdfs:label "sync behavior default" ;
  rdfs:subPropertyOf svg:attributes ;
.
svg:syncMaster
  a svg:Attribute ;
  rdfs:label "sync master" ;
  rdfs:subPropertyOf svg:attributes ;
.
svg:syncTolerance
  a svg:Attribute ;
  rdfs:label "sync tolerance" ;
  rdfs:subPropertyOf svg:attributes ;
.
svg:syncToleranceDefault
  a svg:Attribute ;
  rdfs:label "sync tolerance default" ;
  rdfs:subPropertyOf svg:attributes ;
.
svg:systemLanguage
  a svg:Attribute ;
  rdfs:label "system language" ;
  rdfs:subPropertyOf svg:attributes ;
.
svg:target
  a svg:Attribute ;
  rdfs:label "target" ;
  rdfs:subPropertyOf svg:attributes ;
.
svg:timelineBegin
  a svg:Attribute ;
  rdfs:label "timeline begin" ;
  rdfs:subPropertyOf svg:attributes ;
.
svg:to
  a svg:Attribute ;
  rdfs:label "to" ;
  rdfs:subPropertyOf svg:attributes ;
.
svg:transform
  a svg:Attribute ;
  rdfs:label "transform" ;
  rdfs:subPropertyOf svg:attributes ;
.
svg:transformBehavior
  a svg:Attribute ;
  rdfs:label "transform behavior" ;
  rdfs:subPropertyOf svg:attributes ;
.
svg:type
  a svg:Attribute ;
  rdfs:label "type" ;
  rdfs:subPropertyOf svg:attributes ;
.
svg:typeof
  a svg:Attribute ;
  rdfs:label "typeof" ;
  rdfs:subPropertyOf svg:attributes ;
.
svg:u1
  a svg:Attribute ;
  rdfs:label "u1" ;
  rdfs:subPropertyOf svg:attributes ;
.
svg:u2
  a svg:Attribute ;
  rdfs:label "u2" ;
  rdfs:subPropertyOf svg:attributes ;
.
svg:underline-position
  a svg:Attribute ;
  rdfs:label "underline-position" ;
  rdfs:subPropertyOf svg:attributes ;
.
svg:underline-thickness
  a svg:Attribute ;
  rdfs:label "underline-thickness" ;
  rdfs:subPropertyOf svg:attributes ;
.
svg:unicode
  a svg:Attribute ;
  rdfs:label "unicode" ;
  rdfs:subPropertyOf svg:attributes ;
.
svg:unicode-range
  a svg:Attribute ;
  rdfs:label "unicode-range" ;
  rdfs:subPropertyOf svg:attributes ;
.
svg:units-per-em
  a svg:Attribute ;
  rdfs:label "units-per-em" ;
  rdfs:subPropertyOf svg:attributes ;
.
svg:values
  a svg:Attribute ;
  rdfs:label "values" ;
  rdfs:subPropertyOf svg:attributes ;
.
svg:version
  a svg:Attribute ;
  rdfs:label "version" ;
  rdfs:subPropertyOf svg:attributes ;
.
svg:viewBox
  a svg:Attribute ;
  rdfs:label "view box" ;
  rdfs:subPropertyOf svg:attributes ;
.
svg:width
  a svg:Attribute ;
  rdfs:label "width" ;
  rdfs:subPropertyOf svg:attributes ;
.
svg:widths
  a svg:Attribute ;
  rdfs:label "widths" ;
  rdfs:subPropertyOf svg:attributes ;
.
svg:x
  a svg:Attribute ;
  rdfs:label "x" ;
  rdfs:subPropertyOf svg:attributes ;
.
svg:x-height
  a svg:Attribute ;
  rdfs:label "x-height" ;
  rdfs:subPropertyOf svg:attributes ;
.
svg:x1
  a svg:Attribute ;
  rdfs:label "x1" ;
  rdfs:subPropertyOf svg:attributes ;
.
svg:x2
  a svg:Attribute ;
  rdfs:label "x2" ;
  rdfs:subPropertyOf svg:attributes ;
.
svg:y
  a svg:Attribute ;
  rdfs:label "y" ;
  rdfs:subPropertyOf svg:attributes ;
.
svg:y1
  a svg:Attribute ;
  rdfs:label "y1" ;
  rdfs:subPropertyOf svg:attributes ;
.
svg:y2
  a svg:Attribute ;
  rdfs:label "y2" ;
  rdfs:subPropertyOf svg:attributes ;
.
svg:zoomAndPan
  a svg:Attribute ;
  rdfs:label "zoom and pan" ;
  rdfs:subPropertyOf svg:attributes ;
.
xlink:actuate
  a svg:Attribute ;
  rdfs:label "actuate" ;
  rdfs:subPropertyOf svg:attributes ;
.
xlink:arcrole
  a svg:Attribute ;
  rdfs:label "arcrole" ;
  rdfs:subPropertyOf svg:attributes ;
.
xlink:href
  a svg:Attribute ;
  rdfs:label "href" ;
  rdfs:subPropertyOf svg:attributes ;
.
xlink:role
  a svg:Attribute ;
  rdfs:label "role" ;
  rdfs:subPropertyOf svg:attributes ;
.
xlink:show
  a svg:Attribute ;
  rdfs:label "show" ;
  rdfs:subPropertyOf svg:attributes ;
.
xlink:title
  a svg:Attribute ;
  rdfs:label "title" ;
  rdfs:subPropertyOf svg:attributes ;
.
xlink:type
  a svg:Attribute ;
  rdfs:label "type" ;
  rdfs:subPropertyOf svg:attributes ;
.
