# baseURI: http://uispin.org/uilink

@prefix owl: <http://www.w3.org/2002/07/owl#> .
@prefix rdf: <http://www.w3.org/1999/02/22-rdf-syntax-ns#> .
@prefix rdfs: <http://www.w3.org/2000/01/rdf-schema#> .
@prefix ui: <http://uispin.org/ui#> .
@prefix xsd: <http://www.w3.org/2001/XMLSchema#> .

ui:instanceView
  a rdf:Property ;
  rdfs:comment "Links a class with elements that can be used to display instances of that class. In those elements, the variable ?this points to the instance being displayed." ;
  rdfs:domain rdfs:Class ;
  rdfs:label "instance view" ;
  rdfs:range rdfs:Resource ;
.
ui:view
  a rdf:Property ;
  rdfs:comment "Links a resource (instance) with an element that can be used to render the resource on the screen. Queries associated with the element can access the resource with the variable ?this." ;
  rdfs:domain rdfs:Resource ;
  rdfs:label "view" ;
  rdfs:range rdfs:Resource ;
.
<http://uispin.org/uilink>
  a owl:Ontology ;
  rdfs:comment "A light-weight fraction of the http://uispin.org/ui schema, defining properties that can be used to link RDF resources with user interface elements." ;
.
