# baseURI: http://evn.topbraidlive.org/tagger/acjob

@prefix acjob: <http://evn.topbraidlive.org/tagger/acjob#> .
@prefix owl: <http://www.w3.org/2002/07/owl#> .
@prefix rdf: <http://www.w3.org/1999/02/22-rdf-syntax-ns#> .
@prefix rdfs: <http://www.w3.org/2000/01/rdf-schema#> .
@prefix taggerprojects: <http://evn.topbraidlive.org/taggerprojects#> .
@prefix teamwork: <http://topbraid.org/teamwork#> .
@prefix xsd: <http://www.w3.org/2001/XMLSchema#> .

<http://evn.topbraidlive.org/tagger/acjob>
  rdf:type owl:Ontology ;
  rdfs:comment "A system namespace used to represent status information and summary data on AutoClassifier jobs."^^xsd:string ;
  owl:versionInfo "0.1.0"^^xsd:string ;
.
acjob:AutoClassifierJob
  rdf:type rdfs:Class ;
  rdfs:comment "A batch job for the AutoClassifier, possibly in progress, completed or cancelled."^^xsd:string ;
  rdfs:label "AutoClassifier job"^^xsd:string ;
  rdfs:subClassOf rdfs:Resource ;
.
acjob:JobScope
  rdf:type rdfs:Class ;
  rdfs:comment "The scope of an AutoClassifier job, that is, a characterization of the content resources covered by the job."^^xsd:string ;
  rdfs:label "Job scope"^^xsd:string ;
.
acjob:JobStatus
  rdf:type rdfs:Class ;
  rdfs:comment "An enumeration of status values for AutoClassifier jobs."^^xsd:string ;
  rdfs:label "Job status"^^xsd:string ;
.
acjob:all
  rdf:type acjob:JobScope ;
  rdfs:comment "Indicates a scope covering all content resources in a corpus."^^xsd:string ;
  rdfs:label "All"^^xsd:string ;
.
acjob:completed
  rdf:type acjob:JobStatus ;
  rdfs:label "Completed"^^xsd:string ;
.
acjob:finished
  rdf:type owl:DatatypeProperty ;
  rdfs:comment "The date and time when a completed AutoClassifier job was finished."^^xsd:string ;
  rdfs:domain acjob:AutoClassifierJob ;
  rdfs:label "finished"^^xsd:string ;
  rdfs:range xsd:dateTime ;
.
acjob:job
  rdf:type owl:ObjectProperty ;
  rdfs:comment "Connects an AutoClassifier job to the content tag set that provides the taxonomy and documents to be tagged."^^xsd:string ;
  rdfs:domain taggerprojects:ContentTagSet ;
  rdfs:label "job"^^xsd:string ;
  rdfs:range acjob:AutoClassifierJob ;
.
acjob:merged
  rdf:type acjob:JobStatus ;
  rdfs:label "Merged"^^xsd:string ;
.
acjob:resources
  rdf:type owl:DatatypeProperty ;
  rdfs:comment "The number of content resources to be tagged in an AutoClassifier job."^^xsd:string ;
  rdfs:domain acjob:AutoClassifierJob ;
  rdfs:label "resources"^^xsd:string ;
  rdfs:range xsd:integer ;
.
acjob:results
  rdf:type owl:ObjectProperty ;
  rdfs:comment "Connects a completed AutoClassifier job to a working copy containing its results."^^xsd:string ;
  rdfs:domain acjob:AutoClassifierJob ;
  rdfs:label "results"^^xsd:string ;
  rdfs:range teamwork:Tag ;
.
acjob:running
  rdf:type acjob:JobStatus ;
  rdfs:label "Running"^^xsd:string ;
.
acjob:scope
  rdf:type owl:ObjectProperty ;
  rdfs:comment "Connects an AutoClassifier job to its scope, that is, a characterization of the content resources covered by the job."^^xsd:string ;
  rdfs:domain acjob:AutoClassifierJob ;
  rdfs:label "scope"^^xsd:string ;
  rdfs:range acjob:JobScope ;
.
acjob:search
  rdf:type acjob:JobScope ;
  rdfs:comment "Indicates a scope covering the results of a (not specified in detail) search."^^xsd:string ;
  rdfs:label "Search"^^xsd:string ;
.
acjob:started
  rdf:type owl:DatatypeProperty ;
  rdfs:comment "The date and time when an AutoClassifier job was started."^^xsd:string ;
  rdfs:domain acjob:AutoClassifierJob ;
  rdfs:label "started"^^xsd:string ;
  rdfs:range xsd:dateTime ;
.
acjob:status
  rdf:type owl:ObjectProperty ;
  rdfs:comment "Connects an AutoClassifier job to its job status."^^xsd:string ;
  rdfs:domain acjob:AutoClassifierJob ;
  rdfs:label "status"^^xsd:string ;
  rdfs:range acjob:JobStatus ;
.
