# baseURI: http://itil.edg.topbraid.solutions/models/1.0/glossary
# imports: http://edg.topbraid.solutions/1.0/schema/glossary
# imports: http://www.w3.org/2004/02/skos/core

@prefix dcterms: <http://purl.org/dc/terms/> .
@prefix edg: <http://edg.topbraid.solutions/model/> .
@prefix hcare: <http://healthcare.edg.topbraid.solutions/hcare/> .
@prefix itil: <http://itil.edg.topbraid.solutions/models/> .
@prefix owl: <http://www.w3.org/2002/07/owl#> .
@prefix rdf: <http://www.w3.org/1999/02/22-rdf-syntax-ns#> .
@prefix rdfs: <http://www.w3.org/2000/01/rdf-schema#> .
@prefix skos: <http://www.w3.org/2004/02/skos/core#> .
@prefix vaem: <http://www.linkedmodel.org/schema/vaem#> .
@prefix xsd: <http://www.w3.org/2001/XMLSchema#> .

<http://itil.edg.topbraid.solutions/models/1.0/glossary>
  rdf:type owl:Ontology ;
  vaem:hasGraphMetadata <http://itil.edg.topbraid.solutions/models/glossary/GMD_glossary> ;
  owl:imports <http://edg.topbraid.solutions/1.0/schema/glossary> ;
  owl:imports <http://www.w3.org/2004/02/skos/core> ;
  owl:versionInfo "Created with TopBraid Composer" ;
.
itil:GlossaryConcept
  rdf:type owl:Class ;
  rdfs:label "ITIL Glossary Term" ;
  rdfs:subClassOf edg:GlossaryTerm ;
  rdfs:subClassOf skos:Concept ;
  skos:prefLabel "ITIL Glossary Term" ;
.
itil:TERM_Acceptance
  rdf:type itil:GlossaryConcept ;
  rdfs:label "Acceptance" ;
  skos:definition "Formal agreement that an IT Service, Process, Plan, or other Deliverable is complete, accurate, Reliable and meets its specified Requirements. Acceptance is usually preceded by Evaluation or Testing and is often required before proceeding to the next stage of a Project or Process. See Service Acceptance Criteria." ;
  skos:prefLabel "Acceptance" ;
.
itil:TERM_Access_Management
  rdf:type itil:GlossaryConcept ;
  rdfs:label "Access Management" ;
  skos:definition "(Service Operation) The Process responsible for allowing Users to make use of IT Services, data, or other Assets. Access Management helps to protect the Confidentiality, Integrity and Availability of Assets by ensuring that only authorized Users are able to access or modify the Assets. Access Management is sometimes referred to as Rights Management or Identity Management." ;
  skos:prefLabel "Access Management" ;
.
itil:TERM_Account_Manager
  rdf:type itil:GlossaryConcept ;
  rdfs:label "Account Manager" ;
  skos:definition "(Service Strategy) A Role that is very similar to Business Relationship Manager, but includes more commercial aspects. Most commonly used when dealing with External Customers." ;
  skos:prefLabel "Account Manager" ;
.
itil:TERM_Accounting
  rdf:type itil:GlossaryConcept ;
  rdfs:label "Accounting" ;
  skos:definition "(Service Strategy) The Process responsible for identifying actual Costs of delivering IT Services, comparing these with budgeted costs, and managing variance from the Budget." ;
  skos:prefLabel "Accounting" ;
.
itil:TERM_Accredited
  rdf:type itil:GlossaryConcept ;
  rdfs:label "Accredited" ;
  skos:definition "Officially authorised to carry out a Role. For example an Accredited body may be authorised to provide training or to conduct Audits." ;
  skos:prefLabel "Accredited" ;
.
itil:TERM_Active_Monitoring
  rdf:type itil:GlossaryConcept ;
  rdfs:label "Active Monitoring" ;
  skos:definition "(Service Operation) Monitoring of a Configuration Item or an IT Service that uses automated regular checks to discover the current status. See Passive Monitoring." ;
  skos:prefLabel "Active Monitoring" ;
.
itil:TERM_Activity
  rdf:type itil:GlossaryConcept ;
  rdfs:label "Activity" ;
  skos:definition "A set of actions designed to achieve a particular result. Activities are usually defined as part of Processes or Plans, and are documented in Procedures." ;
  skos:prefLabel "Activity" ;
.
itil:TERM_Agreed_Service_Time
  rdf:type itil:GlossaryConcept ;
  rdfs:label "Agreed Service Time" ;
  skos:definition "(Service Design) A synonym for Service Hours, commonly used in formal calculations of Availability. See Downtime." ;
  skos:prefLabel "Agreed Service Time" ;
.
itil:TERM_Agreement
  rdf:type itil:GlossaryConcept ;
  rdfs:label "Agreement" ;
  skos:definition "A Document that describes a formal understanding between two or more parties. An Agreement is not legally binding, unless it forms part of a Contract. See Service Level Agreement, Operational Level Agreement." ;
  skos:prefLabel "Agreement" ;
.
itil:TERM_Alert
  rdf:type itil:GlossaryConcept ;
  rdfs:label "Alert" ;
  skos:definition "(Service Operation) A warning that a threshold has been reached, something has changed, or a Failure has occurred. Alerts are often created and managed by System Management tools and are managed by the Event Management Process." ;
  skos:prefLabel "Alert" ;
.
itil:TERM_Analytical_Modelling
  rdf:type itil:GlossaryConcept ;
  rdfs:label "Analytical Modelling" ;
  skos:definition "(Service Strategy) (Service Design) (Continual Service Improvement) A technique that uses mathematical Models to predict the behaviour of a Configuration Item or IT Service. Analytical Models are commonly used in Capacity Management and Availability Management. See Modelling." ;
  skos:prefLabel "Analytical Modelling" ;
.
itil:TERM_Application
  rdf:type itil:GlossaryConcept ;
  rdfs:label "Application" ;
  skos:definition "Software that provides Functions that are required by an IT Service. Each Application may be part of more than one IT Service. An Application runs on one or more Servers or Clients. See Application Management, Application Portfolio." ;
  skos:prefLabel "Application" ;
.
itil:TERM_Application_Management
  rdf:type itil:GlossaryConcept ;
  rdfs:label "Application Management" ;
  skos:definition "(Service Design) (Service Operation) The Function responsible for managing Applications throughout their Lifecycle." ;
  skos:prefLabel "Application Management" ;
.
itil:TERM_Application_Portfolio
  rdf:type itil:GlossaryConcept ;
  rdfs:label "Application Portfolio" ;
  skos:definition "(Service Design) A database or structured Document used to manage Applications throughout their Lifecycle. The Application Portfolio contains key Attributes of all Applications. The Application Portfolio is sometimes implemented as part of the Service Portfolio, or as part of the Configuration Management System." ;
  skos:prefLabel "Application Portfolio" ;
.
itil:TERM_Application_Service_Provider
  rdf:type itil:GlossaryConcept ;
  rdfs:label "Application Service Provider (ASP)" ;
  skos:definition "(Service Design) An External Service Provider that provides IT Services using Applications running at the Service Provider's premises. Users access the Applications by network connections to the Service Provider." ;
  skos:prefLabel "Application Service Provider (ASP)" ;
.
itil:TERM_Application_Sizing
  rdf:type itil:GlossaryConcept ;
  rdfs:label "Application Sizing" ;
  skos:definition "(Service Design) The Activity responsible for understanding the Resource Requirements needed to support a new Application, or a major Change to an existing Application. Application Sizing helps to ensure that the IT Service can meet its agreed Service Level Targets for Capacity and Performance." ;
  skos:prefLabel "Application Sizing" ;
.
itil:TERM_Architecture
  rdf:type itil:GlossaryConcept ;
  rdfs:label "Architecture" ;
  skos:definition "(Service Design) The structure of a System or IT Service, including the Relationships of Components to each other and to the environment they are in. Architecture also includes the Standards and Guidelines which guide the design and evolution of the System." ;
  skos:prefLabel "Architecture" ;
.
itil:TERM_Assembly
  rdf:type itil:GlossaryConcept ;
  rdfs:label "Assembly" ;
  skos:definition "(Service Transition) A Configuration Item that is made up from a number of other CIs. For example a Server CI may contain CIs for CPUs, Disks, Memory etc.; an IT Service CI may contain many Hardware, Software and other CIs. See Component CI, Build." ;
  skos:prefLabel "Assembly" ;
.
itil:TERM_Assessment
  rdf:type itil:GlossaryConcept ;
  rdfs:label "Assessment" ;
  skos:definition "Inspection and analysis to check whether a Standard or set of Guidelines is being followed, that Records are accurate, or that Efficiency and Effectiveness targets are being met. See Audit." ;
  skos:prefLabel "Assessment" ;
.
itil:TERM_Asset
  rdf:type itil:GlossaryConcept ;
  rdfs:label "Asset" ;
  skos:definition "(Service Strategy) Any Resource or Capability. Assets of a Service Provider include anything that could contribute to the delivery of a Service. Assets can be one of the following types: Management, Organisation, Process, Knowledge, People, Information, Applications, Infrastructure, and Financial Capital." ;
  skos:prefLabel "Asset" ;
.
itil:TERM_Asset_Management
  rdf:type itil:GlossaryConcept ;
  rdfs:label "Asset Management" ;
  skos:definition "(Service Transition) Asset Management is the Process responsible for tracking and reporting the value and ownership of financial Assets throughout their Lifecycle. Asset Management is part of an overall Service Asset and Configuration Management Process. See Asset Register." ;
  skos:prefLabel "Asset Management" ;
.
itil:TERM_Asset_Register
  rdf:type itil:GlossaryConcept ;
  rdfs:label "Asset Register" ;
  skos:definition "(Service Transition) A list of Assets, which includes their ownership and value. The Asset Register is maintained by Asset Management." ;
  skos:prefLabel "Asset Register" ;
.
itil:TERM_Attribute
  rdf:type itil:GlossaryConcept ;
  rdfs:label "Attribute" ;
  skos:definition "(Service Transition) A piece of information about a Configuration Item. Examples are name, location, Version number, and Cost. Attributes of CIs are recorded in the Configuration Management Database (CMDB). See Relationship." ;
  skos:prefLabel "Attribute" ;
.
itil:TERM_Audit
  rdf:type itil:GlossaryConcept ;
  rdfs:label "Audit" ;
  skos:definition "Formal inspection and verification to check whether a Standard or set of Guidelines is being followed, that Records are accurate, or that Efficiency and Effectiveness targets are being met. An Audit may be carried out by internal or external groups. See Certification, Assessment." ;
  skos:prefLabel "Audit" ;
.
itil:TERM_Authority_Matrix
  rdf:type itil:GlossaryConcept ;
  rdfs:label "Authority Matrix" ;
  skos:definition "Synonym for RACI." ;
  skos:prefLabel "Authority Matrix" ;
.
itil:TERM_Automatic_Call_Distribution
  rdf:type itil:GlossaryConcept ;
  rdfs:label "Automatic Call Distribution (ACD)" ;
  skos:definition "(Service Operation) Use of Information Technology to direct an incoming telephone call to the most appropriate person in the shortest possible time. ACD is sometimes called Automated Call Distribution." ;
  skos:prefLabel "Automatic Call Distribution (ACD)" ;
.
itil:TERM_Availability
  rdf:type itil:GlossaryConcept ;
  rdfs:label "Availability" ;
  skos:definition "(Service Design) Ability of a Configuration Item or IT Service to perform its agreed Function when required. Availability is determined by Reliability, Maintainability, Serviceability, Performance, and Security. Availability is usually calculated as a percentage. This calculation is often based on Agreed Service Time and Downtime. It is Best Practice to calculate Availability using measurements of the Business output of the IT Service." ;
  skos:prefLabel "Availability" ;
.
itil:TERM_Availability_Management
  rdf:type itil:GlossaryConcept ;
  rdfs:label "Availability Management" ;
  skos:definition "(Service Design) The Process responsible for defining, analysing, Planning, measuring and improving all aspects of the Availability of IT Services. Availability Management is responsible for ensuring that all IT Infrastructure, Processes, Tools, Roles etc are appropriate for the agreed Service Level Targets for Availability." ;
  skos:prefLabel "Availability Management" ;
.
itil:TERM_Availability_Management_Information_System
  rdf:type itil:GlossaryConcept ;
  rdfs:label "Availability Management Information System (AMIS)" ;
  skos:definition "(Service Design) A virtual repository of all Availability Management data, usually stored in multiple physical locations. See Service Knowledge Management System." ;
  skos:prefLabel "Availability Management Information System (AMIS)" ;
.
itil:TERM_Availability_Plan
  rdf:type itil:GlossaryConcept ;
  rdfs:label "Availability Plan" ;
  skos:definition "(Service Design) A Plan to ensure that existing and future Availability Requirements for IT Services can be provided Cost Effectively." ;
  skos:prefLabel "Availability Plan" ;
.
itil:TERM_Back-out
  rdf:type itil:GlossaryConcept ;
  rdfs:label "Back-out" ;
  skos:definition "Synonym for Remediation." ;
  skos:prefLabel "Back-out" ;
.
itil:TERM_Backup
  rdf:type itil:GlossaryConcept ;
  rdfs:label "Backup" ;
  skos:definition "(Service Design) (Service Operation) Copying data to protect against loss of Integrity or Availability of the original." ;
  skos:prefLabel "Backup" ;
.
itil:TERM_Balanced_Scorecard
  rdf:type itil:GlossaryConcept ;
  rdfs:label "Balanced Scorecard" ;
  skos:definition "(Continual Service Improvement) A management tool developed by Drs. Robert Kaplan (Harvard Business School) and David Norton. A Balanced Scorecard enables a Strategy to be broken down into Key Performance Indicators. Performance against the KPIs is used to demonstrate how well the Strategy is being achieved. A Balanced Scorecard has 4 major areas, each of which has a small number of KPIs. The same 4 areas are considered at different levels of detail throughout the Organisation." ;
  skos:prefLabel "Balanced Scorecard" ;
.
itil:TERM_Baseline
  rdf:type itil:GlossaryConcept ;
  rdfs:label "Baseline" ;
  skos:definition "(Continual Service Improvement) A Benchmark used as a reference point. For example: � An ITSM Baseline can be used as a starting point to measure the effect of a Service Improvement Plan � A Performance Baseline can be used to measure changes in Performance over the lifetime of an IT Service � A Configuration Management Baseline can be used to enable the IT Infrastructure to be restored to a known Configuration if a Change or Release fails" ;
  skos:prefLabel "Baseline" ;
.
itil:TERM_Benchmark
  rdf:type itil:GlossaryConcept ;
  rdfs:label "Benchmark" ;
  skos:definition "(Continual Service Improvement) The recorded state of something at a specific point in time. A Benchmark can be created for a Configuration, a Process, or any other set of data. For example, a benchmark can be used in: � Continual Service Improvement, to establish the current state for managing improvements. � Capacity Management, to document Performance characteristics during normal operations. � See Benchmarking, Baseline." ;
  skos:prefLabel "Benchmark" ;
.
itil:TERM_Benchmarking
  rdf:type itil:GlossaryConcept ;
  rdfs:label "Benchmarking" ;
  skos:definition "(Continual Service Improvement) Comparing a Benchmark with a Baseline or with Best Practice. The term Benchmarking is also used to mean creating a series of Benchmarks over time, and comparing the results to measure progress or improvement." ;
  skos:prefLabel "Benchmarking" ;
.
itil:TERM_Best_Practice
  rdf:type itil:GlossaryConcept ;
  rdfs:label "Best Practice" ;
  skos:definition "Proven Activities or Processes that have been successfully used by multiple Organisations. ITIL is an example of Best Practice." ;
  skos:prefLabel "Best Practice" ;
.
itil:TERM_Brainstorming
  rdf:type itil:GlossaryConcept ;
  rdfs:label "Brainstorming" ;
  skos:definition "(Service Design) A technique that helps a team to generate ideas. Ideas are not reviewed during the Brainstorming session, but at a later stage. Brainstorming is often used by Problem Management to identify possible causes." ;
  skos:prefLabel "Brainstorming" ;
.
itil:TERM_British_Standards_Institution
  rdf:type itil:GlossaryConcept ;
  rdfs:label "British Standards Institution (BSI)" ;
  skos:definition "The UK National Standards body, responsible for creating and maintaining British Standards. See http://www.bsi-global.com for more information. See ISO." ;
  skos:prefLabel "British Standards Institution (BSI)" ;
.
itil:TERM_Budget
  rdf:type itil:GlossaryConcept ;
  rdfs:label "Budget" ;
  skos:definition "A list of all the money an Organisation or Business Unit plans to receive, and plans to pay out, over a specified period of time. See Budgeting, Planning." ;
  skos:prefLabel "Budget" ;
.
itil:TERM_Budgeting
  rdf:type itil:GlossaryConcept ;
  rdfs:label "Budgeting" ;
  skos:definition "The Activity of predicting and controlling the spending of money. Consists of a periodic negotiation cycle to set future Budgets (usually annual) and the day-to-day monitoring and adjusting of current Budgets." ;
  skos:prefLabel "Budgeting" ;
.
itil:TERM_Build
  rdf:type itil:GlossaryConcept ;
  rdfs:label "Build" ;
  skos:definition "(Service Transition) The Activity of assembling a number of Configuration Items to create part of an IT Service. The term Build is also used to refer to a Release that is authorised for distribution. For example Server Build or laptop Build. See Configuration Baseline." ;
  skos:prefLabel "Build" ;
.
itil:TERM_Build_Environment
  rdf:type itil:GlossaryConcept ;
  rdfs:label "Build Environment" ;
  skos:definition "(Service Transition) A controlled Environment where Applications, IT Services and other Builds are assembled prior to being moved into a Test or Live Environment." ;
  skos:prefLabel "Build Environment" ;
.
itil:TERM_Business
  rdf:type itil:GlossaryConcept ;
  rdfs:label "Business" ;
  skos:definition "(Service Strategy) An overall corporate entity or Organisation formed of a number of Business Units. In the context of ITSM, the term Business includes public sector and not-for-profit organisations, as well as companies. An IT Service Provider provides IT Services to a Customer within a Business. The IT Service Provider may be part of the same Business as their Customer (Internal Service Provider), or part of another Business (External Service Provider)." ;
  skos:prefLabel "Business" ;
.
itil:TERM_Business_Capacity_Management
  rdf:type itil:GlossaryConcept ;
  rdfs:label "Business Capacity Management (BCM)" ;
  skos:definition "(Service Design) In the context of ITSM, Business Capacity Management is the Activity responsible for understanding future Business Requirements for use in the Capacity Plan. See Service Capacity Management." ;
  skos:prefLabel "Business Capacity Management (BCM)" ;
.
itil:TERM_Business_Case
  rdf:type itil:GlossaryConcept ;
  rdfs:label "Business Case" ;
  skos:definition "(Service Strategy) Justification for a significant item of expenditure. Includes information about Costs, benefits, options, issues, Risks, and possible problems. See Cost Benefit Analysis." ;
  skos:prefLabel "Business Case" ;
.
itil:TERM_Business_Continuity_Management
  rdf:type itil:GlossaryConcept ;
  rdfs:label "Business Continuity Management (BCM)" ;
  skos:definition "(Service Design) The Business Process responsible for managing Risks that could seriously impact the Business. BCM safeguards the interests of key stakeholders, reputation, brand and value creating activities. The BCM Process involves reducing Risks to an acceptable level and planning for the recovery of Business Processes should a disruption to the Business occur. BCM sets the Objectives, Scope and Requirements for IT Service Continuity Management." ;
  skos:prefLabel "Business Continuity Management (BCM)" ;
.
itil:TERM_Business_Continuity_Plan
  rdf:type itil:GlossaryConcept ;
  rdfs:label "Business Continuity Plan (BCP)" ;
  skos:definition "(Service Design) A Plan defining the steps required to Restore Business Processes following a disruption. The Plan will also identify the triggers for Invocation, people to be involved, communications etc. IT Service Continuity Plans form a significant part of Business Continuity Plans." ;
  skos:prefLabel "Business Continuity Plan (BCP)" ;
.
itil:TERM_Business_Customer
  rdf:type itil:GlossaryConcept ;
  rdfs:label "Business Customer" ;
  skos:definition "(Service Strategy) A recipient of a product or a Service from the Business. For example if the Business is a car manufacturer then the Business Customer is someone who buys a car." ;
  skos:prefLabel "Business Customer" ;
.
itil:TERM_Business_Impact_Analysis
  rdf:type itil:GlossaryConcept ;
  rdfs:label "Business Impact Analysis (BIA)" ;
  skos:definition "(Service Strategy) BIA is the Activity in Business Continuity Management that identifies Vital Business Functions and their dependencies. These dependencies may include Suppliers, people, other Business Processes, IT Services etc. BIA defines the recovery requirements for IT Services. These requirements include Recovery Time Objectives, Recovery Point Objectives and minimum Service Level Targets for each IT Service." ;
  skos:prefLabel "Business Impact Analysis (BIA)" ;
.
itil:TERM_Business_Objective
  rdf:type itil:GlossaryConcept ;
  rdfs:label "Business Objective" ;
  skos:definition "(Service Strategy) The Objective of a Business Process, or of the Business as a whole. Business Objectives support the Business Vision, provide guidance for the IT Strategy, and are often supported by IT Services." ;
  skos:prefLabel "Business Objective" ;
.
itil:TERM_Business_Operations
  rdf:type itil:GlossaryConcept ;
  rdfs:label "Business Operations" ;
  skos:definition "(Service Strategy) The day-to-day execution, monitoring and management of Business Processes." ;
  skos:prefLabel "Business Operations" ;
.
itil:TERM_Business_Perspective
  rdf:type itil:GlossaryConcept ;
  rdfs:label "Business Perspective" ;
  skos:definition "(Continual Service Improvement) An understanding of the Service Provider and IT Services from the point of view of the Business, and an understanding of the Business from the point of view of the Service Provider." ;
  skos:prefLabel "Business Perspective" ;
.
itil:TERM_Business_Process
  rdf:type itil:GlossaryConcept ;
  rdfs:label "Business Process" ;
  skos:definition "A Process that is owned and carried out by the Business. A Business Process contributes to the delivery of a product or Service to a Business Customer. For example, a retailer may have a purchasing Process which helps to deliver Services to their Business Customers. Many Business Processes rely on IT Services." ;
  skos:prefLabel "Business Process" ;
.
itil:TERM_Business_Relationship_Management
  rdf:type itil:GlossaryConcept ;
  rdfs:label "Business Relationship Management" ;
  skos:definition "(Service Strategy) The Process or Function responsible for maintaining a Relationship with the Business. BRM usually includes: � Managing personal Relationships with Business managers � Providing input to Service Portfolio Management � Ensuring that the IT Service Provider is satisfying the Business needs of the Customers This Process has strong links with Service Level Management." ;
  skos:prefLabel "Business Relationship Management" ;
.
itil:TERM_Business_Relationship_Manager
  rdf:type itil:GlossaryConcept ;
  rdfs:label "Business Relationship Manager (BRM)" ;
  skos:definition "(Service Strategy) A Role responsible for maintaining the Relationship with one or more Customers. This Role is often combined with the Service Level Manager Role. See Account Manager." ;
  skos:prefLabel "Business Relationship Manager (BRM)" ;
.
itil:TERM_Business_Service
  rdf:type itil:GlossaryConcept ;
  rdfs:label "Business Service" ;
  skos:definition "An IT Service that directly supports a Business Process, as opposed to an Infrastructure Service which is used internally by the IT Service Provider and is not usually visible to the Business. The term Business Service is also used to mean a Service that is delivered to Business Customers by Business Units. For example delivery of financial services to Customers of a bank, or goods to the Customers of a retail store. Successful delivery of Business Services often depends on one or more IT Services." ;
  skos:prefLabel "Business Service" ;
.
itil:TERM_Business_Service_Management
  rdf:type itil:GlossaryConcept ;
  rdfs:label "Business Service Management (BSM)" ;
  skos:definition "(Service Strategy) (Service Design) An approach to the management of IT Services that considers the Business Processes supported and the Business value provided. This term also means the management of Business Services delivered to Business Customers." ;
  skos:prefLabel "Business Service Management (BSM)" ;
.
itil:TERM_Business_Unit
  rdf:type itil:GlossaryConcept ;
  rdfs:label "Business Unit" ;
  skos:definition "(Service Strategy) A segment of the Business which has its own Plans, Metrics, income and Costs. Each Business Unit owns Assets and uses these to create value for Customers in the form of goods and Services." ;
  skos:prefLabel "Business Unit" ;
.
itil:TERM_CI_Type
  rdf:type itil:GlossaryConcept ;
  rdfs:label "CI Type" ;
  skos:definition "(Service Transition) A Category that is used to Classify CIs. The CI Type identifies the required Attributes and Relationships for a Configuration Record. Common CI Types include: hardware, Document, User etc." ;
  skos:prefLabel "CI Type" ;
.
itil:TERM_COBIT
  rdf:type itil:GlossaryConcept ;
  rdfs:label "COBIT" ;
  skos:definition "(Continual Service Improvement) Control Objectives for Information and related Technology (COBIT) provides guidance and Best Practice for the management of IT Processes. COBIT is published by the IT Governance Institute. See http://www.isaca.org/ for more information." ;
  skos:prefLabel "COBIT" ;
.
itil:TERM_CRAMM
  rdf:type itil:GlossaryConcept ;
  rdfs:label "CRAMM" ;
  skos:definition "A methodology and tool for analysing and managing Risks. CRAMM was developed by the UK Government, but is now privately owned. Further information is available from http://www.cramm.com/" ;
  skos:prefLabel "CRAMM" ;
.
itil:TERM_Call
  rdf:type itil:GlossaryConcept ;
  rdfs:label "Call" ;
  skos:definition "(Service Operation) A telephone call to the Service Desk from a User. A Call could result in an Incident or a Service Request being logged." ;
  skos:prefLabel "Call" ;
.
itil:TERM_Call_Centre
  rdf:type itil:GlossaryConcept ;
  rdfs:label "Call Centre" ;
  skos:definition "(Service Operation) An Organisation or Business Unit which handles large numbers of incoming and outgoing telephone calls. See Service Desk." ;
  skos:prefLabel "Call Centre" ;
.
itil:TERM_Call_Type
  rdf:type itil:GlossaryConcept ;
  rdfs:label "Call Type" ;
  skos:definition "(Service Operation) A Category that is used to distinguish incoming requests to a Service Desk. Common Call Types are Incident, Service Request and Complaint." ;
  skos:prefLabel "Call Type" ;
.
itil:TERM_Capability
  rdf:type itil:GlossaryConcept ;
  rdfs:label "Capability" ;
  skos:definition "(Service Strategy) The ability of an Organisation, person, Process, Application, Configuration Item or IT Service to carry out an Activity. Capabilities are intangible Assets of an Organisation. See Resource." ;
  skos:prefLabel "Capability" ;
.
itil:TERM_Capability_Maturity_Model
  rdf:type itil:GlossaryConcept ;
  rdfs:label "Capability Maturity Model (CMM)" ;
  skos:definition "(Continual Service Improvement) The Capability Maturity Model for Software (also known as the CMM and SW-CMM) is a model used to identify Best Practices to help increase Process Maturity. CMM was developed at the Software Engineering Institute (SEI) of Carnegie Mellon University. In 2000, the SW-CMM was upgraded to CMMI� (Capability Maturity Model Integration). The SEI no longer maintains the SW-CMM model, its associated appraisal methods, or training materials." ;
  skos:prefLabel "Capability Maturity Model (CMM)" ;
.
itil:TERM_Capability_Maturity_Model_Integration
  rdf:type itil:GlossaryConcept ;
  rdfs:label "Capability Maturity Model Integration (CMMI)" ;
  skos:definition "(Continual Service Improvement) Capability Maturity Model� Integration (CMMI) is a process improvement approach developed by the Software Engineering Institute (SEI) of Carnegie Melon University. CMMI provides organizations with the essential elements of effective processes. It can be used to guide process improvement across a project, a division, or an entire organization. CMMI helps integrate traditionally separate organizational functions, set process improvement goals and priorities, provide guidance for quality processes, and provide a point of reference for appraising current processes. See http://www.sei.cmu.edu/cmmi/ for more information. See CMM, Continuous Improvement, Maturity." ;
  skos:prefLabel "Capability Maturity Model Integration (CMMI)" ;
.
itil:TERM_Capacity
  rdf:type itil:GlossaryConcept ;
  rdfs:label "Capacity" ;
  skos:definition "(Service Design) The maximum Throughput that a Configuration Item or IT Service can deliver whilst meeting agreed Service Level Targets. For some types of CI, Capacity may be the size or volume, for example a disk drive." ;
  skos:prefLabel "Capacity" ;
.
itil:TERM_Capacity_Management
  rdf:type itil:GlossaryConcept ;
  rdfs:label "Capacity Management" ;
  skos:definition "(Service Design) The Process responsible for ensuring that the Capacity of IT Services and the IT Infrastructure is able to deliver agreed Service Level Targets in a Cost Effective and timely manner. Capacity Management considers all Resources required to deliver the IT Service, and plans for short, medium and long term Business Requirements." ;
  skos:prefLabel "Capacity Management" ;
.
itil:TERM_Capacity_Management_Information_System
  rdf:type itil:GlossaryConcept ;
  rdfs:label "Capacity Management Information System (CMIS)" ;
  skos:definition "(Service Design) A virtual repository of all Capacity Management data, usually stored in multiple physical locations. See Service Knowledge Management System." ;
  skos:prefLabel "Capacity Management Information System (CMIS)" ;
.
itil:TERM_Capacity_Plan
  rdf:type itil:GlossaryConcept ;
  rdfs:label "Capacity Plan" ;
  skos:definition "(Service Design) A Capacity Plan is used to manage the Resources required to deliver IT Services. The Plan contains scenarios for different predictions of Business demand, and costed options to deliver the agreed Service Level Targets." ;
  skos:prefLabel "Capacity Plan" ;
.
itil:TERM_Capacity_Planning
  rdf:type itil:GlossaryConcept ;
  rdfs:label "Capacity Planning" ;
  skos:definition "(Service Design) The Activity within Capacity Management responsible for creating a Capacity Plan." ;
  skos:prefLabel "Capacity Planning" ;
.
itil:TERM_Capital_Expenditure
  rdf:type itil:GlossaryConcept ;
  rdfs:label "Capital Expenditure (CAPEX)" ;
  skos:definition "(Service Strategy) The Cost of purchasing something that will become a financial Asset, for example computer equipment and buildings. The value of the Asset is Depreciated over multiple accounting periods." ;
  skos:prefLabel "Capital Expenditure (CAPEX)" ;
.
itil:TERM_Capital_Item
  rdf:type itil:GlossaryConcept ;
  rdfs:label "Capital Item" ;
  skos:definition "(Service Strategy) An Asset that is of interest to Financial Management because it is above an agreed financial value." ;
  skos:prefLabel "Capital Item" ;
.
itil:TERM_Capitalization
  rdf:type itil:GlossaryConcept ;
  rdfs:label "Capitalization" ;
  skos:definition "(Service Strategy) Identifying major Cost as capital, even though no Asset is purchased. This is done to spread the impact of the Cost over multiple accounting periods. The most common example of this is software development, or purchase of a software license." ;
  skos:prefLabel "Capitalization" ;
.
itil:TERM_Category
  rdf:type itil:GlossaryConcept ;
  rdfs:label "Category" ;
  skos:definition "A named group of things that have something in common. Categories are used to group similar things together. For example Cost Types are used to group similar types of Cost. Incident Categories are used to group similar types of Incident, CI Types are used to group similar types of Configuration Item." ;
  skos:prefLabel "Category" ;
.
itil:TERM_Certification
  rdf:type itil:GlossaryConcept ;
  rdfs:label "Certification" ;
  skos:definition "Issuing a certificate to confirm Compliance to a Standard. Certification includes a formal Audit by an independent and Accredited body. The term Certification is also used to mean awarding a certificate to verify that a person has achieved a qualification." ;
  skos:prefLabel "Certification" ;
.
itil:TERM_Change
  rdf:type itil:GlossaryConcept ;
  rdfs:label "Change" ;
  skos:definition "(Service Transition) The addition, modification or removal of anything that could have an effect on IT Services. The Scope should include all IT Services, Configuration Items, Processes, Documentation etc." ;
  skos:prefLabel "Change" ;
.
itil:TERM_Change_Advisory_Board
  rdf:type itil:GlossaryConcept ;
  rdfs:label "Change Advisory Board (CAB)" ;
  skos:definition "(Service Transition) A group of people that advises the Change Manager in the Assessment, prioritisation and scheduling of Changes. This board is usually made up of representatives from all areas within the IT Service Provider, the Business, and Third Parties such as Suppliers." ;
  skos:prefLabel "Change Advisory Board (CAB)" ;
.
itil:TERM_Change_Case
  rdf:type itil:GlossaryConcept ;
  rdfs:label "Change Case" ;
  skos:definition "(Service Operation) A technique used to predict the impact of proposed Changes. Change Cases use specific scenarios to clarify the scope of proposed Changes and to help with Cost Benefit Analysis. See Use Case." ;
  skos:prefLabel "Change Case" ;
.
itil:TERM_Change_History
  rdf:type itil:GlossaryConcept ;
  rdfs:label "Change History" ;
  skos:definition "(Service Transition) Information about all changes made to a Configuration Item during its life. Change History consists of all those Change Records that apply to the CI." ;
  skos:prefLabel "Change History" ;
.
itil:TERM_Change_Management
  rdf:type itil:GlossaryConcept ;
  rdfs:label "Change Management" ;
  skos:definition "(Service Transition) The Process responsible for controlling the Lifecycle of all Changes. The primary objective of Change Management is to enable beneficial Changes to be made, with minimum disruption to IT Services." ;
  skos:prefLabel "Change Management" ;
.
itil:TERM_Change_Model
  rdf:type itil:GlossaryConcept ;
  rdfs:label "Change Model" ;
  skos:definition "(Service Transition) A repeatable way of dealing with a particular Category of Change. A Change Model defines specific pre-defined steps that will be followed for a Change of this Category. Change Models may be very simple, with no requirement for approval (e.g. Password Reset) or may be very complex with many steps that require approval (e.g. major software Release). See Standard Change, Change Advisory Board." ;
  skos:prefLabel "Change Model" ;
.
itil:TERM_Change_Record
  rdf:type itil:GlossaryConcept ;
  rdfs:label "Change Record" ;
  skos:definition "(Service Transition) A Record containing the details of a Change. Each Change Record documents the Lifecycle of a single Change. A Change Record is created for every Request for Change that is received, even those that are subsequently rejected. Change Records should reference the Configuration Items that are affected by the Change. Change Records are stored in the Configuration Management System." ;
  skos:prefLabel "Change Record" ;
.
itil:TERM_Change_Request
  rdf:type itil:GlossaryConcept ;
  rdfs:label "Change Request" ;
  skos:definition "Synonym for Request for Change." ;
  skos:prefLabel "Change Request" ;
.
itil:TERM_Change_Schedule
  rdf:type itil:GlossaryConcept ;
  rdfs:label "Change Schedule" ;
  skos:definition "(Service Transition) A Document that lists all approved Changes and their planned implementation dates. A Change Schedule is sometimes called a Forward Schedule of Change, even though it also contains information about Changes that have already been implemented." ;
  skos:prefLabel "Change Schedule" ;
.
itil:TERM_Change_Window
  rdf:type itil:GlossaryConcept ;
  rdfs:label "Change Window" ;
  skos:definition "(Service Transition) A regular, agreed time when Changes or Releases may be implemented with minimal impact on Services. Change Windows are usually documented in SLAs." ;
  skos:prefLabel "Change Window" ;
.
itil:TERM_Charging
  rdf:type itil:GlossaryConcept ;
  rdfs:label "Charging" ;
  skos:definition "(Service Strategy) Requiring payment for IT Services. Charging for IT Services is optional, and many Organisations choose to treat their IT Service Provider as a Cost Centre." ;
  skos:prefLabel "Charging" ;
.
itil:TERM_Chronological_Analysis
  rdf:type itil:GlossaryConcept ;
  rdfs:label "Chronological Analysis" ;
  skos:definition "(Service Operation) A technique used to help identify possible causes of Problems. All available data about the Problem is collected and sorted by date and time to provide a detailed timeline. This can make it possible to identify which Events may have been triggered by others." ;
  skos:prefLabel "Chronological Analysis" ;
.
itil:TERM_Classification
  rdf:type itil:GlossaryConcept ;
  rdfs:label "Classification" ;
  skos:definition "The act of assigning a Category to something. Classification is used to ensure consistent management and reporting. CIs, Incidents, Problems, Changes etc. are usually classified." ;
  skos:prefLabel "Classification" ;
.
itil:TERM_Client
  rdf:type itil:GlossaryConcept ;
  rdfs:label "Client" ;
  skos:definition "A generic term that means a Customer, the Business or a Business Customer. For example Client Manager may be used as a synonym for Account Manager. The term client is also used to mean: � A computer that is used directly by a User, for example a PC, Handheld Computer, or Workstation. � The part of a Client-Server Application that the User directly interfaces with. For example an email Client" ;
  skos:prefLabel "Client" ;
.
itil:TERM_Closed
  rdf:type itil:GlossaryConcept ;
  rdfs:label "Closed" ;
  skos:definition "(Service Operation) The final Status in the Lifecycle of an Incident, Problem, Change etc. When the Status is Closed, no further action is taken." ;
  skos:prefLabel "Closed" ;
.
itil:TERM_Closure
  rdf:type itil:GlossaryConcept ;
  rdfs:label "Closure" ;
  skos:definition "(Service Operation) The act of changing the Status of an Incident, Problem, Change etc. to Closed." ;
  skos:prefLabel "Closure" ;
.
itil:TERM_Code_of_Practice
  rdf:type itil:GlossaryConcept ;
  rdfs:label "Code of Practice" ;
  skos:definition "A Guideline published by a public body or a Standards Organisation, such as ISO or BSI. Many Standards consist of a Code of Practice and a Specification. The Code of Practice describes recommended Best Practice." ;
  skos:prefLabel "Code of Practice" ;
.
itil:TERM_Cold_Standby
  rdf:type itil:GlossaryConcept ;
  rdfs:label "Cold Standby" ;
  skos:definition "Synonym for Gradual Recovery." ;
  skos:prefLabel "Cold Standby" ;
.
itil:TERM_Commercial_off_the_Shelf
  rdf:type itil:GlossaryConcept ;
  rdfs:label "Commercial off the Shelf (COTS)" ;
  skos:definition "(Service Design) Application software or Middleware that can be purchased from a Third Party." ;
  skos:prefLabel "Commercial off the Shelf (COTS)" ;
.
itil:TERM_Compliance
  rdf:type itil:GlossaryConcept ;
  rdfs:label "Compliance" ;
  skos:definition "Ensuring that a Standard or set of Guidelines is followed, or that proper, consistent accounting or other practices are being employed." ;
  skos:prefLabel "Compliance" ;
.
itil:TERM_Component
  rdf:type itil:GlossaryConcept ;
  rdfs:label "Component" ;
  skos:definition "A general term that is used to mean one part of something more complex. For example, a computer System may be a component of an IT Service, an Application may be a Component of a Release Unit. Components that need to be managed should be Configuration Items." ;
  skos:prefLabel "Component" ;
.
itil:TERM_Component_CI
  rdf:type itil:GlossaryConcept ;
  rdfs:label "Component CI" ;
  skos:definition "(Service Transition) A Configuration Item that is part of an Assembly. For example, a CPU or Memory CI may be part of a Server CI." ;
  skos:prefLabel "Component CI" ;
.
itil:TERM_Component_Capacity_Management
  rdf:type itil:GlossaryConcept ;
  rdfs:label "Component Capacity Management (CCM)" ;
  skos:definition "(Service Design) (Continual Service Improvement) The Process responsible for understanding the Capacity, Utilisation, and Performance of Configuration Items. Data is collected, recorded and analysed for use in the Capacity Plan. See Service Capacity Management." ;
  skos:prefLabel "Component Capacity Management (CCM)" ;
.
itil:TERM_Component_Failure_Impact_Analysis
  rdf:type itil:GlossaryConcept ;
  rdfs:label "Component Failure Impact Analysis (CFIA)" ;
  skos:definition "(Service Design) A technique that helps to identify the impact of CI failure on IT Services. A matrix is created with IT Services on one edge and CIs on the other. This enables the identification of critical CIs (that could cause the failure of multiple IT Services) and of fragile IT Services (that have multiple Single Points of Failure)." ;
  skos:prefLabel "Component Failure Impact Analysis (CFIA)" ;
.
itil:TERM_Computer_Telephony_Integration
  rdf:type itil:GlossaryConcept ;
  rdfs:label "Computer Telephony Integration (CTI)" ;
  skos:definition "(Service Operation) CTI is a general term covering any kind of integration between computers and telephone Systems. It is most commonly used to refer to Systems where an Application displays detailed screens relating to incoming or outgoing telephone calls. See Automatic Call Distribution, Interactive Voice Response." ;
  skos:prefLabel "Computer Telephony Integration (CTI)" ;
.
itil:TERM_Concurrency
  rdf:type itil:GlossaryConcept ;
  rdfs:label "Concurrency" ;
  skos:definition "A measure of the number of Users engaged in the same Operation at the same time." ;
  skos:prefLabel "Concurrency" ;
.
itil:TERM_Confidentiality
  rdf:type itil:GlossaryConcept ;
  rdfs:label "Confidentiality" ;
  skos:definition "(Service Design) A security principle that requires that data should only be accessed by authorised people." ;
  skos:prefLabel "Confidentiality" ;
.
itil:TERM_Configuration
  rdf:type itil:GlossaryConcept ;
  rdfs:label "Configuration" ;
  skos:definition "(Service Transition) A generic term, used to describe a group of Configuration Items that work together to deliver an IT Service, or a recognizable part of an IT Service. Configuration is also used to describe the parameter settings for one or more CIs." ;
  skos:prefLabel "Configuration" ;
.
itil:TERM_Configuration_Baseline
  rdf:type itil:GlossaryConcept ;
  rdfs:label "Configuration Baseline" ;
  skos:definition "(Service Transition) A Baseline of a Configuration that has been formally agreed and is managed through the Change Management process. A Configuration Baseline is used as a basis for future Builds, Releases and Changes." ;
  skos:prefLabel "Configuration Baseline" ;
.
itil:TERM_Configuration_Control
  rdf:type itil:GlossaryConcept ;
  rdfs:label "Configuration Control" ;
  skos:definition "(Service Transition) The Activity responsible for ensuring that adding, modifying or removing a CI is properly managed, for example by submitting a Request for Change or Service Request." ;
  skos:prefLabel "Configuration Control" ;
.
itil:TERM_Configuration_Identification
  rdf:type itil:GlossaryConcept ;
  rdfs:label "Configuration Identification" ;
  skos:definition "(Service Transition) The Activity responsible for collecting information about Configuration Items and their Relationships, and loading this information into the CMDB. Configuration Identification is also responsible for labelling the CIs themselves, so that the corresponding Configuration Records can be found." ;
  skos:prefLabel "Configuration Identification" ;
.
itil:TERM_Configuration_Item
  rdf:type itil:GlossaryConcept ;
  rdfs:label "Configuration Item (CI)" ;
  skos:definition "(Service Transition) Any Component that needs to be managed in order to deliver an IT Service. Information about each CI is recorded in a Configuration Record within the Configuration Management System and is maintained throughout its Lifecycle by Configuration Management. CIs are under the control of Change Management. CIs typically include IT Services, hardware, software, buildings, people, and formal documentation such as Process documentation and SLAs." ;
  skos:prefLabel "Configuration Item (CI)" ;
.
itil:TERM_Configuration_Management
  rdf:type itil:GlossaryConcept ;
  rdfs:label "Configuration Management" ;
  skos:definition "(Service Transition) The Process responsible for maintaining information about Configuration Items required to deliver an IT Service, including their Relationships. This information is managed throughout the Lifecycle of the CI. Configuration Management is part of an overall Service Asset and Configuration Management Process." ;
  skos:prefLabel "Configuration Management" ;
.
itil:TERM_Configuration_Management_Database
  rdf:type itil:GlossaryConcept ;
  rdfs:label "Configuration Management Database (CMDB)" ;
  skos:definition "(Service Transition) A database used to store Configuration Records throughout their Lifecycle. The Configuration Management System maintains one or more CMDBs, and each CMDB stores Attributes of CIs, and Relationships with other CIs." ;
  skos:prefLabel "Configuration Management Database (CMDB)" ;
.
itil:TERM_Configuration_Management_System
  rdf:type itil:GlossaryConcept ;
  rdfs:label "Configuration Management System (CMS)" ;
  skos:definition "(Service Transition) A set of tools and databases that are used to manage an IT Service Provider's Configuration data. The CMS also includes information about Incidents, Problems, Known Errors, Changes and Releases; and may contain data about employees, Suppliers, locations, Business Units, Customers and Users. The CMS includes tools for collecting, storing, managing, updating, and presenting data about all Configuration Items and their Relationships. The CMS is maintained by Configuration Management and is used by all IT Service Management Processes. See Configuration Management Database, Service Knowledge Management System." ;
  skos:prefLabel "Configuration Management System (CMS)" ;
.
itil:TERM_Configuration_Record
  rdf:type itil:GlossaryConcept ;
  rdfs:label "Configuration Record" ;
  skos:definition "(Service Transition) A Record containing the details of a Configuration Item. Each Configuration Record documents the Lifecycle of a single CI. Configuration Records are stored in a Configuration Management Database." ;
  skos:prefLabel "Configuration Record" ;
.
itil:TERM_Configuration_Structure
  rdf:type itil:GlossaryConcept ;
  rdfs:label "Configuration Structure" ;
  skos:definition "(Service Transition) The hierarchy and other Relationships between all the Configuration Items that comprise a Configuration." ;
  skos:prefLabel "Configuration Structure" ;
.
itil:TERM_Continual_Service_Improvement
  rdf:type itil:GlossaryConcept ;
  rdfs:label "Continual Service Improvement (CSI)" ;
  skos:definition "(Continual Service Improvement) A stage in the Lifecycle of an IT Service and the title of one of the Core ITIL publications. Continual Service Improvement is responsible for managing improvements to IT Service Management Processes and IT Services. The Performance of the IT Service Provider is continually measured and improvements are made to Processes, IT Services and IT Infrastructure in order to increase Efficiency, Effectiveness, and Cost Effectiveness. See Plan-Do-Check-Act." ;
  skos:prefLabel "Continual Service Improvement (CSI)" ;
.
itil:TERM_Continuous_Availability
  rdf:type itil:GlossaryConcept ;
  rdfs:label "Continuous Availability" ;
  skos:definition "(Service Design) An approach or design to achieve 100% Availability. A Continuously Available IT Service has no planned or unplanned Downtime." ;
  skos:prefLabel "Continuous Availability" ;
.
itil:TERM_Continuous_Operation
  rdf:type itil:GlossaryConcept ;
  rdfs:label "Continuous Operation" ;
  skos:definition "(Service Design) An approach or design to eliminate planned Downtime of an IT Service. Note that individual Configuration Items may be down even though the IT Service is Available." ;
  skos:prefLabel "Continuous Operation" ;
.
itil:TERM_Contract
  rdf:type itil:GlossaryConcept ;
  rdfs:label "Contract" ;
  skos:definition "A legally binding Agreement between two or more parties." ;
  skos:prefLabel "Contract" ;
.
itil:TERM_Contract_Portfolio
  rdf:type itil:GlossaryConcept ;
  rdfs:label "Contract Portfolio" ;
  skos:definition "(Service Strategy) A database or structured Document used to manage Service Contracts or Agreements between an IT Service Provider and their Customers. Each IT Service delivered to a Customer should have a Contract or other Agreement which is listed in the Contract Portfolio. See Service Portfolio, Service Catalogue." ;
  skos:prefLabel "Contract Portfolio" ;
.
itil:TERM_Control
  rdf:type itil:GlossaryConcept ;
  rdfs:label "Control" ;
  skos:definition "A means of managing a Risk, ensuring that a Business Objective is achieved, or ensuring that a Process is followed. Example Controls include Policies, Procedures, Roles, RAID, door-locks etc. A control is sometimes called a Countermeasure or safeguard. Control also means to manage the utilization or behaviour of a Configuration Item, System or IT Service." ;
  skos:prefLabel "Control" ;
.
itil:TERM_Control_Objectives_for_Information_and_related_Technology
  rdf:type itil:GlossaryConcept ;
  rdfs:label "Control Objectives for Information and related Technology (COBIT)" ;
  skos:definition "See COBIT." ;
  skos:prefLabel "Control Objectives for Information and related Technology (COBIT)" ;
.
itil:TERM_Control_Processes
  rdf:type itil:GlossaryConcept ;
  rdfs:label "Control Processes" ;
  skos:definition "The ISO/IEC 20000 Process group that includes Change Management and Configuration Management." ;
  skos:prefLabel "Control Processes" ;
.
itil:TERM_Control_perspective
  rdf:type itil:GlossaryConcept ;
  rdfs:label "Control perspective" ;
  skos:definition "(Service Strategy) An approach to the management of IT Services, Processes, Functions, Assets etc. There can be several different Control Perspectives on the same IT Service, Process etc., allowing different individuals or teams to focus on what is important and relevant to their specific Role. Example Control Perspectives include Reactive and Proactive management within IT Operations, or a Lifecycle view for an Application Project team." ;
  skos:prefLabel "Control perspective" ;
.
itil:TERM_Core_Service
  rdf:type itil:GlossaryConcept ;
  rdfs:label "Core Service" ;
  skos:definition "(Service Strategy) An IT Service that delivers basic Outcomes desired by one or more Customers. See Supporting Service, Core Service Package." ;
  skos:prefLabel "Core Service" ;
.
itil:TERM_Core_Service_Package
  rdf:type itil:GlossaryConcept ;
  rdfs:label "Core Service Package (CSP)" ;
  skos:definition "(Service Strategy) A detailed description of a Core Service that may be shared by two or more Service Level Packages. See Service Package." ;
  skos:prefLabel "Core Service Package (CSP)" ;
.
itil:TERM_Cost
  rdf:type itil:GlossaryConcept ;
  rdfs:label "Cost" ;
  skos:definition "The amount of money spent on a specific Activity, IT Service, or Business Unit. Costs consist of real cost (money), notional cost such as people's time, and Depreciation." ;
  skos:prefLabel "Cost" ;
.
itil:TERM_Cost_Benefit_Analysis
  rdf:type itil:GlossaryConcept ;
  rdfs:label "Cost Benefit Analysis" ;
  skos:definition "An Activity that analyses and compares the Costs and the benefits involved in one or more alternative courses of action. See Business Case, Net Present Value, Internal Rate of Return, Return on Investment, Value on Investment." ;
  skos:prefLabel "Cost Benefit Analysis" ;
.
itil:TERM_Cost_Centre
  rdf:type itil:GlossaryConcept ;
  rdfs:label "Cost Centre" ;
  skos:definition "(Service Strategy) A Business Unit or Project to which Costs are assigned. A Cost Centre does not charge for Services provided. An IT Service Provider can be run as a Cost Centre or a Profit Centre." ;
  skos:prefLabel "Cost Centre" ;
.
itil:TERM_Cost_Effectiveness
  rdf:type itil:GlossaryConcept ;
  rdfs:label "Cost Effectiveness" ;
  skos:definition "A measure of the balance between the Effectiveness and Cost of a Service, Process or activity, A Cost Effective Process is one which achieves its Objectives at minimum Cost. See KPI, Return on Investment, Value for Money." ;
  skos:prefLabel "Cost Effectiveness" ;
.
itil:TERM_Cost_Element
  rdf:type itil:GlossaryConcept ;
  rdfs:label "Cost Element" ;
  skos:definition "(Service Strategy) The middle level of category to which Costs are assigned in Budgeting and Accounting. The highest level category is Cost Type. For example a Cost Type of �people� could have cost elements of payroll, staff benefits, expenses, training, overtime etc. Cost Elements can be further broken down to give Cost Units. For example the Cost Element �expenses� could include Cost Units of Hotels, Transport, Meals etc." ;
  skos:prefLabel "Cost Element" ;
.
itil:TERM_Cost_Management
  rdf:type itil:GlossaryConcept ;
  rdfs:label "Cost Management" ;
  skos:definition "(Service Strategy) A general term that is used to refer to Budgeting and Accounting, sometimes used as a synonym for Financial Management" ;
  skos:prefLabel "Cost Management" ;
.
itil:TERM_Cost_Type
  rdf:type itil:GlossaryConcept ;
  rdfs:label "Cost Type" ;
  skos:definition "(Service Strategy) The highest level of category to which Costs are assigned in Budgeting and Accounting. For example hardware, software, people, accommodation, external and Transfer. See Cost Element, Cost Type." ;
  skos:prefLabel "Cost Type" ;
.
itil:TERM_Cost_Unit
  rdf:type itil:GlossaryConcept ;
  rdfs:label "Cost Unit" ;
  skos:definition "(Service Strategy) The lowest level of category to which Costs are assigned, Cost Units are usually things that can be easily counted (e.g. staff numbers, software licences) or things easily measured (e.g. CPU usage, Electricity consumed). Cost Units are included within Cost Elements. For example a Cost Element of �expenses� could include Cost Units of Hotels, Transport, Meals etc. See Cost Type." ;
  skos:prefLabel "Cost Unit" ;
.
itil:TERM_Countermeasure
  rdf:type itil:GlossaryConcept ;
  rdfs:label "Countermeasure" ;
  skos:definition "Can be used to refer to any type of Control. The term Countermeasure is most often used when referring to measures that increase Resilience, Fault Tolerance or Reliability of an IT Service." ;
  skos:prefLabel "Countermeasure" ;
.
itil:TERM_Course_Corrections
  rdf:type itil:GlossaryConcept ;
  rdfs:label "Course Corrections" ;
  skos:definition "Changes made to a Plan or Activity that has already started, to ensure that it will meet its Objectives. Course corrections are made as a result of Monitoring progress." ;
  skos:prefLabel "Course Corrections" ;
.
itil:TERM_Crisis_Management
  rdf:type itil:GlossaryConcept ;
  rdfs:label "Crisis Management" ;
  skos:definition "The Process responsible for managing the wider implications of Business Continuity. A Crisis Management team is responsible for Strategic issues such as managing media relations and shareholder confidence, and decides when to invoke Business Continuity Plans." ;
  skos:prefLabel "Crisis Management" ;
.
itil:TERM_Critical_Success_Factor
  rdf:type itil:GlossaryConcept ;
  rdfs:label "Critical Success Factor (CSF)" ;
  skos:definition "Something that must happen if a Process, Project, Plan, or IT Service is to succeed. KPIs are used to measure the achievement of each CSF. For example a CSF of \"protect IT Services when making Changes\" could be measured by KPIs such as \"percentage reduction of unsuccessful Changes\", \"percentage reduction in Changes causing Incidents\" etc." ;
  skos:prefLabel "Critical Success Factor (CSF)" ;
.
itil:TERM_Culture
  rdf:type itil:GlossaryConcept ;
  rdfs:label "Culture" ;
  skos:definition "A set of values that is shared by a group of people, including expectations about how people should behave, ideas, beliefs, and practices. See Vision." ;
  skos:prefLabel "Culture" ;
.
itil:TERM_Customer
  rdf:type itil:GlossaryConcept ;
  rdfs:label "Customer" ;
  skos:definition "Someone who buys goods or Services. The Customer of an IT Service Provider is the person or group who defines and agrees the Service Level Targets. The term Customers is also sometimes informally used to mean Users, for example \"this is a Customer focussed Organisation\"." ;
  skos:prefLabel "Customer" ;
.
itil:TERM_Customer_Portfolio
  rdf:type itil:GlossaryConcept ;
  rdfs:label "Customer Portfolio" ;
  skos:definition "(Service Strategy) A database or structured Document used to record all Customers of the IT Service Provider. The Customer Portfolio is the Business Relationship Manager's view of the Customers who receive Services from the IT Service Provider. See Contract Portfolio, Service Portfolio." ;
  skos:prefLabel "Customer Portfolio" ;
.
itil:TERM_Dashboard
  rdf:type itil:GlossaryConcept ;
  rdfs:label "Dashboard" ;
  skos:definition "(Service Operation) A graphical representation of overall IT Service Performance and Availability. Dashboard images may be updated in real-time, and can also be included in management reports and web pages. Dashboards can be used to support Service Level Management, Event Management or Incident Diagnosis." ;
  skos:prefLabel "Dashboard" ;
.
itil:TERM_Data-to-_Information-to-_Knowledge-to-_Wisdom
  rdf:type itil:GlossaryConcept ;
  rdfs:label "Data-to- Information-to- Knowledge-to- Wisdom (DIKW)" ;
  skos:definition "A way of understanding the relationships between data, information, knowledge, and wisdom. DIKW shows how each of these builds on the others." ;
  skos:prefLabel "Data-to- Information-to- Knowledge-to- Wisdom (DIKW)" ;
.
itil:TERM_Definitive_Media_Library
  rdf:type itil:GlossaryConcept ;
  rdfs:label "Definitive Media Library (DML)" ;
  skos:definition "(Service Transition) One or more locations in which the definitive and approved versions of all software Configuration Items are securely stored. The DML may also contain associated CIs such as licenses and documentation. The DML is a single logical storage area even if there are multiple locations. All software in the DML is under the control of Change and Release Management and is recorded in the Configuration Management System. Only software from the DML is acceptable for use in a Release." ;
  skos:prefLabel "Definitive Media Library (DML)" ;
.
itil:TERM_Deliverable
  rdf:type itil:GlossaryConcept ;
  rdfs:label "Deliverable" ;
  skos:definition "Something that must be provided to meet a commitment in a Service Level Agreement or a Contract. Deliverable is also used in a more informal way to mean a planned output of any Process." ;
  skos:prefLabel "Deliverable" ;
.
itil:TERM_Demand_Management
  rdf:type itil:GlossaryConcept ;
  rdfs:label "Demand Management" ;
  skos:definition "Activities that understand and influence Customer demand for Services and the provision of Capacity to meet these demands. At a Strategic level Demand Management can involve analysis of Patterns of Business Activity and User Profiles. At a Tactical level it can involve use of Differential Charging to encourage Customers to use IT Services at less busy times. See Capacity Management." ;
  skos:prefLabel "Demand Management" ;
.
itil:TERM_Deming_Cycle
  rdf:type itil:GlossaryConcept ;
  rdfs:label "Deming Cycle" ;
  skos:definition "Synonym for Plan Do Check Act." ;
  skos:prefLabel "Deming Cycle" ;
.
itil:TERM_Dependency
  rdf:type itil:GlossaryConcept ;
  rdfs:label "Dependency" ;
  skos:definition "The direct or indirect reliance of one Process or Activity upon another." ;
  skos:prefLabel "Dependency" ;
.
itil:TERM_Deployment
  rdf:type itil:GlossaryConcept ;
  rdfs:label "Deployment" ;
  skos:definition "(Service Transition) The Activity responsible for movement of new or changed hardware, software, documentation, Process, etc to the Live Environment. Deployment is part of the Release and Deployment Management Process. See Rollout." ;
  skos:prefLabel "Deployment" ;
.
itil:TERM_Depreciation
  rdf:type itil:GlossaryConcept ;
  rdfs:label "Depreciation" ;
  skos:definition "(Service Strategy) A measure of the reduction in value of an Asset over its life. This is based on wearing out, consumption or other reduction in the useful economic value." ;
  skos:prefLabel "Depreciation" ;
.
itil:TERM_Design
  rdf:type itil:GlossaryConcept ;
  rdfs:label "Design" ;
  skos:definition "(Service Design) An Activity or Process that identifies Requirements and then defines a solution that is able to meet these Requirements. See Service Design." ;
  skos:prefLabel "Design" ;
.
itil:TERM_Detection
  rdf:type itil:GlossaryConcept ;
  rdfs:label "Detection" ;
  skos:definition "(Service Operation) A stage in the Incident Lifecycle. Detection results in the Incident becoming known to the Service Provider. Detection can be automatic, or can be the result of a User logging an Incident." ;
  skos:prefLabel "Detection" ;
.
itil:TERM_Development
  rdf:type itil:GlossaryConcept ;
  rdfs:label "Development" ;
  skos:definition "(Service Design) The Process responsible for creating or modifying an IT Service or Application. Also used to mean the Role or group that carries out Development work." ;
  skos:prefLabel "Development" ;
.
itil:TERM_Development_Environment
  rdf:type itil:GlossaryConcept ;
  rdfs:label "Development Environment" ;
  skos:definition "(Service Design) An Environment used to create or modify IT Services or Applications. Development Environments are not typically subjected to the same degree of control as Test Environments or Live Environments. See Development." ;
  skos:prefLabel "Development Environment" ;
.
itil:TERM_Diagnosis
  rdf:type itil:GlossaryConcept ;
  rdfs:label "Diagnosis" ;
  skos:definition "(Service Operation) A stage in the Incident and Problem Lifecycles. The purpose of Diagnosis is to identify a Workaround for an Incident or the Root Cause of a Problem." ;
  skos:prefLabel "Diagnosis" ;
.
itil:TERM_Diagnostic_Script
  rdf:type itil:GlossaryConcept ;
  rdfs:label "Diagnostic Script" ;
  skos:definition "(Service Operation) A structured set of questions used by Service Desk staff to ensure they ask the correct questions, and to help them Classify, Resolve and assign Incidents. Diagnostic Scripts may also be made available to Users to help them diagnose and resolve their own Incidents." ;
  skos:prefLabel "Diagnostic Script" ;
.
itil:TERM_Differential_Charging
  rdf:type itil:GlossaryConcept ;
  rdfs:label "Differential Charging" ;
  skos:definition "A technique used to support Demand Management by charging different amounts for the same IT Service Function at different times." ;
  skos:prefLabel "Differential Charging" ;
.
itil:TERM_Direct_Cost
  rdf:type itil:GlossaryConcept ;
  rdfs:label "Direct Cost" ;
  skos:definition "(Service Strategy) A cost of providing an IT Service which can be allocated in full to a specific Customer, Cost Centre, Project etc. For example cost of providing non-shared servers or software licenses. See Indirect Cost." ;
  skos:prefLabel "Direct Cost" ;
.
itil:TERM_Directory_Service
  rdf:type itil:GlossaryConcept ;
  rdfs:label "Directory Service" ;
  skos:definition "(Service Operation) An Application that manages information about IT Infrastructure available on a network, and corresponding User access Rights." ;
  skos:prefLabel "Directory Service" ;
.
itil:TERM_Do_Nothing
  rdf:type itil:GlossaryConcept ;
  rdfs:label "Do Nothing" ;
  skos:definition "(Service Design) A Recovery Option. The Service Provider formally agrees with the Customer that Recovery of this IT Service will not be performed." ;
  skos:prefLabel "Do Nothing" ;
.
itil:TERM_Document
  rdf:type itil:GlossaryConcept ;
  rdfs:label "Document" ;
  skos:definition "Information in readable form. A Document may be paper or electronic. For example a Policy statement, Service Level Agreement, Incident Record, diagram of computer room layout. See Record." ;
  skos:prefLabel "Document" ;
.
itil:TERM_Downtime
  rdf:type itil:GlossaryConcept ;
  rdfs:label "Downtime" ;
  skos:definition "(Service Design) (Service Operation) The time when a Configuration Item or IT Service is not Available during its Agreed Service Time. The Availability of an IT Service is often calculated from Agreed Service Time and Downtime." ;
  skos:prefLabel "Downtime" ;
.
itil:TERM_Driver
  rdf:type itil:GlossaryConcept ;
  rdfs:label "Driver" ;
  skos:definition "Something that influences Strategy, Objectives or Requirements. For example new legislation or the actions of competitors." ;
  skos:prefLabel "Driver" ;
.
itil:TERM_Early_Life_Support
  rdf:type itil:GlossaryConcept ;
  rdfs:label "Early Life Support" ;
  skos:definition "(Service Transition) Support provided for a new or Changed IT Service for a period of time after it is Released. During Early Life Support the IT Service Provider may review the KPIs, Service Levels and Monitoring Thresholds, and provide additional Resources for Incident and Problem Management." ;
  skos:prefLabel "Early Life Support" ;
.
itil:TERM_Economies_of_scale
  rdf:type itil:GlossaryConcept ;
  rdfs:label "Economies of scale" ;
  skos:definition "(Service Strategy) The reduction in average Cost that is possible from increasing the usage of an IT Service or Asset. See Economies of Scope." ;
  skos:prefLabel "Economies of scale" ;
.
itil:TERM_Economies_of_scope
  rdf:type itil:GlossaryConcept ;
  rdfs:label "Economies of scope" ;
  skos:definition "(Service Strategy) The reduction in Cost that is allocated to an IT Service by using an existing Asset for an additional purpose. For example delivering a new IT Service from existing IT Infrastructure. See Economies of Scale." ;
  skos:prefLabel "Economies of scope" ;
.
itil:TERM_Effectiveness
  rdf:type itil:GlossaryConcept ;
  rdfs:label "Effectiveness" ;
  skos:definition "(Continual Service Improvement) A measure of whether the Objectives of a Process, Service or Activity have been achieved. An Effective Process or Activity is one that achieves its agreed Objectives. See KPI." ;
  skos:prefLabel "Effectiveness" ;
.
itil:TERM_Efficiency
  rdf:type itil:GlossaryConcept ;
  rdfs:label "Efficiency" ;
  skos:definition "(Continual Service Improvement) A measure of whether the right amount of resources have been used to deliver a Process, Service or Activity. An Efficient Process achieves its Objectives with the minimum amount of time, money, people or other resources. See KPI." ;
  skos:prefLabel "Efficiency" ;
.
itil:TERM_Emergency_Change
  rdf:type itil:GlossaryConcept ;
  rdfs:label "Emergency Change" ;
  skos:definition "(Service Transition) A Change that must be introduced as soon as possible. For example to resolve a Major Incident or implement a Security patch. The Change Management Process will normally have a specific Procedure for handling Emergency Changes. See Emergency Change Advisory Board (ECAB)." ;
  skos:prefLabel "Emergency Change" ;
.
itil:TERM_Emergency_Change_Advisory_Board
  rdf:type itil:GlossaryConcept ;
  rdfs:label "Emergency Change Advisory Board (ECAB)" ;
  skos:definition "(Service Transition) A sub-set of the Change Advisory Board who make decisions about high impact Emergency Changes. Membership of the ECAB may be decided at the time a meeting is called, and depends on the nature of the Emergency Change." ;
  skos:prefLabel "Emergency Change Advisory Board (ECAB)" ;
.
itil:TERM_Environment
  rdf:type itil:GlossaryConcept ;
  rdfs:label "Environment" ;
  skos:definition "(Service Transition) A subset of the IT Infrastructure that is used for a particular purpose. For Example: Live Environment, Test Environment, Build Environment. It is possible for multiple Environments to share a Configuration Item, for example Test and Live Environments may use different partitions on a single mainframe computer. Also used in the term Physical Environment to mean the accommodation, air conditioning, power system etc. Environment is also used as a generic term to mean the external conditions that influence or affect something." ;
  skos:prefLabel "Environment" ;
.
itil:TERM_Error
  rdf:type itil:GlossaryConcept ;
  rdfs:label "Error" ;
  skos:definition "(Service Operation) A design flaw or malfunction that causes a Failure of one or more Configuration Items or IT Services. A mistake made by a person or a faulty Process that impacts a CI or IT Service is also an Error." ;
  skos:prefLabel "Error" ;
.
itil:TERM_Escalation
  rdf:type itil:GlossaryConcept ;
  rdfs:label "Escalation" ;
  skos:definition "(Service Operation) An Activity that obtains additional Resources when these are needed to meet Service Level Targets or Customer expectations. Escalation may be needed within any IT Service Management Process, but is most commonly associated with Incident Management, Problem Management and the management of Customer complaints. There are two types of Escalation, Functional Escalation and Hierarchic Escalation." ;
  skos:prefLabel "Escalation" ;
.
itil:TERM_Estimation
  rdf:type itil:GlossaryConcept ;
  rdfs:label "Estimation" ;
  skos:definition "The use of experience to provide an approximate value for a Metric or Cost. Estimation is also used in Capacity and Availability Management as the cheapest and least accurate Modelling method." ;
  skos:prefLabel "Estimation" ;
.
itil:TERM_Evaluation
  rdf:type itil:GlossaryConcept ;
  rdfs:label "Evaluation" ;
  skos:definition "(Service Transition) The Process responsible for assessing a new or Changed IT Service to ensure that Risks have been managed and to help determine whether to proceed with the Change. Evaluation is also used to mean comparing an actual Outcome with the intended Outcome, or comparing one alternative with another." ;
  skos:prefLabel "Evaluation" ;
.
itil:TERM_Event
  rdf:type itil:GlossaryConcept ;
  rdfs:label "Event" ;
  skos:definition "(Service Operation) A change of state which has significance for the management of a Configuration Item or IT Service. The term Event is also used to mean an Alert or notification created by any IT Service, Configuration Item or Monitoring tool. Events typically require IT Operations personnel to take actions, and often lead to Incidents being logged." ;
  skos:prefLabel "Event" ;
.
itil:TERM_Event_Management
  rdf:type itil:GlossaryConcept ;
  rdfs:label "Event Management" ;
  skos:definition "(Service Operation) The Process responsible for managing Events throughout their Lifecycle. Event Management is one of the main Activities of IT Operations." ;
  skos:prefLabel "Event Management" ;
  skos:related itil:TERM_Event_correlation ;
  skos:related itil:TERM_Event_filtering ;
  skos:related itil:TERM_Exception ;
  skos:related itil:TERM_Reporting ;
  skos:related itil:TERM_Warning ;
.
itil:TERM_Event_correlation
  rdf:type itil:GlossaryConcept ;
  rdfs:label "Event correlation" ;
  skos:prefLabel "Event correlation" ;
.
itil:TERM_Event_filtering
  rdf:type itil:GlossaryConcept ;
  rdfs:label "Event filtering" ;
  skos:prefLabel "Event filtering" ;
.
itil:TERM_Exception
  rdf:type itil:GlossaryConcept ;
  rdfs:label "Exception" ;
  skos:prefLabel "Exception" ;
.
itil:TERM_Exception_Report
  rdf:type itil:GlossaryConcept ;
  rdfs:label "Exception Report" ;
  skos:definition "A Document containing details of one or more KPIs or other important targets that have exceeded defined Thresholds. Examples include SLA targets being missed or about to be missed, and a Performance Metric indicating a potential Capacity problem." ;
  skos:prefLabel "Exception Report" ;
.
itil:TERM_Expanded_Incident_Lifecycle
  rdf:type itil:GlossaryConcept ;
  rdfs:label "Expanded Incident Lifecycle" ;
  skos:definition "(Availability Management) Detailed stages in the Lifecycle of an Incident. The stages are Detection, Diagnosis, Repair, Recovery, Restoration. The Expanded Incident Lifecycle is used to help understand all contributions to the Impact of Incidents and to Plan how these could be controlled or reduced." ;
  skos:prefLabel "Expanded Incident Lifecycle" ;
.
itil:TERM_External_Customer
  rdf:type itil:GlossaryConcept ;
  rdfs:label "External Customer" ;
  skos:definition "A Customer who works for a different Business to the IT Service Provider. See External Service Provider, Internal Customer." ;
  skos:prefLabel "External Customer" ;
.
itil:TERM_External_Metric
  rdf:type itil:GlossaryConcept ;
  rdfs:label "External Metric" ;
  skos:definition "A Metric that is used to measure the delivery of IT Service to a Customer. External Metrics are usually defined in SLAs and reported to Customers. See Internal Metric." ;
  skos:prefLabel "External Metric" ;
.
itil:TERM_External_Service_Provider
  rdf:type itil:GlossaryConcept ;
  rdfs:label "External Service Provider" ;
  skos:definition "(Service Strategy) An IT Service Provider which is part of a different Organisation to their Customer. An IT Service Provider may have both Internal Customers and External Customers. See Type III Service Provider." ;
  skos:prefLabel "External Service Provider" ;
.
itil:TERM_External_Sourcing
  rdf:type itil:GlossaryConcept ;
  rdfs:label "External Sourcing" ;
  skos:definition "Synonym for Outsourcing." ;
  skos:prefLabel "External Sourcing" ;
.
itil:TERM_Facilities_Management
  rdf:type itil:GlossaryConcept ;
  rdfs:label "Facilities Management" ;
  skos:definition "(Service Operation) The Function responsible for managing the physical Environment where the IT Infrastructure is located. Facilities Management includes all aspects of managing the physical Environment, for example power and cooling, building Access Management, and environmental Monitoring." ;
  skos:prefLabel "Facilities Management" ;
.
itil:TERM_Failure
  rdf:type itil:GlossaryConcept ;
  rdfs:label "Failure" ;
  skos:definition "(Service Operation) Loss of ability to Operate to Specification, or to deliver the required output. The term Failure may be used when referring to IT Services, Processes, Activities, Configuration Items etc. A Failure often causes an Incident." ;
  skos:prefLabel "Failure" ;
.
itil:TERM_Failure_Modes_and_Effects_Analysis
  rdf:type itil:GlossaryConcept ;
  rdfs:label "Failure Modes and Effects Analysis (FMEA)" ;
  skos:definition "An approach to assessing the potential Impact of Failures. FMEA involves analysing what would happen after Failure of each Configuration Item, all the way up to the effect on the Business. FMEA is often used in Information Security Management and in IT Service Continuity Planning." ;
  skos:prefLabel "Failure Modes and Effects Analysis (FMEA)" ;
.
itil:TERM_Fast_Recovery
  rdf:type itil:GlossaryConcept ;
  rdfs:label "Fast Recovery" ;
  skos:definition "(Service Design) A Recovery Option which is also known as Hot Standby. Provision is made to Recover the IT Service in a short period of time, typically less than 24 hours. Fast Recovery typically uses a dedicated Fixed Facility with computer Systems, and software configured ready to run the IT Services. Immediate Recovery may take up to 24 hours if there is a need to Restore data from Backups." ;
  skos:prefLabel "Fast Recovery" ;
.
itil:TERM_Fault
  rdf:type itil:GlossaryConcept ;
  rdfs:label "Fault" ;
  skos:definition "Synonym for Error." ;
  skos:prefLabel "Fault" ;
.
itil:TERM_Fault_Tolerance
  rdf:type itil:GlossaryConcept ;
  rdfs:label "Fault Tolerance" ;
  skos:definition "(Service Design) The ability of an IT Service or Configuration Item to continue to Operate correctly after Failure of a Component part. See Resilience, Countermeasure." ;
  skos:prefLabel "Fault Tolerance" ;
.
itil:TERM_Fault_Tree_Analysis
  rdf:type itil:GlossaryConcept ;
  rdfs:label "Fault Tree Analysis (FTA)" ;
  skos:definition "(Service Design) (Continual Service Improvement) A technique that can be used to determine the chain of Events that leads to a Problem. Fault Tree Analysis represents a chain of Events using Boolean notation in a diagram." ;
  skos:prefLabel "Fault Tree Analysis (FTA)" ;
.
itil:TERM_Financial_Management
  rdf:type itil:GlossaryConcept ;
  rdfs:label "Financial Management" ;
  skos:definition "(Service Strategy) The Function and Processes responsible for managing an IT Service Provider's Budgeting, Accounting and Charging Requirements." ;
  skos:prefLabel "Financial Management" ;
.
itil:TERM_First-line_Support
  rdf:type itil:GlossaryConcept ;
  rdfs:label "First-line Support" ;
  skos:definition "(Service Operation) The first level in a hierarchy of Support Groups involved in the resolution of Incidents. Each level contains more specialist skills, or has more time or other Resources. See Escalation." ;
  skos:prefLabel "First-line Support" ;
.
itil:TERM_Fishbone_Diagram
  rdf:type itil:GlossaryConcept ;
  rdfs:label "Fishbone Diagram" ;
  skos:definition "Synonym for Ishikawa Diagram." ;
  skos:prefLabel "Fishbone Diagram" ;
.
itil:TERM_Fit_for_Purpose
  rdf:type itil:GlossaryConcept ;
  rdfs:label "Fit for Purpose" ;
  skos:definition "An informal term used to describe a Process, Configuration Item, IT Service etc. that is capable of meeting its Objectives or Service Levels. Being Fit for Purpose requires suitable Design, implementation, Control and maintenance." ;
  skos:prefLabel "Fit for Purpose" ;
.
itil:TERM_Fixed_Cost
  rdf:type itil:GlossaryConcept ;
  rdfs:label "Fixed Cost" ;
  skos:definition "(Service Strategy) A Cost that does not vary with IT Service usage. For example the cost of Server hardware. See Variable Cost." ;
  skos:prefLabel "Fixed Cost" ;
.
itil:TERM_Fixed_Facility
  rdf:type itil:GlossaryConcept ;
  rdfs:label "Fixed Facility" ;
  skos:definition "(Service Design) A permanent building, available for use when needed by an IT Service Continuity Plan. See Recovery Option, Portable Facility." ;
  skos:prefLabel "Fixed Facility" ;
.
itil:TERM_Follow_the_Sun
  rdf:type itil:GlossaryConcept ;
  rdfs:label "Follow the Sun" ;
  skos:definition "(Service Operation) A methodology for using Service Desks and Support Groups around the world to provide seamless 24 * 7 Service. Calls, Incidents, Problems and Service Requests are passed between groups in different time zones." ;
  skos:prefLabel "Follow the Sun" ;
.
itil:TERM_Fulfilment
  rdf:type itil:GlossaryConcept ;
  rdfs:label "Fulfilment" ;
  skos:definition "Performing Activities to meet a need or Requirement. For example by providing a new IT Service, or meeting a Service Request." ;
  skos:prefLabel "Fulfilment" ;
.
itil:TERM_Function
  rdf:type itil:GlossaryConcept ;
  rdfs:label "Function" ;
  skos:definition "A team or group of people and the tools they use to carry out one or more Processes or Activities. For example the Service Desk. The term Function also has two other meanings � An intended purpose of a Configuration Item, Person, Team, Process, or IT Service. For example one Function of an Email Service may be to store and forward outgoing mails, one Function of a Business Process may be to dispatch goods to Customers. � To perform the intended purpose correctly, \"The computer is Functioning\"" ;
  skos:prefLabel "Function" ;
.
itil:TERM_Functional_Escalation
  rdf:type itil:GlossaryConcept ;
  rdfs:label "Functional Escalation" ;
  skos:definition "(Service Operation) Transferring an Incident, Problem or Change to a technical team with a higher level of expertise to assist in an Escalation." ;
  skos:prefLabel "Functional Escalation" ;
.
itil:TERM_Gap_Analysis
  rdf:type itil:GlossaryConcept ;
  rdfs:label "Gap Analysis" ;
  skos:definition "(Continual Service Improvement) An Activity which compares two sets of data and identifies the differences. Gap Analysis is commonly used to compare a set of Requirements with actual delivery. See Benchmarking." ;
  skos:prefLabel "Gap Analysis" ;
.
itil:TERM_Governance
  rdf:type itil:GlossaryConcept ;
  rdfs:label "Governance" ;
  skos:definition "Ensuring that Policies and Strategy are actually implemented, and that required Processes are correctly followed. Governance includes defining Roles and responsibilities, measuring and reporting, and taking actions to resolve any issues identified." ;
  skos:prefLabel "Governance" ;
.
itil:TERM_Gradual_Recovery
  rdf:type itil:GlossaryConcept ;
  rdfs:label "Gradual Recovery" ;
  skos:definition "(Service Design) A Recovery Option which is also known as Cold Standby. Provision is made to Recover the IT Service in a period of time greater than 72 hours. Gradual Recovery typically uses a Portable or Fixed Facility that has environmental support and network cabling, but no computer Systems. The hardware and software are installed as part of the IT Service Continuity Plan." ;
  skos:prefLabel "Gradual Recovery" ;
.
itil:TERM_Guideline
  rdf:type itil:GlossaryConcept ;
  rdfs:label "Guideline" ;
  skos:definition "A Document describing Best Practice, that recommends what should be done. Compliance to a guideline is not normally enforced. See Standard." ;
  skos:prefLabel "Guideline" ;
.
itil:TERM_Help_Desk
  rdf:type itil:GlossaryConcept ;
  rdfs:label "Help Desk" ;
  skos:definition "(Service Operation) A point of contact for Users to log Incidents. A Help Desk is usually more technically focussed than a Service Desk and does not provide a Single Point of Contact for all interaction. The term Help Desk is often used as a synonym for Service Desk." ;
  skos:prefLabel "Help Desk" ;
.
itil:TERM_Hierarchic_Escalation
  rdf:type itil:GlossaryConcept ;
  rdfs:label "Hierarchic Escalation" ;
  skos:definition "(Service Operation) Informing or involving more senior levels of management to assist in an Escalation." ;
  skos:prefLabel "Hierarchic Escalation" ;
.
itil:TERM_High_Availability
  rdf:type itil:GlossaryConcept ;
  rdfs:label "High Availability" ;
  skos:definition "(Service Design) An approach or Design that minimises or hides the effects of Configuration Item Failure on the Users of an IT Service. High Availability solutions are Designed to achieve an agreed level of Availability and make use of techniques such as Fault Tolerance, Resilience and fast Recovery to reduce the number of Incidents, and the Impact of Incidents." ;
  skos:prefLabel "High Availability" ;
.
itil:TERM_Hot_Standby
  rdf:type itil:GlossaryConcept ;
  rdfs:label "Hot Standby" ;
  skos:definition "Synonym for Fast Recovery or Immediate Recovery." ;
  skos:prefLabel "Hot Standby" ;
.
itil:TERM_ISOIEC_17799
  rdf:type itil:GlossaryConcept ;
  rdfs:label "ISO/IEC 17799" ;
  skos:definition "(Continual Service Improvement) ISO Code of Practice for Information Security Management. See Standard." ;
  skos:prefLabel "ISO/IEC 17799" ;
.
itil:TERM_ISOIEC_20000
  rdf:type itil:GlossaryConcept ;
  rdfs:label "ISO/IEC 20000" ;
  skos:definition "ISO Specification and Code of Practice for IT Service Management. ISO/IEC 20000 is aligned with ITIL Best Practice." ;
  skos:prefLabel "ISO/IEC 20000" ;
.
itil:TERM_ISOIEC_27001
  rdf:type itil:GlossaryConcept ;
  rdfs:label "ISO/IEC 27001" ;
  skos:definition "(Service Design) (Continual Service Improvement) ISO Specification for Information Security Management. The corresponding Code of Practice is ISO/IEC 17799. See Standard." ;
  skos:prefLabel "ISO/IEC 27001" ;
.
itil:TERM_ISO_9000
  rdf:type itil:GlossaryConcept ;
  rdfs:label "ISO 9000" ;
  skos:definition "A generic term that refers to a number of international Standards and Guidelines for Quality Management Systems. See http://www.iso.org/ for more information. See ISO." ;
  skos:prefLabel "ISO 9000" ;
.
itil:TERM_ISO_9001
  rdf:type itil:GlossaryConcept ;
  rdfs:label "ISO 9001" ;
  skos:definition "An international Standard for Quality Management Systems. See ISO 9000, Standard." ;
  skos:prefLabel "ISO 9001" ;
.
itil:TERM_ITIL
  rdf:type itil:GlossaryConcept ;
  rdfs:label "ITIL" ;
  skos:definition "A set of Best Practice guidance for IT Service Management. ITIL is owned by the OGC and consists of a series of publications giving guidance on the provision of Quality IT Services, and on the Processes and facilities needed to support them. See http://www.itil.co.uk/ for more information." ;
  skos:prefLabel "ITIL" ;
.
itil:TERM_IT_Directorate
  rdf:type itil:GlossaryConcept ;
  rdfs:label "IT Directorate" ;
  skos:definition "(Continual Service Improvement) Senior Management within a Service Provider, charged with developing and delivering IT services. Most commonly used in UK Government departments." ;
  skos:prefLabel "IT Directorate" ;
.
itil:TERM_IT_Infrastructure
  rdf:type itil:GlossaryConcept ;
  rdfs:label "IT Infrastructure" ;
  skos:definition "All of the hardware, software, networks, facilities etc. that are required to Develop, Test, deliver, Monitor, Control or support IT Services. The term IT Infrastructure includes all of the Information Technology but not the associated people, Processes and documentation." ;
  skos:prefLabel "IT Infrastructure" ;
.
itil:TERM_IT_Operations
  rdf:type itil:GlossaryConcept ;
  rdfs:label "IT Operations" ;
  skos:definition "(Service Operation) Activities carried out by IT Operations Control, including Console Management, Job Scheduling, Backup and Restore, and Print and Output Management. IT Operations is also used as a synonym for Service Operation." ;
  skos:prefLabel "IT Operations" ;
.
itil:TERM_IT_Operations_Control
  rdf:type itil:GlossaryConcept ;
  rdfs:label "IT Operations Control" ;
  skos:definition "(Service Operation) The Function responsible for Monitoring and Control of the IT Services and IT Infrastructure. See Operations Bridge." ;
  skos:prefLabel "IT Operations Control" ;
.
itil:TERM_IT_Operations_Management
  rdf:type itil:GlossaryConcept ;
  rdfs:label "IT Operations Management" ;
  skos:definition "(Service Operation) The Function within an IT Service Provider which performs the daily Activities needed to manage IT Services and the supporting IT Infrastructure. IT Operations Management includes IT Operations Control and Facilities Management." ;
  skos:prefLabel "IT Operations Management" ;
.
itil:TERM_IT_Service
  rdf:type itil:GlossaryConcept ;
  rdfs:label "IT Service" ;
  skos:definition "A Service provided to one or more Customers by an IT Service Provider. An IT Service is based on the use of Information Technology and supports the Customer's Business Processes. An IT Service is made up from a combination of people, Processes and technology and should be defined in a Service Level Agreement." ;
  skos:prefLabel "IT Service" ;
.
itil:TERM_IT_Service_Continuity_Management
  rdf:type itil:GlossaryConcept ;
  rdfs:label "IT Service Continuity Management (ITSCM)" ;
  skos:definition "(Service Design) The Process responsible for managing Risks that could seriously impact IT Services. ITSCM ensures that the IT Service Provider can always provide minimum agreed Service Levels, by reducing the Risk to an acceptable level and Planning for the Recovery of IT Services. ITSCM should be designed to support Business Continuity Management." ;
  skos:prefLabel "IT Service Continuity Management (ITSCM)" ;
.
itil:TERM_IT_Service_Continuity_Plan
  rdf:type itil:GlossaryConcept ;
  rdfs:label "IT Service Continuity Plan" ;
  skos:definition "(Service Design) A Plan defining the steps required to Recover one or more IT Services. The Plan will also identify the triggers for Invocation, people to be involved, communications etc. The IT Service Continuity Plan should be part of a Business Continuity Plan." ;
  skos:prefLabel "IT Service Continuity Plan" ;
.
itil:TERM_IT_Service_Management
  rdf:type itil:GlossaryConcept ;
  rdfs:label "IT Service Management (ITSM)" ;
  skos:definition "The implementation and management of Quality IT Services that meet the needs of the Business. IT Service Management is performed by IT Service Providers through an appropriate mix of people, Process and Information Technology. See Service Management." ;
  skos:prefLabel "IT Service Management (ITSM)" ;
.
itil:TERM_IT_Service_Management_Forum
  rdf:type itil:GlossaryConcept ;
  rdfs:label "IT Service Management Forum (itSMF)" ;
  skos:definition "The IT Service Management Forum is an independent Organisation dedicated to promoting a professional approach to IT Service Management. The itSMF is a not-for-profit membership Organisation with representation in many countries around the world (itSMF Chapters). The itSMF and its membership contribute to the development of ITIL and associated IT Service Management Standards. See http://www.itsmf.com/ for more information." ;
  skos:prefLabel "IT Service Management Forum (itSMF)" ;
.
itil:TERM_IT_Service_Provider
  rdf:type itil:GlossaryConcept ;
  rdfs:label "IT Service Provider" ;
  skos:definition "(Service Strategy) A Service Provider that provides IT Services to Internal Customers or External Customers." ;
  skos:prefLabel "IT Service Provider" ;
.
itil:TERM_IT_Steering_Group
  rdf:type itil:GlossaryConcept ;
  rdfs:label "IT Steering Group (ISG)" ;
  skos:definition "A formal group that is responsible for ensuring that Business and IT Service Provider Strategies and Plans are closely aligned. An IT Steering Group includes senior representatives from the Business and the IT Service Provider." ;
  skos:prefLabel "IT Steering Group (ISG)" ;
.
itil:TERM_Identity
  rdf:type itil:GlossaryConcept ;
  rdfs:label "Identity" ;
  skos:definition "(Service Operation) A unique name that is used to identify a User, person or Role. The Identity is used to grant Rights to that User, person, or Role. Example identities might be the username SmithJ or the Role \"Change manager\"." ;
  skos:prefLabel "Identity" ;
.
itil:TERM_Immediate_Recovery
  rdf:type itil:GlossaryConcept ;
  rdfs:label "Immediate Recovery" ;
  skos:definition "(Service Design) A Recovery Option which is also known as Hot Standby. Provision is made to Recover the IT Service with no loss of Service. Immediate Recovery typically uses mirroring, load balancing and split site technologies." ;
  skos:prefLabel "Immediate Recovery" ;
.
itil:TERM_Impact
  rdf:type itil:GlossaryConcept ;
  rdfs:label "Impact" ;
  skos:definition "(Service Operation) (Service Transition) A measure of the effect of an Incident, Problem or Change on Business Processes. Impact is often based on how Service Levels will be affected. Impact and Urgency are used to assign Priority." ;
  skos:prefLabel "Impact" ;
.
itil:TERM_Incident
  rdf:type itil:GlossaryConcept ;
  rdfs:label "Incident" ;
  skos:definition "(Service Operation) An unplanned interruption to an IT Service or a reduction in the Quality of an IT Service. Failure of a Configuration Item that has not yet impacted Service is also an Incident. For example Failure of one disk from a mirror set." ;
  skos:prefLabel "Incident" ;
.
itil:TERM_Incident_Management
  rdf:type itil:GlossaryConcept ;
  rdfs:label "Incident Management" ;
  skos:definition "(Service Operation) The Process responsible for managing the Lifecycle of all Incidents. The primary Objective of Incident Management is to return the IT Service to Users as quickly as possible." ;
  skos:prefLabel "Incident Management" ;
.
itil:TERM_Incident_Record
  rdf:type itil:GlossaryConcept ;
  rdfs:label "Incident Record" ;
  skos:definition "(Service Operation) A Record containing the details of an Incident. Each Incident record documents the Lifecycle of a single Incident." ;
  skos:prefLabel "Incident Record" ;
.
itil:TERM_Indirect_Cost
  rdf:type itil:GlossaryConcept ;
  rdfs:label "Indirect Cost" ;
  skos:definition "(Service Strategy) A Cost of providing an IT Service which cannot be allocated in full to a specific Customer. For example Cost of providing shared Servers or software licenses. Also known as Overhead. See Direct Cost." ;
  skos:prefLabel "Indirect Cost" ;
.
itil:TERM_Information_Security_Management
  rdf:type itil:GlossaryConcept ;
  rdfs:label "Information Security Management (ISM)" ;
  skos:definition "(Service Design) The Process that ensures the Confidentiality, Integrity and Availability of an Organisation's Assets, information, data and IT Services. Information Security Management usually forms part of an Organisational approach to Security Management which has a wider scope than the IT Service Provider, and includes handling of paper, building access, phone calls etc., for the entire Organisation." ;
  skos:prefLabel "Information Security Management (ISM)" ;
.
itil:TERM_Information_Security_Management_System
  rdf:type itil:GlossaryConcept ;
  rdfs:label "Information Security Management System (ISMS)" ;
  skos:definition "(Service Design) The framework of Policy, Processes, Standards, Guidelines and tools that ensures an Organisation can achieve its Information Security Management Objectives." ;
  skos:prefLabel "Information Security Management System (ISMS)" ;
.
itil:TERM_Information_Security_Policy
  rdf:type itil:GlossaryConcept ;
  rdfs:label "Information Security Policy" ;
  skos:definition "(Service Design) The Policy that governs the Organisation�s approach to Information Security Management." ;
  skos:prefLabel "Information Security Policy" ;
.
itil:TERM_Information_Technology
  rdf:type itil:GlossaryConcept ;
  rdfs:label "Information Technology (IT)" ;
  skos:definition "The use of technology for the storage, communication or processing of information. The technology typically includes computers, telecommunications, Applications and other software. The information may include Business data, voice, images, video, etc. Information Technology is often used to support Business Processes through IT Services." ;
  skos:prefLabel "Information Technology (IT)" ;
.
itil:TERM_Infrastructure_Service
  rdf:type itil:GlossaryConcept ;
  rdfs:label "Infrastructure Service" ;
  skos:definition "An IT Service that is not directly used by the Business, but is required by the IT Service Provider so they can provide other IT Services. For example Directory Services, naming services, or communication services." ;
  skos:prefLabel "Infrastructure Service" ;
.
itil:TERM_Insourcing
  rdf:type itil:GlossaryConcept ;
  rdfs:label "Insourcing" ;
  skos:definition "Synonym for Internal Sourcing." ;
  skos:prefLabel "Insourcing" ;
.
itil:TERM_Integrity
  rdf:type itil:GlossaryConcept ;
  rdfs:label "Integrity" ;
  skos:definition "(Service Design) A security principle that ensures data and Configuration Items are only modified by authorised personnel and Activities. Integrity considers all possible causes of modification, including software and hardware Failure, environmental Events, and human intervention." ;
  skos:prefLabel "Integrity" ;
.
itil:TERM_Interactive_Voice_Response
  rdf:type itil:GlossaryConcept ;
  rdfs:label "Interactive Voice Response (IVR)" ;
  skos:definition "(Service Operation) A form of Automatic Call Distribution that accepts User input, such as key presses and spoken commands, to identify the correct destination for incoming Calls." ;
  skos:prefLabel "Interactive Voice Response (IVR)" ;
.
itil:TERM_Intermediate_Recovery
  rdf:type itil:GlossaryConcept ;
  rdfs:label "Intermediate Recovery" ;
  skos:definition "(Service Design) A Recovery Option which is also known as Warm Standby. Provision is made to Recover the IT Service in a period of time between 24 and 72 hours. Intermediate Recovery typically uses a shared Portable or Fixed Facility that has computer Systems and network Components. The hardware and software will need to be configured, and data will need to be restored, as part of the IT Service Continuity Plan." ;
  skos:prefLabel "Intermediate Recovery" ;
.
itil:TERM_Internal_Customer
  rdf:type itil:GlossaryConcept ;
  rdfs:label "Internal Customer" ;
  skos:definition "A Customer who works for the same Business as the IT Service Provider. See Internal Service Provider, External Customer." ;
  skos:prefLabel "Internal Customer" ;
.
itil:TERM_Internal_Metric
  rdf:type itil:GlossaryConcept ;
  rdfs:label "Internal Metric" ;
  skos:definition "A Metric that is used within the IT Service Provider to Monitor the Efficiency, Effectiveness or Cost Effectiveness of the IT Service Provider's internal Processes. Internal Metrics are not normally reported to the Customer of the IT Service. See External Metric." ;
  skos:prefLabel "Internal Metric" ;
.
itil:TERM_Internal_Rate_of_Return
  rdf:type itil:GlossaryConcept ;
  rdfs:label "Internal Rate of Return (IRR)" ;
  skos:definition "(Service Strategy) A technique used to help make decisions about Capital Expenditure. IRR calculates a figure that allows two or more alternative investments to be compared. A larger IRR indicates a better investment. See Net Present Value, Return on Investment." ;
  skos:prefLabel "Internal Rate of Return (IRR)" ;
.
itil:TERM_Internal_Service_Provider
  rdf:type itil:GlossaryConcept ;
  rdfs:label "Internal Service Provider" ;
  skos:definition "(Service Strategy) An IT Service Provider which is part of the same Organisation as their Customer. An IT Service Provider may have both Internal Customers and External Customers. See Type I Service Provider, Type II Service Provider, Insource." ;
  skos:prefLabel "Internal Service Provider" ;
.
itil:TERM_Internal_Sourcing
  rdf:type itil:GlossaryConcept ;
  rdfs:label "Internal Sourcing" ;
  skos:definition "(Service Strategy) Using an Internal Service Provider to manage IT Services. See Service Sourcing, Type I Service Provider, Type II Service Provider." ;
  skos:prefLabel "Internal Sourcing" ;
.
itil:TERM_International_Organization_for_Standardization
  rdf:type itil:GlossaryConcept ;
  rdfs:label "International Organization for Standardization (ISO)" ;
  skos:definition "The International Organization for Standardization (ISO) is the world's largest developer of Standards. ISO is a non-governmental organization which is a network of the national standards institutes of 156 countries. Further information about ISO is available from http://www.iso.org/" ;
  skos:prefLabel "International Organization for Standardization (ISO)" ;
.
itil:TERM_International_Standards_Organisation
  rdf:type itil:GlossaryConcept ;
  rdfs:label "International Standards Organisation" ;
  skos:definition "See International Organization for Standardization (ISO)" ;
  skos:prefLabel "International Standards Organisation" ;
.
itil:TERM_Internet_Service_Provider
  rdf:type itil:GlossaryConcept ;
  rdfs:label "Internet Service Provider (ISP)" ;
  skos:definition "An External Service Provider that provides access to the Internet. Most ISPs also provide other IT Services such as web hosting." ;
  skos:prefLabel "Internet Service Provider (ISP)" ;
.
itil:TERM_Invocation
  rdf:type itil:GlossaryConcept ;
  rdfs:label "Invocation" ;
  skos:definition "(Service Design) Initiation of the steps defined in a plan. For example initiating the IT Service Continuity Plan for one or more IT Services." ;
  skos:prefLabel "Invocation" ;
.
itil:TERM_Ishikawa_Diagram
  rdf:type itil:GlossaryConcept ;
  rdfs:label "Ishikawa Diagram" ;
  skos:definition "(Service Operation) (Continual Service Improvement) A technique that helps a team to identify all the possible causes of a Problem. Originally devised by Kaoru Ishikawa, the output of this technique is a diagram that looks like a fishbone." ;
  skos:prefLabel "Ishikawa Diagram" ;
.
itil:TERM_Job_Description
  rdf:type itil:GlossaryConcept ;
  rdfs:label "Job Description" ;
  skos:definition "A Document which defines the Roles, responsibilities, skills and knowledge required by a particular person. One Job Description can include multiple Roles, for example the Roles of Configuration Manager and Change Manager may be carried out by one person." ;
  skos:prefLabel "Job Description" ;
.
itil:TERM_Job_Scheduling
  rdf:type itil:GlossaryConcept ;
  rdfs:label "Job Scheduling" ;
  skos:definition "(Service Operation) Planning and managing the execution of software tasks that are required as part of an IT Service. Job Scheduling is carried out by IT Operations Management, and is often automated using software tools that run batch or online tasks at specific times of the day, week, month or year." ;
  skos:prefLabel "Job Scheduling" ;
.
itil:TERM_Kano_Model
  rdf:type itil:GlossaryConcept ;
  rdfs:label "Kano Model" ;
  skos:definition "(Service Strategy) A Model developed by Noriaki Kano that is used to help understand Customer preferences. The Kano Model considers Attributes of an IT Service grouped into areas such as Basic Factors, Excitement Factors, Performance Factors etc." ;
  skos:prefLabel "Kano Model" ;
.
itil:TERM_Kepner__Tregoe_Analysis
  rdf:type itil:GlossaryConcept ;
  rdfs:label "Kepner & Tregoe Analysis" ;
  skos:definition "(Service Operation) (Continual Service Improvement) A structured approach to Problem solving. The Problem is analysed in terms of what, where, when and extent. Possible causes are identified. The most probable cause is tested. The true cause is verified." ;
  skos:prefLabel "Kepner & Tregoe Analysis" ;
.
itil:TERM_Key_Performance_Indicator
  rdf:type itil:GlossaryConcept ;
  rdfs:label "Key Performance Indicator (KPI)" ;
  skos:definition "(Continual Service Improvement) A Metric that is used to help manage a Process, IT Service or Activity. Many Metrics may be measured, but only the most important of these are defined as KPIs and used to actively manage and report on the Process, IT Service or Activity. KPIs should be selected to ensure that Efficiency, Effectiveness, and Cost Effectiveness are all managed. See Critical Success Factor." ;
  skos:prefLabel "Key Performance Indicator (KPI)" ;
.
itil:TERM_Knowledge_Base
  rdf:type itil:GlossaryConcept ;
  rdfs:label "Knowledge Base" ;
  skos:definition "(Service Transition) A logical database containing the data used by the Service Knowledge Management System." ;
  skos:prefLabel "Knowledge Base" ;
.
itil:TERM_Knowledge_Management
  rdf:type itil:GlossaryConcept ;
  rdfs:label "Knowledge Management" ;
  skos:definition "(Service Transition) The Process responsible for gathering, analysing, storing and sharing knowledge and information within an Organisation. The primary purpose of Knowledge Management is to improve Efficiency by reducing the need to rediscover knowledge. See Data-to-Information-to-Knowledge-to-Wisdom, Service Knowledge Management System." ;
  skos:prefLabel "Knowledge Management" ;
.
itil:TERM_Known_Error
  rdf:type itil:GlossaryConcept ;
  rdfs:label "Known Error" ;
  skos:definition "(Service Operation) A Problem that has a documented Root Cause and a Workaround. Known Errors are created and managed throughout their Lifecycle by Problem Management. Known Errors may also be identified by Development or Suppliers." ;
  skos:prefLabel "Known Error" ;
.
itil:TERM_Known_Error_Database
  rdf:type itil:GlossaryConcept ;
  rdfs:label "Known Error Database (KEDB)" ;
  skos:definition "(Service Operation) A database containing all Known Error Records. This database is created by Problem Management and used by Incident and Problem Management. The Known Error Database is part of the Service Knowledge Management System." ;
  skos:prefLabel "Known Error Database (KEDB)" ;
.
itil:TERM_Known_Error_Record
  rdf:type itil:GlossaryConcept ;
  rdfs:label "Known Error Record" ;
  skos:definition "(Service Operation) A Record containing the details of a Known Error. Each Known Error Record documents the Lifecycle of a Known Error, including the Status, Root Cause and Workaround. In some implementations a Known Error is documented using additional fields in a Problem Record." ;
  skos:prefLabel "Known Error Record" ;
.
itil:TERM_Lifecycle
  rdf:type itil:GlossaryConcept ;
  rdfs:label "Lifecycle" ;
  skos:definition "The various stages in the life of an IT Service, Configuration Item, Incident, Problem, Change etc. The Lifecycle defines the Categories for Status and the Status transitions that are permitted. For example: � The Lifecycle of an Application includes Requirements, Design, Build, Deploy, Operate, Optimise. � The Expanded Incident Lifecycle includes Detect, Respond, Diagnose, Repair, Recover, Restore. � The lifecycle of a Server may include: Ordered, Received, In Test, Live, Disposed etc." ;
  skos:prefLabel "Lifecycle" ;
.
itil:TERM_Line_of_Service
  rdf:type itil:GlossaryConcept ;
  rdfs:label "Line of Service (LOS)" ;
  skos:definition "(Service Strategy) A Core Service or Supporting Service that has multiple Service Level Packages. A line of Service is managed by a Product Manager and each Service Level Package is designed to support a particular market segment." ;
  skos:prefLabel "Line of Service (LOS)" ;
.
itil:TERM_Live
  rdf:type itil:GlossaryConcept ;
  rdfs:label "Live" ;
  skos:definition "(Service Transition) Refers to an IT Service or Configuration Item that is being used to deliver Service to a Customer." ;
  skos:prefLabel "Live" ;
.
itil:TERM_Live_Environment
  rdf:type itil:GlossaryConcept ;
  rdfs:label "Live Environment" ;
  skos:definition "(Service Transition) A controlled Environment containing Live Configuration Items used to deliver IT Services to Customers." ;
  skos:prefLabel "Live Environment" ;
.
itil:TERM_Maintainability
  rdf:type itil:GlossaryConcept ;
  rdfs:label "Maintainability" ;
  skos:definition "(Service Design) A measure of how quickly and Effectively a Configuration Item or IT Service can be restored to normal working after a Failure. Maintainability is often measured and reported as MTRS. Maintainability is also used in the context of Software or IT Service Development to mean ability to be Changed or Repaired easily." ;
  skos:prefLabel "Maintainability" ;
.
itil:TERM_Major_Incident
  rdf:type itil:GlossaryConcept ;
  rdfs:label "Major Incident" ;
  skos:broader itil:TERM_Incident ;
  skos:definition "(Service Operation) The highest Category of Impact for an Incident. A Major Incident results in significant disruption to the Business." ;
  skos:prefLabel "Major Incident" ;
.
itil:TERM_Managed_Services
  rdf:type itil:GlossaryConcept ;
  rdfs:label "Managed Services" ;
  skos:definition "(Service Strategy) A perspective on IT Services which emphasizes the fact that they are managed. The term Managed Services is also used as a synonym for Outsourced IT Services." ;
  skos:prefLabel "Managed Services" ;
.
itil:TERM_Management_Information
  rdf:type itil:GlossaryConcept ;
  rdfs:label "Management Information" ;
  skos:definition "Information that is used to support decision making by managers. Management Information is often generated automatically by tools supporting the various IT Service Management Processes. Management Information often includes the values of KPIs such as \"Percentage of Changes leading to Incidents\", or \"first time fix rate\"." ;
  skos:prefLabel "Management Information" ;
.
itil:TERM_Management_System
  rdf:type itil:GlossaryConcept ;
  rdfs:label "Management System" ;
  skos:definition "The framework of Policy, Processes and Functions that ensures an Organisation can achieve its Objectives." ;
  skos:prefLabel "Management System" ;
.
itil:TERM_Management_of_Risk
  rdf:type itil:GlossaryConcept ;
  rdfs:label "Management of Risk (MoR)" ;
  skos:definition "The OGC methodology for managing Risks. MoR includes all the Activities required to identify and Control the exposure to Risk which may have an impact on the achievement of an Organisation�s Business Objectives. See http://www.m-o-r.org/ for more details." ;
  skos:prefLabel "Management of Risk (MoR)" ;
.
itil:TERM_Manual_Workaround
  rdf:type itil:GlossaryConcept ;
  rdfs:label "Manual Workaround" ;
  skos:broader itil:TERM_Workaround ;
  skos:definition "A Workaround that requires manual intervention. Manual Workaround is also used as the name of a Recovery Option in which The Business Process Operates without the use of IT Services. This is a temporary measure and is usually combined with another Recovery Option." ;
  skos:prefLabel "Manual Workaround" ;
.
itil:TERM_Marginal_Cost
  rdf:type itil:GlossaryConcept ;
  rdfs:label "Marginal Cost" ;
  skos:definition "(Service Strategy) The Cost of continuing to provide the IT Service. Marginal Cost does not include investment already made, for example the cost of developing new software and delivering training." ;
  skos:prefLabel "Marginal Cost" ;
.
itil:TERM_Market_Space
  rdf:type itil:GlossaryConcept ;
  rdfs:label "Market Space" ;
  skos:definition "(Service Strategy) All opportunities that an IT Service Provider could exploit to meet business needs of Customers. The Market Space identifies the possible IT Services that an IT Service Provider may wish to consider delivering." ;
  skos:prefLabel "Market Space" ;
.
itil:TERM_Maturity
  rdf:type itil:GlossaryConcept ;
  rdfs:label "Maturity" ;
  skos:definition "(Continual Service Improvement) A measure of the Reliability, Efficiency and Effectiveness of a Process, Function, Organisation etc. The most mature Processes and Functions are formally aligned to Business Objectives and Strategy, and are supported by a framework for continual improvement." ;
  skos:prefLabel "Maturity" ;
.
itil:TERM_Maturity_Level
  rdf:type itil:GlossaryConcept ;
  rdfs:label "Maturity Level" ;
  skos:definition "A named level in a Maturity model such as the Carnegie Mellon Capability Maturity Model Integration." ;
  skos:prefLabel "Maturity Level" ;
.
itil:TERM_Mean_Time
  rdf:type itil:GlossaryConcept ;
  rdfs:label "Mean Time" ;
  skos:definition "(Service Design) A Metric for measuring and reporting Reliability. Mean Time is the average time." ;
  skos:prefLabel "Mean Time" ;
.
itil:TERM_Mean_Time_Between_Failures
  rdf:type itil:GlossaryConcept ;
  rdfs:label "Mean Time Between Failures (MTBF)" ;
  skos:broader itil:TERM_Mean_Time ;
  skos:definition "(Service Design) A Metric for measuring and reporting Reliability. MTBF is the average time that a Configuration Item or IT Service can perform its agreed Function without interruption. This is measured from when the CI or IT Service starts working, until it next fails." ;
  skos:prefLabel "Mean Time Between Failures (MTBF)" ;
.
itil:TERM_Mean_Time_Between_Service_Incidents
  rdf:type itil:GlossaryConcept ;
  rdfs:label "Mean Time Between Service Incidents (MTBSI)" ;
  skos:broader itil:TERM_Mean_Time ;
  skos:definition "(Service Design) A Metric used for measuring and reporting Reliability. MTBSI is the mean time from when a System or IT Service fails, until it next fails. MTBSI is equal to MTBF + MTRS." ;
  skos:prefLabel "Mean Time Between Service Incidents (MTBSI)" ;
.
itil:TERM_Mean_Time_To_Repair
  rdf:type itil:GlossaryConcept ;
  rdfs:label "Mean Time To Repair (MTTR)" ;
  skos:broader itil:TERM_Mean_Time ;
  skos:definition "The average time taken to repair a Configuration Item or IT Service after a Failure. MTTR is measured from when the CI or IT Service fails until it is Repaired. MTTR does not include the time required to Recover or Restore. MTTR is sometimes incorrectly used to mean Mean Time to Restore Service." ;
  skos:prefLabel "Mean Time To Repair (MTTR)" ;
.
itil:TERM_Mean_Time_to_Restore_Service
  rdf:type itil:GlossaryConcept ;
  rdfs:label "Mean Time to Restore Service (MTRS)" ;
  skos:broader itil:TERM_Mean_Time ;
  skos:definition "The average time taken to Restore a Configuration Item or IT Service after a Failure. MTRS is measured from when the CI or IT Service fails until it is fully Restored and delivering its normal functionality. See Maintainability, Mean Time to Repair." ;
  skos:prefLabel "Mean Time to Restore Service (MTRS)" ;
.
itil:TERM_Metric
  rdf:type itil:GlossaryConcept ;
  rdfs:label "Metric" ;
  skos:definition "(Continual Service Improvement) Something that is measured and reported to help manage a Process, IT Service or Activity. See KPI." ;
  skos:prefLabel "Metric" ;
.
itil:TERM_Middleware
  rdf:type itil:GlossaryConcept ;
  rdfs:label "Middleware" ;
  skos:definition "(Service Design) Software that connects two or more software Components or Applications. Middleware is usually purchased from a Supplier, rather than developed within the IT Service Provider. See Off the Shelf." ;
  skos:prefLabel "Middleware" ;
.
itil:TERM_Mission_Statement
  rdf:type itil:GlossaryConcept ;
  rdfs:label "Mission Statement" ;
  skos:definition "The Mission Statement of an Organisation is a short but complete description of the overall purpose and intentions of that Organisation. It states what is to be achieved, but not how this should be done." ;
  skos:prefLabel "Mission Statement" ;
.
itil:TERM_Model
  rdf:type itil:GlossaryConcept ;
  rdfs:label "Model" ;
  skos:definition "A representation of a System, Process, IT Service, Configuration Item etc. that is used to help understand or predict future behaviour." ;
  skos:prefLabel "Model" ;
.
itil:TERM_Modelling
  rdf:type itil:GlossaryConcept ;
  rdfs:label "Modelling" ;
  skos:definition "A technique that is used to predict the future behaviour of a System, Process, IT Service, Configuration Item etc. Modelling is commonly used in Financial Management, Capacity Management and Availability Management." ;
  skos:prefLabel "Modelling" ;
.
itil:TERM_Monitor_Control_Loop
  rdf:type itil:GlossaryConcept ;
  rdfs:label "Monitor Control Loop" ;
  skos:definition "(Service Operation) Monitoring the output of a Task, Process, IT Service or Configuration Item; comparing this output to a predefined norm; and taking appropriate action based on this comparison." ;
  skos:prefLabel "Monitor Control Loop" ;
.
itil:TERM_Monitoring
  rdf:type itil:GlossaryConcept ;
  rdfs:label "Monitoring" ;
  skos:definition "(Service Operation) Repeated observation of a Configuration Item, IT Service or Process to detect Events and to ensure that the current status is known." ;
  skos:prefLabel "Monitoring" ;
.
itil:TERM_Near-Shore
  rdf:type itil:GlossaryConcept ;
  rdfs:label "Near-Shore" ;
  skos:definition "(Service Strategy) Provision of Services from a country near the country where the Customer is based. This can be the provision of an IT Service, or of supporting Functions such as Service Desk. See On-shore, Off-shore." ;
  skos:prefLabel "Near-Shore" ;
.
itil:TERM_Net_Present_Value
  rdf:type itil:GlossaryConcept ;
  rdfs:label "Net Present Value (NPV)" ;
  skos:definition "(Service Strategy) A technique used to help make decisions about Capital Expenditure. NPV compares cash inflows to cash outflows. Positive NPV indicates that an investment is worthwhile. See Internal Rate of Return, Return on Investment." ;
  skos:prefLabel "Net Present Value (NPV)" ;
.
itil:TERM_Notional_Charging
  rdf:type itil:GlossaryConcept ;
  rdfs:label "Notional Charging" ;
  skos:definition "(Service Strategy) An approach to Charging for IT Services. Charges to Customers are calculated and Customers are informed of the charge, but no money is actually transferred. Notional Charging is sometimes introduced to ensure that Customers are aware of the Costs they incur, or as a stage during the introduction of real Charging." ;
  skos:prefLabel "Notional Charging" ;
.
itil:TERM_Objective
  rdf:type itil:GlossaryConcept ;
  rdfs:label "Objective" ;
  skos:definition "The defined purpose or aim of a Process, an Activity or an Organisation as a whole. Objectives are usually expressed as measurable targets. The term Objective is also informally used to mean a Requirement. See Outcome." ;
  skos:prefLabel "Objective" ;
.
itil:TERM_Off-shore
  rdf:type itil:GlossaryConcept ;
  rdfs:label "Off-shore" ;
  skos:definition "(Service Strategy) Provision of Services from a location outside the country where the Customer is based, often in a different continent. This can be the provision of an IT Service, or of supporting Functions such as Service Desk. See On-shore, Near-shore." ;
  skos:prefLabel "Off-shore" ;
.
itil:TERM_Off_the_Shelf
  rdf:type itil:GlossaryConcept ;
  rdfs:label "Off the Shelf" ;
  skos:definition "Synonym for Commercial Off the Shelf." ;
  skos:prefLabel "Off the Shelf" ;
.
itil:TERM_Office_of_Government_Commerce
  rdf:type itil:GlossaryConcept ;
  rdfs:label "Office of Government Commerce (OGC)" ;
  skos:definition "OGC owns the ITIL brand (copyright and trademark). OGC is a UK Government department that supports the delivery of the government's procurement agenda through its work in collaborative procurement and in raising levels of procurement skills and capability with departments. It also provides support for complex public sector projects." ;
  skos:prefLabel "Office of Government Commerce (OGC)" ;
.
itil:TERM_Office_of_Public_Sector_Information
  rdf:type itil:GlossaryConcept ;
  rdfs:label "Office of Public Sector Information (OPSI)" ;
  skos:definition "OPSI license the Crown Copyright material used in the ITIL publications. They are a UK Government department who provide online access to UK legislation, license the re-use of Crown copyright material, manage the Information Fair Trader Scheme, maintain the Government�s Information Asset Register and provide advice and guidance on official publishing and Crown copyright." ;
  skos:prefLabel "Office of Public Sector Information (OPSI)" ;
.
itil:TERM_On-shore
  rdf:type itil:GlossaryConcept ;
  rdfs:label "On-shore" ;
  skos:definition "(Service Strategy) Provision of Services from a location within the country where the Customer is based. See Off-shore, Near-shore." ;
  skos:prefLabel "On-shore" ;
.
itil:TERM_Operate
  rdf:type itil:GlossaryConcept ;
  rdfs:label "Operate" ;
  skos:definition "To perform as expected. A Process or Configuration Item is said to Operate if it is delivering the Required outputs. Operate also means to perform one or more Operations. For example, to Operate a computer is to do the day-to-day Operations needed for it to perform as expected." ;
  skos:prefLabel "Operate" ;
.
itil:TERM_Operation
  rdf:type itil:GlossaryConcept ;
  rdfs:label "Operation" ;
  skos:definition "(Service Operation) Day-to-day management of an IT Service, System, or other Configuration Item. Operation is also used to mean any pre- defined Activity or Transaction. For example loading a magnetic tape, accepting money at a point of sale, or reading data from a disk drive." ;
  skos:prefLabel "Operation" ;
.
itil:TERM_Operational
  rdf:type itil:GlossaryConcept ;
  rdfs:label "Operational" ;
  skos:definition "The lowest of three levels of Planning and delivery (Strategic, Tactical, Operational). Operational Activities include the day-to-day or short term Planning or delivery of a Business Process or IT Service Management Process. The term Operational is also a synonym for Live." ;
  skos:prefLabel "Operational" ;
.
itil:TERM_Operational_Cost
  rdf:type itil:GlossaryConcept ;
  rdfs:label "Operational Cost" ;
  skos:definition "Cost resulting from running the IT Services. Often repeating payments. For example staff costs, hardware maintenance and electricity (also known as \"current expenditure\" or \"revenue expenditure\"). See Capital Expenditure." ;
  skos:prefLabel "Operational Cost" ;
.
itil:TERM_Operational_Expenditure
  rdf:type itil:GlossaryConcept ;
  rdfs:label "Operational Expenditure (OPEX)" ;
  skos:definition "Synonym for Operational Cost." ;
  skos:prefLabel "Operational Expenditure (OPEX)" ;
.
itil:TERM_Operational_Level_Agreement
  rdf:type itil:GlossaryConcept ;
  rdfs:label "Operational Level Agreement (OLA)" ;
  skos:definition "(Service Design) (Continual Service Improvement) An Agreement between an IT Service Provider and another part of the same Organisation. An OLA supports the IT Service Provider's delivery of IT Services to Customers. The OLA defines the goods or Services to be provided and the responsibilities of both parties. For example there could be an OLA � between the IT Service Provider and a procurement department to obtain hardware in agreed times � between the Service Desk and a Support Group to provide Incident Resolution in agreed times. See Service Level Agreement." ;
  skos:prefLabel "Operational Level Agreement (OLA)" ;
.
itil:TERM_Operations_Bridge
  rdf:type itil:GlossaryConcept ;
  rdfs:label "Operations Bridge" ;
  skos:definition "(Service Operation) A physical location where IT Services and IT Infrastructure are monitored and managed." ;
  skos:prefLabel "Operations Bridge" ;
.
itil:TERM_Operations_Control
  rdf:type itil:GlossaryConcept ;
  rdfs:label "Operations Control" ;
  skos:definition "Synonym for IT Operations Control." ;
  skos:prefLabel "Operations Control" ;
.
itil:TERM_Operations_Management
  rdf:type itil:GlossaryConcept ;
  rdfs:label "Operations Management" ;
  skos:definition "Synonym for IT Operations Management." ;
  skos:prefLabel "Operations Management" ;
.
itil:TERM_Opportunity_Cost
  rdf:type itil:GlossaryConcept ;
  rdfs:label "Opportunity Cost" ;
  skos:definition "(Service Strategy) A Cost that is used in deciding between investment choices. Opportunity Cost represents the revenue that would have been generated by using the Resources in a different way. For example the Opportunity Cost of purchasing a new Server may include not carrying out a Service Improvement activity that the money could have been spent on. Opportunity cost analysis is used as part of a decision making processes, but is not treated as an actual Cost in any financial statement." ;
  skos:prefLabel "Opportunity Cost" ;
.
itil:TERM_Optimise
  rdf:type itil:GlossaryConcept ;
  rdfs:label "Optimise" ;
  skos:definition "Review, Plan and request Changes, in order to obtain the maximum Efficiency and Effectiveness from a Process, Configuration Item, Application etc." ;
  skos:prefLabel "Optimise" ;
.
itil:TERM_Organisation
  rdf:type itil:GlossaryConcept ;
  rdfs:label "Organisation" ;
  skos:definition "A company, legal entity or other institution. Examples of Organisations that are not companies include International Standards Organisation or itSMF. The term Organisation is sometimes used to refer to any entity which has People, Resources and Budgets. For example a Project or Business Unit." ;
  skos:prefLabel "Organisation" ;
.
itil:TERM_Outcome
  rdf:type itil:GlossaryConcept ;
  rdfs:label "Outcome" ;
  skos:definition "The result of carrying out an Activity; following a Process; delivering an IT Service etc. The term Outcome is used to refer to intended results, as well as to actual results. See Objective." ;
  skos:prefLabel "Outcome" ;
.
itil:TERM_Outsourcing
  rdf:type itil:GlossaryConcept ;
  rdfs:label "Outsourcing" ;
  skos:definition "(Service Strategy) Using an External Service Provider to manage IT Services. See Service Sourcing, Type III Service Provider." ;
  skos:prefLabel "Outsourcing" ;
.
itil:TERM_Overhead
  rdf:type itil:GlossaryConcept ;
  rdfs:label "Overhead" ;
  skos:definition "Synonym for Indirect cost" ;
  skos:prefLabel "Overhead" ;
.
itil:TERM_PMBOK
  rdf:type itil:GlossaryConcept ;
  rdfs:label "PMBOK" ;
  skos:definition "A Project management Standard maintained and published by the Project Management Institute. PMBOK stands for Project Management Body of Knowledge. See http://www.pmi.org/ for more information. See PRINCE2." ;
  skos:prefLabel "PMBOK" ;
.
itil:TERM_PRINCE2
  rdf:type itil:GlossaryConcept ;
  rdfs:label "PRINCE2" ;
  skos:definition "The standard UK government methodology for Project management. See http://www.ogc.gov.uk/prince2/ for more information. See PMBOK." ;
  skos:prefLabel "PRINCE2" ;
.
itil:TERM_PRojects_IN_Controlled_Environments
  rdf:type itil:GlossaryConcept ;
  rdfs:label "PRojects IN Controlled Environments (PRINCE2)" ;
  skos:definition "See PRINCE2" ;
  skos:prefLabel "PRojects IN Controlled Environments (PRINCE2)" ;
.
itil:TERM_Pain_Value_Analysis
  rdf:type itil:GlossaryConcept ;
  rdfs:label "Pain Value Analysis" ;
  skos:definition "(Service Operation) A technique used to help identify the Business Impact of one or more Problems. A formula is used to calculate Pain Value based on the number of Users affected, the duration of the Downtime, the Impact on each User, and the cost to the Business (if known)." ;
  skos:prefLabel "Pain Value Analysis" ;
.
itil:TERM_Pareto_Principle
  rdf:type itil:GlossaryConcept ;
  rdfs:label "Pareto Principle" ;
  skos:definition "(Service Operation) A technique used to prioritise Activities. The Pareto Principle says that 80% of the value of any Activity is created with 20% of the effort. Pareto Analysis is also used in Problem Management to prioritise possible Problem causes for investigation." ;
  skos:prefLabel "Pareto Principle" ;
.
itil:TERM_Partnership
  rdf:type itil:GlossaryConcept ;
  rdfs:label "Partnership" ;
  skos:definition "A relationship between two Organisations which involves working closely together for common goals or mutual benefit. The IT Service Provider should have a Partnership with the Business, and with Third Parties who are critical to the delivery of IT Services. See Value Network." ;
  skos:prefLabel "Partnership" ;
.
itil:TERM_Passive_Monitoring
  rdf:type itil:GlossaryConcept ;
  rdfs:label "Passive Monitoring" ;
  skos:definition "(Service Operation) Monitoring of a Configuration Item, an IT Service or a Process that relies on an Alert or notification to discover the current status. See Active Monitoring." ;
  skos:prefLabel "Passive Monitoring" ;
.
itil:TERM_Pattern_of_Business_Activity
  rdf:type itil:GlossaryConcept ;
  rdfs:label "Pattern of Business Activity (PBA)" ;
  skos:definition "(Service Strategy) A Workload profile of one or more Business Activities. Patterns of Business Activity are used to help the IT Service Provider understand and plan for different levels of Business Activity. See User Profile." ;
  skos:prefLabel "Pattern of Business Activity (PBA)" ;
.
itil:TERM_Percentage_utilisation
  rdf:type itil:GlossaryConcept ;
  rdfs:label "Percentage utilisation" ;
  skos:definition "(Service Design) The amount of time that a Component is busy over a given period of time. For example, if a CPU is busy for 1800 seconds in a one hour period, its utilisation is 50%" ;
  skos:prefLabel "Percentage utilisation" ;
.
itil:TERM_Performance
  rdf:type itil:GlossaryConcept ;
  rdfs:label "Performance" ;
  skos:definition "A measure of what is achieved or delivered by a System, person, team, Process, or IT Service." ;
  skos:prefLabel "Performance" ;
.
itil:TERM_Performance_Anatomy
  rdf:type itil:GlossaryConcept ;
  rdfs:label "Performance Anatomy" ;
  skos:definition "(Service Strategy) An approach to Organisational Culture that integrates, and actively manages, leadership and strategy, people development, technology enablement, performance management and innovation." ;
  skos:prefLabel "Performance Anatomy" ;
.
itil:TERM_Performance_Management
  rdf:type itil:GlossaryConcept ;
  rdfs:label "Performance Management" ;
  skos:definition "(Continual Service Improvement) The Process responsible for day-to- day Capacity Management Activities. These include Monitoring, Threshold detection, Performance analysis and Tuning, and implementing Changes related to Performance and Capacity." ;
  skos:prefLabel "Performance Management" ;
.
itil:TERM_Pilot
  rdf:type itil:GlossaryConcept ;
  rdfs:label "Pilot" ;
  skos:definition "(Service Transition) A limited Deployment of an IT Service, a Release or a Process to the Live Environment. A Pilot is used to reduce Risk and to gain User feedback and Acceptance. See Test, Evaluation." ;
  skos:prefLabel "Pilot" ;
.
itil:TERM_Plan
  rdf:type itil:GlossaryConcept ;
  rdfs:label "Plan" ;
  skos:definition "A detailed proposal which describes the Activities and Resources needed to achieve an Objective. For example a Plan to implement a new IT Service or Process. ISO/IEC 20000 requires a Plan for the management of each IT Service Management Process." ;
  skos:prefLabel "Plan" ;
.
itil:TERM_Plan-Do-Check-_Act
  rdf:type itil:GlossaryConcept ;
  rdfs:label "Plan-Do-Check- Act" ;
  skos:definition "(Continual Service Improvement) A four stage cycle for Process management, attributed to Edward Deming. Plan-Do-Check-Act is also called the Deming Cycle. PLAN: Design or revise Processes that support the IT Services. DO: Implement the Plan and manage the Processes. CHECK: Measure the Processes and IT Services, compare with Objectives and produce reports ACT: Plan and implement Changes to improve the Processes." ;
  skos:prefLabel "Plan-Do-Check- Act" ;
.
itil:TERM_Planned_Downtime
  rdf:type itil:GlossaryConcept ;
  rdfs:label "Planned Downtime" ;
  skos:definition "(Service Design) Agreed time when an IT Service will not be available. Planned Downtime is often used for maintenance, upgrades and testing. See Change Window, Downtime." ;
  skos:prefLabel "Planned Downtime" ;
.
itil:TERM_Planning
  rdf:type itil:GlossaryConcept ;
  rdfs:label "Planning" ;
  skos:definition "An Activity responsible for creating one or more Plans. For example, Capacity Planning." ;
  skos:prefLabel "Planning" ;
.
itil:TERM_Policy
  rdf:type itil:GlossaryConcept ;
  rdfs:label "Policy" ;
  skos:definition "Formally documented management expectations and intentions. Policies are used to direct decisions, and to ensure consistent and appropriate development and implementation of Processes, Standards, Roles, Activities, IT Infrastructure etc." ;
  skos:prefLabel "Policy" ;
.
itil:TERM_Portable_Facility
  rdf:type itil:GlossaryConcept ;
  rdfs:label "Portable Facility" ;
  skos:definition "(Service Design) A prefabricated building, or a large vehicle, provided by a Third Party and moved to a site when needed by an IT Service Continuity Plan. See Recovery Option, Fixed Facility." ;
  skos:prefLabel "Portable Facility" ;
.
itil:TERM_Post_Implementation_Review
  rdf:type itil:GlossaryConcept ;
  rdfs:label "Post Implementation Review (PIR)" ;
  skos:definition "A Review that takes place after a Change or a Project has been implemented. A PIR determines if the Change or Project was successful, and identifies opportunities for improvement." ;
  skos:prefLabel "Post Implementation Review (PIR)" ;
.
itil:TERM_Practice
  rdf:type itil:GlossaryConcept ;
  rdfs:label "Practice" ;
  skos:definition "A way of working, or a way in which work must be done. Practices can include Activities, Processes, Functions, Standards and Guidelines. See Best Practice." ;
  skos:prefLabel "Practice" ;
.
itil:TERM_Prerequisite_for_Success
  rdf:type itil:GlossaryConcept ;
  rdfs:label "Prerequisite for Success (PFS)" ;
  skos:definition "An Activity that needs to be completed, or a condition that needs to be met, to enable successful implementation of a Plan or Process. A PFS is often an output from one Process that is a required input to another Process." ;
  skos:prefLabel "Prerequisite for Success (PFS)" ;
.
itil:TERM_Pricing
  rdf:type itil:GlossaryConcept ;
  rdfs:label "Pricing" ;
  skos:definition "(Service Strategy) The Activity for establishing how much Customers will be Charged." ;
  skos:prefLabel "Pricing" ;
.
itil:TERM_Priority
  rdf:type itil:GlossaryConcept ;
  rdfs:label "Priority" ;
  skos:definition "(Service Transition) (Service Operation) A Category used to identify the relative importance of an Incident, Problem or Change. Priority is based on Impact and Urgency, and is used to identify required times for actions to be taken. For example the SLA may state that Priority2 Incidents must be resolved within 12 hours." ;
  skos:prefLabel "Priority" ;
.
itil:TERM_Proactive_Monitoring
  rdf:type itil:GlossaryConcept ;
  rdfs:label "Proactive Monitoring" ;
  skos:definition "(Service Operation) Monitoring that looks for patterns of Events to predict possible future Failures. See Reactive Monitoring." ;
  skos:prefLabel "Proactive Monitoring" ;
.
itil:TERM_Proactive_Problem_Management
  rdf:type itil:GlossaryConcept ;
  rdfs:label "Proactive Problem Management" ;
  skos:definition "(Service Operation) Part of the Problem Management Process. The Objective of Proactive Problem Management is to identify Problems that might otherwise be missed. Proactive Problem Management analyses Incident Records, and uses data collected by other IT Service Management Processes to identify trends or significant Problems." ;
  skos:prefLabel "Proactive Problem Management" ;
.
itil:TERM_Problem
  rdf:type itil:GlossaryConcept ;
  rdfs:label "Problem" ;
  skos:definition "(Service Operation) A cause of one or more Incidents. The cause is not usually known at the time a Problem Record is created, and the Problem Management Process is responsible for further investigation." ;
  skos:prefLabel "Problem" ;
.
itil:TERM_Problem_Management
  rdf:type itil:GlossaryConcept ;
  rdfs:label "Problem Management" ;
  skos:definition "(Service Operation) The Process responsible for managing the Lifecycle of all Problems. The primary Objectives of Problem Management are to prevent Incidents from happening, and to minimise the Impact of Incidents that cannot be prevented." ;
  skos:prefLabel "Problem Management" ;
.
itil:TERM_Problem_Record
  rdf:type itil:GlossaryConcept ;
  rdfs:label "Problem Record" ;
  skos:definition "(Service Operation) A Record containing the details of a Problem. Each Problem Record documents the Lifecycle of a single Problem." ;
  skos:prefLabel "Problem Record" ;
.
itil:TERM_Procedure
  rdf:type itil:GlossaryConcept ;
  rdfs:label "Procedure" ;
  skos:definition "A Document containing steps that specify how to achieve an Activity. Procedures are defined as part of Processes. See Work Instruction." ;
  skos:prefLabel "Procedure" ;
.
itil:TERM_Process
  rdf:type itil:GlossaryConcept ;
  rdfs:label "Process" ;
  skos:definition "A structured set of Activities designed to accomplish a specific Objective. A Process takes one or more defined inputs and turns them into defined outputs. A Process may include any of the Roles, responsibilities, tools and management Controls required to reliably deliver the outputs. A Process may define Policies, Standards, Guidelines, Activities, and Work Instructions if they are needed." ;
  skos:prefLabel "Process" ;
.
itil:TERM_Process_Control
  rdf:type itil:GlossaryConcept ;
  rdfs:label "Process Control" ;
  skos:definition "The Activity of planning and regulating a Process, with the Objective of performing the Process in an Effective, Efficient, and consistent manner." ;
  skos:prefLabel "Process Control" ;
.
itil:TERM_Process_Manager
  rdf:type itil:GlossaryConcept ;
  rdfs:label "Process Manager" ;
  skos:definition "A Role responsible for Operational management of a Process. The Process Manager's responsibilities include Planning and co-ordination of all Activities required to carry out, monitor and report on the Process. There may be several Process Managers for one Process, for example regional Change Managers or IT Service Continuity Managers for each data centre. The Process Manager Role is often assigned to the person who carries out the Process Owner Role, but the two Roles may be separate in larger Organisations." ;
  skos:prefLabel "Process Manager" ;
.
itil:TERM_Process_Owner
  rdf:type itil:GlossaryConcept ;
  rdfs:label "Process Owner" ;
  skos:definition "A Role responsible for ensuring that a Process is Fit for Purpose. The Process Owner�s responsibilities include sponsorship, Design, Change Management and continual improvement of the Process and its Metrics. This Role is often assigned to the same person who carries out the Process Manager Role, but the two Roles may be separate in larger Organisations." ;
  skos:prefLabel "Process Owner" ;
.
itil:TERM_Production_Environment
  rdf:type itil:GlossaryConcept ;
  rdfs:label "Production Environment" ;
  skos:definition "Synonym for Live Environment." ;
  skos:prefLabel "Production Environment" ;
.
itil:TERM_Profit_Centre
  rdf:type itil:GlossaryConcept ;
  rdfs:label "Profit Centre" ;
  skos:definition "(Service Strategy) A Business Unit which charges for Services provided. A Profit Centre can be created with the objective of making a profit, recovering Costs, or running at a loss. An IT Service Provider can be run as a Cost Centre or a Profit Centre." ;
  skos:prefLabel "Profit Centre" ;
.
itil:TERM_Programme
  rdf:type itil:GlossaryConcept ;
  rdfs:label "Programme" ;
  skos:definition "A number of Projects and Activities that are planned and managed together to achieve an overall set of related Objectives and other Outcomes." ;
  skos:prefLabel "Programme" ;
.
itil:TERM_Project
  rdf:type itil:GlossaryConcept ;
  rdfs:label "Project" ;
  skos:definition "A temporary Organisation, with people and other Assets required to achieve an Objective or other Outcome. Each Project has a Lifecycle that typically includes initiation, Planning, execution, Closure etc. Projects are usually managed using a formal methodology such as PRINCE2." ;
  skos:prefLabel "Project" ;
.
itil:TERM_Projected_Service_Outage
  rdf:type itil:GlossaryConcept ;
  rdfs:label "Projected Service Outage (PSO)" ;
  skos:definition "(Service Transition) A Document that identifies the effect of planned Changes, maintenance Activities and Test Plans on agreed Service Levels." ;
  skos:prefLabel "Projected Service Outage (PSO)" ;
.
itil:TERM_Qualification
  rdf:type itil:GlossaryConcept ;
  rdfs:label "Qualification" ;
  skos:definition "(Service Transition) An Activity that ensures that IT Infrastructure is appropriate, and correctly configured, to support an Application or IT Service. See Validation." ;
  skos:prefLabel "Qualification" ;
.
itil:TERM_Quality
  rdf:type itil:GlossaryConcept ;
  rdfs:label "Quality" ;
  skos:definition "The ability of a product, Service, or Process to provide the intended value. For example, a hardware Component can be considered to be of high Quality if it performs as expected and delivers the required Reliability. Process Quality also requires an ability to monitor Effectiveness and Efficiency, and to improve them if necessary. See Quality Management System." ;
  skos:prefLabel "Quality" ;
.
itil:TERM_Quality_Assurance
  rdf:type itil:GlossaryConcept ;
  rdfs:label "Quality Assurance (QA)" ;
  skos:definition "(Service Transition) The Process responsible for ensuring that the Quality of a product, Service or Process will provide its intended Value." ;
  skos:prefLabel "Quality Assurance (QA)" ;
.
itil:TERM_Quality_Management_System
  rdf:type itil:GlossaryConcept ;
  rdfs:label "Quality Management System (QMS)" ;
  skos:definition "(Continual Service Improvement) The set of Processes responsible for ensuring that all work carried out by an Organisation is of a suitable Quality to reliably meet Business Objectives or Service Levels. See ISO 9000." ;
  skos:prefLabel "Quality Management System (QMS)" ;
.
itil:TERM_Quick_Win
  rdf:type itil:GlossaryConcept ;
  rdfs:label "Quick Win" ;
  skos:definition "(Continual Service Improvement) An improvement Activity which is expected to provide a Return on Investment in a short period of time with relatively small Cost and effort. See Pareto Principle." ;
  skos:prefLabel "Quick Win" ;
.
itil:TERM_RACI
  rdf:type itil:GlossaryConcept ;
  rdfs:label "RACI" ;
  skos:definition "(Service Design) (Continual Service Improvement) A Model used to help define Roles and Responsibilities. RACI stands for Responsible, Accountable, Consulted and Informed. See Stakeholder." ;
  skos:prefLabel "RACI" ;
.
itil:TERM_Reactive_Monitoring
  rdf:type itil:GlossaryConcept ;
  rdfs:label "Reactive Monitoring" ;
  skos:definition "(Service Operation) Monitoring that takes action in response to an Event. For example submitting a batch job when the previous job completes, or logging an Incident when an Error occurs. See Proactive Monitoring." ;
  skos:prefLabel "Reactive Monitoring" ;
.
itil:TERM_Reciprocal_Arrangement
  rdf:type itil:GlossaryConcept ;
  rdfs:label "Reciprocal Arrangement" ;
  skos:definition "(Service Design) A Recovery Option. An agreement between two Organisations to share resources in an emergency. For example, Computer Room space or use of a mainframe." ;
  skos:prefLabel "Reciprocal Arrangement" ;
.
itil:TERM_Record
  rdf:type itil:GlossaryConcept ;
  rdfs:label "Record" ;
  skos:definition "A Document containing the results or other output from a Process or Activity. Records are evidence of the fact that an Activity took place and may be paper or electronic. For example, an Audit report, an Incident Record, or the minutes of a meeting." ;
  skos:prefLabel "Record" ;
.
itil:TERM_Recovery
  rdf:type itil:GlossaryConcept ;
  rdfs:label "Recovery" ;
  skos:definition "(Service Design) (Service Operation) Returning a Configuration Item or an IT Service to a working state. Recovery of an IT Service often includes recovering data to a known consistent state. After Recovery, further steps may be needed before the IT Service can be made available to the Users (Restoration)." ;
  skos:prefLabel "Recovery" ;
.
itil:TERM_Recovery_Option
  rdf:type itil:GlossaryConcept ;
  rdfs:label "Recovery Option" ;
  skos:definition "(Service Design) A Strategy for responding to an interruption to Service. Commonly used Strategies are Do Nothing, Manual Workaround, Reciprocal Arrangement, Gradual Recovery, Intermediate Recovery, Fast Recovery, Immediate Recovery. Recovery Options may make use of dedicated facilities, or Third Party facilities shared by multiple Businesses." ;
  skos:prefLabel "Recovery Option" ;
.
itil:TERM_Recovery_Point_Objective
  rdf:type itil:GlossaryConcept ;
  rdfs:label "Recovery Point Objective (RPO)" ;
  skos:definition "(Service Operation) The maximum amount of data that may be lost when Service is Restored after an interruption. Recovery Point Objective is expressed as a length of time before the Failure. For example a Recovery Point Objective of one day may be supported by daily Backups, and up to 24 hours of data may be lost. Recovery Point Objectives for each IT Service should be negotiated, agreed and documented, and used as Requirements for Service Design and IT Service Continuity Plans." ;
  skos:prefLabel "Recovery Point Objective (RPO)" ;
.
itil:TERM_Recovery_Time_Objective
  rdf:type itil:GlossaryConcept ;
  rdfs:label "Recovery Time Objective (RTO)" ;
  skos:definition "(Service Operation) The maximum time allowed for recovery of an IT Service following an interruption. The Service Level to be provided may be less than normal Service Level Targets. Recovery Time Objectives for each IT Service should be negotiated, agreed and documented. See Business Impact Analysis." ;
  skos:prefLabel "Recovery Time Objective (RTO)" ;
.
itil:TERM_Redundancy
  rdf:type itil:GlossaryConcept ;
  rdfs:label "Redundancy" ;
  skos:definition "Synonym for Fault Tolerance. The term Redundant also has a generic meaning of obsolete, or no longer needed." ;
  skos:prefLabel "Redundancy" ;
.
itil:TERM_Relationship
  rdf:type itil:GlossaryConcept ;
  rdfs:label "Relationship" ;
  skos:definition "A connection or interaction between two people or things. In Business Relationship Management it is the interaction between the IT Service Provider and the Business. In Configuration Management it is a link between two Configuration Items that identifies a dependency or connection between them. For example Applications may be linked to the Servers they run on, IT Services have many links to all the CIs that contribute to them." ;
  skos:prefLabel "Relationship" ;
.
itil:TERM_Relationship_Processes
  rdf:type itil:GlossaryConcept ;
  rdfs:label "Relationship Processes" ;
  skos:definition "The ISO/IEC 20000 Process group that includes Business Relationship Management and Supplier Management." ;
  skos:prefLabel "Relationship Processes" ;
.
itil:TERM_Release
  rdf:type itil:GlossaryConcept ;
  rdfs:label "Release" ;
  skos:definition "(Service Transition) A collection of hardware, software, documentation, Processes or other Components required to implement one or more approved Changes to IT Services. The contents of each Release are managed, Tested, and Deployed as a single entity." ;
  skos:prefLabel "Release" ;
.
itil:TERM_Release_Identification
  rdf:type itil:GlossaryConcept ;
  rdfs:label "Release Identification" ;
  skos:definition "(Service Transition) A naming convention used to uniquely identify a Release. The Release Identification typically includes a reference to the Configuration Item and a version number. For example Microsoft Office 2003 SR2." ;
  skos:prefLabel "Release Identification" ;
.
itil:TERM_Release_Management
  rdf:type itil:GlossaryConcept ;
  rdfs:label "Release Management" ;
  skos:definition "(Service Transition) The Process responsible for Planning, scheduling and controlling the movement of Releases to Test and Live Environments. The primary Objective of Release Management is to ensure that the integrity of the Live Environment is protected and that the correct Components are released. Release Management is part of the Release and Deployment Management Process." ;
  skos:prefLabel "Release Management" ;
.
itil:TERM_Release_Process
  rdf:type itil:GlossaryConcept ;
  rdfs:label "Release Process" ;
  skos:definition "The name used by ISO/IEC 20000 for the Process group that includes Release Management. This group does not include any other Processes. Release Process is also used as a synonym for Release Management Process." ;
  skos:prefLabel "Release Process" ;
.
itil:TERM_Release_Record
  rdf:type itil:GlossaryConcept ;
  rdfs:label "Release Record" ;
  skos:definition "(Service Transition) A Record in the CMDB that defines the content of a Release. A Release Record has Relationships with all Configuration Items that are affected by the Release." ;
  skos:prefLabel "Release Record" ;
.
itil:TERM_Release_Unit
  rdf:type itil:GlossaryConcept ;
  rdfs:label "Release Unit" ;
  skos:definition "(Service Transition) Components of an IT Service that are normally Released together. A Release Unit typically includes sufficient Components to perform a useful Function. For example one Release Unit could be a Desktop PC, including Hardware, Software, Licenses, Documentation etc. A different Release Unit may be the complete Payroll Application, including IT Operations Procedures and User training." ;
  skos:prefLabel "Release Unit" ;
.
itil:TERM_Release_Window
  rdf:type itil:GlossaryConcept ;
  rdfs:label "Release Window" ;
  skos:definition "Synonym for Change Window." ;
  skos:prefLabel "Release Window" ;
.
itil:TERM_Release_and_Deployment_Management
  rdf:type itil:GlossaryConcept ;
  rdfs:label "Release and Deployment Management" ;
  skos:definition "(Service Transition) The Process responsible for both Release Management and Deployment." ;
  skos:prefLabel "Release and Deployment Management" ;
.
itil:TERM_Reliability
  rdf:type itil:GlossaryConcept ;
  rdfs:label "Reliability" ;
  skos:definition "(Service Design) (Continual Service Improvement) A measure of how long a Configuration Item or IT Service can perform its agreed Function without interruption. Usually measured as MTBF or MTBSI. The term Reliability can also be used to state how likely it is that a Process, Function etc. will deliver its required outputs. See Availability." ;
  skos:prefLabel "Reliability" ;
.
itil:TERM_Remediation
  rdf:type itil:GlossaryConcept ;
  rdfs:label "Remediation" ;
  skos:definition "(Service Transition) Recovery to a known state after a failed Change or Release." ;
  skos:prefLabel "Remediation" ;
.
itil:TERM_Repair
  rdf:type itil:GlossaryConcept ;
  rdfs:label "Repair" ;
  skos:definition "(Service Operation) The replacement or correction of a failed Configuration Item." ;
  skos:prefLabel "Repair" ;
.
itil:TERM_Reporting
  rdf:type itil:GlossaryConcept ;
  rdfs:label "Reporting" ;
  skos:prefLabel "Reporting" ;
.
itil:TERM_Request_Fulfilment
  rdf:type itil:GlossaryConcept ;
  rdfs:label "Request Fulfilment" ;
  skos:definition "(Service Operation) The Process responsible for managing the Lifecycle of all Service Requests." ;
  skos:prefLabel "Request Fulfilment" ;
.
itil:TERM_Request_for_Change
  rdf:type itil:GlossaryConcept ;
  rdfs:label "Request for Change (RFC)" ;
  skos:definition "(Service Transition) A formal proposal for a Change to be made. An RFC includes details of the proposed Change, and may be recorded on paper or electronically. The term RFC is often misused to mean a Change Record, or the Change itself." ;
  skos:prefLabel "Request for Change (RFC)" ;
.
itil:TERM_Requirement
  rdf:type itil:GlossaryConcept ;
  rdfs:label "Requirement" ;
  skos:definition "(Service Design) A formal statement of what is needed. For example a Service Level Requirement, a Project Requirement or the required Deliverables for a Process. See Statement of Requirements." ;
  skos:prefLabel "Requirement" ;
.
itil:TERM_Resilience
  rdf:type itil:GlossaryConcept ;
  rdfs:label "Resilience" ;
  skos:definition "(Service Design) The ability of a Configuration Item or IT Service to resist Failure or to Recover quickly following a Failure. For example, an armoured cable will resist failure when put under stress. See Fault Tolerance." ;
  skos:prefLabel "Resilience" ;
.
itil:TERM_Resolution
  rdf:type itil:GlossaryConcept ;
  rdfs:label "Resolution" ;
  skos:definition "(Service Operation) Action taken to repair the Root Cause of an Incident or Problem, or to implement a Workaround. In ISO/IEC 20000, Resolution Processes is the Process group that includes Incident and Problem Management." ;
  skos:prefLabel "Resolution" ;
.
itil:TERM_Resolution_Processes
  rdf:type itil:GlossaryConcept ;
  rdfs:label "Resolution Processes" ;
  skos:definition "The ISO/IEC 20000 Process group that includes Incident Management and Problem Management." ;
  skos:prefLabel "Resolution Processes" ;
.
itil:TERM_Resource
  rdf:type itil:GlossaryConcept ;
  rdfs:label "Resource" ;
  skos:definition "(Service Strategy) A generic term that includes IT Infrastructure, people, money or anything else that might help to deliver an IT Service. Resources are considered to be Assets of an Organisation. See Capability, Service Asset." ;
  skos:prefLabel "Resource" ;
.
itil:TERM_Response_Time
  rdf:type itil:GlossaryConcept ;
  rdfs:label "Response Time" ;
  skos:definition "A measure of the time taken to complete an Operation or Transaction. Used in Capacity Management as a measure of IT Infrastructure Performance, and in Incident Management as a measure of the time taken to answer the phone, or to start Diagnosis." ;
  skos:prefLabel "Response Time" ;
.
itil:TERM_Responsiveness
  rdf:type itil:GlossaryConcept ;
  rdfs:label "Responsiveness" ;
  skos:definition "A measurement of the time taken to respond to something. This could be Response Time of a Transaction, or the speed with which an IT Service Provider responds to an Incident or Request for Change etc." ;
  skos:prefLabel "Responsiveness" ;
.
itil:TERM_Restoration_of_Service
  rdf:type itil:GlossaryConcept ;
  rdfs:label "Restoration of Service" ;
  skos:definition "See Restore." ;
  skos:prefLabel "Restoration of Service" ;
.
itil:TERM_Restore
  rdf:type itil:GlossaryConcept ;
  rdfs:label "Restore" ;
  skos:definition "(Service Operation) Taking action to return an IT Service to the Users after Repair and Recovery from an Incident. This is the primary Objective of Incident Management." ;
  skos:prefLabel "Restore" ;
.
itil:TERM_Retire
  rdf:type itil:GlossaryConcept ;
  rdfs:label "Retire" ;
  skos:definition "(Service Transition) Permanent removal of an IT Service, or other Configuration Item, from the Live Environment. Retired is a stage in the Lifecycle of many Configuration Items." ;
  skos:prefLabel "Retire" ;
.
itil:TERM_Return_on_Investment
  rdf:type itil:GlossaryConcept ;
  rdfs:label "Return on Investment (ROI)" ;
  skos:definition "(Service Strategy) (Continual Service Improvement) A measurement of the expected benefit of an investment. In the simplest sense it is the net profit of an investment divided by the net worth of the assets invested. See Net Present Value, Value on Investment." ;
  skos:prefLabel "Return on Investment (ROI)" ;
.
itil:TERM_Return_to_Normal
  rdf:type itil:GlossaryConcept ;
  rdfs:label "Return to Normal" ;
  skos:definition "(Service Design) The phase of an IT Service Continuity Plan during which full normal operations are resumed. For example, if an alternate data centre has been in use, then this phase will bring the primary data centre back into operation, and restore the ability to invoke IT Service Continuity Plans again." ;
  skos:prefLabel "Return to Normal" ;
.
itil:TERM_Review
  rdf:type itil:GlossaryConcept ;
  rdfs:label "Review" ;
  skos:definition "An evaluation of a Change, Problem, Process, Project etc. Reviews are typically carried out at predefined points in the Lifecycle, and especially after Closure. The purpose of a Review is to ensure that all Deliverables have been provided, and to identify opportunities for improvement. See Post Implementation Review." ;
  skos:prefLabel "Review" ;
.
itil:TERM_Rights
  rdf:type itil:GlossaryConcept ;
  rdfs:label "Rights" ;
  skos:definition "(Service Operation) Entitlements, or permissions, granted to a User or Role. For example the Right to modify particular data, or to authorize a Change." ;
  skos:prefLabel "Rights" ;
.
itil:TERM_Risk
  rdf:type itil:GlossaryConcept ;
  rdfs:label "Risk" ;
  skos:definition "A possible Event that could cause harm or loss, or affect the ability to achieve Objectives. A Risk is measured by the probability of a Threat, the Vulnerability of the Asset to that Threat, and the Impact it would have if it occurred." ;
  skos:prefLabel "Risk" ;
.
itil:TERM_Risk_Assessment
  rdf:type itil:GlossaryConcept ;
  rdfs:label "Risk Assessment" ;
  skos:definition "The initial steps of Risk Management. Analysing the value of Assets to the business, identifying Threats to those Assets, and evaluating how Vulnerable each Asset is to those Threats. Risk Assessment can be quantitative (based on numerical data) or qualitative." ;
  skos:prefLabel "Risk Assessment" ;
.
itil:TERM_Risk_Management
  rdf:type itil:GlossaryConcept ;
  rdfs:label "Risk Management" ;
  skos:definition "The Process responsible for identifying, assessing and controlling Risks. See Risk Assessment." ;
  skos:prefLabel "Risk Management" ;
.
itil:TERM_Role
  rdf:type itil:GlossaryConcept ;
  rdfs:label "Role" ;
  skos:definition "A set of responsibilities, Activities and authorities granted to a person or team. A Role is defined in a Process. One person or team may have multiple Roles, for example the Roles of Configuration Manager and Change Manager may be carried out by a single person." ;
  skos:prefLabel "Role" ;
.
itil:TERM_Rollout
  rdf:type itil:GlossaryConcept ;
  rdfs:label "Rollout" ;
  skos:definition "(Service Transition) Synonym for Deployment. Most often used to refer to complex or phased Deployments or Deployments to multiple locations." ;
  skos:prefLabel "Rollout" ;
.
itil:TERM_Root_Cause
  rdf:type itil:GlossaryConcept ;
  rdfs:label "Root Cause" ;
  skos:definition "(Service Operation) The underlying or original cause of an Incident or Problem." ;
  skos:prefLabel "Root Cause" ;
.
itil:TERM_Root_Cause_Analysis
  rdf:type itil:GlossaryConcept ;
  rdfs:label "Root Cause Analysis (RCA)" ;
  skos:definition "(Service Operation) An Activity that identifies the Root Cause of an Incident or Problem. RCA typically concentrates on IT Infrastructure failures. See Service Failure Analysis." ;
  skos:prefLabel "Root Cause Analysis (RCA)" ;
.
itil:TERM_Running_Costs
  rdf:type itil:GlossaryConcept ;
  rdfs:label "Running Costs" ;
  skos:definition "Synonym for Operational Costs" ;
  skos:prefLabel "Running Costs" ;
.
itil:TERM_SLAM_Chart
  rdf:type itil:GlossaryConcept ;
  rdfs:label "SLAM Chart" ;
  skos:definition "(Continual Service Improvement) A Service Level Agreement Monitoring Chart is used to help monitor and report achievements against Service Level Targets. A SLAM Chart is typically colour coded to show whether each agreed Service Level Target has been met, missed, or nearly missed during each of the previous 12 months." ;
  skos:prefLabel "SLAM Chart" ;
.
itil:TERM_SMART
  rdf:type itil:GlossaryConcept ;
  rdfs:label "SMART" ;
  skos:definition "(Service Design) (Continual Service Improvement) An acronym for helping to remember that targets in Service Level Agreements and Project Plans should be Specific, Measurable, Achievable, Relevant and Timely." ;
  skos:prefLabel "SMART" ;
.
itil:TERM_SWOT_Analysis
  rdf:type itil:GlossaryConcept ;
  rdfs:label "SWOT Analysis" ;
  skos:definition "(Continual Service Improvement) A technique that reviews and analyses the internal strengths and weaknesses of an Organisation and the external opportunities and threats which it faces SWOT stands for Strengths, Weaknesses, Opportunities and Threats." ;
  skos:prefLabel "SWOT Analysis" ;
.
itil:TERM_Scalability
  rdf:type itil:GlossaryConcept ;
  rdfs:label "Scalability" ;
  skos:definition "The ability of an IT Service, Process, Configuration Item etc. to perform its agreed Function when the Workload or Scope changes." ;
  skos:prefLabel "Scalability" ;
.
itil:TERM_Scope
  rdf:type itil:GlossaryConcept ;
  rdfs:label "Scope" ;
  skos:definition "The boundary, or extent, to which a Process, Procedure, Certification, Contract etc. applies. For example the Scope of Change Management may include all Live IT Services and related Configuration Items, the Scope of an ISO/IEC 20000 Certificate may include all IT Services delivered out of a named data centre." ;
  skos:prefLabel "Scope" ;
.
itil:TERM_Second-line_Support
  rdf:type itil:GlossaryConcept ;
  rdfs:label "Second-line Support" ;
  skos:definition "(Service Operation) The second level in a hierarchy of Support Groups involved in the resolution of Incidents and investigation of Problems. Each level contains more specialist skills, or has more time or other Resources." ;
  skos:prefLabel "Second-line Support" ;
.
itil:TERM_Security
  rdf:type itil:GlossaryConcept ;
  rdfs:label "Security" ;
  skos:definition "See Information Security Management" ;
  skos:prefLabel "Security" ;
.
itil:TERM_Security_Management
  rdf:type itil:GlossaryConcept ;
  rdfs:label "Security Management" ;
  skos:definition "Synonym for Information Security Management" ;
  skos:prefLabel "Security Management" ;
.
itil:TERM_Security_Policy
  rdf:type itil:GlossaryConcept ;
  rdfs:label "Security Policy" ;
  skos:definition "Synonym for Information Security Policy" ;
  skos:prefLabel "Security Policy" ;
.
itil:TERM_Separation_of_Concerns
  rdf:type itil:GlossaryConcept ;
  rdfs:label "Separation of Concerns (SoC)" ;
  skos:definition "(Service Strategy) An approach to Designing a solution or IT Service that divides the problem into pieces that can be solved independently. This approach separates \"what\" is to be done from \"how\" it is to be done." ;
  skos:prefLabel "Separation of Concerns (SoC)" ;
.
itil:TERM_Server
  rdf:type itil:GlossaryConcept ;
  rdfs:label "Server" ;
  skos:definition "(Service Operation) A computer that is connected to a network and provides software Functions that are used by other computers." ;
  skos:prefLabel "Server" ;
.
itil:TERM_Service
  rdf:type itil:GlossaryConcept ;
  rdfs:label "Service" ;
  skos:definition "A means of delivering value to Customers by facilitating Outcomes Customers want to achieve without the ownership of specific Costs and Risks." ;
  skos:prefLabel "Service" ;
.
itil:TERM_Service_Acceptance_Criteria
  rdf:type itil:GlossaryConcept ;
  rdfs:label "Service Acceptance Criteria (SAC)" ;
  skos:definition "(Service Transition) A set of criteria used to ensure that an IT Service meets its functionality and Quality Requirements and that the IT Service Provider is ready to Operate the new IT Service when it has been Deployed. See Acceptance." ;
  skos:prefLabel "Service Acceptance Criteria (SAC)" ;
.
itil:TERM_Service_Analytics
  rdf:type itil:GlossaryConcept ;
  rdfs:label "Service Analytics" ;
  skos:definition "(Service Strategy) A technique used in the Assessment of the Business Impact of Incidents. Service Analytics Models the dependencies between Configuration Items, and the dependencies of IT Services on Configuration Items." ;
  skos:prefLabel "Service Analytics" ;
.
itil:TERM_Service_Asset
  rdf:type itil:GlossaryConcept ;
  rdfs:label "Service Asset" ;
  skos:definition "Any Capability or Resource of a Service Provider. See Asset." ;
  skos:prefLabel "Service Asset" ;
.
itil:TERM_Service_Asset_and_Configuration_Management
  rdf:type itil:GlossaryConcept ;
  rdfs:label "Service Asset and Configuration Management (SACM)" ;
  skos:definition "(Service Transition) The Process responsible for both Configuration Management and Asset Management." ;
  skos:prefLabel "Service Asset and Configuration Management (SACM)" ;
.
itil:TERM_Service_Capacity_Management
  rdf:type itil:GlossaryConcept ;
  rdfs:label "Service Capacity Management (SCM)" ;
  skos:definition "(Service Design) (Continual Service Improvement) The Activity responsible for understanding the Performance and Capacity of IT Services. The Resources used by each IT Service and the pattern of usage over time are collected, recorded, and analysed for use in the Capacity Plan. See Business Capacity Management, Component Capacity Management." ;
  skos:prefLabel "Service Capacity Management (SCM)" ;
.
itil:TERM_Service_Catalogue
  rdf:type itil:GlossaryConcept ;
  rdfs:label "Service Catalogue" ;
  skos:definition "(Service Design) A database or structured Document with information about all Live IT Services, including those available for Deployment. The Service Catalogue is the only part of the Service Portfolio published to Customers, and is used to support the sale and delivery of IT Services. The Service Catalogue includes information about deliverables, prices, contact points, ordering and request Processes. See Contract Portfolio." ;
  skos:prefLabel "Service Catalogue" ;
.
itil:TERM_Service_Continuity_Management
  rdf:type itil:GlossaryConcept ;
  rdfs:label "Service Continuity Management" ;
  skos:definition "Synonym for IT Service Continuity Management." ;
  skos:prefLabel "Service Continuity Management" ;
.
itil:TERM_Service_Contract
  rdf:type itil:GlossaryConcept ;
  rdfs:label "Service Contract" ;
  skos:definition "(Service Strategy) A Contract to deliver one or more IT Services. The term Service Contract is also used to mean any Agreement to deliver IT Services, whether this is a legal Contract or an SLA. See Contract Portfolio." ;
  skos:prefLabel "Service Contract" ;
.
itil:TERM_Service_Culture
  rdf:type itil:GlossaryConcept ;
  rdfs:label "Service Culture" ;
  skos:definition "A Customer oriented Culture. The major Objectives of a Service Culture are Customer satisfaction and helping the Customer to achieve their Business Objectives." ;
  skos:prefLabel "Service Culture" ;
.
itil:TERM_Service_Design
  rdf:type itil:GlossaryConcept ;
  rdfs:label "Service Design" ;
  skos:definition "(Service Design) A stage in the Lifecycle of an IT Service. Service Design includes a number of Processes and Functions and is the title of one of the Core ITIL publications. See Design." ;
  skos:prefLabel "Service Design" ;
.
itil:TERM_Service_Design_Package
  rdf:type itil:GlossaryConcept ;
  rdfs:label "Service Design Package" ;
  skos:definition "(Service Design) Document(s) defining all aspects of an IT Service and its Requirements through each stage of its Lifecycle. A Service Design Package is produced for each new IT Service, major Change, or IT Service Retirement." ;
  skos:prefLabel "Service Design Package" ;
.
itil:TERM_Service_Desk
  rdf:type itil:GlossaryConcept ;
  rdfs:label "Service Desk" ;
  skos:definition "(Service Operation) The Single Point of Contact between the Service Provider and the Users. A typical Service Desk manages Incidents and Service Requests, and also handles communication with the Users." ;
  skos:prefLabel "Service Desk" ;
.
itil:TERM_Service_Failure_Analysis
  rdf:type itil:GlossaryConcept ;
  rdfs:label "Service Failure Analysis (SFA)" ;
  skos:broader itil:TERM_Root_Cause_Analysis ;
  skos:definition "(Service Design) An Activity that identifies underlying causes of one or more IT Service interruptions. SFA identifies opportunities to improve the IT Service Provider's Processes and tools, and not just the IT Infrastructure. SFA is a time constrained, project-like activity, rather than an ongoing process of analysis. See Root Cause Analysis." ;
  skos:prefLabel "Service Failure Analysis (SFA)" ;
.
itil:TERM_Service_Hours
  rdf:type itil:GlossaryConcept ;
  rdfs:label "Service Hours" ;
  skos:definition "(Service Design) (Continual Service Improvement) An agreed time period when a particular IT Service should be Available. For example, \"Monday-Friday 08:00 to 17:00 except public holidays\". Service Hours should be defined in a Service Level Agreement." ;
  skos:prefLabel "Service Hours" ;
.
itil:TERM_Service_Improvement_Plan
  rdf:type itil:GlossaryConcept ;
  rdfs:label "Service Improvement Plan (SIP)" ;
  skos:definition "(Continual Service Improvement) A formal Plan to implement improvements to a Process or IT Service." ;
  skos:prefLabel "Service Improvement Plan (SIP)" ;
.
itil:TERM_Service_Knowledge_Management_System
  rdf:type itil:GlossaryConcept ;
  rdfs:label "Service Knowledge Management System (SKMS)" ;
  skos:definition "(Service Transition) A set of tools and databases that are used to manage knowledge and information. The SKMS includes the Configuration Management System, as well as other tools and databases. The SKMS stores, manages, updates, and presents all information that an IT Service Provider needs to manage the full Lifecycle of IT Services." ;
  skos:prefLabel "Service Knowledge Management System (SKMS)" ;
.
itil:TERM_Service_Level
  rdf:type itil:GlossaryConcept ;
  rdfs:label "Service Level" ;
  skos:definition "Measured and reported achievement against one or more Service Level Targets. The term Service Level is sometimes used informally to mean Service Level Target." ;
  skos:prefLabel "Service Level" ;
.
itil:TERM_Service_Level_Agreement
  rdf:type itil:GlossaryConcept ;
  rdfs:label "Service Level Agreement (SLA)" ;
  skos:broader itil:TERM_Operational_Level_Agreement ;
  skos:definition "(Service Design) (Continual Service Improvement) An Agreement between an IT Service Provider and a Customer. The SLA describes the IT Service, documents Service Level Targets, and specifies the responsibilities of the IT Service Provider and the Customer. A single SLA may cover multiple IT Services or multiple Customers. See Operational Level Agreement." ;
  skos:prefLabel "Service Level Agreement (SLA)" ;
.
itil:TERM_Service_Level_Management
  rdf:type itil:GlossaryConcept ;
  rdfs:label "Service Level Management (SLM)" ;
  skos:definition "(Service Design) (Continual Service Improvement) The Process responsible for negotiating Service Level Agreements, and ensuring that these are met. SLM is responsible for ensuring that all IT Service Management Processes, Operational Level Agreements, and Underpinning Contracts, are appropriate for the agreed Service Level Targets. SLM monitors and reports on Service Levels, and holds regular Customer reviews." ;
  skos:prefLabel "Service Level Management (SLM)" ;
.
itil:TERM_Service_Level_Package
  rdf:type itil:GlossaryConcept ;
  rdfs:label "Service Level Package (SLP)" ;
  skos:definition "(Service Strategy) A defined level of Utility and Warranty for a particular Service Package. Each SLP is designed to meet the needs of a particular Pattern of Business Activity. See Line of Service." ;
  skos:prefLabel "Service Level Package (SLP)" ;
.
itil:TERM_Service_Level_Requirement
  rdf:type itil:GlossaryConcept ;
  rdfs:label "Service Level Requirement (SLR)" ;
  skos:definition "(Service Design) (Continual Service Improvement) A Customer Requirement for an aspect of an IT Service. SLRs are based on Business Objectives and are used to negotiate agreed Service Level Targets." ;
  skos:prefLabel "Service Level Requirement (SLR)" ;
.
itil:TERM_Service_Level_Target
  rdf:type itil:GlossaryConcept ;
  rdfs:label "Service Level Target" ;
  skos:definition "(Service Design) (Continual Service Improvement) A commitment that is documented in a Service Level Agreement. Service Level Targets are based on Service Level Requirements, and are needed to ensure that the IT Service design is Fit for Purpose. Service Level Targets should be SMART, and are usually based on KPIs." ;
  skos:prefLabel "Service Level Target" ;
.
itil:TERM_Service_Maintenance_Objective
  rdf:type itil:GlossaryConcept ;
  rdfs:label "Service Maintenance Objective" ;
  skos:definition "(Service Operation) The expected time that a Configuration Item will be unavailable due to planned maintenance Activity." ;
  skos:prefLabel "Service Maintenance Objective" ;
.
itil:TERM_Service_Management
  rdf:type itil:GlossaryConcept ;
  rdfs:label "Service Management" ;
  skos:definition "Service Management is a set of specialized organizational capabilities for providing value to customers in the form of services." ;
  skos:prefLabel "Service Management" ;
.
itil:TERM_Service_Management_Lifecycle
  rdf:type itil:GlossaryConcept ;
  rdfs:label "Service Management Lifecycle" ;
  skos:definition "An approach to IT Service Management that emphasizes the importance of coordination and Control across the various Functions, Processes, and Systems necessary to manage the full Lifecycle of IT Services. The Service Management Lifecycle approach considers the Strategy, Design, Transition, Operation and Continuous Improvement of IT Services." ;
  skos:prefLabel "Service Management Lifecycle" ;
.
itil:TERM_Service_Manager
  rdf:type itil:GlossaryConcept ;
  rdfs:label "Service Manager" ;
  skos:definition "A manager who is responsible for managing the end-to-end Lifecycle of one or more IT Services. The term Service Manager is also used to mean any manager within the IT Service Provider. Most commonly used to refer to a Business Relationship Manager, a Process Manager, an Account Manager or a senior manager with responsibility for IT Services overall." ;
  skos:prefLabel "Service Manager" ;
.
itil:TERM_Service_Operation
  rdf:type itil:GlossaryConcept ;
  rdfs:label "Service Operation" ;
  skos:definition "(Service Operation) A stage in the Lifecycle of an IT Service. Service Operation includes a number of Processes and Functions and is the title of one of the Core ITIL publications. See Operation." ;
  skos:prefLabel "Service Operation" ;
.
itil:TERM_Service_Owner
  rdf:type itil:GlossaryConcept ;
  rdfs:label "Service Owner" ;
  skos:definition "(Continual Service Improvement) A Role which is accountable for the delivery of a specific IT Service." ;
  skos:prefLabel "Service Owner" ;
.
itil:TERM_Service_Package
  rdf:type itil:GlossaryConcept ;
  rdfs:label "Service Package" ;
  skos:definition "(Service Strategy) A detailed description of an IT Service that is available to be delivered to Customers. A Service Package includes a Service Level Package and one or more Core Services and Supporting Services." ;
  skos:prefLabel "Service Package" ;
.
itil:TERM_Service_Pipeline
  rdf:type itil:GlossaryConcept ;
  rdfs:label "Service Pipeline" ;
  skos:definition "(Service Strategy) A database or structured Document listing all IT Services that are under consideration or Development, but are not yet available to Customers. The Service Pipeline provides a Business view of possible future IT Services and is part of the Service Portfolio which is not normally published to Customers." ;
  skos:prefLabel "Service Pipeline" ;
.
itil:TERM_Service_Portfolio
  rdf:type itil:GlossaryConcept ;
  rdfs:label "Service Portfolio" ;
  skos:definition "(Service Strategy) The complete set of Services that are managed by a Service Provider. The Service Portfolio is used to manage the entire Lifecycle of all Services, and includes three Categories: Service Pipeline (proposed or in Development); Service Catalogue (Live or available for Deployment); and Retired Services. See Service Portfolio Management, Contract Portfolio." ;
  skos:prefLabel "Service Portfolio" ;
.
itil:TERM_Service_Portfolio_Management
  rdf:type itil:GlossaryConcept ;
  rdfs:label "Service Portfolio Management (SPM)" ;
  skos:definition "(Service Strategy) The Process responsible for managing the Service Portfolio. Service Portfolio Management considers Services in terms of the Business value that they provide." ;
  skos:prefLabel "Service Portfolio Management (SPM)" ;
.
itil:TERM_Service_Potential
  rdf:type itil:GlossaryConcept ;
  rdfs:label "Service Potential" ;
  skos:definition "(Service Strategy) The total possible value of the overall Capabilities and Resources of the IT Service Provider." ;
  skos:prefLabel "Service Potential" ;
.
itil:TERM_Service_Provider
  rdf:type itil:GlossaryConcept ;
  rdfs:label "Service Provider" ;
  skos:definition "(Service Strategy) An Organisation supplying Services to one or more Internal Customers or External Customers. Service Provider is often used as an abbreviation for IT Service Provider. See Type I Service Provider, Type II Service Provider, Type III Service Provider." ;
  skos:prefLabel "Service Provider" ;
.
itil:TERM_Service_Provider_Interface
  rdf:type itil:GlossaryConcept ;
  rdfs:label "Service Provider Interface (SPI)" ;
  skos:definition "(Service Strategy) An interface between the IT Service Provider and a User, Customer, Business Process, or a Supplier. Analysis of Service Provider Interfaces helps to coordinate end-to-end management of IT Services." ;
  skos:prefLabel "Service Provider Interface (SPI)" ;
.
itil:TERM_Service_Provisioning_Optimization
  rdf:type itil:GlossaryConcept ;
  rdfs:label "Service Provisioning Optimization (SPO)" ;
  skos:definition "(Service Strategy) Analysing the finances and constraints of an IT Service to decide if alternative approaches to Service delivery might reduce Costs or improve Quality." ;
  skos:prefLabel "Service Provisioning Optimization (SPO)" ;
.
itil:TERM_Service_Reporting
  rdf:type itil:GlossaryConcept ;
  rdfs:label "Service Reporting" ;
  skos:definition "(Continual Service Improvement) The Process responsible for producing and delivering reports of achievement and trends against Service Levels. Service Reporting should agree the format, content and frequency of reports with Customers." ;
  skos:prefLabel "Service Reporting" ;
.
itil:TERM_Service_Request
  rdf:type itil:GlossaryConcept ;
  rdfs:label "Service Request" ;
  skos:definition "(Service Operation) A request from a User for information, or advice, or for a Standard Change or for Access to an IT Service. For example to reset a password, or to provide standard IT Services for a new User. Service Requests are usually handled by a Service Desk, and do not require an RFC to be submitted. See Request Fulfilment." ;
  skos:prefLabel "Service Request" ;
.
itil:TERM_Service_Sourcing
  rdf:type itil:GlossaryConcept ;
  rdfs:label "Service Sourcing" ;
  skos:definition "(Service Strategy) The Strategy and approach for deciding whether to provide a Service internally or to Outsource it to an External Service Provider. Service Sourcing also means the execution of this Strategy. Service Sourcing includes: � Internal Sourcing - Internal or Shared Services using Type I or Type II Service Providers. � Traditional Sourcing - Full Service Outsourcing using a Type III Service Provider. � Multivendor Sourcing - Prime, Consortium or Selective Outsourcing using Type III Service Providers." ;
  skos:prefLabel "Service Sourcing" ;
.
itil:TERM_Service_Strategy
  rdf:type itil:GlossaryConcept ;
  rdfs:label "Service Strategy" ;
  skos:definition "(Service Strategy) The title of one of the Core ITIL publications. Service Strategy establishes an overall Strategy for IT Services and for IT Service Management." ;
  skos:prefLabel "Service Strategy" ;
.
itil:TERM_Service_Transition
  rdf:type itil:GlossaryConcept ;
  rdfs:label "Service Transition" ;
  skos:definition "(Service Transition) A stage in the Lifecycle of an IT Service. Service Transition includes a number of Processes and Functions and is the title of one of the Core ITIL publications. See Transition." ;
  skos:prefLabel "Service Transition" ;
.
itil:TERM_Service_Utility
  rdf:type itil:GlossaryConcept ;
  rdfs:label "Service Utility" ;
  skos:definition "(Service Strategy) The Functionality of an IT Service from the Customer's perspective. The Business value of an IT Service is created by the combination of Service Utility (what the Service does) and Service Warranty (how well it does it). See Utility." ;
  skos:prefLabel "Service Utility" ;
.
itil:TERM_Service_Validation_and_Testing
  rdf:type itil:GlossaryConcept ;
  rdfs:label "Service Validation and Testing" ;
  skos:definition "(Service Transition) The Process responsible for Validation and Testing of a new or Changed IT Service. Service Validation and Testing ensures that the IT Service matches its Design Specification and will meet the needs of the Business." ;
  skos:prefLabel "Service Validation and Testing" ;
.
itil:TERM_Service_Valuation
  rdf:type itil:GlossaryConcept ;
  rdfs:label "Service Valuation" ;
  skos:definition "(Service Strategy) A measurement of the total Cost of delivering an IT Service, and the total value to the Business of that IT Service. Service Valuation is used to help the Business and the IT Service Provider agree on the value of the IT Service." ;
  skos:prefLabel "Service Valuation" ;
.
itil:TERM_Service_Warranty
  rdf:type itil:GlossaryConcept ;
  rdfs:label "Service Warranty" ;
  skos:definition "(Service Strategy) Assurance that an IT Service will meet agreed Requirements. This may be a formal Agreement such as a Service Level Agreement or Contract, or may be a marketing message or brand image. The Business value of an IT Service is created by the combination of Service Utility (what the Service does) and Service Warranty (how well it does it). See Warranty." ;
  skos:prefLabel "Service Warranty" ;
.
itil:TERM_Serviceability
  rdf:type itil:GlossaryConcept ;
  rdfs:label "Serviceability" ;
  skos:definition "(Service Design) (Continual Service Improvement) The ability of a Third Party Supplier to meet the terms of their Contract. This Contract will include agreed levels of Reliability, Maintainability or Availability for a Configuration Item." ;
  skos:prefLabel "Serviceability" ;
.
itil:TERM_Shift
  rdf:type itil:GlossaryConcept ;
  rdfs:label "Shift" ;
  skos:definition "(Service Operation) A group or team of people who carry out a specific Role for a fixed period of time. For example there could be four shifts of IT Operations Control personnel to support an IT Service that is used 24 hours a day." ;
  skos:prefLabel "Shift" ;
.
itil:TERM_Simulation_modelling
  rdf:type itil:GlossaryConcept ;
  rdfs:label "Simulation modelling" ;
  skos:definition "(Service Design) (Continual Service Improvement) A technique that creates a detailed Model to predict the behaviour of a Configuration Item or IT Service. Simulation Models can be very accurate but are expensive and time consuming to create. A Simulation Model is often created by using the actual Configuration Items that are being modelled, with artificial Workloads or Transactions. They are used in Capacity Management when accurate results are important. A simulation model is sometimes called a Performance Benchmark." ;
  skos:prefLabel "Simulation modelling" ;
.
itil:TERM_Single_Point_of_Contact
  rdf:type itil:GlossaryConcept ;
  rdfs:label "Single Point of Contact" ;
  skos:definition "(Service Operation) Providing a single consistent way to communicate with an Organisation or Business Unit. For example, a Single Point of Contact for an IT Service Provider is usually called a Service Desk." ;
  skos:prefLabel "Single Point of Contact" ;
.
itil:TERM_Single_Point_of_Failure
  rdf:type itil:GlossaryConcept ;
  rdfs:label "Single Point of Failure (SPOF)" ;
  skos:definition "(Service Design) Any Configuration Item that can cause an Incident when it fails, and for which a Countermeasure has not been implemented. A SPOF may be a person, or a step in a Process or Activity, as well as a Component of the IT Infrastructure. See Failure." ;
  skos:prefLabel "Single Point of Failure (SPOF)" ;
.
itil:TERM_Snapshot
  rdf:type itil:GlossaryConcept ;
  rdfs:label "Snapshot" ;
  skos:definition "(Service Transition) The current state of a Configuration as captured by a discovery tool. Also used as a synonym for Benchmark. See Baseline." ;
  skos:prefLabel "Snapshot" ;
.
itil:TERM_Source
  rdf:type itil:GlossaryConcept ;
  rdfs:label "Source" ;
  skos:definition "See Service Sourcing." ;
  skos:prefLabel "Source" ;
.
itil:TERM_Specification
  rdf:type itil:GlossaryConcept ;
  rdfs:label "Specification" ;
  skos:definition "A formal definition of Requirements. A Specification may be used to define technical or Operational Requirements, and may be internal or external. Many public Standards consist of a Code of Practice and a Specification. The Specification defines the Standard against which an Organisation can be Audited." ;
  skos:prefLabel "Specification" ;
.
itil:TERM_Stakeholder
  rdf:type itil:GlossaryConcept ;
  rdfs:label "Stakeholder" ;
  skos:definition "All people who have an interest in an Organisation, Project, IT Service etc. Stakeholders may be interested in the Activities, targets, Resources, or Deliverables. Stakeholders may include Customers, Partners, employees, shareholders, owners, etc. See RACI." ;
  skos:prefLabel "Stakeholder" ;
.
itil:TERM_Standard
  rdf:type itil:GlossaryConcept ;
  rdfs:label "Standard" ;
  skos:definition "A mandatory Requirement. Examples include ISO/IEC 20000 (an international Standard), an internal security Standard for Unix configuration, or a government Standard for how financial Records should be maintained. The term Standard is also used to refer to a Code of Practice or Specification published by a Standards Organisation such as ISO or BSI. See Guideline." ;
  skos:prefLabel "Standard" ;
.
itil:TERM_Standard_Change
  rdf:type itil:GlossaryConcept ;
  rdfs:label "Standard Change" ;
  skos:definition "(Service Transition) A pre-approved Change that is low Risk, relatively common and follows a Procedure or Work Instruction. For example password reset or provision of standard equipment to a new employee. RFCs are not required to implement a Standard Change, and they are logged and tracked using a different mechanism, such as a Service Request. See Change Model." ;
  skos:prefLabel "Standard Change" ;
.
itil:TERM_Standard_Operating_Procedures
  rdf:type itil:GlossaryConcept ;
  rdfs:label "Standard Operating Procedures (SOP)" ;
  skos:definition "(Service Operation) Procedures used by IT Operations Management." ;
  skos:prefLabel "Standard Operating Procedures (SOP)" ;
.
itil:TERM_Standby
  rdf:type itil:GlossaryConcept ;
  rdfs:label "Standby" ;
  skos:definition "(Service Design) Used to refer to Resources that are not required to deliver the Live IT Services, but are available to support IT Service Continuity Plans. For example a Standby data centre may be maintained to support Hot Standby, Warm Standby or Cold Standby arrangements." ;
  skos:prefLabel "Standby" ;
.
itil:TERM_Statement_of_requirements
  rdf:type itil:GlossaryConcept ;
  rdfs:label "Statement of requirements (SOR)" ;
  skos:definition "(Service Design) A Document containing all Requirements for a product purchase, or a new or changed IT Service. See Terms of Reference." ;
  skos:prefLabel "Statement of requirements (SOR)" ;
.
itil:TERM_Status
  rdf:type itil:GlossaryConcept ;
  rdfs:label "Status" ;
  skos:definition "The name of a required field in many types of Record. It shows the current stage in the Lifecycle of the associated Configuration Item, Incident, Problem etc." ;
  skos:prefLabel "Status" ;
.
itil:TERM_Status_Accounting
  rdf:type itil:GlossaryConcept ;
  rdfs:label "Status Accounting" ;
  skos:definition "(Service Transition) The Activity responsible for recording and reporting the Lifecycle of each Configuration Item." ;
  skos:prefLabel "Status Accounting" ;
.
itil:TERM_Storage_Management
  rdf:type itil:GlossaryConcept ;
  rdfs:label "Storage Management" ;
  skos:definition "(Service Operation) The Process responsible for managing the storage and maintenance of data throughout its Lifecycle." ;
  skos:prefLabel "Storage Management" ;
.
itil:TERM_Strategic
  rdf:type itil:GlossaryConcept ;
  rdfs:label "Strategic" ;
  skos:definition "(Service Strategy) The highest of three levels of Planning and delivery (Strategic, Tactical, Operational). Strategic Activities include Objective setting and long term Planning to achieve the overall Vision." ;
  skos:prefLabel "Strategic" ;
.
itil:TERM_Strategy
  rdf:type itil:GlossaryConcept ;
  rdfs:label "Strategy" ;
  skos:definition "(Service Strategy) A Strategic Plan designed to achieve defined Objectives." ;
  skos:prefLabel "Strategy" ;
.
itil:TERM_Super_User
  rdf:type itil:GlossaryConcept ;
  rdfs:label "Super User" ;
  skos:definition "(Service Operation) A User who helps other Users, and assists in communication with the Service Desk or other parts of the IT Service Provider. Super Users typically provide support for minor Incidents and training." ;
  skos:prefLabel "Super User" ;
.
itil:TERM_Supplier
  rdf:type itil:GlossaryConcept ;
  rdfs:label "Supplier" ;
  skos:definition "(Service Strategy) (Service Design) A Third Party responsible for supplying goods or Services that are required to deliver IT services. Examples of suppliers include commodity hardware and software vendors, network and telecom providers, and Outsourcing Organisations. See Underpinning Contract, Supply Chain." ;
  skos:prefLabel "Supplier" ;
.
itil:TERM_Supplier_Management
  rdf:type itil:GlossaryConcept ;
  rdfs:label "Supplier Management" ;
  skos:definition "(Service Design) The Process responsible for ensuring that all Contracts with Suppliers support the needs of the Business, and that all Suppliers meet their contractual commitments." ;
  skos:prefLabel "Supplier Management" ;
.
itil:TERM_Supplier_and_Contract_Database
  rdf:type itil:GlossaryConcept ;
  rdfs:label "Supplier and Contract Database (SCD)" ;
  skos:definition "(Service Design) A database or structured Document used to manage Supplier Contracts throughout their Lifecycle. The SCD contains key Attributes of all Contracts with Suppliers, and should be part of the Service Knowledge Management System." ;
  skos:prefLabel "Supplier and Contract Database (SCD)" ;
.
itil:TERM_Supply_Chain
  rdf:type itil:GlossaryConcept ;
  rdfs:label "Supply Chain" ;
  skos:definition "(Service Strategy) The Activities in a Value Chain carried out by Suppliers. A Supply Chain typically involves multiple Suppliers, each adding value to the product or Service. See Value Network." ;
  skos:prefLabel "Supply Chain" ;
.
itil:TERM_Support_Group
  rdf:type itil:GlossaryConcept ;
  rdfs:label "Support Group" ;
  skos:definition "(Service Operation) A group of people with technical skills. Support Groups provide the Technical Support needed by all of the IT Service Management Processes. See Technical Management." ;
  skos:prefLabel "Support Group" ;
.
itil:TERM_Support_Hours
  rdf:type itil:GlossaryConcept ;
  rdfs:label "Support Hours" ;
  skos:definition "(Service Design) (Service Operation) The times or hours when support is available to the Users. Typically this is the hours when the Service Desk is available. Support Hours should be defined in a Service Level Agreement, and may be different from Service Hours. For example, Service Hours may be 24 hours a day, but the Support Hours may be 07:00 to 19:00." ;
  skos:prefLabel "Support Hours" ;
.
itil:TERM_Supporting_Service
  rdf:type itil:GlossaryConcept ;
  rdfs:label "Supporting Service" ;
  skos:definition "(Service Strategy) A Service that enables or enhances a Core Service. For example a Directory Service or a Backup Service. See Service Package." ;
  skos:prefLabel "Supporting Service" ;
.
itil:TERM_System
  rdf:type itil:GlossaryConcept ;
  rdfs:label "System" ;
  skos:definition "A number of related things that work together to achieve an overall Objective. For example: � A computer System including hardware, software and Applications. � A management System, including multiple Processes that are planned and managed together. For example a Quality Management System. � A Database Management System or Operating System that includes many software modules that are designed to perform a set of related Functions." ;
  skos:prefLabel "System" ;
.
itil:TERM_System_Management
  rdf:type itil:GlossaryConcept ;
  rdfs:label "System Management" ;
  skos:definition "The part of IT Service Management that focuses on the management of IT Infrastructure rather than Process." ;
  skos:prefLabel "System Management" ;
.
itil:TERM_Tactical
  rdf:type itil:GlossaryConcept ;
  rdfs:label "Tactical" ;
  skos:definition "The middle of three levels of Planning and delivery (Strategic, Tactical, Operational). Tactical Activities include the medium term Plans required to achieve specific Objectives, typically over a period of weeks to months." ;
  skos:prefLabel "Tactical" ;
.
itil:TERM_Tag
  rdf:type itil:GlossaryConcept ;
  rdfs:label "Tag" ;
  skos:definition "(Service Strategy) A short code used to identify a Category. For example tags EC1, EC2, EC3 etc. might be used to identify different Customer outcomes when analysing and comparing Strategies. The term Tag is also used to refer to the Activity of assigning Tags to things." ;
  skos:prefLabel "Tag" ;
.
itil:TERM_Technical_Management
  rdf:type itil:GlossaryConcept ;
  rdfs:label "Technical Management" ;
  skos:definition "(Service Operation) The Function responsible for providing technical skills in support of IT Services and management of the IT Infrastructure. Technical Management defines the Roles of Support Groups, as well as the tools, Processes and Procedures required." ;
  skos:prefLabel "Technical Management" ;
.
itil:TERM_Technical_Observation
  rdf:type itil:GlossaryConcept ;
  rdfs:label "Technical Observation (TO)" ;
  skos:definition "(Continual Service Improvement) A technique used in Service Improvement, Problem investigation and Availability Management. Technical support staff meet to monitor the behaviour and Performance of an IT Service and make recommendations for improvement." ;
  skos:prefLabel "Technical Observation (TO)" ;
.
itil:TERM_Technical_Service
  rdf:type itil:GlossaryConcept ;
  rdfs:label "Technical Service" ;
  skos:definition "Synonym for Infrastructure Service." ;
  skos:prefLabel "Technical Service" ;
.
itil:TERM_Technical_Support
  rdf:type itil:GlossaryConcept ;
  rdfs:label "Technical Support" ;
  skos:definition "Synonym for Technical Management." ;
  skos:prefLabel "Technical Support" ;
.
itil:TERM_Tension_Metrics
  rdf:type itil:GlossaryConcept ;
  rdfs:label "Tension Metrics" ;
  skos:definition "(Continual Service Improvement) A set of related Metrics, in which improvements to one Metric have a negative effect on another. Tension Metrics are designed to ensure that an appropriate balance is achieved." ;
  skos:prefLabel "Tension Metrics" ;
.
itil:TERM_Terms_of_Reference
  rdf:type itil:GlossaryConcept ;
  rdfs:label "Terms of Reference (TOR)" ;
  skos:definition "(Service Design) A Document specifying the Requirements, Scope, Deliverables, Resources and schedule for a Project or Activity." ;
  skos:prefLabel "Terms of Reference (TOR)" ;
.
itil:TERM_Test
  rdf:type itil:GlossaryConcept ;
  rdfs:label "Test" ;
  skos:definition "(Service Transition) An Activity that verifies that a Configuration Item, IT Service, Process, etc. meets its Specification or agreed Requirements. See Service Validation and Testing, Acceptance." ;
  skos:prefLabel "Test" ;
.
itil:TERM_Test_Environment
  rdf:type itil:GlossaryConcept ;
  rdfs:label "Test Environment" ;
  skos:definition "(Service Transition) A controlled Environment used to Test Configuration Items, Builds, IT Services, Processes etc." ;
  skos:prefLabel "Test Environment" ;
.
itil:TERM_Third-line_Support
  rdf:type itil:GlossaryConcept ;
  rdfs:label "Third-line Support" ;
  skos:definition "(Service Operation) The third level in a hierarchy of Support Groups involved in the resolution of Incidents and investigation of Problems. Each level contains more specialist skills, or has more time or other Resources." ;
  skos:prefLabel "Third-line Support" ;
.
itil:TERM_Third_Party
  rdf:type itil:GlossaryConcept ;
  rdfs:label "Third Party" ;
  skos:definition "A person, group, or Business who is not part of the Service Level Agreement for an IT Service, but is required to ensure successful delivery of that IT Service. For example a software Supplier, a hardware maintenance company, or a facilities department. Requirements for Third Parties are typically specified in Underpinning Contracts or Operational Level Agreements." ;
  skos:prefLabel "Third Party" ;
.
itil:TERM_Threat
  rdf:type itil:GlossaryConcept ;
  rdfs:label "Threat" ;
  skos:definition "Anything that might exploit a Vulnerability. Any potential cause of an Incident can be considered to be a Threat. For example a fire is a Threat that could exploit the Vulnerability of flammable floor coverings. This term is commonly used in Information Security Management and IT Service Continuity Management, but also applies to other areas such as Problem and Availability Management." ;
  skos:prefLabel "Threat" ;
.
itil:TERM_Threshold
  rdf:type itil:GlossaryConcept ;
  rdfs:label "Threshold" ;
  skos:definition "The value of a Metric which should cause an Alert to be generated, or management action to be taken. For example \"Priority1 Incident not solved within 4 hours\", \"more than 5 soft disk errors in an hour\", or \"more than 10 failed changes in a month\"." ;
  skos:prefLabel "Threshold" ;
.
itil:TERM_Throughput
  rdf:type itil:GlossaryConcept ;
  rdfs:label "Throughput" ;
  skos:definition "(Service Design) A measure of the number of Transactions, or other Operations, performed in a fixed time. For example 5000 emails sent per hour, or 200 disk I/Os per second." ;
  skos:prefLabel "Throughput" ;
.
itil:TERM_Total_Cost_of_Ownership
  rdf:type itil:GlossaryConcept ;
  rdfs:label "Total Cost of Ownership (TCO)" ;
  skos:definition "(Service Strategy) A methodology used to help make investment decisions. TCO assesses the full Lifecycle Cost of owning a Configuration Item, not just the initial Cost or purchase price. See Total Cost of Utilization." ;
  skos:prefLabel "Total Cost of Ownership (TCO)" ;
.
itil:TERM_Total_Cost_of_Utilization
  rdf:type itil:GlossaryConcept ;
  rdfs:label "Total Cost of Utilization (TCU)" ;
  skos:definition "(Service Strategy) A methodology used to help make investment and Service Sourcing decisions. TCU assesses the full Lifecycle Cost to the Customer of using an IT Service. See Total Cost of Ownership." ;
  skos:prefLabel "Total Cost of Utilization (TCU)" ;
.
itil:TERM_Total_Quality_Management
  rdf:type itil:GlossaryConcept ;
  rdfs:label "Total Quality Management (TQM)" ;
  skos:definition "(Continual Service Improvement) A methodology for managing continual Improvement by using a Quality Management System. TQM establishes a Culture involving all people in the Organisation in a Process of continual monitoring and improvement." ;
  skos:prefLabel "Total Quality Management (TQM)" ;
.
itil:TERM_Transaction
  rdf:type itil:GlossaryConcept ;
  rdfs:label "Transaction" ;
  skos:definition "A discrete Function performed by an IT Service. For example transferring money from one bank account to another. A single Transaction may involve numerous additions, deletions and modifications of data. Either all of these complete successfully or none of them is carried out." ;
  skos:prefLabel "Transaction" ;
.
itil:TERM_Transition
  rdf:type itil:GlossaryConcept ;
  rdfs:label "Transition" ;
  skos:definition "(Service Transition) A change in state, corresponding to a movement of an IT Service or other Configuration Item from one Lifecycle status to the next." ;
  skos:prefLabel "Transition" ;
.
itil:TERM_Transition_Planning_and_Support
  rdf:type itil:GlossaryConcept ;
  rdfs:label "Transition Planning and Support" ;
  skos:definition "(Service Transition) The Process responsible for Planning all Service Transition Processes and co-ordinating the resources that they require. These Service Transition Processes are Change Management, Service Asset and Configuration Management, Release and Deployment Management, Service Validation and Testing, Evaluation, and Knowledge Management." ;
  skos:prefLabel "Transition Planning and Support" ;
.
itil:TERM_Trend_Analysis
  rdf:type itil:GlossaryConcept ;
  rdfs:label "Trend Analysis" ;
  skos:definition "(Continual Service Improvement) Analysis of data to identify time related patterns. Trend Analysis is used in Problem Management to identify common Failures or fragile Configuration Items, and in Capacity Management as a Modelling tool to predict future behaviour. It is also used as a management tool for identifying deficiencies in IT Service Management Processes." ;
  skos:prefLabel "Trend Analysis" ;
.
itil:TERM_Tuning
  rdf:type itil:GlossaryConcept ;
  rdfs:label "Tuning" ;
  skos:definition "The Activity responsible for Planning Changes to make the most efficient use of Resources. Tuning is part of Performance Management, which also includes Performance Monitoring and implementation of the required Changes." ;
  skos:prefLabel "Tuning" ;
.
itil:TERM_Type_III_Service_Provider
  rdf:type itil:GlossaryConcept ;
  rdfs:label "Type III Service Provider" ;
  skos:broader itil:TERM_Service_Provider ;
  skos:definition "(Service Strategy) A Service Provider that provides IT Services to External Customers." ;
  skos:prefLabel "Type III Service Provider" ;
.
itil:TERM_Type_II_Service_Provider
  rdf:type itil:GlossaryConcept ;
  rdfs:label "Type II Service Provider" ;
  skos:broader itil:TERM_Service_Provider ;
  skos:definition "(Service Strategy) An Internal Service Provider that provides shared IT Services to more than one Business Unit." ;
  skos:prefLabel "Type II Service Provider" ;
.
itil:TERM_Type_I_Service_Provider
  rdf:type itil:GlossaryConcept ;
  rdfs:label "Type I Service Provider" ;
  skos:broader itil:TERM_Service_Provider ;
  skos:definition "(Service Strategy) An Internal Service Provider that is embedded within a Business Unit. There may be several Type I Service Providers within an Organisation." ;
  skos:prefLabel "Type I Service Provider" ;
.
itil:TERM_Underpinning_Contract
  rdf:type itil:GlossaryConcept ;
  rdfs:label "Underpinning Contract (UC)" ;
  skos:definition "(Service Design) A Contract between an IT Service Provider and a Third Party. The Third Party provides goods or Services that support delivery of an IT Service to a Customer. The Underpinning Contract defines targets and responsibilities that are required to meet agreed Service Level Targets in an SLA." ;
  skos:prefLabel "Underpinning Contract (UC)" ;
.
itil:TERM_Unit_Cost
  rdf:type itil:GlossaryConcept ;
  rdfs:label "Unit Cost" ;
  skos:definition "(Service Strategy) The Cost to the IT Service Provider of providing a single Component of an IT Service. For example the Cost of a single desktop PC, or of a single Transaction." ;
  skos:prefLabel "Unit Cost" ;
.
itil:TERM_Urgency
  rdf:type itil:GlossaryConcept ;
  rdfs:label "Urgency" ;
  skos:definition "(Service Transition) (Service Design) A measure of how long it will be until an Incident, Problem or Change has a significant Impact on the Business. For example a high Impact Incident may have low Urgency, if the Impact will not affect the Business until the end of the financial year. Impact and Urgency are used to assign Priority." ;
  skos:prefLabel "Urgency" ;
.
itil:TERM_Usability
  rdf:type itil:GlossaryConcept ;
  rdfs:label "Usability" ;
  skos:definition "(Service Design) The ease with which an Application, product, or IT Service can be used. Usability Requirements are often included in a Statement of Requirements." ;
  skos:prefLabel "Usability" ;
.
itil:TERM_Use_Case
  rdf:type itil:GlossaryConcept ;
  rdfs:label "Use Case" ;
  skos:definition "(Service Design) A technique used to define required functionality and Objectives, and to Design Tests. Use Cases define realistic scenarios that describe interactions between Users and an IT Service or other System. See Change Case." ;
  skos:prefLabel "Use Case" ;
.
itil:TERM_User
  rdf:type itil:GlossaryConcept ;
  rdfs:label "User" ;
  skos:definition "A person who uses the IT Service on a day-to-day basis. Users are distinct from Customers, as some Customers do not use the IT Service directly." ;
  skos:prefLabel "User" ;
.
itil:TERM_User_Profile
  rdf:type itil:GlossaryConcept ;
  rdfs:label "User Profile (UP)" ;
  skos:definition "(Service Strategy) A pattern of User demand for IT Services. Each User Profile includes one or more Patterns of Business Activity." ;
  skos:prefLabel "User Profile (UP)" ;
.
itil:TERM_Utility
  rdf:type itil:GlossaryConcept ;
  rdfs:label "Utility" ;
  skos:definition "(Service Strategy) Functionality offered by a Product or Service to meet a particular need. Utility is often summarised as \"what it does\". See Service Utility." ;
  skos:prefLabel "Utility" ;
.
itil:TERM_Validation
  rdf:type itil:GlossaryConcept ;
  rdfs:label "Validation" ;
  skos:definition "(Service Transition) An Activity that ensures a new or changed IT Service, Process, Plan, or other Deliverable meets the needs of the Business. Validation ensures that Business Requirements are met even though these may have changed since the original Design. See Verification, Acceptance, Qualification, Service Validation and Testing." ;
  skos:prefLabel "Validation" ;
.
itil:TERM_Value_Chain
  rdf:type itil:GlossaryConcept ;
  rdfs:label "Value Chain" ;
  skos:definition "(Service Strategy) A sequence of Processes that creates a product or Service that is of value to a Customer. Each step of the sequence builds on the previous steps and contributes to the overall product or Service. See Value Network." ;
  skos:prefLabel "Value Chain" ;
.
itil:TERM_Value_Network
  rdf:type itil:GlossaryConcept ;
  rdfs:label "Value Network" ;
  skos:definition "(Service Strategy) A complex set of Relationships between two or more groups or organisations. Value is generated through exchange of knowledge, information, goods or Services. See Value Chain, Partnership." ;
  skos:prefLabel "Value Network" ;
.
itil:TERM_Value_for_Money
  rdf:type itil:GlossaryConcept ;
  rdfs:label "Value for Money" ;
  skos:definition "An informal measure of Cost Effectiveness. Value for Money is often based on a comparison with the Cost of alternatives. See Cost Benefit Analysis." ;
  skos:prefLabel "Value for Money" ;
.
itil:TERM_Value_on_Investment
  rdf:type itil:GlossaryConcept ;
  rdfs:label "Value on Investment (VOI)" ;
  skos:definition "(Continual Service Improvement) A measurement of the expected benefit of an investment. VOI considers both financial and intangible benefits. See Return on Investment." ;
  skos:prefLabel "Value on Investment (VOI)" ;
.
itil:TERM_Variable_Cost
  rdf:type itil:GlossaryConcept ;
  rdfs:label "Variable Cost" ;
  skos:definition "(Service Strategy) A Cost that depends on how much the IT Service is used, how many products are produced, the number and type of Users, or something else that cannot be fixed in advance. See Variable Cost Dynamics." ;
  skos:prefLabel "Variable Cost" ;
.
itil:TERM_Variable_Cost_Dynamics
  rdf:type itil:GlossaryConcept ;
  rdfs:label "Variable Cost Dynamics" ;
  skos:definition "(Service Strategy) A technique used to understand how overall Costs are impacted by the many complex variable elements that contribute to the provision of IT Services." ;
  skos:prefLabel "Variable Cost Dynamics" ;
.
itil:TERM_Variance
  rdf:type itil:GlossaryConcept ;
  rdfs:label "Variance" ;
  skos:definition "The difference between a planned value and the actual measured value. Commonly used in Financial Management, Capacity Management and Service Level Management, but could apply in any area where Plans are in place." ;
  skos:prefLabel "Variance" ;
.
itil:TERM_Verification
  rdf:type itil:GlossaryConcept ;
  rdfs:label "Verification" ;
  skos:definition "(Service Transition) An Activity that ensures a new or changed IT Service, Process, Plan, or other Deliverable is complete, accurate, Reliable and matches its Design Specification. See Validation, Acceptance, Service Validation and Testing." ;
  skos:prefLabel "Verification" ;
.
itil:TERM_Verification_and_Audit
  rdf:type itil:GlossaryConcept ;
  rdfs:label "Verification and Audit" ;
  skos:definition "(Service Transition) The Activities responsible for ensuring that information in the CMDB is accurate and that all Configuration Items have been identified and recorded in the CMDB. Verification includes routine checks that are part of other Processes. For example, verifying the serial number of a desktop PC when a User logs an Incident. Audit is a periodic, formal check." ;
  skos:prefLabel "Verification and Audit" ;
.
itil:TERM_Version
  rdf:type itil:GlossaryConcept ;
  rdfs:label "Version" ;
  skos:definition "(Service Transition) A Version is used to identify a specific Baseline of a Configuration Item. Versions typically use a naming convention that enables the sequence or date of each Baseline to be identified. For example Payroll Application Version 3 contains updated functionality from Version 2." ;
  skos:prefLabel "Version" ;
.
itil:TERM_Vision
  rdf:type itil:GlossaryConcept ;
  rdfs:label "Vision" ;
  skos:definition "A description of what the Organisation intends to become in the future. A Vision is created by senior management and is used to help influence Culture and Strategic Planning." ;
  skos:prefLabel "Vision" ;
.
itil:TERM_Vital_Business_Function
  rdf:type itil:GlossaryConcept ;
  rdfs:label "Vital Business Function (VBF)" ;
  skos:definition "(Service Design) A Function of a Business Process which is critical to the success of the Business. Vital Business Functions are an important consideration of Business Continuity Management, IT Service Continuity Management and Availability Management." ;
  skos:prefLabel "Vital Business Function (VBF)" ;
.
itil:TERM_Vulnerability
  rdf:type itil:GlossaryConcept ;
  rdfs:label "Vulnerability" ;
  skos:definition "A weakness that could be exploited by a Threat. For example an open firewall port, a password that is never changed, or a flammable carpet. A missing Control is also considered to be a Vulnerability." ;
  skos:prefLabel "Vulnerability" ;
.
itil:TERM_Warm_Standby
  rdf:type itil:GlossaryConcept ;
  rdfs:label "Warm Standby" ;
  skos:definition "Synonym for Intermediate Recovery." ;
  skos:prefLabel "Warm Standby" ;
.
itil:TERM_Warning
  rdf:type itil:GlossaryConcept ;
  rdfs:label "Warning" ;
  skos:prefLabel "Warning" ;
.
itil:TERM_Warranty
  rdf:type itil:GlossaryConcept ;
  rdfs:label "Warranty" ;
  skos:definition "(Service Strategy) A promise or guarantee that a product or Service will meet its agreed Requirements. See Service Validation and Testing, Service Warranty." ;
  skos:prefLabel "Warranty" ;
.
itil:TERM_Work_Instruction
  rdf:type itil:GlossaryConcept ;
  rdfs:label "Work Instruction" ;
  skos:definition "A Document containing detailed instructions that specify exactly what steps to follow to carry out an Activity. A Work Instruction contains much more detail than a Procedure and is only created if very detailed instructions are needed." ;
  skos:prefLabel "Work Instruction" ;
.
itil:TERM_Work_in_Progress
  rdf:type itil:GlossaryConcept ;
  rdfs:label "Work in Progress (WIP)" ;
  skos:definition "A Status that means Activities have started but are not yet complete. It is commonly used as a Status for Incidents, Problems, Changes etc." ;
  skos:prefLabel "Work in Progress (WIP)" ;
.
itil:TERM_Workaround
  rdf:type itil:GlossaryConcept ;
  rdfs:label "Workaround" ;
  skos:definition "(Service Operation) Reducing or eliminating the Impact of an Incident or Problem for which a full Resolution is not yet available. For example by restarting a failed Configuration Item. Workarounds for Problems are documented in Known Error Records. Workarounds for Incidents that do not have associated Problem Records are documented in the Incident Record." ;
  skos:prefLabel "Workaround" ;
.
itil:TERM_Workload
  rdf:type itil:GlossaryConcept ;
  rdfs:label "Workload" ;
  skos:definition "The Resources required to deliver an identifiable part of an IT Service. Workloads may be Categorised by Users, groups of Users, or Functions within the IT Service. This is used to assist in analysing and managing the Capacity, Performance and Utilisation of Configuration Items and IT Services. The term Workload is sometimes used as a synonym for Throughput." ;
  skos:prefLabel "Workload" ;
.
itil:TERM_eSourcing_Capability_Model_for_Client_Organizations
  rdf:type itil:GlossaryConcept ;
  rdfs:label "eSourcing Capability Model for Client Organizations (eSCM-CL)" ;
  skos:definition "(Service Strategy) A framework to help Organisations guide their analysis and decisions on Service Sourcing Models and Strategies. eSCM-CL was developed by Carnegie Mellon University. See eSCM-SP." ;
  skos:prefLabel "eSourcing Capability Model for Client Organizations (eSCM-CL)" ;
.
itil:TERM_eSourcing_Capability_Model_for_Service_Providers
  rdf:type itil:GlossaryConcept ;
  rdfs:label "eSourcing Capability Model for Service Providers (eSCM- SP)" ;
  skos:definition "(Service Strategy) A framework to help IT Service Providers develop their IT Service Management Capabilities from a Service Sourcing perspective. eSCM-SP was developed by Carnegie Mellon University. See eSCM-CL." ;
  skos:prefLabel "eSourcing Capability Model for Service Providers (eSCM- SP)" ;
.
itil:TERM_pro-forma
  rdf:type itil:GlossaryConcept ;
  rdfs:label "pro-forma" ;
  skos:definition "A template, or example Document containing example data that will be replaced with the real values when these are available." ;
  skos:prefLabel "pro-forma" ;
.
<http://itil.edg.topbraid.solutions/models/glossary/GMD_glossary>
  rdf:type vaem:GraphMetaData ;
  dcterms:modified "2016-12-18"^^xsd:date ;
  dcterms:rights "<p>This ontology is issued under a restricted copyright license that prohibits reproduction, distribution, copying and any other form of sharing. The license agreement can be found at <a href='http://www.topquadrant.com/docs/legal/EULA.pdf'>http://www.topquadrant.com/docs/legal/EULA.pdf.</p>"^^rdf:HTML ;
  vaem:hasGraphRole vaem:ModelGraph ;
  vaem:hasLicenseType <voag:TopQuadrant_ONTOLOGY-LICENSE> ;
  vaem:hasOwner vaem:TopQuadrant ;
  vaem:hasSteward vaem:TopQuadrant ;
  vaem:isMetadataFor <http://itil.edg.topbraid.solutions/models/1.0/glossary> ;
  vaem:name "EDG" ;
  vaem:namespace "http://edg.topbraid.solutions/model/" ;
  vaem:namespacePrefix "edg" ;
  vaem:owner "TopQuadrant, Inc." ;
  vaem:releaseDate "2016-12-18"^^xsd:date ;
  vaem:revision "1.0" ;
  vaem:usesNonImportedResource dcterms:abstract ;
  vaem:usesNonImportedResource dcterms:author ;
  vaem:usesNonImportedResource dcterms:created ;
  vaem:usesNonImportedResource dcterms:modified ;
  vaem:usesNonImportedResource dcterms:rights ;
  vaem:usesNonImportedResource dcterms:title ;
  vaem:usesNonImportedResource <http://voag.linkedmodel.org/voag#TopQuadrant_ONTOLOGY-LICENSE> ;
  vaem:withAttributionTo "Any references to this ontology should give attribution to TopQuadrant, Inc." ;
.
