# baseURI: http://eds.topbraidlive.org/1.0/quantitykinds/maeco
# imports: http://edg.topbraid.solutions/1.0/schema/maeco
# imports: http://spinrdf.org/spl
# imports: http://www.w3.org/2004/02/skos/core

@prefix dc: <http://purl.org/dc/elements/1.1/> .
@prefix dcterms: <http://purl.org/dc/terms/> .
@prefix maeco: <http://edg.topbraid.solutions/maeco/> .
@prefix maecot: <http://edg.topbraid.solutions/maeco/term/> .
@prefix owl: <http://www.w3.org/2002/07/owl#> .
@prefix prov: <http://www.w3.org/ns/prov#> .
@prefix rdf: <http://www.w3.org/1999/02/22-rdf-syntax-ns#> .
@prefix rdfs: <http://www.w3.org/2000/01/rdf-schema#> .
@prefix skos: <http://www.w3.org/2004/02/skos/core#> .
@prefix spin: <http://spinrdf.org/spin#> .
@prefix spl: <http://spinrdf.org/spl#> .
@prefix swa: <http://topbraid.org/swa#> .
@prefix taxonomies: <http://evn.topbraidlive.org/evnprojects#> .
@prefix teamwork: <http://topbraid.org/teamwork#> .
@prefix xsd: <http://www.w3.org/2001/XMLSchema#> .

rdf:type
  rdfs:isDefinedBy <http://eds.topbraidlive.org/1.0/taxonomy/maeco> ;
  rdfs:isDefinedBy <http://eds.topbraidlive.org/taxonomy/maeco> ;
  rdfs:label "type" ;
.
maeco:BankOfEnglandPRAglossary
  rdf:type maeco:Resource ;
  dcterms:description "The glossary at the Bank of England's Prudential Regulation Authority (PRA)." ;
  dcterms:source "http://www.prarulebook.co.uk/rulebook/Glossary/Rulebook/0/13-04-2016/A"^^xsd:anyURI ;
  dcterms:title "Bank of England's Prudential Regulation Authority (PRA) Glossary" ;
  rdfs:label "Bank of England's Prudential Regulation Authority (PRA) Glossary" ;
.
maeco:BankOfEnglandWorkingPapers
  rdf:type maeco:Resource ;
  dcterms:description "The Bank of England's Working Papers" ;
  dcterms:source "http://www.bankofengland.co.uk/research/Pages/workingpapers/default.aspx"^^xsd:anyURI ;
  dcterms:title "The Bank of England's Working Papers" ;
  rdfs:label "The Bank of England's Working Papers" ;
.
maeco:Buffer
  maeco:representedBy maecot:ANY_Buffer ;
  rdfs:isDefinedBy <http://eds.topbraidlive.org/1.0/taxonomy/maeco> ;
  rdfs:isDefinedBy <http://eds.topbraidlive.org/taxonomy/maeco> ;
.
maeco:CombinedBuffer
  rdf:type maeco:Buffer ;
  dcterms:source "http://www.prarulebook.co.uk/rulebook/Content/Part/211272/13-04-2016"^^xsd:anyURI ;
  rdfs:isDefinedBy <http://eds.topbraidlive.org/1.0/taxonomy/maeco> ;
  rdfs:isDefinedBy <http://eds.topbraidlive.org/taxonomy/maeco> ;
  rdfs:label "Capital Conservation Buffer" ;
  rdfs:seeAlso maecot:CapitalConservationBuffer ;
  rdfs:seeAlso maecot:CounterCyclicalCapitalBuffer ;
  skos:broader maecot:ANY_Buffer ;
  skos:definition "The \"Combined Buffer\" is the sum of (a) the capital conservation buffer; and (b) the countercyclical capital buffer." ;
  skos:prefLabel "Capital Conservation Buffer"@en ;
.
maeco:Cost
  maeco:representedBy maecot:ANY_Cost ;
  rdfs:isDefinedBy <http://eds.topbraidlive.org/1.0/taxonomy/maeco> ;
  rdfs:isDefinedBy <http://eds.topbraidlive.org/taxonomy/maeco> ;
.
maeco:CounterCyclicalBufferRate
  rdf:type maeco:Rate ;
  dcterms:source "http://www.prarulebook.co.uk/rulebook/Content/Part/211272/13-04-2016"^^xsd:anyURI ;
  rdfs:isDefinedBy <http://eds.topbraidlive.org/1.0/taxonomy/maeco> ;
  rdfs:isDefinedBy <http://eds.topbraidlive.org/taxonomy/maeco> ;
  rdfs:label "Counter-cyclical buffer rate" ;
  rdfs:seeAlso maecot:CounterCyclicalCapitalBuffer ;
  skos:broader maecot:ANY_Rate ;
  skos:definition "The \"countercyclical buffer rate\" means (in accordance with point (7) of Article 128 of the CRD) the rate: (a) expressed as a percentage of total risk exposure amount set by the FPC or an EEA countercyclical buffer authority; or (b) expressed in terms equivalent to a percentage of total risk exposure amount set by a third country countercyclical buffer authority; that a firm must apply in order to calculate its countercyclical capital buffer." ;
  skos:prefLabel "Counter-cyclical buffer rate" ;
.
maeco:Demand
  maeco:representedBy maecot:ANY_Demand ;
  rdfs:isDefinedBy <http://eds.topbraidlive.org/1.0/taxonomy/maeco> ;
  rdfs:isDefinedBy <http://eds.topbraidlive.org/taxonomy/maeco> ;
.
maeco:EuropeanCentralBank
  rdf:type maeco:Resource ;
  dcterms:source "https://www.ecb.europa.eu/home/glossary/html/index.en.html"^^xsd:anyURI ;
  dcterms:source "https://www.ecb.europa.eu/home/html/index.en.html"^^xsd:anyURI ;
  dcterms:source "https://www.ecb.europa.eu/pub/research/working-papers/html/all-papers.en.html"^^xsd:anyURI ;
  rdfs:isDefinedBy <http://eds.topbraidlive.org/1.0/taxonomy/maeco> ;
  rdfs:isDefinedBy <http://eds.topbraidlive.org/taxonomy/maeco> ;
  rdfs:label "European Central Bank" ;
  skos:definition "The central bank of the <a href='http://edg.topbraid.solutions/maeco/term/EuroZone'>Euro Zone</a> ." ;
  skos:prefLabel "European Central Bank" ;
.
maeco:FRED
  rdf:type maeco:Resource ;
  dcterms:description "The Research Division of the Federal Reserve Bank of St. Louis is responsible for advising the Bank president on matters of economic policy. The Division monitors the economic and financial literature and produces research in the areas of money and banking, macroeconomics, and international and regional economics. A diverse group of Bank publications allows the Research Division to address quickly changing economic trends, explore the relevance of historical and current data for economic policy, and expand the understanding of issues relevant to the Eighth District and beyond. The Research Division also furnishes its working papers to provide insight into current Bank interests and developing theories and to stimulate discussion." ;
  dcterms:source "https://research.stlouisfed.org/"^^xsd:anyURI ;
  dcterms:source "https://research.stlouisfed.org/fred2/categories/33490?t=debt&ob=pv&od=desc"^^xsd:anyURI ;
  dcterms:title "Federal Reserve Economic Data" ;
  rdfs:label "FRED" ;
.
maeco:IMF-SDDS
  rdf:type maeco:Resource ;
  dcterms:source "http://dsbb.imf.org/Pages/SDDS/Home.aspx"^^xsd:anyURI ;
  rdfs:label "IMF-SDDS" ;
  skos:definition "￼￼￼￼￼￼￼￼￼￼￼￼￼￼￼￼￼￼￼￼￼￼￼￼￼￼￼￼￼￼￼￼￼￼￼￼￼￼￼￼￼￼￼￼￼￼￼￼￼￼￼￼￼￼￼￼￼￼￼￼￼￼￼" ;
.
maeco:IMFER
  rdf:type maeco:Resource ;
  dcterms:source "http://www.palgrave-journals.com/imfer/index.html"^^xsd:anyURI ;
  dcterms:source "http://www.palgrave-journals.com/imfer/journal/v61/n2/full/imfer201312a.html"^^xsd:anyURI ;
  rdfs:label "IMF Economic Review" ;
  skos:definition "￼￼￼￼￼￼￼￼￼￼￼￼￼￼￼￼￼￼￼￼￼￼￼￼￼￼￼￼￼￼￼￼￼￼￼￼￼￼￼￼￼￼￼￼￼￼￼￼￼￼￼￼￼￼￼￼￼￼￼￼￼￼￼IMF Economic Review (IMFER) is the official research journal of the International Monetary Fund, bringing you policy-relevant and innovative academic research on global macroeconomics." ;
.
maeco:LiquidityMeasure
  maeco:representedBy maecot:ANY_LiquidityMeasure ;
  rdfs:isDefinedBy <http://eds.topbraidlive.org/1.0/taxonomy/maeco> ;
  rdfs:isDefinedBy <http://eds.topbraidlive.org/taxonomy/maeco> ;
.
maeco:LongSaleCapitalGainsOverhang
  rdf:type maeco:QuantityKind ;
  maeco:citation """von Beschwitz, Bastian and Massimo Massa (2015). Biased Shorts: Short sellers’ Disposition Effect and Limits to Arbitrage. International Finance Discussion Papers 1147.   
<a href=\"http://dx.doi.org/10.17016/IFDP.2015.1147\">http://dx.doi.org/10.17016/IFDP.2015.1147</a>."""^^rdf:HTML ;
  dcterms:source "http://dx.doi.org/10.17016/IFDP.2015.1147"^^xsd:anyURI ;
  rdfs:isDefinedBy <http://eds.topbraidlive.org/1.0/taxonomy/maeco> ;
  rdfs:isDefinedBy <http://eds.topbraidlive.org/taxonomy/maeco> ;
  rdfs:label "Long sale capital gains overhang" ;
  rdfs:seeAlso maeco:ShortSaleCapitalGainsOverhang ;
  skos:altLabel "LCGO" ;
  skos:altLabel "capital gains of long traders" ;
  skos:broader maecot:ANY_QuantityKind ;
  skos:definition "Long sale Capital Gains Overhang (LCGO) is defined as the average percentage gains of short sellers relative to the price at which they entered their positions." ;
  skos:prefLabel "Long Sale Capital Gains Overhang" ;
.
maeco:Measure
  maeco:representedBy maecot:ANY_Measure ;
  rdfs:isDefinedBy <http://eds.topbraidlive.org/1.0/taxonomy/maeco> ;
  rdfs:isDefinedBy <http://eds.topbraidlive.org/taxonomy/maeco> ;
.
maeco:PercentageOLossRealized
  rdf:type maeco:QuantityKind ;
  maeco:citation """von Beschwitz, Bastian and Massimo Massa (2015). Biased Shorts: Short sellers’ Disposition Effect and Limits to Arbitrage. International Finance Discussion Papers 1147.   
<a href=\"http://dx.doi.org/10.17016/IFDP.2015.1147\">http://dx.doi.org/10.17016/IFDP.2015.1147</a>."""^^rdf:HTML ;
  dcterms:source "http://dx.doi.org/10.17016/IFDP.2015.1147"^^xsd:anyURI ;
  rdfs:isDefinedBy <http://eds.topbraidlive.org/1.0/taxonomy/maeco> ;
  rdfs:isDefinedBy <http://eds.topbraidlive.org/taxonomy/maeco> ;
  rdfs:label "Percentage of loss realized" ;
  rdfs:seeAlso maeco:PercentageOfGainRealized ;
  skos:altLabel "PGR" ;
  skos:broader maecot:ANY_QuantityKind ;
  skos:definition "Percentage of loss realized (PLR) is defined as the percentage of open (long) positions with negative capital gains that are sold. " ;
  skos:prefLabel "Percentage Of Loss Realized" ;
.
maeco:PercentageOfGainRealized
  rdf:type maeco:QuantityKind ;
  maeco:citation """von Beschwitz, Bastian and Massimo Massa (2015). Biased Shorts: Short sellers’ Disposition Effect and Limits to Arbitrage. International Finance Discussion Papers 1147.   
<a href=\"http://dx.doi.org/10.17016/IFDP.2015.1147\">http://dx.doi.org/10.17016/IFDP.2015.1147</a>."""^^rdf:HTML ;
  dcterms:source "http://dx.doi.org/10.17016/IFDP.2015.1147"^^xsd:anyURI ;
  rdfs:isDefinedBy <http://eds.topbraidlive.org/1.0/taxonomy/maeco> ;
  rdfs:isDefinedBy <http://eds.topbraidlive.org/taxonomy/maeco> ;
  rdfs:label "Percentage of gains realized" ;
  rdfs:seeAlso maeco:PercentageOLossRealized ;
  skos:altLabel "PGR" ;
  skos:broader maecot:ANY_QuantityKind ;
  skos:definition "Percentage of gains realized (PGR) is defined as the percentage of open (long) positions with positive capital gains that are sold. " ;
  skos:prefLabel "Percentage Of Gains Realized" ;
.
maeco:QuantityKind
  rdf:type owl:Class ;
  rdfs:isDefinedBy <http://eds.topbraidlive.org/1.0/taxonomy/maeco> ;
  rdfs:isDefinedBy <http://eds.topbraidlive.org/taxonomy/maeco> ;
  rdfs:subClassOf skos:Concept ;
.
maeco:RESOURCE_CEPR
  rdf:type maeco:Resource ;
  dcterms:source "http://cepr.org/active/publications/discussion_papers/dp.php?dpno=1001"^^xsd:anyURI ;
  dcterms:source "http://cepr.org/active/publications/discussion_papers/dp.php?dpno=11249"^^xsd:anyURI ;
  rdfs:label "RESOURCE CEPR" ;
.
maeco:Rate
  maeco:representedBy maecot:ANY_Rate ;
  rdfs:isDefinedBy <http://eds.topbraidlive.org/1.0/taxonomy/maeco> ;
  rdfs:isDefinedBy <http://eds.topbraidlive.org/taxonomy/maeco> ;
.
maeco:Ratio
  maeco:representedBy maecot:ANY_Ratio ;
  rdfs:isDefinedBy <http://eds.topbraidlive.org/1.0/taxonomy/maeco> ;
  rdfs:isDefinedBy <http://eds.topbraidlive.org/taxonomy/maeco> ;
.
maeco:ReDIF
  rdf:type maeco:Resource ;
  dcterms:description "A resource that describes current version of the Research Documents Information Format (ReDIF). This is a simple \"field: value\" data format inspired from the IAFA templates. A primitive nesting stucture syntax is enabled through the use of clusters of fields. ReDIF is currently used by RePEc." ;
  dcterms:source "https://ideas.repec.org/p/rpc/rdfdoc/redif.html"^^xsd:anyURI ;
  dcterms:source "https://ideas.repec.org/top/top.journals.simple.html"^^xsd:anyURI ;
  dcterms:title "Research Documents Information Format (ReDIF)" ;
  rdfs:label "ReDIF" ;
.
maeco:Reserves
  maeco:representedBy maecot:ANY_Reserves ;
  rdfs:isDefinedBy <http://eds.topbraidlive.org/1.0/taxonomy/maeco> ;
  rdfs:isDefinedBy <http://eds.topbraidlive.org/taxonomy/maeco> ;
.
maeco:Resource
  rdf:type owl:Class ;
  rdfs:label "Resource" ;
  rdfs:subClassOf owl:Thing ;
.
maeco:SCHEME_Agreement
  rdf:type skos:ConceptScheme ;
  rdfs:isDefinedBy <http://eds.topbraidlive.org/1.0/taxonomy/maeco> ;
  rdfs:isDefinedBy <http://eds.topbraidlive.org/taxonomy/maeco> ;
  rdfs:label "Economic Agreement" ;
.
maeco:SCHEME_Organization
  rdf:type skos:ConceptScheme ;
  rdfs:isDefinedBy <http://eds.topbraidlive.org/1.0/taxonomy/maeco> ;
  rdfs:isDefinedBy <http://eds.topbraidlive.org/taxonomy/maeco> ;
  rdfs:label "Organization" ;
.
maeco:ShortSaleCapitalGainsOverhang
  rdf:type maeco:QuantityKind ;
  maeco:citation """von Beschwitz, Bastian and Massimo Massa (2015). Biased Shorts: Short sellers’ Disposition Effect and Limits to Arbitrage. International Finance Discussion Papers 1147.   
<a href=\"http://dx.doi.org/10.17016/IFDP.2015.1147\">http://dx.doi.org/10.17016/IFDP.2015.1147</a>."""^^rdf:HTML ;
  dcterms:source "http://dx.doi.org/10.17016/IFDP.2015.1147"^^xsd:anyURI ;
  rdfs:isDefinedBy <http://eds.topbraidlive.org/1.0/taxonomy/maeco> ;
  rdfs:isDefinedBy <http://eds.topbraidlive.org/taxonomy/maeco> ;
  rdfs:label "Short sale capital gains overhang" ;
  rdfs:seeAlso maeco:LongSaleCapitalGainsOverhang ;
  skos:altLabel "SCGO" ;
  skos:altLabel "capital gains of short traders" ;
  skos:broader maecot:ANY_QuantityKind ;
  skos:definition "Short sale Capital Gains Overhang (SCGO) is defined as the average percentage gains of short sellers relative to the price at which they entered their positions." ;
  skos:prefLabel "Short Sale Capital Gains Overhang" ;
.
maeco:StatisticsCanadaThesaurus
  rdf:type maeco:Resource ;
  dcterms:description "The Statistics Canada Thesaurus was developed to provide subject access to Statistics Canada's information resources. The Thesaurus is a bilingual, fully structured, indexing and information retrieval tool which conforms to internationally accepted standards and conventions for thesaurus construction. It consists of descriptors and non-descriptors, accompanied by their hierarchical, associative and prescriptive relationships." ;
  dcterms:source "http://www47.statcan.gc.ca/th_r001-eng.htm"^^xsd:anyURI ;
  dcterms:title "Statistics Canada Thesaurus" ;
  rdfs:label "Statistics Canada Thesaurus" ;
.
maeco:TradeMeasure
  maeco:representedBy maecot:ANY_TradeMeasure ;
  rdfs:isDefinedBy <http://eds.topbraidlive.org/1.0/taxonomy/maeco> ;
  rdfs:isDefinedBy <http://eds.topbraidlive.org/taxonomy/maeco> ;
.
maeco:UN-SNA2008
  rdf:type maeco:Resource ;
  dcterms:source "http://unstats.un.org/unsd/nationalaccount/docs/SNA2008.pdf"^^xsd:anyURI ;
  rdfs:label "UN SNA 2008" ;
  skos:definition "￼￼￼￼￼￼￼￼￼￼￼￼￼￼￼￼￼￼￼￼￼￼￼￼￼￼￼￼￼￼￼￼￼￼￼￼￼￼￼￼￼￼￼￼￼￼￼￼￼￼￼￼￼￼￼￼￼￼￼￼￼￼" ;
.
maeco:ZBWeconomicSubjectThesaurus
  rdf:type maeco:Resource ;
  dcterms:description "The thesaurus provides vocabulary on any economic subject: more than 6,000 standardized subject headings and about 20,000 additional entry terms to support individual keywords. You can also find technical terms used in law, sociology, or politics, and geographic names. When selecting terms from this vocabulary, you can be sure to get results matching your search query. The information on the web pages is also embedded as data in RDFa format in order to support multiple re-use in the economics and business communities and within the semantic web.." ;
  dcterms:source "http://zbw.eu/stw/version/latest/about"^^xsd:anyURI ;
  dcterms:title "ZBW Economic Subject Thesaurus" ;
  rdfs:label "ZBW Economic Subject Thesaurus" ;
.
maecot:ANY_Average
  rdf:type maeco:QuantityKind ;
  rdfs:isDefinedBy <http://eds.topbraidlive.org/1.0/taxonomy/maeco> ;
  rdfs:isDefinedBy <http://eds.topbraidlive.org/taxonomy/maeco> ;
  rdfs:label "Average" ;
  skos:broader maecot:ANY_QuantityKind ;
  skos:prefLabel "Average" ;
.
maecot:ANY_Buffer
  rdf:type maeco:Buffer ;
  rdfs:isDefinedBy <http://eds.topbraidlive.org/1.0/taxonomy/maeco> ;
  rdfs:isDefinedBy <http://eds.topbraidlive.org/taxonomy/maeco> ;
  rdfs:label "Buffer" ;
  skos:broader maecot:ANY_QuantityKind ;
  skos:prefLabel "Buffer"@en ;
.
maecot:ANY_Cash
  rdf:type maeco:QuantityKind ;
  rdfs:isDefinedBy <http://eds.topbraidlive.org/1.0/taxonomy/maeco> ;
  rdfs:isDefinedBy <http://eds.topbraidlive.org/taxonomy/maeco> ;
  rdfs:label "Cash" ;
  skos:broader maecot:ANY_QuantityKind ;
  skos:prefLabel "Cash Value"@en ;
.
maecot:ANY_Cost
  rdf:type maeco:Cost ;
  rdfs:isDefinedBy <http://eds.topbraidlive.org/1.0/taxonomy/maeco> ;
  rdfs:isDefinedBy <http://eds.topbraidlive.org/taxonomy/maeco> ;
  rdfs:label "cost" ;
  skos:broader maecot:ANY_QuantityKind ;
  skos:prefLabel "Cost" ;
.
maecot:ANY_Demand
  rdf:type maeco:Demand ;
  dcterms:source "http://www.wwnorton.com/college/econ/stec4/macroeconomics/glossary.asp"^^xsd:anyURI ;
  rdfs:isDefinedBy <http://eds.topbraidlive.org/1.0/taxonomy/maeco> ;
  rdfs:isDefinedBy <http://eds.topbraidlive.org/taxonomy/maeco> ;
  rdfs:label "demand" ;
  skos:definition "<STRONG>1.</STRONG> The act of offering to buy a product.  <STRONG>2.</STRONG> The quantity offered to buy.  <STRONG>3.</STRONG> The quantities offered to buy at various prices; the <a href='http://edg.topbraid.solutions/maeco/term/DemandCurve'>demand curve</a> . <STRONG>Demand</STRONG> - the quantity of a good or service that a household or firm chooses to buy at a given price." ;
  skos:prefLabel "Demand" ;
.
maecot:ANY_LiquidityMeasure
  rdf:type maeco:LiquidityMeasure ;
  rdfs:isDefinedBy <http://eds.topbraidlive.org/1.0/taxonomy/maeco> ;
  rdfs:isDefinedBy <http://eds.topbraidlive.org/taxonomy/maeco> ;
  rdfs:label "Liquidity Measure" ;
  skos:broader maecot:ANY_Measure ;
  skos:prefLabel "Liquidity Measure"@en ;
.
maecot:ANY_Measure
  rdf:type maeco:Measure ;
  rdfs:isDefinedBy <http://eds.topbraidlive.org/1.0/taxonomy/maeco> ;
  rdfs:isDefinedBy <http://eds.topbraidlive.org/taxonomy/maeco> ;
  rdfs:label "Measure" ;
  skos:prefLabel "Measure"@en ;
.
maecot:ANY_Premium
  rdf:type maeco:QuantityKind ;
  dcterms:source "http://www.cftc.gov/LawRegulation/DoddFrankAct/index.htm"^^xsd:anyURI ;
  rdfs:isDefinedBy <http://eds.topbraidlive.org/1.0/taxonomy/maeco> ;
  rdfs:isDefinedBy <http://eds.topbraidlive.org/taxonomy/maeco> ;
  rdfs:label "Premium" ;
  skos:broader maecot:ANY_QuantityKind ;
  skos:prefLabel "Premium"@en ;
.
maecot:ANY_QuantityKind
  rdf:type maeco:QuantityKind ;
  dcterms:source "http://www.cftc.gov/LawRegulation/DoddFrankAct/index.htm"^^xsd:anyURI ;
  rdfs:isDefinedBy <http://eds.topbraidlive.org/1.0/taxonomy/maeco> ;
  rdfs:isDefinedBy <http://eds.topbraidlive.org/taxonomy/maeco> ;
  rdfs:label "Quantity Kind" ;
  skos:prefLabel "Quantity Kind"@en ;
.
maecot:ANY_Rate
  rdf:type maeco:Rate ;
  rdfs:isDefinedBy <http://eds.topbraidlive.org/1.0/taxonomy/maeco> ;
  rdfs:isDefinedBy <http://eds.topbraidlive.org/taxonomy/maeco> ;
  rdfs:label "rate" ;
  skos:broader maecot:ANY_QuantityKind ;
  skos:prefLabel "Rate" ;
.
maecot:ANY_Ratio
  rdf:type maeco:Ratio ;
  rdfs:isDefinedBy <http://eds.topbraidlive.org/1.0/taxonomy/maeco> ;
  rdfs:isDefinedBy <http://eds.topbraidlive.org/taxonomy/maeco> ;
  rdfs:label "Ratio" ;
  skos:broader maecot:ANY_QuantityKind ;
  skos:prefLabel "Ratio"@en ;
.
maecot:ANY_Reserves
  rdf:type maeco:Reserves ;
  rdfs:isDefinedBy <http://eds.topbraidlive.org/1.0/taxonomy/maeco> ;
  rdfs:isDefinedBy <http://eds.topbraidlive.org/taxonomy/maeco> ;
  rdfs:label "Reserves" ;
  skos:broader maecot:ANY_QuantityKind ;
  skos:prefLabel "Reserves"@en ;
.
maecot:ANY_TradeMeasure
  rdf:type maeco:TradeMeasure ;
  rdfs:isDefinedBy <http://eds.topbraidlive.org/1.0/taxonomy/maeco> ;
  rdfs:isDefinedBy <http://eds.topbraidlive.org/taxonomy/maeco> ;
  rdfs:label "Trade Measure" ;
  skos:broader maecot:ANY_Measure ;
  skos:prefLabel "Trade Measure" ;
.
maecot:AboveAverageRiskWeight
  rdf:type maeco:RiskMeasure ;
  rdfs:isDefinedBy <http://eds.topbraidlive.org/1.0/taxonomy/maeco> ;
  rdfs:isDefinedBy <http://eds.topbraidlive.org/taxonomy/maeco> ;
  rdfs:label "Above Average Risk Weight" ;
  skos:broader maecot:RiskWeightingFactor ;
  skos:prefLabel "Above average risk weight"@en ;
.
maecot:AbsoluteAmount
  rdf:type maeco:QuantityKind ;
  rdfs:isDefinedBy <http://eds.topbraidlive.org/1.0/taxonomy/maeco> ;
  rdfs:isDefinedBy <http://eds.topbraidlive.org/taxonomy/maeco> ;
  rdfs:label "Absolute Amount" ;
  skos:broader maecot:ANY_QuantityKind ;
  skos:prefLabel "Absolute amount"@en ;
.
maecot:AbsoluteLevels
  rdf:type maeco:QuantityKind ;
  rdfs:isDefinedBy <http://eds.topbraidlive.org/1.0/taxonomy/maeco> ;
  rdfs:isDefinedBy <http://eds.topbraidlive.org/taxonomy/maeco> ;
  rdfs:label "Absolute Levels" ;
  skos:prefLabel "Absolute levels"@en ;
.
maecot:AbsoluteRisk
  rdf:type maeco:RiskMeasure ;
  rdfs:isDefinedBy <http://eds.topbraidlive.org/1.0/taxonomy/maeco> ;
  rdfs:isDefinedBy <http://eds.topbraidlive.org/taxonomy/maeco> ;
  rdfs:label "Absolute Risk" ;
  skos:prefLabel "Absolute risk"@en ;
.
maecot:AbsoluteRiskWeight
  rdf:type maeco:RiskMeasure ;
  rdfs:isDefinedBy <http://eds.topbraidlive.org/1.0/taxonomy/maeco> ;
  rdfs:isDefinedBy <http://eds.topbraidlive.org/taxonomy/maeco> ;
  rdfs:label "Absolute Risk Weight" ;
  skos:broader maecot:RiskWeightingFactor ;
  skos:prefLabel "Absolute risk weight"@en ;
.
maecot:AbsoluteVariation
  rdf:type maeco:QuantityKind ;
  rdfs:isDefinedBy <http://eds.topbraidlive.org/1.0/taxonomy/maeco> ;
  rdfs:isDefinedBy <http://eds.topbraidlive.org/taxonomy/maeco> ;
  rdfs:label "Absolute Variation" ;
  skos:broader maecot:ANY_QuantityKind ;
  skos:prefLabel "Absolute variation"@en ;
.
maecot:Absorption
  rdf:type maeco:QuantityKind ;
  rdfs:isDefinedBy <http://eds.topbraidlive.org/1.0/taxonomy/maeco> ;
  rdfs:isDefinedBy <http://eds.topbraidlive.org/taxonomy/maeco> ;
  rdfs:label "Absorption" ;
  skos:broader maecot:ANY_QuantityKind ;
  skos:definition """<ol><li>Total demand for final goods and services by all residents (consumers, producers, and government) of a country (as opposed to total demand for that country's output). The term was introduced as part of the <a href='http://edg.topbraid.solutions/maeco/term/AbsorptionApproach'>Absorption Approach</a> .</li>
<li><a href='http://edg.topbraid.solutions/maeco/term/RollUp'>Roll-up</a></li></ol>""" ;
  skos:prefLabel "Absorption" ;
.
maecot:AcceptableLevel
  rdf:type maeco:QuantityKind ;
  rdfs:isDefinedBy <http://eds.topbraidlive.org/1.0/taxonomy/maeco> ;
  rdfs:isDefinedBy <http://eds.topbraidlive.org/taxonomy/maeco> ;
  rdfs:label "Acceptable Level" ;
  skos:prefLabel "Acceptable level"@en ;
.
maecot:AccommodateDifferences
  rdf:type maeco:QuantityKind ;
  rdfs:isDefinedBy <http://eds.topbraidlive.org/1.0/taxonomy/maeco> ;
  rdfs:isDefinedBy <http://eds.topbraidlive.org/taxonomy/maeco> ;
  rdfs:label "Accommodate Differences" ;
  skos:prefLabel "Accommodate differences"@en ;
.
maecot:AccumulatedOtherComprehensiveIncome
  rdf:type maeco:QuantityKind ;
  dcterms:source "http://www.cftc.gov/LawRegulation/DoddFrankAct/index.htm"^^xsd:anyURI ;
  rdfs:isDefinedBy <http://eds.topbraidlive.org/1.0/taxonomy/maeco> ;
  rdfs:isDefinedBy <http://eds.topbraidlive.org/taxonomy/maeco> ;
  rdfs:label "Accumulated Other Comprehensive Income" ;
  skos:altLabel "AOCI"@en ;
  skos:broader maecot:Income ;
  skos:definition "Accumulated other comprehensive income. The US bank capital rules eliminate the AOCI filter for advanced approaches banks, which lets banks reverse fair value adjustments to shareholders' equity in their capital calculations. Non-advanced approaches banks can make a one-time election to opt out of the provisions removing the AOCI filter."@en ;
  skos:prefLabel "Accumulated other comprehensive income"@en ;
.
maecot:ActionableSubsidy
  rdf:type maeco:Subsidy ;
  rdfs:isDefinedBy <http://eds.topbraidlive.org/1.0/taxonomy/maeco> ;
  rdfs:isDefinedBy <http://eds.topbraidlive.org/taxonomy/maeco> ;
  rdfs:label "Actionable subsidy" ;
  skos:broader maecot:Subsidy ;
  skos:definition "A <a href='http://edg.topbraid.solutions/maeco/term/Subsidy'>subsidy</a> <a href='http://edg.topbraid.solutions/maeco/term/Wto'>WTO</a> that is neither prohibited by the <a href='http://edg.topbraid.solutions/maeco/term/Cvd2'>countervailing duties</a> nor explicitly permitted, but that member countries are permitted to levy against. Said to be in the <a href='http://edg.topbraid.solutions/maeco/term/AmberBox'>amber box</a>." ;
  skos:prefLabel "Actionable Subsidy" ;
.
maecot:ActualAverageRiskWeight
  rdf:type maeco:RiskMeasure ;
  rdfs:isDefinedBy <http://eds.topbraidlive.org/1.0/taxonomy/maeco> ;
  rdfs:isDefinedBy <http://eds.topbraidlive.org/taxonomy/maeco> ;
  rdfs:label "Actual Average Risk Weight" ;
  skos:broader maecot:RiskWeightingFactor ;
  skos:prefLabel "Actual Average Risk Weight"@en ;
.
maecot:ActualDefault
  rdf:type maeco:QuantityKind ;
  rdfs:isDefinedBy <http://eds.topbraidlive.org/1.0/taxonomy/maeco> ;
  rdfs:isDefinedBy <http://eds.topbraidlive.org/taxonomy/maeco> ;
  rdfs:label "Actual Default" ;
  skos:prefLabel "Actual Default"@en ;
.
maecot:ActualExposure
  rdf:type maeco:QuantityKind ;
  rdfs:isDefinedBy <http://eds.topbraidlive.org/1.0/taxonomy/maeco> ;
  rdfs:isDefinedBy <http://eds.topbraidlive.org/taxonomy/maeco> ;
  rdfs:label "Actual Exposure" ;
  skos:prefLabel "Actual Exposure"@en ;
.
maecot:ActualExposureAmount
  rdf:type maeco:QuantityKind ;
  rdfs:isDefinedBy <http://eds.topbraidlive.org/1.0/taxonomy/maeco> ;
  rdfs:isDefinedBy <http://eds.topbraidlive.org/taxonomy/maeco> ;
  rdfs:label "Actual Exposure Amount" ;
  skos:prefLabel "Actual Exposure Amount"@en ;
.
maecot:ActualProtectionRate
  rdf:type maeco:Rate ;
  rdfs:isDefinedBy <http://eds.topbraidlive.org/1.0/taxonomy/maeco> ;
  rdfs:isDefinedBy <http://eds.topbraidlive.org/taxonomy/maeco> ;
  rdfs:label "Actual protection rate" ;
  skos:broader maecot:ANY_Rate ;
  skos:definition "<a href='http://edg.topbraid.solutions/maeco/term/ImplicitTariff'>Implicit tariff</a> ." ;
  skos:prefLabel "Actual Protection Rate" ;
.
maecot:ActualRisk
  rdf:type maeco:RiskMeasure ;
  rdfs:isDefinedBy <http://eds.topbraidlive.org/1.0/taxonomy/maeco> ;
  rdfs:isDefinedBy <http://eds.topbraidlive.org/taxonomy/maeco> ;
  rdfs:label "Actual Risk" ;
  skos:prefLabel "Actual Risk"@en ;
.
maecot:ActualRiskWeight
  rdf:type maeco:RiskMeasure ;
  rdfs:isDefinedBy <http://eds.topbraidlive.org/1.0/taxonomy/maeco> ;
  rdfs:isDefinedBy <http://eds.topbraidlive.org/taxonomy/maeco> ;
  rdfs:label "Actual Risk Weight" ;
  skos:broader maecot:RiskWeightingFactor ;
  skos:prefLabel "Actual Risk Weights"@en ;
.
maecot:ActualRiskWeightDensity
  rdf:type maeco:RiskMeasure ;
  rdfs:isDefinedBy <http://eds.topbraidlive.org/1.0/taxonomy/maeco> ;
  rdfs:isDefinedBy <http://eds.topbraidlive.org/taxonomy/maeco> ;
  rdfs:label "Actual Risk Weight Density" ;
  skos:broader maecot:RiskWeightingFactor ;
  skos:prefLabel "Actual Risk Weight Density"@en ;
.
maecot:AdValorem
  rdf:type maeco:QuantityKind ;
  rdfs:isDefinedBy <http://eds.topbraidlive.org/1.0/taxonomy/maeco> ;
  rdfs:isDefinedBy <http://eds.topbraidlive.org/taxonomy/maeco> ;
  rdfs:label "Ad valorem" ;
  skos:definition "Per unit of value (i.e., divided by the price)." ;
  skos:prefLabel "Ad Valorem" ;
.
maecot:AdValoremTariff
  rdf:type maeco:Tariff ;
  rdfs:isDefinedBy <http://eds.topbraidlive.org/1.0/taxonomy/maeco> ;
  rdfs:isDefinedBy <http://eds.topbraidlive.org/taxonomy/maeco> ;
  rdfs:label "Ad valorem tariff" ;
  skos:broader maecot:AdValorem ;
  skos:definition "<a href='http://edg.topbraid.solutions/maeco/term/Tariff'>Tariff</a> defined as a percentage of the value of an imported good." ;
  skos:prefLabel "Ad Valorem Tariff" ;
.
maecot:AdditionalTier1Capital
  rdf:type maeco:QuantityKind ;
  dcterms:source "http://www.cftc.gov/LawRegulation/DoddFrankAct/index.htm"^^xsd:anyURI ;
  rdfs:isDefinedBy <http://eds.topbraidlive.org/1.0/taxonomy/maeco> ;
  rdfs:isDefinedBy <http://eds.topbraidlive.org/taxonomy/maeco> ;
  rdfs:label "Additional Tier1Capital" ;
  skos:broader maecot:Capital ;
  skos:definition "Additional Tier 1 capital. AT1 is one of the two components of Tier 1 capital, the highest quality capital under the Basel framework, with the other being common equity Tier 1 (or CET1). In order for an instrument to constitute AT1 it must meet the prescriptive criteria identified in the final Basel III framework, such as an ability to absorb losses, subordination, fully discretionary non-cumulative dividend payments, no incentive to repay or redeem, etc. AT1 also may be referred to as non-core Tier 1. AT1 is subordinate to depositors, general creditors and subordinated debt of the bank."@en ;
  skos:prefLabel "Additional Tier 1 capital"@en ;
.
maecot:AdjustablePeg
  rdf:type maeco:Rate ;
  rdfs:isDefinedBy <http://eds.topbraidlive.org/1.0/taxonomy/maeco> ;
  rdfs:isDefinedBy <http://eds.topbraidlive.org/taxonomy/maeco> ;
  rdfs:label "Adjustable peg" ;
  skos:broader maecot:ExchangeRate ;
  skos:definition "An exchange rate that is <a href='http://edg.topbraid.solutions/maeco/term/PeggedExchangeRate'>pegged</a>, but for which it is understood that the <a href='http://edg.topbraid.solutions/maeco/term/ParValue'>par value</a> will be changed occasionally. This system can be subject to extreme <a href='http://edg.topbraid.solutions/maeco/term/SpeculativeAttack'>speculative attack</a> and <a href='http://edg.topbraid.solutions/maeco/term/FinancialCrisis'>financial crisis</a>, since speculators may easily anticipate these changes." ;
  skos:prefLabel "Adjustable Peg" ;
.
maecot:AdjustmentCost
  rdf:type maeco:Cost ;
  rdfs:isDefinedBy <http://eds.topbraidlive.org/1.0/taxonomy/maeco> ;
  rdfs:isDefinedBy <http://eds.topbraidlive.org/taxonomy/maeco> ;
  rdfs:label "Adjustment cost" ;
  skos:broader maecot:ANY_Cost ;
  skos:definition "<a href='http://edg.topbraid.solutions/maeco/term/TradeLiberalization'>trade liberalization</a> The cost -- temporary but sometimes severe -- incurred by a person or firm in moving from one equilibrium to another. Many of the costs associated with <a href='http://edg.topbraid.solutions/maeco/term/GainsFromTrade'>gains from trade</a> are adjustment costs and are not accounted for in the usual measures of ." ;
  skos:prefLabel "Adjustment Cost" ;
.
maecot:AdministeredPrice
  rdf:type maeco:Price ;
  rdfs:isDefinedBy <http://eds.topbraidlive.org/1.0/taxonomy/maeco> ;
  rdfs:isDefinedBy <http://eds.topbraidlive.org/taxonomy/maeco> ;
  rdfs:label "Administered price" ;
  skos:broader maecot:Price ;
  skos:definition "<a href='http://edg.topbraid.solutions/maeco/term/RestrictedTrade'>restrictions on trade</a> A price for a good or service that is set and maintained by government, usually requiring accompanying  if the administered price differs from the world price." ;
  skos:prefLabel "Administered Price" ;
.
maecot:AggregateDemand
  rdf:type maeco:Demand ;
  rdfs:isDefinedBy <http://eds.topbraidlive.org/1.0/taxonomy/maeco> ;
  rdfs:isDefinedBy <http://eds.topbraidlive.org/taxonomy/maeco> ;
  rdfs:label "Aggregate demand" ;
  skos:definition "The total demand for a country's output, including demands for consumption, investment, government purchases, and net exports." ;
  skos:prefLabel "Aggregate Demand" ;
.
maecot:AggregateSupply
  rdf:type maeco:Supply ;
  rdfs:isDefinedBy <http://eds.topbraidlive.org/1.0/taxonomy/maeco> ;
  rdfs:isDefinedBy <http://eds.topbraidlive.org/taxonomy/maeco> ;
  rdfs:label "Aggregate supply" ;
  skos:definition "The total supply of a country's output of all industries combined, usually assumed to be an increasing function of its price level in the short run but independent of the price level in the long run." ;
  skos:prefLabel "Aggregate Supply" ;
.
maecot:AllInCost
  rdf:type maeco:QuantityKind ;
  dcterms:source "http://www.isda.org/c_and_a/oper_commit-dcg-glossary.html"^^xsd:anyURI ;
  rdfs:isDefinedBy <http://eds.topbraidlive.org/1.0/taxonomy/maeco> ;
  rdfs:isDefinedBy <http://eds.topbraidlive.org/taxonomy/maeco> ;
  rdfs:label "All In Cost" ;
  skos:definition "The cost of funds in a bond issue after fees and expenses."@en ;
  skos:prefLabel "All-in cost"@en ;
.
maecot:AmihudIlliquidity
  rdf:type maeco:Ratio ;
  dcterms:source "http://www.cis.upenn.edu/~mkearns/finread/amihud.pdf"^^xsd:anyURI ;
  dcterms:source "http://www.federalreserve.gov/pubs/feds/2008/200840/200840pap.pdf"^^xsd:anyURI ;
  rdfs:isDefinedBy <http://eds.topbraidlive.org/1.0/taxonomy/maeco> ;
  rdfs:isDefinedBy <http://eds.topbraidlive.org/taxonomy/maeco> ;
  rdfs:label "Amihud Illiquidity" ;
  skos:altLabel "Amihud Measure" ;
  skos:altLabel "ILLIQ" ;
  skos:broader maecot:ANY_Ratio ;
  skos:definition "Amihud Illiquity is defined as the quarterly mean of the ratio of the daily return to the daily dollar volume of trading. Alterante forms of this measure have been defined. For example, the Amihud measure can be defined , on a daily basis, as the ratio of the absolute percentage change in bond price to the dollar size of a trade (in million dollars)." ;
  skos:prefLabel "Amihud Illiquidity" ;
.
maecot:AppliedTariffRate
  rdf:type maeco:Rate ;
  rdfs:isDefinedBy <http://eds.topbraidlive.org/1.0/taxonomy/maeco> ;
  rdfs:isDefinedBy <http://eds.topbraidlive.org/taxonomy/maeco> ;
  rdfs:label "Applied tariff rate" ;
  skos:broader maecot:ANY_Rate ;
  skos:definition "<a href='http://edg.topbraid.solutions/maeco/term/Tariff'>tariff</a> The actual <a href='http://edg.topbraid.solutions/maeco/term/BoundTariff'>bound tariff</a> rate in effect at a country's border, which may be lower than the ." ;
  skos:prefLabel "Applied Tariff Rate" ;
.
maecot:ArmsLengthPrice
  rdf:type maeco:Price ;
  rdfs:isDefinedBy <http://eds.topbraidlive.org/1.0/taxonomy/maeco> ;
  rdfs:isDefinedBy <http://eds.topbraidlive.org/taxonomy/maeco> ;
  rdfs:label "Arm's length price" ;
  skos:broader maecot:Price ;
  skos:definition "<a href='http://edg.topbraid.solutions/maeco/term/TransferPrice'>transfer price</a> The price of a product in a transaction between unrelated buyer and seller. Contrasts with ." ;
  skos:prefLabel "Arm's Length Price" ;
.
maecot:AssetBackedIndex
  rdf:type maeco:IndexMeasure ;
  dcterms:source "http://www.isda.org/c_and_a/oper_commit-dcg-glossary.html"^^xsd:anyURI ;
  rdfs:isDefinedBy <http://eds.topbraidlive.org/1.0/taxonomy/maeco> ;
  rdfs:isDefinedBy <http://eds.topbraidlive.org/taxonomy/maeco> ;
  rdfs:label "Asset Backed Index (ABX)" ;
  skos:altLabel "ABX" ;
  skos:definition "A credit derivative index based on 20 underlying ABS bonds that are backed by subprime mortgages. There are five separate tradable tranches in each series and a new series is issued approximately every six months, market conditions permitting.   "@en ;
  skos:prefLabel "Asset Backed Index" ;
.
maecot:AssetsUnderManagement
  rdf:type maeco:QuantityKind ;
  dcterms:source "http://www.cftc.gov/LawRegulation/DoddFrankAct/index.htm"^^xsd:anyURI ;
  rdfs:isDefinedBy <http://eds.topbraidlive.org/1.0/taxonomy/maeco> ;
  rdfs:isDefinedBy <http://eds.topbraidlive.org/taxonomy/maeco> ;
  rdfs:label "Assets Under Management" ;
  skos:altLabel "AUM" ;
  skos:definition "Assets under management. The value of the assets that an investment adviser manages on behalf of clients."@en ;
  skos:prefLabel "Assets under management"@en ;
.
maecot:AsymmetricPriceAdjustment
  rdf:type maeco:QuantityKind ;
  rdfs:isDefinedBy <http://eds.topbraidlive.org/1.0/taxonomy/maeco> ;
  rdfs:isDefinedBy <http://eds.topbraidlive.org/taxonomy/maeco> ;
  rdfs:label "Asymmetric Price Adjustment" ;
  skos:broader maecot:Price ;
  skos:prefLabel "Asymmetric Price Adjustment" ;
.
maecot:AsymmetricPriceChange
  rdf:type maeco:QuantityKind ;
  rdfs:isDefinedBy <http://eds.topbraidlive.org/1.0/taxonomy/maeco> ;
  rdfs:isDefinedBy <http://eds.topbraidlive.org/taxonomy/maeco> ;
  rdfs:label "Asymmetric Price Change" ;
  skos:broader maecot:Price ;
  skos:prefLabel "Asymmetric Price Change" ;
.
maecot:AttachmentPoint
  rdf:type maeco:Measure ;
  dcterms:source "http://www.isda.org/c_and_a/oper_commit-dcg-glossary.html"^^xsd:anyURI ;
  rdfs:isDefinedBy <http://eds.topbraidlive.org/1.0/taxonomy/maeco> ;
  rdfs:isDefinedBy <http://eds.topbraidlive.org/taxonomy/maeco> ;
  rdfs:label "Attachment Point" ;
  skos:broader maecot:ANY_Measure ;
  skos:definition "A defined point at which the level of losses in the underlying portfolio reduces the notional of a tranche. For example, the notional in a tranche with an attachment point of 3% will reduce after 3% of losses in the portfolio have occurred."@en ;
  skos:prefLabel "Attachment point"@en ;
.
maecot:AutarkyPrice
  rdf:type maeco:Price ;
  rdfs:isDefinedBy <http://eds.topbraidlive.org/1.0/taxonomy/maeco> ;
  rdfs:isDefinedBy <http://eds.topbraidlive.org/taxonomy/maeco> ;
  rdfs:label "Autarky price" ;
  skos:broader maecot:Price ;
  skos:definition "<a href='http://edg.topbraid.solutions/maeco/term/ComparativeAdvantage'>comparative advantage</a> Price in autarky; that is, the price of something within a country when it is not traded by that country. Relative autarky prices turn out to be the most theoretically robust (but empirically elusive) measures of ." ;
  skos:prefLabel "Autarky Price" ;
.
maecot:AverageConversionFactor
  rdf:type maeco:QuantityKind ;
  rdfs:isDefinedBy <http://eds.topbraidlive.org/1.0/taxonomy/maeco> ;
  rdfs:isDefinedBy <http://eds.topbraidlive.org/taxonomy/maeco> ;
  rdfs:label "Average Conversion Factor" ;
  skos:broader maecot:ANY_QuantityKind ;
  skos:prefLabel "Average conversion factor"@en ;
.
maecot:AverageCost
  rdf:type maeco:Cost ;
  dcterms:source "http://www.wwnorton.com/college/econ/stec4/macroeconomics/glossary.asp"^^xsd:anyURI ;
  rdfs:isDefinedBy <http://eds.topbraidlive.org/1.0/taxonomy/maeco> ;
  rdfs:isDefinedBy <http://eds.topbraidlive.org/taxonomy/maeco> ;
  rdfs:label "average cost" ;
  skos:broader maecot:ANY_Average ;
  skos:broader maecot:ANY_Cost ;
  skos:definition "Total cost divided by output." ;
  skos:prefLabel "Average Cost" ;
.
maecot:AverageDefaultRate
  rdf:type maeco:Rate ;
  rdfs:isDefinedBy <http://eds.topbraidlive.org/1.0/taxonomy/maeco> ;
  rdfs:isDefinedBy <http://eds.topbraidlive.org/taxonomy/maeco> ;
  rdfs:label "Average Default Rate" ;
  skos:broader maecot:DefaultRate ;
  skos:prefLabel "Average default rate"@en ;
.
maecot:AverageDeviation
  rdf:type maeco:QuantityKind ;
  rdfs:isDefinedBy <http://eds.topbraidlive.org/1.0/taxonomy/maeco> ;
  rdfs:isDefinedBy <http://eds.topbraidlive.org/taxonomy/maeco> ;
  rdfs:label "Average Deviation" ;
  skos:broader maecot:ANY_QuantityKind ;
  skos:prefLabel "Average deviation"@en ;
.
maecot:AverageLendingFee
  rdf:type maeco:QuantityKind ;
  rdfs:isDefinedBy <http://eds.topbraidlive.org/1.0/taxonomy/maeco> ;
  rdfs:isDefinedBy <http://eds.topbraidlive.org/taxonomy/maeco> ;
  rdfs:label "Average Lending Fee" ;
  skos:broader maecot:ANY_Average ;
  skos:prefLabel "Average Lending Fee" ;
.
maecot:AverageRiskWeight
  rdf:type maeco:RiskMeasure ;
  rdfs:isDefinedBy <http://eds.topbraidlive.org/1.0/taxonomy/maeco> ;
  rdfs:isDefinedBy <http://eds.topbraidlive.org/taxonomy/maeco> ;
  rdfs:label "Average Risk Weight" ;
  skos:broader maecot:RiskWeightingFactor ;
  skos:prefLabel "Average risk weight"@en ;
.
maecot:AverageRiskWeightDeviation
  rdf:type maeco:RiskMeasure ;
  rdfs:isDefinedBy <http://eds.topbraidlive.org/1.0/taxonomy/maeco> ;
  rdfs:isDefinedBy <http://eds.topbraidlive.org/taxonomy/maeco> ;
  rdfs:label "Average Risk Weight Deviation" ;
  skos:broader maecot:RiskWeightingFactor ;
  skos:prefLabel "Average risk weight deviation"@en ;
.
maecot:AverageShortSaleDuration
  rdf:type maeco:QuantityKind ;
  rdfs:isDefinedBy <http://eds.topbraidlive.org/1.0/taxonomy/maeco> ;
  rdfs:isDefinedBy <http://eds.topbraidlive.org/taxonomy/maeco> ;
  rdfs:label "Average Short Sale Duration" ;
  skos:broader maecot:ANY_Average ;
  skos:prefLabel "Average Short Sale Duration" ;
.
maecot:AverageTariff
  rdf:type maeco:Tariff ;
  rdfs:isDefinedBy <http://eds.topbraidlive.org/1.0/taxonomy/maeco> ;
  rdfs:isDefinedBy <http://eds.topbraidlive.org/taxonomy/maeco> ;
  rdfs:label "Average tariff" ;
  skos:broader maecot:ANY_Average ;
  skos:broader maecot:Tariff ;
  skos:definition "<a href='http://edg.topbraid.solutions/maeco/term/TradeWeightedAverageTariff'>trade-weighted average tariff</a> An average of a country's tariff rates. This can be calculated in several ways, of which none are ideal for representing how protective the country's tariffs are. Most common is the <a href='http://edg.topbraid.solutions/maeco/term/ProhibitiveTariff'>prohibitive tariffs</a> , which under-represents , since they get zero weight." ;
  skos:prefLabel "Average Tariff" ;
.
maecot:AverageTaxRate
  rdf:type maeco:Rate ;
  dcterms:source "http://www.wwnorton.com/college/econ/stec4/macroeconomics/glossary.asp"^^xsd:anyURI ;
  rdfs:isDefinedBy <http://eds.topbraidlive.org/1.0/taxonomy/maeco> ;
  rdfs:isDefinedBy <http://eds.topbraidlive.org/taxonomy/maeco> ;
  rdfs:label "average tax rate" ;
  skos:broader maecot:ANY_Average ;
  skos:broader maecot:ANY_Rate ;
  skos:definition "The amount paid as tax as a fraction of the amount being taxed. In the case of an <a href='http://edg.topbraid.solutions/maeco/term/MarginalTaxRate'>marginal tax rate</a> , the total amount of tax as a fraction of total income. Contrasts with <a href='http://edg.topbraid.solutions/maeco/term/IncomeTax'>income tax</a> ." ;
  skos:prefLabel "Average Tax Rate" ;
.
maecot:AverageVariableCost
  rdf:type maeco:Cost ;
  dcterms:source "http://www.wwnorton.com/college/econ/stec4/macroeconomics/glossary.asp"^^xsd:anyURI ;
  rdfs:isDefinedBy <http://eds.topbraidlive.org/1.0/taxonomy/maeco> ;
  rdfs:isDefinedBy <http://eds.topbraidlive.org/taxonomy/maeco> ;
  rdfs:label "Average Variable Cost" ;
  skos:broader maecot:VariableCost ;
  skos:definition "<STRONG>Average Variable Costs</STRONG> - total variable costs divided by total output" ;
  skos:prefLabel "Average Variable Cost" ;
.
maecot:BankCapitalRatio
  rdf:type maeco:Ratio ;
  rdfs:isDefinedBy <http://eds.topbraidlive.org/1.0/taxonomy/maeco> ;
  rdfs:isDefinedBy <http://eds.topbraidlive.org/taxonomy/maeco> ;
  rdfs:label "Bank Capital Ratio" ;
  skos:broader maecot:ANY_Ratio ;
  skos:prefLabel "Bank capital ratio" ;
.
maecot:BankRate
  rdf:type maeco:Rate ;
  rdfs:isDefinedBy <http://eds.topbraidlive.org/1.0/taxonomy/maeco> ;
  rdfs:isDefinedBy <http://eds.topbraidlive.org/taxonomy/maeco> ;
  rdfs:label "Bank rate" ;
  skos:broader maecot:ANY_Rate ;
  skos:definition "The interest rate charged by a central bank to commercial banks for very short term loans; the <a href='http://edg.topbraid.solutions/maeco/term/DiscountRate'>discount rate</a> ." ;
  skos:prefLabel "Bank Rate" ;
.
maecot:BaselRiskWeightings
  rdf:type maeco:RiskMeasure ;
  rdfs:isDefinedBy <http://eds.topbraidlive.org/1.0/taxonomy/maeco> ;
  rdfs:isDefinedBy <http://eds.topbraidlive.org/taxonomy/maeco> ;
  rdfs:label "Basel Risk Weightings" ;
  skos:broader maecot:RiskWeightingFactor ;
  skos:prefLabel "Basel risk weightings"@en ;
.
maecot:BasicImportPrice
  rdf:type maeco:Price ;
  rdfs:isDefinedBy <http://eds.topbraidlive.org/1.0/taxonomy/maeco> ;
  rdfs:isDefinedBy <http://eds.topbraidlive.org/taxonomy/maeco> ;
  rdfs:label "Basic import price" ;
  skos:broader maecot:Price ;
  skos:definition "See <a href='http://edg.topbraid.solutions/maeco/term/MinimumPriceSystem'>minimum price system</a> ." ;
  skos:prefLabel "Basic Import Price" ;
.
maecot:BasisPoint
  rdf:type maeco:QuantityKind ;
  dcterms:source "http://www.isda.org/c_and_a/oper_commit-dcg-glossary.html"^^xsd:anyURI ;
  rdfs:isDefinedBy <http://eds.topbraidlive.org/1.0/taxonomy/maeco> ;
  rdfs:isDefinedBy <http://eds.topbraidlive.org/taxonomy/maeco> ;
  rdfs:label "Basis point" ;
  skos:broader maecot:ANY_QuantityKind ;
  skos:definition "One basis point is one hundredth of one percent, or 0.01%.   "@en ;
  skos:definition "One one-hundredth of a percentage point.  Small changes in <a href='http://edg.topbraid.solutions/maeco/term/InterestRate'>interest rates</a> are commonly measured in basis points." ;
  skos:prefLabel "Basis point"@en ;
.
maecot:BenchmarkCapitalRatio
  rdf:type maeco:Ratio ;
  rdfs:isDefinedBy <http://eds.topbraidlive.org/1.0/taxonomy/maeco> ;
  rdfs:isDefinedBy <http://eds.topbraidlive.org/taxonomy/maeco> ;
  rdfs:label "Benchmark Capital Ratio" ;
  skos:broader maecot:ANY_Ratio ;
  skos:prefLabel "Benchmark capital ratio"@en ;
.
maecot:BenchmarkRiskWeight
  rdf:type maeco:RiskMeasure ;
  rdfs:isDefinedBy <http://eds.topbraidlive.org/1.0/taxonomy/maeco> ;
  rdfs:isDefinedBy <http://eds.topbraidlive.org/taxonomy/maeco> ;
  rdfs:label "Benchmark Risk Weight" ;
  skos:broader maecot:RiskWeightingFactor ;
  skos:prefLabel "Benchmark risk weight"@en ;
.
maecot:Bid-askSpread
  rdf:type maeco:QuantityKind ;
  rdfs:isDefinedBy <http://eds.topbraidlive.org/1.0/taxonomy/maeco> ;
  rdfs:isDefinedBy <http://eds.topbraidlive.org/taxonomy/maeco> ;
  rdfs:label "Bid/ask spread" ;
  skos:definition "The difference between the price that a buyer must pay on a market and the price that a seller will receive for the same thing.  The difference covers the cost of, and provides profit for, the broker or other intermediary, such as a bank on the foreign exchange market." ;
  skos:prefLabel "bid-ask spread" ;
.
maecot:BidOffer
  rdf:type maeco:QuantityKind ;
  dcterms:source "http://www.isda.org/c_and_a/oper_commit-dcg-glossary.html"^^xsd:anyURI ;
  rdfs:isDefinedBy <http://eds.topbraidlive.org/1.0/taxonomy/maeco> ;
  rdfs:isDefinedBy <http://eds.topbraidlive.org/taxonomy/maeco> ;
  rdfs:label "Bid Offer" ;
  skos:broader maecot:ANY_QuantityKind ;
  skos:definition "The difference between the bid and the offer rate.  The bid offer spread is a measure of liquidity and counterparty risk."@en ;
  skos:prefLabel "Spread (bid offer)"@en ;
.
maecot:BidPrice
  rdf:type maeco:QuantityKind ;
  dcterms:source "http://www.isda.org/c_and_a/oper_commit-dcg-glossary.html"^^xsd:anyURI ;
  rdfs:isDefinedBy <http://eds.topbraidlive.org/1.0/taxonomy/maeco> ;
  rdfs:isDefinedBy <http://eds.topbraidlive.org/taxonomy/maeco> ;
  rdfs:label "Bid Price" ;
  skos:broader maecot:Price ;
  skos:definition "The price at which a trader or market maker is willing to purchase a contract."@en ;
  skos:prefLabel "Bid price"@en ;
.
maecot:BilateralExchangeRate
  rdf:type maeco:Rate ;
  rdfs:isDefinedBy <http://eds.topbraidlive.org/1.0/taxonomy/maeco> ;
  rdfs:isDefinedBy <http://eds.topbraidlive.org/taxonomy/maeco> ;
  rdfs:label "Bilateral exchange rate" ;
  skos:broader maecot:ANY_Rate ;
  skos:definition "The <a href='http://edg.topbraid.solutions/maeco/term/ExchangeRate'>exchange rate</a> between two countries' currencies, defined as the number of units of either currency needed to purchase one unit of the other." ;
  skos:prefLabel "Bilateral Exchange Rate" ;
.
maecot:BilateralTradeBalance
  rdf:type maeco:QuantityKind ;
  rdfs:isDefinedBy <http://eds.topbraidlive.org/1.0/taxonomy/maeco> ;
  rdfs:isDefinedBy <http://eds.topbraidlive.org/taxonomy/maeco> ;
  rdfs:label "Bilateral trade balance" ;
  skos:definition "The value of a country's exports to a single other country, minus the value of its imports from that country.  While data on bilateral trade imbalances are often reported, economists discount them as essentially meaningless, due to the potential for <a href='http://edg.topbraid.solutions/maeco/term/TriangularTrade'>triangular trade</a> ." ;
  skos:prefLabel "Bilateral Trade Balance" ;
.
maecot:BondDuration
  rdf:type maeco:QuantityKind ;
  dcterms:source "http://www.isda.org/c_and_a/oper_commit-dcg-glossary.html"^^xsd:anyURI ;
  rdfs:isDefinedBy <http://eds.topbraidlive.org/1.0/taxonomy/maeco> ;
  rdfs:isDefinedBy <http://eds.topbraidlive.org/taxonomy/maeco> ;
  rdfs:label "Bond Duration" ;
  skos:broader maecot:ANY_QuantityKind ;
  skos:definition "A measure of the effective maturity of a bond. Duration is an approximation for the price change of a bond for a given change in the interest rate, and is used as a measure of sensitivity of bond prices to market changes. Duration is measured in units of time. It includes the effects of time until maturity, cash flows and the yield to maturity."@en ;
  skos:prefLabel "Bond Duration"@en ;
.
maecot:BondLiquidity
  rdf:type maeco:LiquidityMeasure ;
  rdfs:isDefinedBy <http://eds.topbraidlive.org/1.0/taxonomy/maeco> ;
  rdfs:isDefinedBy <http://eds.topbraidlive.org/taxonomy/maeco> ;
  rdfs:label "Bond Liquidity" ;
  skos:broader maecot:ANY_LiquidityMeasure ;
  skos:prefLabel "Bond Liquidity" ;
.
maecot:BorderPrice
  rdf:type maeco:Price ;
  rdfs:isDefinedBy <http://eds.topbraidlive.org/1.0/taxonomy/maeco> ;
  rdfs:isDefinedBy <http://eds.topbraidlive.org/taxonomy/maeco> ;
  rdfs:label "Border price" ;
  skos:broader maecot:Price ;
  skos:definition "The price of a good at a country's border." ;
  skos:prefLabel "Border Price" ;
.
maecot:BoundRate
  rdf:type maeco:Rate ;
  rdfs:isDefinedBy <http://eds.topbraidlive.org/1.0/taxonomy/maeco> ;
  rdfs:isDefinedBy <http://eds.topbraidlive.org/taxonomy/maeco> ;
  rdfs:label "Bound rate" ;
  skos:broader maecot:ANY_Rate ;
  skos:definition "See <a href='http://edg.topbraid.solutions/maeco/term/TariffBinding'>tariff binding</a> ." ;
  skos:prefLabel "Bound Rate" ;
.
maecot:BoundTariff
  rdf:type maeco:Tariff ;
  rdfs:isDefinedBy <http://eds.topbraidlive.org/1.0/taxonomy/maeco> ;
  rdfs:isDefinedBy <http://eds.topbraidlive.org/taxonomy/maeco> ;
  rdfs:label "Bound tariff" ;
  skos:broader maecot:Tariff ;
  skos:definition "See <a href='http://edg.topbraid.solutions/maeco/term/TariffBinding'>tariff binding</a> ." ;
  skos:prefLabel "Bound Tariff" ;
.
maecot:BreadthOfOwnership
  rdf:type maeco:QuantityKind ;
  rdfs:isDefinedBy <http://eds.topbraidlive.org/1.0/taxonomy/maeco> ;
  rdfs:isDefinedBy <http://eds.topbraidlive.org/taxonomy/maeco> ;
  rdfs:label "Average" ;
  skos:broader maecot:ANY_QuantityKind ;
  skos:definition "Breadth of Ownership" ;
  skos:prefLabel "Average" ;
.
maecot:CalculationPeriod
  rdf:type maeco:QuantityKind ;
  dcterms:source "http://www.isda.org/c_and_a/oper_commit-dcg-glossary.html"^^xsd:anyURI ;
  rdfs:isDefinedBy <http://eds.topbraidlive.org/1.0/taxonomy/maeco> ;
  rdfs:isDefinedBy <http://eds.topbraidlive.org/taxonomy/maeco> ;
  rdfs:label "Calculation Period" ;
  skos:broader maecot:ANY_QuantityKind ;
  skos:definition "The number of days between payment dates or between effective date and the first payment date. The first day is generally included and the last day generally excluded."@en ;
  skos:prefLabel "Calculation period"@en ;
.
maecot:Cap
  rdf:type maeco:QuantityKind ;
  dcterms:source "http://www.isda.org/c_and_a/oper_commit-dcg-glossary.html"^^xsd:anyURI ;
  rdfs:isDefinedBy <http://eds.topbraidlive.org/1.0/taxonomy/maeco> ;
  rdfs:isDefinedBy <http://eds.topbraidlive.org/taxonomy/maeco> ;
  rdfs:label "Cap" ;
  skos:broader maecot:ANY_QuantityKind ;
  skos:definition "An upper limit placed on the payoff of a trade, limiting the upside to the buyer and thus the downside to the seller."@en ;
  skos:prefLabel "Cap"@en ;
.
maecot:Capital
  rdf:type maeco:QuantityKind ;
  dcterms:source "http://www.cftc.gov/LawRegulation/DoddFrankAct/index.htm"^^xsd:anyURI ;
  rdfs:isDefinedBy <http://eds.topbraidlive.org/1.0/taxonomy/maeco> ;
  rdfs:isDefinedBy <http://eds.topbraidlive.org/taxonomy/maeco> ;
  rdfs:label "Capital" ;
  skos:definition "<STRONG>1.</STRONG> The plant and equipment used in production.  <STRONG>2.</STRONG> One of the main <a href='http://edg.topbraid.solutions/maeco/term/PrimaryFactor'>primary factors</a> , the availability of which contributes to the <a href='http://edg.topbraid.solutions/maeco/term/LaborProductivity'>productivity of labor</a> , <a href='http://edg.topbraid.solutions/maeco/term/ComparativeAdvantage'>comparative advantage</a> , and the <a href='http://edg.topbraid.solutions/maeco/term/TradePattern'>pattern of international trade</a> .  <STRONG>3.</STRONG> A stock of financial assets.  <STRONG>4.</STRONG> Of a bank, its <a href='http://edg.topbraid.solutions/maeco/term/Asset'>assets</a> minus its <a href='http://edg.topbraid.solutions/maeco/term/Liability'>liabilities</a> ." ;
  skos:prefLabel "Capital" ;
.
maecot:CapitalAdequacy
  rdf:type maeco:QuantityKind ;
  rdfs:isDefinedBy <http://eds.topbraidlive.org/1.0/taxonomy/maeco> ;
  rdfs:isDefinedBy <http://eds.topbraidlive.org/taxonomy/maeco> ;
  rdfs:label "Capital Adequacy" ;
  skos:broader maecot:Capital ;
  skos:prefLabel "Capital adequacy"@en ;
.
maecot:CapitalAssetsManagementEarningsLiquidityMarketSensitivity
  rdf:type maeco:QuantityKind ;
  dcterms:source "http://www.cftc.gov/LawRegulation/DoddFrankAct/index.htm"^^xsd:anyURI ;
  rdfs:isDefinedBy <http://eds.topbraidlive.org/1.0/taxonomy/maeco> ;
  rdfs:isDefinedBy <http://eds.topbraidlive.org/taxonomy/maeco> ;
  rdfs:label "Capital, Assets, Management, Earnings, Liquidity, Market Sensitivity (Regulatory Bank Ratings)." ;
  skos:altLabel "CAMELS" ;
  skos:broader maecot:ANY_QuantityKind ;
  skos:definition "Capital adequacy, Assets, Management capability, Earnings, Liquidity, market Sensitivity. The CAMELS rating system (from 1 to 5) is a supervisory system for US banks to evaluate the banks' condition. A CAMEL 1 rating is the strongest and a CAMEL 4 or 5 indicates serious concerns. These ratings are not published."@en ;
  skos:prefLabel "Capital, Assets, Management, Earnings, Liquidity, Market Sensitivity (Regulatory Bank Ratings)"@en ;
.
maecot:CapitalConservationBuffer
  rdf:type maeco:Buffer ;
  dcterms:source "http://www.cftc.gov/LawRegulation/DoddFrankAct/index.htm"^^xsd:anyURI ;
  dcterms:source "http://www.prarulebook.co.uk/rulebook/Content/Part/211272/13-04-2016"^^xsd:anyURI ;
  rdfs:isDefinedBy <http://eds.topbraidlive.org/1.0/taxonomy/maeco> ;
  rdfs:isDefinedBy <http://eds.topbraidlive.org/taxonomy/maeco> ;
  rdfs:label "Capital Conservation Buffer" ;
  skos:broader maecot:ANY_Buffer ;
  skos:definition "The capital conservation buffer is a buffer of capital above the minimum conservation Tier 1 capital requirement, consisting of CET1, that can be drawn on buffer in times of stress, and is formulated as 2.5% of total RWA (or TRWA). This is an entirely new element introduced by Basel III. The aim of the buffer is to prevent firms from making distributions during times when they are experiencing financial difficulties."@en ;
  skos:prefLabel "Capital Conservation Buffer"@en ;
.
maecot:CapitalDeductions
  rdf:type maeco:QuantityKind ;
  rdfs:isDefinedBy <http://eds.topbraidlive.org/1.0/taxonomy/maeco> ;
  rdfs:isDefinedBy <http://eds.topbraidlive.org/taxonomy/maeco> ;
  rdfs:label "Capital Deductions" ;
  skos:broader maecot:Capital ;
  skos:prefLabel "Capital deductions"@en ;
.
maecot:CapitalFloor
  rdf:type maeco:QuantityKind ;
  rdfs:isDefinedBy <http://eds.topbraidlive.org/1.0/taxonomy/maeco> ;
  rdfs:isDefinedBy <http://eds.topbraidlive.org/taxonomy/maeco> ;
  rdfs:label "Capital Floor" ;
  skos:broader maecot:Capital ;
  skos:prefLabel "Capital floor"@en ;
.
maecot:CapitalRatio
  rdf:type maeco:Ratio ;
  rdfs:isDefinedBy <http://eds.topbraidlive.org/1.0/taxonomy/maeco> ;
  rdfs:isDefinedBy <http://eds.topbraidlive.org/taxonomy/maeco> ;
  rdfs:label "Capital Ratio" ;
  skos:broader maecot:ANY_Ratio ;
  skos:prefLabel "Capital ratio"@en ;
.
maecot:CapitalRatioDeviation
  rdf:type maeco:Ratio ;
  rdfs:isDefinedBy <http://eds.topbraidlive.org/1.0/taxonomy/maeco> ;
  rdfs:isDefinedBy <http://eds.topbraidlive.org/taxonomy/maeco> ;
  rdfs:label "Capital Ratio Deviation" ;
  skos:broader maecot:ANY_Ratio ;
  skos:prefLabel "Capital ratio deviation"@en ;
.
maecot:CapitalRatioReduction
  rdf:type maeco:Ratio ;
  rdfs:isDefinedBy <http://eds.topbraidlive.org/1.0/taxonomy/maeco> ;
  rdfs:isDefinedBy <http://eds.topbraidlive.org/taxonomy/maeco> ;
  rdfs:label "Capital Ratio Reduction" ;
  skos:broader maecot:ANY_Ratio ;
  skos:prefLabel "Capital ratio reduction"@en ;
.
maecot:CarbonTariff
  rdf:type maeco:Tariff ;
  rdfs:isDefinedBy <http://eds.topbraidlive.org/1.0/taxonomy/maeco> ;
  rdfs:isDefinedBy <http://eds.topbraidlive.org/taxonomy/maeco> ;
  rdfs:label "Carbon tariff" ;
  skos:broader maecot:Tariff ;
  skos:definition "A <a href='http://edg.topbraid.solutions/maeco/term/Tariff'>tariff</a> levied on the basis of carbon dioxide that an import's production emits into the atmosphere.  The purposes are to treat imports equally with domestic goods that are subject to costly environmental regulation or tax, and also to motivate other countries to use such environmental policies." ;
  skos:prefLabel "Carbon Tariff" ;
.
maecot:CashInflow
  rdf:type maeco:QuantityKind ;
  rdfs:isDefinedBy <http://eds.topbraidlive.org/1.0/taxonomy/maeco> ;
  rdfs:isDefinedBy <http://eds.topbraidlive.org/taxonomy/maeco> ;
  rdfs:label "Cash Inflow" ;
  skos:broader maecot:ANY_QuantityKind ;
  skos:definition "When considering its available cash inflows, the bank should only include contractual inflows (including interest payments) from outstanding exposures that are fully performing and for which the bank has no reason to expect a default within the 30-day time horizon. Contingent inflows are not included in total net cash inflows."@en ;
  skos:prefLabel "Cash inflow"@en ;
  prov:wasInfluencedBy "<http://www.bis.org/publ/bcbs238.pdf>" ;
.
maecot:CleanPrice
  rdf:type maeco:QuantityKind ;
  dcterms:source "http://www.isda.org/c_and_a/oper_commit-dcg-glossary.html"^^xsd:anyURI ;
  rdfs:isDefinedBy <http://eds.topbraidlive.org/1.0/taxonomy/maeco> ;
  rdfs:isDefinedBy <http://eds.topbraidlive.org/taxonomy/maeco> ;
  rdfs:label "Clean Price" ;
  skos:broader maecot:ANY_QuantityKind ;
  skos:definition "The price of a bond net of accrued interest."@en ;
  skos:prefLabel "Clean price"@en ;
.
maecot:CommercialMortgageBackedIndex
  rdf:type maeco:IndexMeasure ;
  dcterms:source "http://www.isda.org/c_and_a/oper_commit-dcg-glossary.html"^^xsd:anyURI ;
  rdfs:isDefinedBy <http://eds.topbraidlive.org/1.0/taxonomy/maeco> ;
  rdfs:isDefinedBy <http://eds.topbraidlive.org/taxonomy/maeco> ;
  rdfs:label "Commercial Mortgage Backed Index (CMBX)" ;
  skos:altLabel "CMBX" ;
  skos:definition "A credit derivative index which is referenced to 25 underlying CMBS bonds. There are five separate tradable tranches in each series and a new series is issued every six months. The index is based on the PAUG product."@en ;
  skos:prefLabel "Commercial Mortgage Backed Index"@en ;
.
maecot:CommittedCreditFacilities
  rdf:type maeco:QuantityKind ;
  rdfs:isDefinedBy <http://eds.topbraidlive.org/1.0/taxonomy/maeco> ;
  rdfs:isDefinedBy <http://eds.topbraidlive.org/taxonomy/maeco> ;
  rdfs:label "Committed Credit Facilities" ;
  skos:broader maecot:ANY_QuantityKind ;
  skos:definition "Committed credit and liquidity facilities to retail and small business customers."@en ;
  skos:prefLabel "Committed Credit Facilities" ;
  prov:wasInfluencedBy "<http://www.bis.org/publ/bcbs238.pdf>" ;
.
maecot:CommittedCreditFacilitiesType1
  rdf:type maeco:QuantityKind ;
  rdfs:isDefinedBy <http://eds.topbraidlive.org/1.0/taxonomy/maeco> ;
  rdfs:isDefinedBy <http://eds.topbraidlive.org/taxonomy/maeco> ;
  rdfs:label "Committed Credit Facilities Type1" ;
  skos:broader maecot:CommittedCreditFacilities ;
  skos:definition "Committed credit and liquidity facilities to retail and small business customers: Banks should assume a 5% drawdown of the undrawn portion of these facilities."@en ;
  skos:prefLabel "Committed credit and liquidity facilities to retail and small business customers"@en ;
  prov:wasInfluencedBy "<http://www.bis.org/publ/bcbs238.pdf>" ;
.
maecot:CommittedCreditFacilitiesType2
  rdf:type maeco:QuantityKind ;
  rdfs:isDefinedBy <http://eds.topbraidlive.org/1.0/taxonomy/maeco> ;
  rdfs:isDefinedBy <http://eds.topbraidlive.org/taxonomy/maeco> ;
  rdfs:label "Committed Credit Facilities Type2" ;
  skos:broader maecot:CommittedCreditFacilities ;
  skos:definition "Committed credit facilities to non-financial corporates, sovereigns and central banks: PSEs and multilateral development banks: Banks should assume a 10% drawdown of the undrawn portion of these credit facilities."@en ;
  skos:prefLabel "Committed credit facilities to non-financial corporates, sovereigns and central banks"@en ;
  prov:wasInfluencedBy "<http://www.bis.org/publ/bcbs238.pdf>" ;
.
maecot:CommittedCreditFacilitiesType3
  rdf:type maeco:QuantityKind ;
  rdfs:isDefinedBy <http://eds.topbraidlive.org/1.0/taxonomy/maeco> ;
  rdfs:isDefinedBy <http://eds.topbraidlive.org/taxonomy/maeco> ;
  rdfs:label "Committed Credit Facilities Type3" ;
  skos:broader maecot:CommittedCreditFacilities ;
  skos:definition "Committed liquidity facilities to non-financial corporates, sovereigns and central banks, PSEs, and multilateral development banks: Banks should assume a 30% drawdown of the undrawn portion of these liquidity facilities."@en ;
  skos:prefLabel "Committed credit and liquidity facilities to retail and small business customers"@en ;
  prov:wasInfluencedBy "<http://www.bis.org/publ/bcbs238.pdf>" ;
.
maecot:CommittedCreditFacilitiesType4
  rdf:type maeco:QuantityKind ;
  rdfs:isDefinedBy <http://eds.topbraidlive.org/1.0/taxonomy/maeco> ;
  rdfs:isDefinedBy <http://eds.topbraidlive.org/taxonomy/maeco> ;
  rdfs:label "Committed credit and liquidity facilities extended to banks  subject to prudential supervision" ;
  skos:altLabel "Committed Credit Facilities Type 4" ;
  skos:broader maecot:CommittedCreditFacilities ;
  skos:definition "Committed credit and liquidity  facilities  extended  to banks  subject to prudential supervision: Banks should assume a 40% drawdown of the undrawn portion of these facilities."@en ;
  skos:prefLabel "Committed credit and liquidity facilities extended to banks subject to prudential supervision"@en ;
  prov:wasInfluencedBy "<http://www.bis.org/publ/bcbs238.pdf>" ;
.
maecot:CommittedCreditFacilitiesType5
  rdf:type maeco:QuantityKind ;
  rdfs:isDefinedBy <http://eds.topbraidlive.org/1.0/taxonomy/maeco> ;
  rdfs:isDefinedBy <http://eds.topbraidlive.org/taxonomy/maeco> ;
  rdfs:label "Committed Credit Facilities Type5" ;
  skos:broader maecot:CommittedCreditFacilities ;
  skos:definition "Committed credit facilities to other financial institutions including securities firms, insurance companies, fiduciaries, and beneficiaries: Banks should assume a 40% drawdown of the undrawn portion of these credit facilities."@en ;
  skos:prefLabel "Committed credit facilities to other financial institutions including securities firms, insurance companies, fiduciaries, and beneficiaries"@en ;
  prov:wasInfluencedBy "<http://www.bis.org/publ/bcbs238.pdf>" ;
.
maecot:CommittedCreditFacilitiesType6
  rdf:type maeco:QuantityKind ;
  rdfs:isDefinedBy <http://eds.topbraidlive.org/1.0/taxonomy/maeco> ;
  rdfs:isDefinedBy <http://eds.topbraidlive.org/taxonomy/maeco> ;
  rdfs:label "Committed Credit Facilities Type6" ;
  skos:broader maecot:CommittedCreditFacilities ;
  skos:definition "Committed liquidity facilities to other financial institutions including securities firms, insurance companies, fiduciaries, and beneficiaries: Banks should assume a 100% drawdown of the undrawn portion of these liquidity facilities."@en ;
  skos:prefLabel "Committed liquidity facilities to other financial institutions including securities firms, insurance companies, fiduciaries, and beneficiaries"@en ;
  prov:wasInfluencedBy "<http://www.bis.org/publ/bcbs238.pdf>" ;
.
maecot:CommittedCreditFacilitiesType7
  rdf:type maeco:QuantityKind ;
  rdfs:isDefinedBy <http://eds.topbraidlive.org/1.0/taxonomy/maeco> ;
  rdfs:isDefinedBy <http://eds.topbraidlive.org/taxonomy/maeco> ;
  rdfs:label "Committed Credit Facilities Type7" ;
  skos:broader maecot:CommittedCreditFacilities ;
  skos:definition "Committed credit and liquidity facilities to other legal entities (including SPEs conduits and special purpose vehicles, and other entities not included in the prior categories): Banks should assume a 100% drawdown of the undrawn portion of these facilities."@en ;
  skos:prefLabel "Committed credit and liquidity facilities to other legal entities (including SPEs conduits and special purpose vehicles, and other entities not included in the prior categories)"@en ;
  prov:wasInfluencedBy "<http://www.bis.org/publ/bcbs238.pdf>" ;
.
maecot:CommonEffectivePreferentialTariff
  rdf:type maeco:Tariff ;
  rdfs:isDefinedBy <http://eds.topbraidlive.org/1.0/taxonomy/maeco> ;
  rdfs:isDefinedBy <http://eds.topbraidlive.org/taxonomy/maeco> ;
  rdfs:label "Common effective preferential tariff" ;
  skos:broader maecot:Tariff ;
  skos:definition "The CEPT tariff is the <a href='http://edg.topbraid.solutions/maeco/term/Tariff'>tariff</a> that a member of the <a href='http://edg.topbraid.solutions/maeco/term/Afta2'>ASEAN Free Trade Area</a> applies to imports that originate in another AFTA country.  Unlike conventional <a href='http://edg.topbraid.solutions/maeco/term/Fta2'>free trade areas</a> , the CEPT tariff is not required to be zero, but only between zero and 5%.  In addition, countries are permitted to designate products as excluded from the CEPT for several reasons." ;
  skos:prefLabel "Common Effective Preferential Tariff" ;
.
maecot:CommonExternalTariff
  rdf:type maeco:Tariff ;
  rdfs:isDefinedBy <http://eds.topbraidlive.org/1.0/taxonomy/maeco> ;
  rdfs:isDefinedBy <http://eds.topbraidlive.org/taxonomy/maeco> ;
  rdfs:label "Common external tariff" ;
  skos:broader maecot:Tariff ;
  skos:definition "The single tariff rate on a product agreed to by all members of a <a href='http://edg.topbraid.solutions/maeco/term/CustomsUnion'>customs union</a> on imports of that product from outside the union." ;
  skos:prefLabel "Common External Tariff" ;
.
maecot:CompoundTariff
  rdf:type maeco:Tariff ;
  rdfs:isDefinedBy <http://eds.topbraidlive.org/1.0/taxonomy/maeco> ;
  rdfs:isDefinedBy <http://eds.topbraidlive.org/taxonomy/maeco> ;
  rdfs:label "Compound tariff" ;
  skos:broader maecot:Tariff ;
  skos:definition "A <a href='http://edg.topbraid.solutions/maeco/term/Tariff'>tariff</a> that combines both a <a href='http://edg.topbraid.solutions/maeco/term/SpecificTariff'>specific</a> and an <a href='http://edg.topbraid.solutions/maeco/term/AdValorem'>ad valorem</a> component.  Thus, on an import with quantity <em>q</em> and price <em>p</em> , a compound tariff collects a revenue equal to <em>pq</em> , where <em>t</em> is the specific tariff and <em>t</em> is the ad valorem tariff." ;
  skos:prefLabel "Compound Tariff" ;
.
maecot:ConstantCost
  rdf:type maeco:Cost ;
  rdfs:isDefinedBy <http://eds.topbraidlive.org/1.0/taxonomy/maeco> ;
  rdfs:isDefinedBy <http://eds.topbraidlive.org/taxonomy/maeco> ;
  rdfs:label "Constant cost" ;
  skos:broader maecot:ANY_Cost ;
  skos:definition "This could have many meanings, but when stated as an assumption of an economic model, it means that cost of producing a good, per unit, is the same for all units, and thus does not rise or fall with output." ;
  skos:prefLabel "Constant Cost" ;
.
maecot:ContingentFundingObligation
  rdf:type maeco:QuantityKind ;
  rdfs:isDefinedBy <http://eds.topbraidlive.org/1.0/taxonomy/maeco> ;
  rdfs:isDefinedBy <http://eds.topbraidlive.org/taxonomy/maeco> ;
  rdfs:label "Contingent Funding Obligation" ;
  skos:broader maecot:RetailDeposits ;
  skos:definition "Run-off rates at national discretion. National supervisors will work with supervised institutions in their jurisdictions to determine the liquidity risk impact of these contingent liabilities and the resulting stock of HQLA that should accordingly be maintained. Supervisors should disclose the run-off rates they assign to each category publicly."@en ;
  skos:prefLabel "Contingent Funding Obligation"@en ;
  prov:wasInfluencedBy "<http://www.bis.org/publ/bcbs238.pdf>" ;
.
maecot:Convergence
  rdf:type maeco:Measure ;
  dcterms:source "http://www.isda.org/c_and_a/oper_commit-dcg-glossary.html"^^xsd:anyURI ;
  rdfs:isDefinedBy <http://eds.topbraidlive.org/1.0/taxonomy/maeco> ;
  rdfs:isDefinedBy <http://eds.topbraidlive.org/taxonomy/maeco> ;
  rdfs:label "Convergence" ;
  skos:broader maecot:ANY_Measure ;
  skos:definition "The movement of the cash asset price toward the futures price as the expiration date of the futures contract approaches."@en ;
  skos:definition "The process of becoming quantitatively more alike.  In an international context, it often refers to countries becoming more alike in terms of their <a href='http://edg.topbraid.solutions/maeco/term/FactorPrice'>factor prices</a> or in terms of their <a href='http://edg.topbraid.solutions/maeco/term/PerCapitaIncome'>per capita incomes</a> , perhaps as a result of trade or other forms of economic <a href='http://edg.topbraid.solutions/maeco/term/Integration'>integration</a> ." ;
  skos:prefLabel "Convergence"@en ;
.
maecot:Convexity
  rdf:type maeco:QuantityKind ;
  dcterms:source "http://www.isda.org/c_and_a/oper_commit-dcg-glossary.html"^^xsd:anyURI ;
  rdfs:isDefinedBy <http://eds.topbraidlive.org/1.0/taxonomy/maeco> ;
  rdfs:isDefinedBy <http://eds.topbraidlive.org/taxonomy/maeco> ;
  rdfs:label "Convexity" ;
  skos:broader maecot:ANY_QuantityKind ;
  skos:definition "The curvature in the bond price and yield relationship."@en ;
  skos:definition "This is just the state of being <a href='http://edg.topbraid.solutions/maeco/term/Convex'>convex</a> .  More generally in economics it refers to the sets ( <a href='http://edg.topbraid.solutions/maeco/term/ProductionPossibilitySet'>production possibilities</a> , <a href='http://edg.topbraid.solutions/maeco/term/PreferenceSet'>preferences</a> , and <a href='http://edg.topbraid.solutions/maeco/term/ConstraintSet'>constraints</a> ) which, if they are convex, may yield well behaved economic <a href='http://edg.topbraid.solutions/maeco/term/Equilibrium'>equilibria</a> .  In contrast, models that are <a href='http://edg.topbraid.solutions/maeco/term/Nonconvexity'>nonconvex</a> tend to have <a href='http://edg.topbraid.solutions/maeco/term/MultipleEquilibria'>multiple equilibria</a> and display discontinuous behavior (jumps)." ;
  skos:prefLabel "Convexity"@en ;
.
maecot:CorporateCredit
  rdf:type maeco:QuantityKind ;
  rdfs:isDefinedBy <http://eds.topbraidlive.org/1.0/taxonomy/maeco> ;
  rdfs:isDefinedBy <http://eds.topbraidlive.org/taxonomy/maeco> ;
  rdfs:label "Corporate Credit" ;
  skos:broader maecot:ANY_QuantityKind ;
  skos:prefLabel "Corporate credit"@en ;
.
maecot:Correlation
  rdf:type maeco:Measure ;
  dcterms:source "http://www.isda.org/c_and_a/oper_commit-dcg-glossary.html"^^xsd:anyURI ;
  dcterms:source "http://www.wwnorton.com/college/econ/stec4/macroeconomics/glossary.asp"^^xsd:anyURI ;
  rdfs:isDefinedBy <http://eds.topbraidlive.org/1.0/taxonomy/maeco> ;
  rdfs:isDefinedBy <http://eds.topbraidlive.org/taxonomy/maeco> ;
  rdfs:label "correlation" ;
  skos:broader maecot:ANY_Measure ;
  skos:definition "<STRONG>Correlation</STRONG> - the relationship that results when a change in one variable is consistently associated with a change in another variable. A measure of the extent to which two economic or statistical variables move together, normalized so that it ranges from &minus;1 to +1.  It is defined as the <a href='http://edg.topbraid.solutions/maeco/term/Covariance'>covariance</a> of the two variables divided by the square root of the product of their <a href='http://edg.topbraid.solutions/maeco/term/Variance'>variances</a> .  Used in trade theory to express weak relationships among economic variables." ;
  skos:definition "A statistical measure of the relationship between the price movements in two financial instruments."@en ;
  skos:prefLabel "Correlation" ;
  skos:prefLabel "Correlation"@en ;
.
maecot:CounterCyclicalCapitalBuffer
  rdf:type maeco:Buffer ;
  dcterms:source "http://www.cftc.gov/LawRegulation/DoddFrankAct/index.htm"^^xsd:anyURI ;
  rdfs:isDefinedBy <http://eds.topbraidlive.org/1.0/taxonomy/maeco> ;
  rdfs:isDefinedBy <http://eds.topbraidlive.org/taxonomy/maeco> ;
  rdfs:label "Countercyclical Capital Buffer" ;
  skos:broader maecot:ANY_Buffer ;
  skos:definition "This refers to a further buffer (beyond the capital conservation buffer) that is meant to protect the banking sector from periods of excess credit growth associated with a build-up of system-wide risk. The buffer is to be set by national authorities, and is expected to range from 0 to 2.5% of TRWA."@en ;
  skos:prefLabel "Counter-cyclical Capital Buffer"@en ;
.
maecot:CounterfactualRiskWeight
  rdf:type maeco:RiskMeasure ;
  rdfs:isDefinedBy <http://eds.topbraidlive.org/1.0/taxonomy/maeco> ;
  rdfs:isDefinedBy <http://eds.topbraidlive.org/taxonomy/maeco> ;
  rdfs:label "Counterfactual Risk Weight" ;
  skos:broader maecot:RiskWeightingFactor ;
  skos:prefLabel "Counterfactual risk weight"@en ;
.
maecot:CountryRiskClassification
  rdf:type maeco:Measure ;
  dcterms:source "http://www.cftc.gov/LawRegulation/DoddFrankAct/index.htm"^^xsd:anyURI ;
  rdfs:isDefinedBy <http://eds.topbraidlive.org/1.0/taxonomy/maeco> ;
  rdfs:isDefinedBy <http://eds.topbraidlive.org/taxonomy/maeco> ;
  rdfs:label "Country Risk Classification" ;
  skos:altLabel "CRC" ;
  skos:definition "Country Risk Classifications (CRCs) are intended to reflect country risk (the risk that a government will impose capital or exchange controls, for example) and are used for purposes of certain market risk rules for bank capital purposes, since the DFA required that the banking agencies eliminate references to and reliance on external credit ratings."@en ;
  skos:prefLabel "Country Risk Classification"@en ;
.
maecot:Coupon
  rdf:type maeco:QuantityKind ;
  dcterms:source "http://www.isda.org/c_and_a/oper_commit-dcg-glossary.html"^^xsd:anyURI ;
  rdfs:isDefinedBy <http://eds.topbraidlive.org/1.0/taxonomy/maeco> ;
  rdfs:isDefinedBy <http://eds.topbraidlive.org/taxonomy/maeco> ;
  rdfs:label "Coupon" ;
  skos:definition "The interest payment on a <a href='http://edg.topbraid.solutions/maeco/term/Bond'>bond</a> , so-named because bonds originally were pieces of paper with small sections, called coupons, that were cut off and exchanged for the interest payments." ;
  skos:definition "The nominal annual rate of interest paid on a financial instrument and expressed as a percentage of the principal value or as a floating rate based on a reference rate such as LIBOR. The interest is paid to the holder of the security by the borrower. The coupon is generally paid annually, semi-annually or, in some cases, quarterly depending on the type of instrument."@en ;
  skos:prefLabel "Coupon"@en ;
.
maecot:CoveredInterestRate
  rdf:type maeco:Rate ;
  rdfs:isDefinedBy <http://eds.topbraidlive.org/1.0/taxonomy/maeco> ;
  rdfs:isDefinedBy <http://eds.topbraidlive.org/taxonomy/maeco> ;
  rdfs:label "Covered interest rate" ;
  skos:broader maecot:ANY_Rate ;
  skos:definition "The covered interest rate, in a currency other than your own, is the nominal interest rate plus the <a href='http://edg.topbraid.solutions/maeco/term/ForwardPremium'>forward premium</a> on the currency; thus the percent you will earn holding the foreign asset while protecting against exchange-rate change by selling the foreign currency forward." ;
  skos:prefLabel "Covered Interest Rate" ;
.
maecot:CreditConversionFactor
  rdf:type maeco:QuantityKind ;
  dcterms:source "http://www.cftc.gov/LawRegulation/DoddFrankAct/index.htm"^^xsd:anyURI ;
  rdfs:isDefinedBy <http://eds.topbraidlive.org/1.0/taxonomy/maeco> ;
  rdfs:isDefinedBy <http://eds.topbraidlive.org/taxonomy/maeco> ;
  rdfs:label "Credit Conversion Factor" ;
  skos:altLabel "CCF" ;
  skos:definition "Credit conversion factor. In assessing risk weights, off-balance sheet exposures and contingencies are subject to regulatorily defined credit conversion factors."@en ;
  skos:prefLabel "Credit conversion factor"@en ;
.
maecot:CreditDefaultSwapSpread
  rdf:type maeco:QuantityKind ;
  rdfs:isDefinedBy <http://eds.topbraidlive.org/1.0/taxonomy/maeco> ;
  rdfs:isDefinedBy <http://eds.topbraidlive.org/taxonomy/maeco> ;
  rdfs:label "Credit Default Swap Spread" ;
  skos:altLabel "CDS Spread" ;
  skos:broader maecot:CreditSpread ;
  skos:definition "The price which indicates the credit worthiness of an underlying asset."@en ;
  skos:prefLabel "Credit Default Swap Spread" ;
.
maecot:CreditRate
  rdf:type maeco:Rate ;
  rdfs:isDefinedBy <http://eds.topbraidlive.org/1.0/taxonomy/maeco> ;
  rdfs:isDefinedBy <http://eds.topbraidlive.org/taxonomy/maeco> ;
  rdfs:label "Credit Rate" ;
  skos:broader maecot:ANY_Rate ;
  skos:prefLabel "Credit Rate" ;
.
maecot:CreditRating
  rdf:type maeco:Measure ;
  dcterms:source "https://en.wikipedia.org/wiki/Credit_rating"^^xsd:anyURI ;
  rdfs:isDefinedBy <http://eds.topbraidlive.org/1.0/taxonomy/maeco> ;
  rdfs:isDefinedBy <http://eds.topbraidlive.org/taxonomy/maeco> ;
  rdfs:label "Credit Rating" ;
  skos:broader maecot:ANY_Measure ;
  skos:definition "A credit rating is an evaluation of the credit worthiness of a debtor (a business (company) or a government) predicting the debtor's ability to pay back the debt; it thus forecasts implicitly the likelihood of the debtor's default.[3] The credit rating represents the evaluation of the credit rating agency of qualitative and quantitative information for the debtor; including non-public information obtained by the credit rating agencies' analysts." ;
  skos:prefLabel "Credit Rating" ;
.
maecot:CreditRiskCategory
  rdf:type maeco:RiskMeasure ;
  rdfs:isDefinedBy <http://eds.topbraidlive.org/1.0/taxonomy/maeco> ;
  rdfs:isDefinedBy <http://eds.topbraidlive.org/taxonomy/maeco> ;
  rdfs:label "Credit Risk Category" ;
  skos:prefLabel "Credit risk category"@en ;
.
maecot:CreditScore
  rdf:type maeco:RiskMeasure ;
  rdfs:isDefinedBy <http://eds.topbraidlive.org/1.0/taxonomy/maeco> ;
  rdfs:isDefinedBy <http://eds.topbraidlive.org/taxonomy/maeco> ;
  rdfs:label "Credit Score" ;
  skos:broader maecot:ANY_Measure ;
  skos:prefLabel "Credit Score" ;
.
maecot:CreditSpread
  rdf:type maeco:QuantityKind ;
  dcterms:source "http://www.isda.org/c_and_a/oper_commit-dcg-glossary.html"^^xsd:anyURI ;
  rdfs:isDefinedBy <http://eds.topbraidlive.org/1.0/taxonomy/maeco> ;
  rdfs:isDefinedBy <http://eds.topbraidlive.org/taxonomy/maeco> ;
  rdfs:label "Spread (credit)" ;
  skos:altLabel "credit"@en ;
  skos:broader maecot:ANY_QuantityKind ;
  skos:definition "The price which indicates the credit worthiness of an underlying asset."@en ;
  skos:prefLabel "Spread"@en ;
.
maecot:CreditValuationAdjustment
  rdf:type maeco:QuantityKind ;
  dcterms:source "http://www.cftc.gov/LawRegulation/DoddFrankAct/index.htm"^^xsd:anyURI ;
  rdfs:isDefinedBy <http://eds.topbraidlive.org/1.0/taxonomy/maeco> ;
  rdfs:isDefinedBy <http://eds.topbraidlive.org/taxonomy/maeco> ;
  rdfs:label "Credit Valuation Adjustment" ;
  skos:altLabel "CVA" ;
  skos:definition "Credit valuation adjustment. A CVA is a fair value adjustment to reflect counterparty credit risk in valuing an OTC derivatives contract."@en ;
  skos:prefLabel "Credit valuation adjustment"@en ;
.
maecot:CrossBankBenchmark
  rdf:type maeco:QuantityKind ;
  rdfs:isDefinedBy <http://eds.topbraidlive.org/1.0/taxonomy/maeco> ;
  rdfs:isDefinedBy <http://eds.topbraidlive.org/taxonomy/maeco> ;
  rdfs:label "Cross Bank Benchmark" ;
  skos:broader maecot:ANY_QuantityKind ;
  skos:prefLabel "Cross bank benchmark"@en ;
.
maecot:CrossBankMedian
  rdf:type maeco:QuantityKind ;
  rdfs:isDefinedBy <http://eds.topbraidlive.org/1.0/taxonomy/maeco> ;
  rdfs:isDefinedBy <http://eds.topbraidlive.org/taxonomy/maeco> ;
  rdfs:label "Cross Bank Median" ;
  skos:prefLabel "Cross bank median"@en ;
.
maecot:CrossBankMedianBenchmark
  rdf:type maeco:QuantityKind ;
  rdfs:isDefinedBy <http://eds.topbraidlive.org/1.0/taxonomy/maeco> ;
  rdfs:isDefinedBy <http://eds.topbraidlive.org/taxonomy/maeco> ;
  rdfs:label "Cross Bank Median Benchmark" ;
  skos:broader maecot:ANY_QuantityKind ;
  skos:prefLabel "Cross bank median benchmark"@en ;
.
maecot:CrossBankMedianRiskWeight
  rdf:type maeco:RiskMeasure ;
  rdfs:isDefinedBy <http://eds.topbraidlive.org/1.0/taxonomy/maeco> ;
  rdfs:isDefinedBy <http://eds.topbraidlive.org/taxonomy/maeco> ;
  rdfs:label "Cross Bank Median Risk Weight" ;
  skos:broader maecot:RiskWeightingFactor ;
  skos:prefLabel "Cross bank median risk weight"@en ;
.
maecot:CrossRate
  rdf:type maeco:Rate ;
  rdfs:isDefinedBy <http://eds.topbraidlive.org/1.0/taxonomy/maeco> ;
  rdfs:isDefinedBy <http://eds.topbraidlive.org/taxonomy/maeco> ;
  rdfs:label "Cross rate" ;
  skos:broader maecot:ANY_Rate ;
  skos:definition "<STRONG>1.</STRONG> The <a href='http://edg.topbraid.solutions/maeco/term/ExchangeRate'>exchange rate</a> between two currencies as implied by their values with respect to a third currency.  <STRONG>2.</STRONG> Thus, since most currencies are commonly quoted in U.S. dollars, the exchange rate between any two currencies other than the dollar." ;
  skos:prefLabel "Cross Rate" ;
.
maecot:CrossSubsidy
  rdf:type maeco:Subsidy ;
  rdfs:isDefinedBy <http://eds.topbraidlive.org/1.0/taxonomy/maeco> ;
  rdfs:isDefinedBy <http://eds.topbraidlive.org/taxonomy/maeco> ;
  rdfs:label "Cross subsidy" ;
  skos:broader maecot:Subsidy ;
  skos:definition "The use of profits from one activity to cover losses from another.  Thus the use of high prices for some of a firm's products, for example, to permit it to price below cost for others.  In international trade, this could be one explanation for <a href='http://edg.topbraid.solutions/maeco/term/Dumping'>dumping</a> ." ;
  skos:prefLabel "Cross Subsidy" ;
.
maecot:DayCountFraction
  rdf:type maeco:QuantityKind ;
  dcterms:source "http://www.isda.org/c_and_a/oper_commit-dcg-glossary.html"^^xsd:anyURI ;
  rdfs:isDefinedBy <http://eds.topbraidlive.org/1.0/taxonomy/maeco> ;
  rdfs:isDefinedBy <http://eds.topbraidlive.org/taxonomy/maeco> ;
  rdfs:label "Day Count Fraction" ;
  skos:definition "The number of days between coupon payment dates (calculation period) divided by the number of days in the year as specified in the applicable day count convention. Day count fraction is then input to calculate the accrued interest and the present value of the coupon."@en ;
  skos:prefLabel "Day count fraction"@en ;
.
maecot:Debt
  rdf:type maeco:QuantityKind ;
  rdfs:isDefinedBy <http://eds.topbraidlive.org/1.0/taxonomy/maeco> ;
  rdfs:isDefinedBy <http://eds.topbraidlive.org/taxonomy/maeco> ;
  rdfs:label "Debt" ;
  skos:broader maecot:ANY_QuantityKind ;
  skos:definition "The amount that is owed, as a result of previous borrowing.  A country's debt may refer to the debt of its government or to that of the country as a whole." ;
  skos:prefLabel "Debt" ;
.
maecot:DebtBurden
  rdf:type maeco:QuantityKind ;
  rdfs:isDefinedBy <http://eds.topbraidlive.org/1.0/taxonomy/maeco> ;
  rdfs:isDefinedBy <http://eds.topbraidlive.org/taxonomy/maeco> ;
  rdfs:label "Debt burden" ;
  skos:broader maecot:Debt ;
  skos:definition "The <a href='http://edg.topbraid.solutions/maeco/term/Debt'>debt</a> of a country, when large enough that <a href='http://edg.topbraid.solutions/maeco/term/Service'>servicing</a> it has become difficult." ;
  skos:prefLabel "Debt Burden" ;
.
maecot:DebtRatings
  rdf:type maeco:QuantityKind ;
  rdfs:isDefinedBy <http://eds.topbraidlive.org/1.0/taxonomy/maeco> ;
  rdfs:isDefinedBy <http://eds.topbraidlive.org/taxonomy/maeco> ;
  rdfs:label "Debt Ratings" ;
  skos:broader maecot:ANY_QuantityKind ;
  skos:prefLabel "Debt ratings"@en ;
.
maecot:DecreasingCost
  rdf:type maeco:Cost ;
  rdfs:isDefinedBy <http://eds.topbraidlive.org/1.0/taxonomy/maeco> ;
  rdfs:isDefinedBy <http://eds.topbraidlive.org/taxonomy/maeco> ;
  rdfs:label "Decreasing cost" ;
  skos:broader maecot:ANY_Cost ;
  skos:definition "<a href='http://edg.topbraid.solutions/maeco/term/AverageCost'>Average cost</a> that declines as output increases.  Implied by <a href='http://edg.topbraid.solutions/maeco/term/Irts2'>increasing returns to scale</a> ." ;
  skos:prefLabel "Decreasing Cost" ;
.
maecot:DefaultRate
  rdf:type maeco:Rate ;
  rdfs:isDefinedBy <http://eds.topbraidlive.org/1.0/taxonomy/maeco> ;
  rdfs:isDefinedBy <http://eds.topbraidlive.org/taxonomy/maeco> ;
  rdfs:label "Default Rate" ;
  skos:broader maecot:ANY_Rate ;
  skos:prefLabel "Default rate"@en ;
.
maecot:Delta
  rdf:type maeco:QuantityKind ;
  dcterms:source "http://www.isda.org/c_and_a/oper_commit-dcg-glossary.html"^^xsd:anyURI ;
  rdfs:isDefinedBy <http://eds.topbraidlive.org/1.0/taxonomy/maeco> ;
  rdfs:isDefinedBy <http://eds.topbraidlive.org/taxonomy/maeco> ;
  rdfs:label "Delta" ;
  skos:definition "The change in the monetary value of an instrument for a one basis point change in the price of that instrument."@en ;
  skos:prefLabel "Delta"@en ;
.
maecot:DemandPrice
  rdf:type maeco:Price ;
  rdfs:isDefinedBy <http://eds.topbraidlive.org/1.0/taxonomy/maeco> ;
  rdfs:isDefinedBy <http://eds.topbraidlive.org/taxonomy/maeco> ;
  rdfs:label "Demand price" ;
  skos:broader maecot:Price ;
  skos:definition "The price at which a given quantity is demanded; thus the demand curve viewed from the perspective of price as a function of quantity." ;
  skos:prefLabel "Demand Price" ;
.
maecot:DepositReserves
  rdf:type maeco:Reserves ;
  rdfs:isDefinedBy <http://eds.topbraidlive.org/1.0/taxonomy/maeco> ;
  rdfs:isDefinedBy <http://eds.topbraidlive.org/taxonomy/maeco> ;
  rdfs:label "Deposit Reserves" ;
  skos:broader maecot:ANY_Reserves ;
  skos:prefLabel "Deposit Reserves"@us ;
.
maecot:DerivativesCashOutflow
  rdf:type maeco:QuantityKind ;
  rdfs:isDefinedBy <http://eds.topbraidlive.org/1.0/taxonomy/maeco> ;
  rdfs:isDefinedBy <http://eds.topbraidlive.org/taxonomy/maeco> ;
  rdfs:label "Derivatives Cash Outflow" ;
  skos:broader maecot:ANY_QuantityKind ;
  skos:definition "The sum of all net cash outflows should receive a 100% factor. Banks should calculate, in accordance with their existing valuation methodologies, expected contractual derivative cash inflows and outflows. Cash flows may be calculated on a net basis (ie inflows can offset outflows) by counterparty, only where a valid master netting agreement exists. Banks should exclude from such calculations those liquidity requirements that would result from increased collateral needs due to market value movements or falls in value of collateral posted.48 Options should be assumed to be exercised when they are in the money to the option buyer."@en ;
  skos:prefLabel "Derivatives cash outflow"@en ;
  prov:wasInfluencedBy "<http://www.bis.org/publ/bcbs238.pdf>" ;
.
maecot:DerivedDemand
  rdf:type maeco:Demand ;
  rdfs:isDefinedBy <http://eds.topbraidlive.org/1.0/taxonomy/maeco> ;
  rdfs:isDefinedBy <http://eds.topbraidlive.org/taxonomy/maeco> ;
  rdfs:label "Derived demand" ;
  skos:definition "Demand that arises or is defined indirectly from some other demand or underlying behavior; e.g., demand for foreign currency is derived from demand for foreign goods, bonds, etc., while demand for import of a homogeneous good is derived from domestic demand and supply." ;
  skos:prefLabel "Derived Demand" ;
.
maecot:DesignatedMaturity
  rdf:type maeco:QuantityKind ;
  dcterms:source "http://www.isda.org/c_and_a/oper_commit-dcg-glossary.html"^^xsd:anyURI ;
  rdfs:isDefinedBy <http://eds.topbraidlive.org/1.0/taxonomy/maeco> ;
  rdfs:isDefinedBy <http://eds.topbraidlive.org/taxonomy/maeco> ;
  rdfs:label "Designated Maturity" ;
  skos:broader maecot:ANY_QuantityKind ;
  skos:definition "The time period for which the floating rate in a derivative transaction is quoted. For example, six month USD LIBOR."@en ;
  skos:prefLabel "Designated maturity"@en ;
.
maecot:DetachmentPoint
  rdf:type maeco:Measure ;
  dcterms:source "http://www.isda.org/c_and_a/oper_commit-dcg-glossary.html"^^xsd:anyURI ;
  rdfs:isDefinedBy <http://eds.topbraidlive.org/1.0/taxonomy/maeco> ;
  rdfs:isDefinedBy <http://eds.topbraidlive.org/taxonomy/maeco> ;
  rdfs:label "Detachment Point" ;
  skos:broader maecot:ANY_Measure ;
  skos:definition "The detachment point defines the point after the attachment point where losses in the underlying portfolio no longer reduce the notional of a tranche. For example, the notional in a tranche with an attachment point of 3% and a detachment point of 6% will reduce after there has been 3% of losses in the portfolio. The reduction in notional no longer occurs after 6%. "@en ;
  skos:prefLabel "Detachment point"@en ;
.
maecot:DirtyPrice
  rdf:type maeco:QuantityKind ;
  dcterms:source "http://www.isda.org/c_and_a/oper_commit-dcg-glossary.html"^^xsd:anyURI ;
  rdfs:isDefinedBy <http://eds.topbraidlive.org/1.0/taxonomy/maeco> ;
  rdfs:isDefinedBy <http://eds.topbraidlive.org/taxonomy/maeco> ;
  rdfs:label "Dirty Price" ;
  skos:definition "The price of a bond inclusive of accrued interest."@en ;
  skos:prefLabel "Dirty price"@en ;
.
maecot:Discount
  rdf:type maeco:QuantityKind ;
  dcterms:source "http://www.isda.org/c_and_a/oper_commit-dcg-glossary.html"^^xsd:anyURI ;
  rdfs:isDefinedBy <http://eds.topbraidlive.org/1.0/taxonomy/maeco> ;
  rdfs:isDefinedBy <http://eds.topbraidlive.org/taxonomy/maeco> ;
  rdfs:label "Discount" ;
  skos:broader maecot:ANY_QuantityKind ;
  skos:definition "<STRONG>1.</STRONG> Any reduction in price or value, especially when below a stated or normal price.  <STRONG>2.</STRONG> To buy or sell <a href='http://edg.topbraid.solutions/maeco/term/CommercialPaper'>commercial paper</a> at a price below face value to account for <a href='http://edg.topbraid.solutions/maeco/term/Interest'>interest</a> to accrue before maturity.  <STRONG>3.</STRONG> To attach a lower weight to the importance of -- or utility derived from -- one thing compared to another, as in <a href='http://edg.topbraid.solutions/maeco/term/TimePreference'>time preference</a> that discounts later consumption compared to earlier." ;
  skos:definition "The condition of the price of a bond that is lower than par. The discount equals the difference between the price paid for a security and the security's par value. If a bond with a par value of $1,000 is currently selling for $990 dollars (or 99% of par), it is selling at a discount. "@en ;
  skos:prefLabel "Discount"@en ;
.
maecot:DiscountRate
  rdf:type maeco:Rate ;
  rdfs:isDefinedBy <http://eds.topbraidlive.org/1.0/taxonomy/maeco> ;
  rdfs:isDefinedBy <http://eds.topbraidlive.org/taxonomy/maeco> ;
  rdfs:label "Discount rate" ;
  skos:broader maecot:ANY_Rate ;
  skos:definition "<STRONG>1.</STRONG> The rate, per year, at which future values are diminished to make them comparable to values in the present.  Can be either subjective (reflecting personal time preference) or objective (a market interest rate).  <STRONG>2.</STRONG> The interest rate that the <a href='http://edg.topbraid.solutions/maeco/term/Fed'>Fed</a> charges commercial banks for very short-term loans of reserves.  One of the tools of <a href='http://edg.topbraid.solutions/maeco/term/MonetaryPolicy'>monetary policy</a> ." ;
  skos:prefLabel "Discount rate"@en ;
.
maecot:DiscountWindowPrimaryCreditRate
  rdf:type maeco:Rate ;
  rdfs:isDefinedBy <http://eds.topbraidlive.org/1.0/taxonomy/maeco> ;
  rdfs:isDefinedBy <http://eds.topbraidlive.org/taxonomy/maeco> ;
  rdfs:label "Discount Window Primary Credit Rate" ;
  skos:altLabel "Discount window primary credit" ;
  skos:altLabel "FED Discount Rate" ;
  skos:broader maecot:CreditRate ;
  skos:prefLabel "Discount window primary credit rate" ;
.
maecot:DiscriminatoryTariff
  rdf:type maeco:Tariff ;
  rdfs:isDefinedBy <http://eds.topbraidlive.org/1.0/taxonomy/maeco> ;
  rdfs:isDefinedBy <http://eds.topbraidlive.org/taxonomy/maeco> ;
  rdfs:label "Discriminatory tariff" ;
  skos:broader maecot:Tariff ;
  skos:definition "A higher <a href='http://edg.topbraid.solutions/maeco/term/Tariff'>tariff</a> against one source of imports than against another.  Except in special circumstances, such as <a href='http://edg.topbraid.solutions/maeco/term/AntiDumpingDuty'>anti-dumping duties</a> and <a href='http://edg.topbraid.solutions/maeco/term/Cvd2'>countervailing duties</a> , this is a violation of <a href='http://edg.topbraid.solutions/maeco/term/Mfn'>MFN</a> and is prohibited by the <a href='http://edg.topbraid.solutions/maeco/term/Wto'>WTO</a> against other members." ;
  skos:prefLabel "Discriminatory Tariff" ;
.
maecot:DomesticDemand
  rdf:type maeco:Demand ;
  rdfs:isDefinedBy <http://eds.topbraidlive.org/1.0/taxonomy/maeco> ;
  rdfs:isDefinedBy <http://eds.topbraidlive.org/taxonomy/maeco> ;
  rdfs:label "Domestic demand" ;
  skos:definition "Demand for a product by buyers in one's own country." ;
  skos:prefLabel "Domestic Demand" ;
.
maecot:DomesticResourceCost
  rdf:type maeco:Cost ;
  rdfs:isDefinedBy <http://eds.topbraidlive.org/1.0/taxonomy/maeco> ;
  rdfs:isDefinedBy <http://eds.topbraidlive.org/taxonomy/maeco> ;
  rdfs:label "Domestic resource cost" ;
  skos:broader maecot:ANY_Cost ;
  skos:definition "A measure, in terms of real resources, of the <a href='http://edg.topbraid.solutions/maeco/term/OpportunityCost'>opportunity cost</a> of producing or saving <a href='http://edg.topbraid.solutions/maeco/term/ForeignExchange'>foreign exchange</a> .  It is an <a href='http://edg.topbraid.solutions/maeco/term/ExAnteAnalysis'>ex ante</a> measure of <a href='http://edg.topbraid.solutions/maeco/term/ComparativeAdvantage'>comparative advantage</a> , used to evaluate projects and policies.  The term was introduced to the economics literature by <a href='http://edg.topbraid.solutions/maeco/term/Bib.html#Bruno1963'>Bruno</a> (1963, 1972)." ;
  skos:prefLabel "Domestic Resource Cost" ;
.
maecot:DomesticSubsidy
  rdf:type maeco:Subsidy ;
  rdfs:isDefinedBy <http://eds.topbraidlive.org/1.0/taxonomy/maeco> ;
  rdfs:isDefinedBy <http://eds.topbraidlive.org/taxonomy/maeco> ;
  rdfs:label "Domestic subsidy" ;
  skos:broader maecot:Subsidy ;
  skos:definition "A <a href='http://edg.topbraid.solutions/maeco/term/Subsidy'>subsidy</a> to production, independent of where the product is to be sold.  Contrasts with <a href='http://edg.topbraid.solutions/maeco/term/ExportSubsidy'>export subsidy</a> ." ;
  skos:prefLabel "Domestic Subsidy" ;
.
maecot:Ead
  rdf:type maeco:QuantityKind ;
  rdfs:isDefinedBy <http://eds.topbraidlive.org/1.0/taxonomy/maeco> ;
  rdfs:isDefinedBy <http://eds.topbraidlive.org/taxonomy/maeco> ;
  rdfs:label "Ead" ;
  skos:prefLabel "Ead"@en ;
.
maecot:EadSovereign
  rdf:type maeco:QuantityKind ;
  rdfs:isDefinedBy <http://eds.topbraidlive.org/1.0/taxonomy/maeco> ;
  rdfs:isDefinedBy <http://eds.topbraidlive.org/taxonomy/maeco> ;
  rdfs:label "Ead Sovereign" ;
  skos:prefLabel "Ead sovereign"@en ;
.
maecot:EadWeightedIrb
  rdf:type maeco:QuantityKind ;
  rdfs:isDefinedBy <http://eds.topbraidlive.org/1.0/taxonomy/maeco> ;
  rdfs:isDefinedBy <http://eds.topbraidlive.org/taxonomy/maeco> ;
  rdfs:label "Ead Weighted Irb" ;
  skos:broader maecot:RiskWeightingFactor ;
  skos:prefLabel "Ead weighted irb"@en ;
.
maecot:EadWeightedLgds
  rdf:type maeco:QuantityKind ;
  rdfs:isDefinedBy <http://eds.topbraidlive.org/1.0/taxonomy/maeco> ;
  rdfs:isDefinedBy <http://eds.topbraidlive.org/taxonomy/maeco> ;
  rdfs:label "Ead Weighted Lgds" ;
  skos:broader maecot:RiskWeightingFactor ;
  skos:prefLabel "Ead weighted lgds"@en ;
.
maecot:EadWeightedMaturity
  rdf:type maeco:QuantityKind ;
  rdfs:isDefinedBy <http://eds.topbraidlive.org/1.0/taxonomy/maeco> ;
  rdfs:isDefinedBy <http://eds.topbraidlive.org/taxonomy/maeco> ;
  rdfs:label "Ead Weighted Maturity" ;
  skos:broader maecot:RiskWeightingFactor ;
  skos:prefLabel "Ead weighted maturity"@en ;
.
maecot:EadWeightedPds
  rdf:type maeco:QuantityKind ;
  rdfs:isDefinedBy <http://eds.topbraidlive.org/1.0/taxonomy/maeco> ;
  rdfs:isDefinedBy <http://eds.topbraidlive.org/taxonomy/maeco> ;
  rdfs:label "Ead Weighted Pds" ;
  skos:broader maecot:RiskWeightingFactor ;
  skos:prefLabel "Ead weighted pds"@en ;
.
maecot:EarningsPerShare
  rdf:type maeco:QuantityKind ;
  rdfs:isDefinedBy <http://eds.topbraidlive.org/1.0/taxonomy/maeco> ;
  rdfs:isDefinedBy <http://eds.topbraidlive.org/taxonomy/maeco> ;
  rdfs:label "Earnings Per Share" ;
  skos:altLabel "EPS" ;
  skos:broader maecot:ANY_QuantityKind ;
  skos:prefLabel "Earnings per share" ;
.
maecot:EconomicCost
  rdf:type maeco:Cost ;
  rdfs:isDefinedBy <http://eds.topbraidlive.org/1.0/taxonomy/maeco> ;
  rdfs:isDefinedBy <http://eds.topbraidlive.org/taxonomy/maeco> ;
  rdfs:label "Economic cost" ;
  skos:broader maecot:ANY_Cost ;
  skos:definition "The monetary cost of an object or action, including reductions in wages, profits, and property values, but not including such nonmonetary costs as adverse consequences for health or safety, or negative effects on others." ;
  skos:prefLabel "Economic Cost" ;
.
maecot:EffectiveExchangeRate
  rdf:type maeco:Rate ;
  rdfs:isDefinedBy <http://eds.topbraidlive.org/1.0/taxonomy/maeco> ;
  rdfs:isDefinedBy <http://eds.topbraidlive.org/taxonomy/maeco> ;
  rdfs:label "Effective exchange rate" ;
  skos:broader maecot:ANY_Rate ;
  skos:definition "An index of a currency's value relative to a group (or <a href='http://edg.topbraid.solutions/maeco/term/Basket'>basket</a> ) of other currencies, where the currencies in the basket are given weights based on the amount of trade between the countries that use the currencies.  Also called a <a href='http://edg.topbraid.solutions/maeco/term/TradeWeightedExchangeRate'>trade-weighted exchange rate</a> ." ;
  skos:prefLabel "Effective Exchange Rate" ;
.
maecot:EffectiveProtectiveRate
  rdf:type maeco:Rate ;
  rdfs:isDefinedBy <http://eds.topbraidlive.org/1.0/taxonomy/maeco> ;
  rdfs:isDefinedBy <http://eds.topbraidlive.org/taxonomy/maeco> ;
  rdfs:label "Effective protective rate" ;
  skos:broader maecot:ANY_Rate ;
  skos:definition "Same as <a href='http://edg.topbraid.solutions/maeco/term/EffectiveRateOfProtection'>effective rate of protection</a> ." ;
  skos:prefLabel "Effective Protective Rate" ;
.
maecot:EffectiveTariff
  rdf:type maeco:Tariff ;
  rdfs:isDefinedBy <http://eds.topbraidlive.org/1.0/taxonomy/maeco> ;
  rdfs:isDefinedBy <http://eds.topbraidlive.org/taxonomy/maeco> ;
  rdfs:label "Effective tariff" ;
  skos:broader maecot:Tariff ;
  skos:definition "<a href='http://edg.topbraid.solutions/maeco/term/Erp2'>Effective rate of protection</a> ." ;
  skos:prefLabel "Effective Tariff" ;
.
maecot:Elasticity
  rdf:type maeco:QuantityKind ;
  dcterms:source "https://en.wikipedia.org/wiki/Elasticity_(economics)"^^xsd:anyURI ;
  rdfs:isDefinedBy <http://eds.topbraidlive.org/1.0/taxonomy/maeco> ;
  rdfs:isDefinedBy <http://eds.topbraidlive.org/taxonomy/maeco> ;
  rdfs:label "Elasticity" ;
  skos:broader maecot:ANY_QuantityKind ;
  skos:prefLabel "Elasticity" ;
.
maecot:EnvironmentalSubsidy
  rdf:type maeco:Subsidy ;
  rdfs:isDefinedBy <http://eds.topbraidlive.org/1.0/taxonomy/maeco> ;
  rdfs:isDefinedBy <http://eds.topbraidlive.org/taxonomy/maeco> ;
  rdfs:label "Environmental subsidy" ;
  skos:broader maecot:Subsidy ;
  skos:definition "A <a href='http://edg.topbraid.solutions/maeco/term/Subsidy'>subsidy</a> intended for environmental purposes.  A subsidy for adapting existing facilities to new environmental laws or regulations is <a href='http://edg.topbraid.solutions/maeco/term/NonactionableSubsidy'>non-actionable</a> under <a href='http://edg.topbraid.solutions/maeco/term/Wto'>WTO</a> rules." ;
  skos:prefLabel "Environmental Subsidy" ;
.
maecot:EquilibriumExchangeRate
  rdf:type maeco:Rate ;
  rdfs:isDefinedBy <http://eds.topbraidlive.org/1.0/taxonomy/maeco> ;
  rdfs:isDefinedBy <http://eds.topbraidlive.org/taxonomy/maeco> ;
  rdfs:label "Equilibrium exchange rate" ;
  skos:broader maecot:ANY_Rate ;
  skos:definition "This is ambiguous, since there is no single agreed upon model of the <a href='http://edg.topbraid.solutions/maeco/term/ExchangeRate'>exchange rate</a> :  <STRONG>1.</STRONG> The exchange rate at which supply and demand for a currency are equal.  <STRONG>2.</STRONG> The exchange rate at which there is <a href='http://edg.topbraid.solutions/maeco/term/BalanceOfPaymentsEquilibrium'>balance of payments equilibrium</a> .  <STRONG>3.</STRONG> The exchange rate at which <a href='http://edg.topbraid.solutions/maeco/term/Ppp2'>purchasing power parity</a> holds, in some form.  <STRONG>4.</STRONG> The exchange rate at which the expected change in the exchange rate, in the near future, is zero.  <STRONG>5.</STRONG> The exchange rate at which the country's <a href='http://edg.topbraid.solutions/maeco/term/InternationalReserves'>international reserves</a> are neither rising nor falling." ;
  skos:prefLabel "Equilibrium Exchange Rate" ;
.
maecot:EquilibriumPrice
  rdf:type maeco:Price ;
  dcterms:source "http://www.wwnorton.com/college/econ/stec4/macroeconomics/glossary.asp"^^xsd:anyURI ;
  rdfs:isDefinedBy <http://eds.topbraidlive.org/1.0/taxonomy/maeco> ;
  rdfs:isDefinedBy <http://eds.topbraidlive.org/taxonomy/maeco> ;
  rdfs:label "equilibrium price" ;
  skos:broader maecot:Price ;
  skos:definition "<STRONG>Equilibrium Price</STRONG> - the price at which demand equals supply" ;
  skos:prefLabel "Equilibrium Price" ;
.
maecot:EquilibriumRealInterestRate
  rdf:type maeco:Rate ;
  rdfs:isDefinedBy <http://eds.topbraidlive.org/1.0/taxonomy/maeco> ;
  rdfs:isDefinedBy <http://eds.topbraidlive.org/taxonomy/maeco> ;
  rdfs:label "Equilibrium Real Interest Rate" ;
  skos:broader maecot:InterestRate ;
  skos:prefLabel "Equilibrium Real Interest Rate" ;
.
maecot:EquityFirstLossTranche
  rdf:type maeco:QuantityKind ;
  dcterms:source "http://www.isda.org/c_and_a/oper_commit-dcg-glossary.html"^^xsd:anyURI ;
  rdfs:isDefinedBy <http://eds.topbraidlive.org/1.0/taxonomy/maeco> ;
  rdfs:isDefinedBy <http://eds.topbraidlive.org/taxonomy/maeco> ;
  rdfs:label "Equity First Loss Tranche" ;
  skos:definition "The first loss and riskiest tranche in a CDO where there is no subordination. For example, a tranche with a 0% - 4% attachment/detachment point.    "@en ;
  skos:prefLabel "Equity/first loss tranche"@en ;
.
maecot:EquivalentTariff
  rdf:type maeco:Tariff ;
  rdfs:isDefinedBy <http://eds.topbraidlive.org/1.0/taxonomy/maeco> ;
  rdfs:isDefinedBy <http://eds.topbraidlive.org/taxonomy/maeco> ;
  rdfs:label "Equivalent tariff" ;
  skos:broader maecot:Tariff ;
  skos:definition "<a href='http://edg.topbraid.solutions/maeco/term/TariffEquivalent'>Tariff equivalent</a> ." ;
  skos:prefLabel "Equivalent Tariff" ;
.
maecot:ExPostTariff
  rdf:type maeco:Tariff ;
  rdfs:isDefinedBy <http://eds.topbraidlive.org/1.0/taxonomy/maeco> ;
  rdfs:isDefinedBy <http://eds.topbraidlive.org/taxonomy/maeco> ;
  rdfs:label "Ex post tariff" ;
  skos:broader maecot:Tariff ;
  skos:definition "<a href='http://edg.topbraid.solutions/maeco/term/ImplicitTariff'>Implicit tariff</a> ." ;
  skos:prefLabel "Ex Post Tariff" ;
.
maecot:ExchangeRate
  rdf:type maeco:Rate ;
  dcterms:source "http://www.wwnorton.com/college/econ/stec4/macroeconomics/glossary.asp"^^xsd:anyURI ;
  rdfs:isDefinedBy <http://eds.topbraidlive.org/1.0/taxonomy/maeco> ;
  rdfs:isDefinedBy <http://eds.topbraidlive.org/taxonomy/maeco> ;
  rdfs:label "exchange rate" ;
  skos:broader maecot:ANY_Rate ;
  skos:definition "The price at which one country's currency trades for another, typically on the <a href='http://edg.topbraid.solutions/maeco/term/ExchangeMarket'>exchange market</a> ." ;
  skos:prefLabel "Exchange Rate" ;
  skos:prefLabel "Exchange rate" ;
.
maecot:ExciseSubsidy
  rdf:type maeco:Subsidy ;
  rdfs:isDefinedBy <http://eds.topbraidlive.org/1.0/taxonomy/maeco> ;
  rdfs:isDefinedBy <http://eds.topbraidlive.org/taxonomy/maeco> ;
  rdfs:label "Excise subsidy" ;
  skos:broader maecot:Subsidy ;
  skos:definition "A <a href='http://edg.topbraid.solutions/maeco/term/Subsidy'>subsidy</a> paid on production or sale (consumption) of a particular good." ;
  skos:prefLabel "Excise Subsidy" ;
.
maecot:ExercisePrice
  rdf:type maeco:QuantityKind ;
  dcterms:source "http://www.isda.org/c_and_a/oper_commit-dcg-glossary.html"^^xsd:anyURI ;
  rdfs:isDefinedBy <http://eds.topbraidlive.org/1.0/taxonomy/maeco> ;
  rdfs:isDefinedBy <http://eds.topbraidlive.org/taxonomy/maeco> ;
  rdfs:label "Exercise Price" ;
  skos:broader maecot:ANY_QuantityKind ;
  skos:definition "The fixed price, per share or unit, at which an option buyer (holder) has the right to buy (call) or sell (put) the underlying asset."@en ;
  skos:prefLabel "Exercise price"@en ;
.
maecot:ExpectedCreditLoss
  rdf:type maeco:QuantityKind ;
  dcterms:source "http://www.cftc.gov/LawRegulation/DoddFrankAct/index.htm"^^xsd:anyURI ;
  rdfs:isDefinedBy <http://eds.topbraidlive.org/1.0/taxonomy/maeco> ;
  rdfs:isDefinedBy <http://eds.topbraidlive.org/taxonomy/maeco> ;
  rdfs:label "Expected Credit Loss" ;
  skos:altLabel "ECL" ;
  skos:broader maecot:ANY_QuantityKind ;
  skos:definition "Expected credit loss."@en ;
  skos:prefLabel "Expected credit loss"@en ;
.
maecot:ExportParityPrice
  rdf:type maeco:Price ;
  rdfs:isDefinedBy <http://eds.topbraidlive.org/1.0/taxonomy/maeco> ;
  rdfs:isDefinedBy <http://eds.topbraidlive.org/taxonomy/maeco> ;
  rdfs:label "Export parity price" ;
  skos:broader maecot:Price ;
  skos:definition "The price a producer gets or can expect to get for its product if exported, equal to the <a href='http://edg.topbraid.solutions/maeco/term/Fob'>f.o.b.</a> price minus the cost of getting the product from the farm or factory to the border.  This and the <a href='http://edg.topbraid.solutions/maeco/term/ImportParityPrice'>import parity price</a> together define a range of the possible equilibrium prices for an equivalent domestically produced good." ;
  skos:prefLabel "Export Parity Price" ;
.
maecot:ExportSubsidy
  rdf:type maeco:Subsidy ;
  rdfs:isDefinedBy <http://eds.topbraidlive.org/1.0/taxonomy/maeco> ;
  rdfs:isDefinedBy <http://eds.topbraidlive.org/taxonomy/maeco> ;
  rdfs:label "Export subsidy" ;
  skos:broader maecot:Subsidy ;
  skos:definition "<STRONG>1.</STRONG> A subsidy to exports; that is, a payment to exporters of a good per unit of the good exported.  Contrasts with a <a href='http://edg.topbraid.solutions/maeco/term/DomesticSubsidy'>domestic subsidy</a> .  <STRONG>2.</STRONG> Sometimes applied to any payments or other advantages given to producers that lead to an increase in exports." ;
  skos:prefLabel "Export Subsidy" ;
.
maecot:ExportTariff
  rdf:type maeco:Tariff ;
  rdfs:isDefinedBy <http://eds.topbraidlive.org/1.0/taxonomy/maeco> ;
  rdfs:isDefinedBy <http://eds.topbraidlive.org/taxonomy/maeco> ;
  rdfs:label "Export tariff" ;
  skos:broader maecot:Tariff ;
  skos:definition "A tax on exports, more commonly called an <a href='http://edg.topbraid.solutions/maeco/term/ExportTax'>export tax</a> ." ;
  skos:prefLabel "Export Tariff" ;
.
maecot:ExternalCost
  rdf:type maeco:Cost ;
  rdfs:isDefinedBy <http://eds.topbraidlive.org/1.0/taxonomy/maeco> ;
  rdfs:isDefinedBy <http://eds.topbraidlive.org/taxonomy/maeco> ;
  rdfs:label "External cost" ;
  skos:broader maecot:ANY_Cost ;
  skos:definition "A negative (i.e., harmful) <a href='http://edg.topbraid.solutions/maeco/term/Externality'>externality</a> ." ;
  skos:prefLabel "External Cost" ;
.
maecot:FICOscore
  rdf:type maeco:QuantityKind ;
  dcterms:source "http://www.cftc.gov/LawRegulation/DoddFrankAct/index.htm"^^xsd:anyURI ;
  rdfs:isDefinedBy <http://eds.topbraidlive.org/1.0/taxonomy/maeco> ;
  rdfs:isDefinedBy <http://eds.topbraidlive.org/taxonomy/maeco> ;
  rdfs:label "FICOscore" ;
  skos:altLabel "FICO" ;
  skos:broader maecot:ANY_QuantityKind ;
  skos:definition "Fair, Isaac and Company (often used to refer to the score they produce, the FICO score). FICO credit scores are frequently used in connection with mortgage originations or other consumer credit transactions."@en ;
  skos:prefLabel "Fair, Isaac and Company (FICO) Score"@en ;
.
maecot:FactorCost
  rdf:type maeco:Cost ;
  rdfs:isDefinedBy <http://eds.topbraidlive.org/1.0/taxonomy/maeco> ;
  rdfs:isDefinedBy <http://eds.topbraidlive.org/taxonomy/maeco> ;
  rdfs:label "Factor cost" ;
  skos:broader maecot:ANY_Cost ;
  skos:definition "The cost of the <a href='http://edg.topbraid.solutions/maeco/term/Factor'>factors</a> used in production.  The term is used especially when the value of economic activity in a sector or an economy can be measured or valued either at \"factor cost,\" adding up payments to factors, or at \" <STRONG>market value</STRONG> or <STRONG>market price</STRONG> ,\" adding up revenues from goods sold." ;
  skos:prefLabel "Factor Cost" ;
.
maecot:FactorDemand
  rdf:type maeco:Demand ;
  dcterms:source "http://www.wwnorton.com/college/econ/stec4/macroeconomics/glossary.asp"^^xsd:anyURI ;
  rdfs:isDefinedBy <http://eds.topbraidlive.org/1.0/taxonomy/maeco> ;
  rdfs:isDefinedBy <http://eds.topbraidlive.org/taxonomy/maeco> ;
  rdfs:label "factor demand" ;
  skos:definition "<STRONG>Factor Demand</STRONG> - the amount of an input demanded by a firm, given the price of the input and the quantity of output being produced; in a competitive market, an input will be demanded up to the point where the value of the marginal product of that input equals the price of the input." ;
  skos:prefLabel "Factor Demand" ;
.
maecot:FactorPrice
  rdf:type maeco:Price ;
  rdfs:isDefinedBy <http://eds.topbraidlive.org/1.0/taxonomy/maeco> ;
  rdfs:isDefinedBy <http://eds.topbraidlive.org/taxonomy/maeco> ;
  rdfs:label "Factor price" ;
  skos:broader maecot:Price ;
  skos:definition "The price paid for the services of a unit of a <a href='http://edg.topbraid.solutions/maeco/term/PrimaryFactor'>primary factor</a> of production per unit time.  Includes the <a href='http://edg.topbraid.solutions/maeco/term/Wage'>wage</a> or salary of labor and the <a href='http://edg.topbraid.solutions/maeco/term/RentalPrice'>rental prices</a> of land and capital.  Does <em>not</em> normally refer to the price of acquiring ownership of the factor itself, which might be called the \"purchase price.\"" ;
  skos:prefLabel "Factor Price" ;
.
maecot:FactoryGatePrice
  rdf:type maeco:Price ;
  rdfs:isDefinedBy <http://eds.topbraidlive.org/1.0/taxonomy/maeco> ;
  rdfs:isDefinedBy <http://eds.topbraidlive.org/taxonomy/maeco> ;
  rdfs:label "Factory gate price" ;
  skos:broader maecot:Price ;
  skos:definition "<a href='http://edg.topbraid.solutions/maeco/term/ExFactory'>Ex factory</a> price." ;
  skos:prefLabel "Factory Gate Price" ;
.
maecot:FairMarketValue
  rdf:type maeco:QuantityKind ;
  dcterms:source "http://www.cftc.gov/LawRegulation/DoddFrankAct/index.htm"^^xsd:anyURI ;
  rdfs:isDefinedBy <http://eds.topbraidlive.org/1.0/taxonomy/maeco> ;
  rdfs:isDefinedBy <http://eds.topbraidlive.org/taxonomy/maeco> ;
  rdfs:label "Fair Market Value" ;
  skos:altLabel "FMV" ;
  skos:broader maecot:ANY_QuantityKind ;
  skos:definition "Fair market value. FMV is used in the case of securities or other assets that are not publicly traded. It is an estimate of the amount that a seller of a security might reasonably expect to receive upon its current sale."@en ;
  skos:prefLabel "Fair market value"@en ;
.
maecot:FairPrice
  rdf:type maeco:Price ;
  rdfs:isDefinedBy <http://eds.topbraidlive.org/1.0/taxonomy/maeco> ;
  rdfs:isDefinedBy <http://eds.topbraidlive.org/taxonomy/maeco> ;
  rdfs:label "Fair price" ;
  skos:broader maecot:Price ;
  skos:definition "<STRONG>1.</STRONG> In the context of the <a href='http://edg.topbraid.solutions/maeco/term/FairTradeMovement'>Fair Trade Movement</a> , a fair price is a price that, when paid to the individual producers of a product such as coffee or handicrafts, gives them access to a viable standard of living, including nutrition, health care, education, and cultural autonomy.  <STRONG>2.</STRONG> In <a href='http://edg.topbraid.solutions/maeco/term/AntiDumpingSuit'>anti-dumping</a> cases, <a href='http://edg.topbraid.solutions/maeco/term/FairValue'>fair value</a> ." ;
  skos:prefLabel "Fair Price" ;
.
maecot:FarmSubsidy
  rdf:type maeco:Subsidy ;
  rdfs:isDefinedBy <http://eds.topbraidlive.org/1.0/taxonomy/maeco> ;
  rdfs:isDefinedBy <http://eds.topbraidlive.org/taxonomy/maeco> ;
  rdfs:label "Farm subsidy" ;
  skos:broader maecot:Subsidy ;
  skos:definition "Payments by governments to farmers.  These may be in return for producing, as when government buys a crop at a higher-than-market price; for not producing, as when it pays to leave land fallow; or for neither, as when payments are for income maintenance or environmental purposes." ;
  skos:prefLabel "Farm Subsidy" ;
.
maecot:FavorableExchangeRate
  rdf:type maeco:Rate ;
  rdfs:isDefinedBy <http://eds.topbraidlive.org/1.0/taxonomy/maeco> ;
  rdfs:isDefinedBy <http://eds.topbraidlive.org/taxonomy/maeco> ;
  rdfs:label "Favorable exchange rate" ;
  skos:broader maecot:ANY_Rate ;
  skos:definition "A special <a href='http://edg.topbraid.solutions/maeco/term/ExchangeRate'>exchange rate</a> , different from the <a href='http://edg.topbraid.solutions/maeco/term/MarketRate'>market</a> or <a href='http://edg.topbraid.solutions/maeco/term/OfficialRate'>official</a> rate, provided by government on a transaction as an indirect way of providing a <a href='http://edg.topbraid.solutions/maeco/term/Subsidy'>subsidy</a> ." ;
  skos:prefLabel "Favorable Exchange Rate" ;
.
maecot:FederalFundsRate
  rdf:type maeco:Rate ;
  dcterms:source "http://www.wwnorton.com/college/econ/stec4/macroeconomics/glossary.asp"^^xsd:anyURI ;
  rdfs:isDefinedBy <http://eds.topbraidlive.org/1.0/taxonomy/maeco> ;
  rdfs:isDefinedBy <http://eds.topbraidlive.org/taxonomy/maeco> ;
  rdfs:label "federal funds rate" ;
  skos:broader maecot:ANY_Rate ;
  skos:definition "<STRONG>Federal Funds Rate</STRONG> - the interest rate on overnight interbank loans. The interest rate on very short-term loans from one commercial bank to another in the United States.  This rate is used as a target for <a href='http://edg.topbraid.solutions/maeco/term/MonetaryPolicy'>monetary policy</a> by the <a href='http://edg.topbraid.solutions/maeco/term/Fed'>Fed</a> ." ;
  skos:prefLabel "Federal Funds Rate" ;
.
maecot:FillRate
  rdf:type maeco:Rate ;
  rdfs:isDefinedBy <http://eds.topbraidlive.org/1.0/taxonomy/maeco> ;
  rdfs:isDefinedBy <http://eds.topbraidlive.org/taxonomy/maeco> ;
  rdfs:label "Fill rate" ;
  skos:broader maecot:ANY_Rate ;
  skos:definition "See <a href='http://edg.topbraid.solutions/maeco/term/QuotaFillRate'>quota fill rate</a> ." ;
  skos:prefLabel "Fill Rate" ;
.
maecot:FixedCost
  rdf:type maeco:Cost ;
  dcterms:source "http://www.wwnorton.com/college/econ/stec4/macroeconomics/glossary.asp"^^xsd:anyURI ;
  rdfs:isDefinedBy <http://eds.topbraidlive.org/1.0/taxonomy/maeco> ;
  rdfs:isDefinedBy <http://eds.topbraidlive.org/taxonomy/maeco> ;
  rdfs:label "Fixed cost" ;
  skos:altLabel "overhead cost" ;
  skos:broader maecot:ANY_Cost ;
  skos:definition "The cost that a firm bears if it produces at all and that is independent of its output.  The presence of a fixed cost tends to imply <a href='http://edg.topbraid.solutions/maeco/term/Irts2'>increasing returns to scale</a> .  Contrasts with <a href='http://edg.topbraid.solutions/maeco/term/VariableCost'>variable cost</a> . <STRONG>Fixed Costs</STRONG> - the costs resulting from fixed inputs, sometimes called  <em>overhead costs</em>" ;
  skos:prefLabel "Fixed Cost" ;
.
maecot:FixedExchangeRate
  rdf:type maeco:Rate ;
  rdfs:isDefinedBy <http://eds.topbraidlive.org/1.0/taxonomy/maeco> ;
  rdfs:isDefinedBy <http://eds.topbraidlive.org/taxonomy/maeco> ;
  rdfs:label "Fixed exchange rate" ;
  skos:broader maecot:ANY_Rate ;
  skos:definition "Usually synonymous with a <a href='http://edg.topbraid.solutions/maeco/term/PeggedExchangeRate'>pegged exchange rate</a> .  Although \"fixed\" seems to imply less likelihood of change, in practice countries seldom if ever achieve a truly fixed rate." ;
  skos:prefLabel "Fixed Exchange Rate" ;
.
maecot:FlexibleExchangeRate
  rdf:type maeco:Rate ;
  rdfs:isDefinedBy <http://eds.topbraidlive.org/1.0/taxonomy/maeco> ;
  rdfs:isDefinedBy <http://eds.topbraidlive.org/taxonomy/maeco> ;
  rdfs:label "Flexible exchange rate" ;
  skos:broader maecot:ANY_Rate ;
  skos:definition "Same as <a href='http://edg.topbraid.solutions/maeco/term/FloatingExchangeRate'>floating exchange rate</a> ." ;
  skos:prefLabel "Flexible Exchange Rate" ;
.
maecot:FloatingExchangeRate
  rdf:type maeco:Rate ;
  rdfs:isDefinedBy <http://eds.topbraidlive.org/1.0/taxonomy/maeco> ;
  rdfs:isDefinedBy <http://eds.topbraidlive.org/taxonomy/maeco> ;
  rdfs:label "Floating exchange rate" ;
  skos:broader maecot:ANY_Rate ;
  skos:definition "A regime in which a country's exchange rate is allowed to fluctuate freely and be determined without <a href='http://edg.topbraid.solutions/maeco/term/Intervention'>intervention</a> in the exchange market by the government or central bank." ;
  skos:prefLabel "Floating Exchange Rate" ;
.
maecot:Floor
  rdf:type maeco:QuantityKind ;
  dcterms:source "http://www.isda.org/c_and_a/oper_commit-dcg-glossary.html"^^xsd:anyURI ;
  rdfs:isDefinedBy <http://eds.topbraidlive.org/1.0/taxonomy/maeco> ;
  rdfs:isDefinedBy <http://eds.topbraidlive.org/taxonomy/maeco> ;
  rdfs:label "Floor" ;
  skos:definition "A lower limit placed on the payoff of a trade, guaranteeing a minimum payoff to the buyer."@en ;
  skos:definition "See <a href='http://edg.topbraid.solutions/maeco/term/PriceFloor'>price floor</a> ." ;
  skos:prefLabel "Floor"@en ;
.
maecot:FluctuatingExchangeRate
  rdf:type maeco:Rate ;
  rdfs:isDefinedBy <http://eds.topbraidlive.org/1.0/taxonomy/maeco> ;
  rdfs:isDefinedBy <http://eds.topbraidlive.org/taxonomy/maeco> ;
  rdfs:label "Fluctuating exchange rate" ;
  skos:broader maecot:ANY_Rate ;
  skos:definition "Same as <a href='http://edg.topbraid.solutions/maeco/term/FlexibleExchangeRate'>flexible</a> or <a href='http://edg.topbraid.solutions/maeco/term/FloatingExchangeRate'>floating exchange rate</a> ." ;
  skos:prefLabel "Fluctuating Exchange Rate" ;
.
maecot:ForeignExchangeRate
  rdf:type maeco:Rate ;
  rdfs:isDefinedBy <http://eds.topbraidlive.org/1.0/taxonomy/maeco> ;
  rdfs:isDefinedBy <http://eds.topbraidlive.org/taxonomy/maeco> ;
  rdfs:label "Foreign exchange rate" ;
  skos:broader maecot:ANY_Rate ;
  skos:definition "The <a href='http://edg.topbraid.solutions/maeco/term/ExchangeRate'>exchange rate</a> ." ;
  skos:prefLabel "Foreign Exchange Rate" ;
.
maecot:ForwardExchangeRate
  rdf:type maeco:Rate ;
  rdfs:isDefinedBy <http://eds.topbraidlive.org/1.0/taxonomy/maeco> ;
  rdfs:isDefinedBy <http://eds.topbraidlive.org/taxonomy/maeco> ;
  rdfs:label "Forward exchange rate" ;
  skos:broader maecot:ANY_Rate ;
  skos:definition "<a href='http://edg.topbraid.solutions/maeco/term/ForwardRate'>Forward rate</a>" ;
  skos:prefLabel "Forward Exchange Rate" ;
.
maecot:ForwardPrice
  rdf:type maeco:Price ;
  rdfs:isDefinedBy <http://eds.topbraidlive.org/1.0/taxonomy/maeco> ;
  rdfs:isDefinedBy <http://eds.topbraidlive.org/taxonomy/maeco> ;
  rdfs:label "Forward price" ;
  skos:broader maecot:Price ;
  skos:definition "In any <a href='http://edg.topbraid.solutions/maeco/term/ForwardMarket'>forward market</a> , the price of the item being traded for delivery at a future date; in <a href='http://edg.topbraid.solutions/maeco/term/ExchangeMarket'>exchange markets</a> , the <a href='http://edg.topbraid.solutions/maeco/term/ForwardRate'>forward rate</a> ." ;
  skos:prefLabel "Forward Price" ;
.
maecot:ForwardRate
  rdf:type maeco:Rate ;
  rdfs:isDefinedBy <http://eds.topbraidlive.org/1.0/taxonomy/maeco> ;
  rdfs:isDefinedBy <http://eds.topbraidlive.org/taxonomy/maeco> ;
  rdfs:label "Forward rate" ;
  skos:broader maecot:ANY_Rate ;
  skos:definition "Also called the <STRONG>forward exchange rate</STRONG> , this is the <a href='http://edg.topbraid.solutions/maeco/term/ExchangeRate'>exchange rate</a> on a <a href='http://edg.topbraid.solutions/maeco/term/ForwardMarket'>forward market</a> transaction." ;
  skos:prefLabel "Forward Rate" ;
.
maecot:FreeFloatingExchangeRate
  rdf:type maeco:Rate ;
  rdfs:isDefinedBy <http://eds.topbraidlive.org/1.0/taxonomy/maeco> ;
  rdfs:isDefinedBy <http://eds.topbraidlive.org/taxonomy/maeco> ;
  rdfs:label "Free-floating exchange rate" ;
  skos:broader maecot:ANY_Rate ;
  skos:definition "<a href='http://edg.topbraid.solutions/maeco/term/FloatingExchangeRate'>Floating exchange rate</a> .  Contrasts with a <a href='http://edg.topbraid.solutions/maeco/term/ManagedFloat'>managed float</a> ." ;
  skos:prefLabel "Free-Floating Exchange Rate" ;
.
maecot:FrischLaborSupplyElasticity
  rdf:type maeco:QuantityKind ;
  rdfs:isDefinedBy <http://eds.topbraidlive.org/1.0/taxonomy/maeco> ;
  rdfs:isDefinedBy <http://eds.topbraidlive.org/taxonomy/maeco> ;
  rdfs:label "Frisch labor supply elasticity" ;
  skos:broader maecot:Elasticity ;
  skos:prefLabel "Frisch labor supply elasticity" ;
.
maecot:FundamentalEquilibriumExchangeRate
  rdf:type maeco:Rate ;
  rdfs:isDefinedBy <http://eds.topbraidlive.org/1.0/taxonomy/maeco> ;
  rdfs:isDefinedBy <http://eds.topbraidlive.org/taxonomy/maeco> ;
  rdfs:label "Fundamental equilibrium exchange rate" ;
  skos:broader maecot:ANY_Rate ;
  skos:definition "This seems to mean the same as <a href='http://edg.topbraid.solutions/maeco/term/EquilibriumExchangeRate'>equilibrium exchange rate</a> .  Adding \"fundamental\" does not seem to remove its ambiguity." ;
  skos:prefLabel "Fundamental Equilibrium Exchange Rate" ;
.
maecot:Gamma
  rdf:type maeco:QuantityKind ;
  dcterms:source "http://www.isda.org/c_and_a/oper_commit-dcg-glossary.html"^^xsd:anyURI ;
  rdfs:isDefinedBy <http://eds.topbraidlive.org/1.0/taxonomy/maeco> ;
  rdfs:isDefinedBy <http://eds.topbraidlive.org/taxonomy/maeco> ;
  rdfs:label "Gamma" ;
  skos:definition "A term in option theory measuring the rate of change of delta. Gamma is used as a measure of how quickly the outright exposure to the underlying can change. In correlation transactions, gamma can be classified as single name gamma or cross gamma: single name gamma is an exposure to a single name in the basket moving; cross gamma is an exposure to all names in the basket moving simultaneously.  "@en ;
  skos:prefLabel "Gamma"@en ;
.
maecot:Gearing
  rdf:type maeco:QuantityKind ;
  dcterms:source "http://www.isda.org/c_and_a/oper_commit-dcg-glossary.html"^^xsd:anyURI ;
  rdfs:isDefinedBy <http://eds.topbraidlive.org/1.0/taxonomy/maeco> ;
  rdfs:isDefinedBy <http://eds.topbraidlive.org/taxonomy/maeco> ;
  rdfs:label "Gearing" ;
  skos:definition "The characteristic of derivatives which enables a far greater reward (or loss) for the same, or much smaller, initial outlay. It is the ratio of exposure to investment outlay; for example an investment of $1 gives an exposure equivalent to a $10 investment and hence a gearing of 10.  "@en ;
  skos:prefLabel "Gearing"@en ;
.
maecot:GeneralTariff
  rdf:type maeco:Tariff ;
  rdfs:isDefinedBy <http://eds.topbraidlive.org/1.0/taxonomy/maeco> ;
  rdfs:isDefinedBy <http://eds.topbraidlive.org/taxonomy/maeco> ;
  rdfs:label "General tariff" ;
  skos:broader maecot:Tariff ;
  skos:definition "The tariff on a product levied against imports from a country that is not granted <a href='http://edg.topbraid.solutions/maeco/term/Mfn2'>most favored nation</a> status and is not subject to a <a href='http://edg.topbraid.solutions/maeco/term/Pta2'>preferential arrangement</a> .  In the US, these are <a href='http://edg.topbraid.solutions/maeco/term/Column2Rates'>Column 2</a> tariffs." ;
  skos:prefLabel "General Tariff" ;
.
maecot:GlobalValueChainParticipationIndex
  rdf:type maeco:IndexMeasure ;
  rdf:type maeco:TradeMeasure ;
  dcterms:source "http://www.federalreserve.gov/econresdata/ifdp/2015/files/ifdp1154.pdf"^^xsd:anyURI ;
  rdfs:isDefinedBy <http://eds.topbraidlive.org/1.0/taxonomy/maeco> ;
  rdfs:isDefinedBy <http://eds.topbraidlive.org/taxonomy/maeco> ;
  rdfs:label "Global value chain (GVC) participation index" ;
  skos:altLabel "GVC participation index" ;
  skos:broader maecot:ANY_TradeMeasure ;
  skos:prefLabel "Global value chain participation index" ;
.
maecot:GracePeriod
  rdf:type maeco:QuantityKind ;
  dcterms:source "http://www.isda.org/c_and_a/oper_commit-dcg-glossary.html"^^xsd:anyURI ;
  rdfs:isDefinedBy <http://eds.topbraidlive.org/1.0/taxonomy/maeco> ;
  rdfs:isDefinedBy <http://eds.topbraidlive.org/taxonomy/maeco> ;
  rdfs:label "Grace Period" ;
  skos:broader maecot:ANY_QuantityKind ;
  skos:definition "A period, normally 30 days, in which a borrower is permitted to make interest or principal payments that it has missed."@en ;
  skos:prefLabel "Grace period"@en ;
.
maecot:GracePeriodExtension
  rdf:type maeco:QuantityKind ;
  dcterms:source "http://www.isda.org/c_and_a/oper_commit-dcg-glossary.html"^^xsd:anyURI ;
  rdfs:isDefinedBy <http://eds.topbraidlive.org/1.0/taxonomy/maeco> ;
  rdfs:isDefinedBy <http://eds.topbraidlive.org/taxonomy/maeco> ;
  rdfs:label "Grace Period Extension" ;
  skos:definition "An optional term in a credit default swap which applies a grace period to a potential failure to pay credit event in order to determine whether an actual credit event has occurred."@en ;
  skos:prefLabel "Grace period extension"@en ;
.
maecot:GreenExchangeRate
  rdf:type maeco:Rate ;
  rdfs:isDefinedBy <http://eds.topbraidlive.org/1.0/taxonomy/maeco> ;
  rdfs:isDefinedBy <http://eds.topbraidlive.org/taxonomy/maeco> ;
  rdfs:label "Green exchange rate" ;
  skos:broader maecot:ANY_Rate ;
  skos:definition "An exchange rate used within the <a href='http://edg.topbraid.solutions/maeco/term/Eu'>EU's</a> <a href='http://edg.topbraid.solutions/maeco/term/Cap2'>Common Agricultural Policy</a> to convert subsidy and support payments into local currencies, avoiding the variability of the rate set in the <a href='http://edg.topbraid.solutions/maeco/term/ExchangeMarket'>exchange market</a> ." ;
  skos:prefLabel "Green Exchange Rate" ;
.
maecot:GreenTariff
  rdf:type maeco:Tariff ;
  rdfs:isDefinedBy <http://eds.topbraidlive.org/1.0/taxonomy/maeco> ;
  rdfs:isDefinedBy <http://eds.topbraidlive.org/taxonomy/maeco> ;
  rdfs:label "Green tariff" ;
  skos:broader maecot:Tariff ;
  skos:definition "<a href='http://edg.topbraid.solutions/maeco/term/CarbonTariff'>carbon tariff</a>" ;
  skos:prefLabel "Green Tariff" ;
.
maecot:GrossBasis
  rdf:type maeco:QuantityKind ;
  dcterms:source "http://www.isda.org/c_and_a/oper_commit-dcg-glossary.html"^^xsd:anyURI ;
  rdfs:isDefinedBy <http://eds.topbraidlive.org/1.0/taxonomy/maeco> ;
  rdfs:isDefinedBy <http://eds.topbraidlive.org/taxonomy/maeco> ;
  rdfs:label "Basis (Gross)" ;
  skos:altLabel "Gross"@en ;
  skos:broader maecot:ANY_QuantityKind ;
  skos:definition "The difference between the relevant cash instrument price and the futures price. Often used in the context of hedging the cash instrument."@en ;
  skos:prefLabel "Basis"@en ;
.
maecot:GrossDomesticIncome
  rdf:type maeco:QuantityKind ;
  rdfs:isDefinedBy <http://eds.topbraidlive.org/1.0/taxonomy/maeco> ;
  rdfs:isDefinedBy <http://eds.topbraidlive.org/taxonomy/maeco> ;
  rdfs:label "Gross Domestic Income" ;
  skos:altLabel "GDI" ;
  skos:broader maecot:Income ;
  skos:prefLabel "Gross Domestic Income" ;
.
maecot:GrossDomesticProduct
  rdf:type maeco:TradeMeasure ;
  dcterms:source "http://www.wwnorton.com/college/econ/stec4/macroeconomics/glossary.asp"^^xsd:anyURI ;
  rdfs:isDefinedBy <http://eds.topbraidlive.org/1.0/taxonomy/maeco> ;
  rdfs:isDefinedBy <http://eds.topbraidlive.org/taxonomy/maeco> ;
  rdfs:label "Gross Domestic Product" ;
  skos:altLabel "GDP" ;
  skos:broader maecot:ANY_TradeMeasure ;
  skos:definition "<STRONG>Gross Domestic Product (gdp)</STRONG> - the total money value of all final goods and services produced within a nation’s borders during a given period of time. The total value of new goods and services produced in a given year within the borders of a country, regardless of by whom.  It is \"gross\" in the sense that it does <em>not</em> , in contrast to <a href='http://edg.topbraid.solutions/maeco/term/Ndp2'>NDP</a> , deduct <a href='http://edg.topbraid.solutions/maeco/term/Depreciation'>depreciation</a> of previously produced <a href='http://edg.topbraid.solutions/maeco/term/Capital'>capital</a> ." ;
  skos:prefLabel "Gross Domestic Product" ;
.
maecot:GrossPosition
  rdf:type maeco:QuantityKind ;
  dcterms:source "http://www.isda.org/c_and_a/oper_commit-dcg-glossary.html"^^xsd:anyURI ;
  rdfs:isDefinedBy <http://eds.topbraidlive.org/1.0/taxonomy/maeco> ;
  rdfs:isDefinedBy <http://eds.topbraidlive.org/taxonomy/maeco> ;
  rdfs:label "Gross Position" ;
  skos:definition "A derivative or asset position expressed without netting bought and sold trades."@en ;
  skos:prefLabel "Gross"@en ;
.
maecot:Haircut
  rdf:type maeco:QuantityKind ;
  dcterms:source "http://www.isda.org/c_and_a/oper_commit-dcg-glossary.html"^^xsd:anyURI ;
  rdfs:isDefinedBy <http://eds.topbraidlive.org/1.0/taxonomy/maeco> ;
  rdfs:isDefinedBy <http://eds.topbraidlive.org/taxonomy/maeco> ;
  rdfs:label "Haircut" ;
  rdfs:seeAlso maecot:ValuationPercentage ;
  skos:definition "The loss of asset value for a <a href='http://edg.topbraid.solutions/maeco/term/Creditor'>creditor</a> when a <a href='http://edg.topbraid.solutions/maeco/term/Debtor'>debtor</a> <a href='http://edg.topbraid.solutions/maeco/term/Default'>defaults</a> and then renegotiates downward the value of the loan.  Sizable haircuts have been often been experienced by international lenders as the result of <a href='http://edg.topbraid.solutions/maeco/term/DebtCrisis'>debt</a> and <a href='http://edg.topbraid.solutions/maeco/term/FinancialCrisis'>financial crises</a> ." ;
  skos:definition "The percentage by which the market value of the collateral will be reduced to allow for price volatility and instrument liquidity in respect of the relevant collateral between collateral calls."@en ;
  skos:exactMatch maecot:ValuationPercentage ;
  skos:prefLabel "Haircut"@en ;
.
maecot:HistoricalDefaultRate
  rdf:type maeco:Rate ;
  rdfs:isDefinedBy <http://eds.topbraidlive.org/1.0/taxonomy/maeco> ;
  rdfs:isDefinedBy <http://eds.topbraidlive.org/taxonomy/maeco> ;
  rdfs:label "Historical Default Rate" ;
  skos:prefLabel "Historical default rate"@en ;
.
maecot:HistoricalLossRate
  rdf:type maeco:Rate ;
  rdfs:isDefinedBy <http://eds.topbraidlive.org/1.0/taxonomy/maeco> ;
  rdfs:isDefinedBy <http://eds.topbraidlive.org/taxonomy/maeco> ;
  rdfs:label "Historical Loss Rate" ;
  skos:prefLabel "Historical loss rate"@en ;
.
maecot:IcebergTransportCost
  rdf:type maeco:Cost ;
  rdfs:isDefinedBy <http://eds.topbraidlive.org/1.0/taxonomy/maeco> ;
  rdfs:isDefinedBy <http://eds.topbraidlive.org/taxonomy/maeco> ;
  rdfs:label "Iceberg transport cost" ;
  skos:broader maecot:ANY_Cost ;
  skos:definition "A cost of transporting a good that uses up some fraction of the good itself, rather than other resources.  By analogy with floating an iceberg, costless except for the part of the iceberg that melts.  Far from realistic, but a tractable way of modeling transport costs since it impacts no other market.  Due to <a href='http://edg.topbraid.solutions/maeco/term/Bib.html#Samuelson1954'>Samuelson (1954)</a> ." ;
  skos:prefLabel "Iceberg Transport Cost" ;
.
maecot:ImplicitTariff
  rdf:type maeco:Tariff ;
  rdfs:isDefinedBy <http://eds.topbraidlive.org/1.0/taxonomy/maeco> ;
  rdfs:isDefinedBy <http://eds.topbraidlive.org/taxonomy/maeco> ;
  rdfs:label "Implicit tariff" ;
  skos:broader maecot:Tariff ;
  skos:definition "<STRONG>1.</STRONG> <a href='http://edg.topbraid.solutions/maeco/term/TariffRevenue'>Tariff revenue</a> on a good or group of goods, divided by the corresponding value of imports.  Often lower than the official or statutory tariff, due both to <a href='http://edg.topbraid.solutions/maeco/term/Pta'>PTAs</a> and to failures in <a href='http://edg.topbraid.solutions/maeco/term/CustomsProcedure'>customs collection</a> .  <STRONG>2.</STRONG> The difference between the price just inside a border and the price just outside it, especially in the case of a good protected by an import <a href='http://edg.topbraid.solutions/maeco/term/Quota'>quota</a> ." ;
  skos:prefLabel "Implicit Tariff" ;
.
maecot:ImportParityPrice
  rdf:type maeco:Price ;
  rdfs:isDefinedBy <http://eds.topbraidlive.org/1.0/taxonomy/maeco> ;
  rdfs:isDefinedBy <http://eds.topbraidlive.org/taxonomy/maeco> ;
  rdfs:label "Import parity price" ;
  skos:broader maecot:Price ;
  skos:definition "The price that a purchaser pays or can expect to pay for an imported good, thus the <a href='http://edg.topbraid.solutions/maeco/term/Cif'>c.i.f.</a> import price plus tariff plus transport cost to the purchaser's location.  This and the <a href='http://edg.topbraid.solutions/maeco/term/ExportParityPrice'>export parity price</a> together define a range of the possible equilibrium prices for an equivalent domestically produced good." ;
  skos:prefLabel "Import Parity Price" ;
.
maecot:ImportTariff
  rdf:type maeco:Tariff ;
  rdfs:isDefinedBy <http://eds.topbraidlive.org/1.0/taxonomy/maeco> ;
  rdfs:isDefinedBy <http://eds.topbraidlive.org/taxonomy/maeco> ;
  rdfs:label "Import tariff" ;
  skos:broader maecot:Tariff ;
  skos:definition "<a href='http://edg.topbraid.solutions/maeco/term/Tariff'>Tariff</a>" ;
  skos:prefLabel "Import Tariff" ;
.
maecot:ImportWeightedAverageTariff
  rdf:type maeco:Tariff ;
  rdfs:isDefinedBy <http://eds.topbraidlive.org/1.0/taxonomy/maeco> ;
  rdfs:isDefinedBy <http://eds.topbraidlive.org/taxonomy/maeco> ;
  rdfs:label "Import-weighted average tariff" ;
  skos:broader maecot:Tariff ;
  skos:definition "See <a href='http://edg.topbraid.solutions/maeco/term/TradeWeightedAverageTariff'>trade weighted average tariff</a> ." ;
  skos:prefLabel "Import-Weighted Average Tariff" ;
.
maecot:Income
  rdf:type maeco:QuantityKind ;
  dcterms:source "http://www.cftc.gov/LawRegulation/DoddFrankAct/index.htm"^^xsd:anyURI ;
  rdfs:isDefinedBy <http://eds.topbraidlive.org/1.0/taxonomy/maeco> ;
  rdfs:isDefinedBy <http://eds.topbraidlive.org/taxonomy/maeco> ;
  rdfs:label "Income" ;
  skos:broader maecot:ANY_QuantityKind ;
  skos:definition "<STRONG>1.</STRONG> The amount of money ( <a href='http://edg.topbraid.solutions/maeco/term/Nominal'>nominal</a> or <a href='http://edg.topbraid.solutions/maeco/term/Real'>real</a> ) received by a person, household, or other economic unit per unit time.  May or may not be in return for services provided or goods sold.  <STRONG>2.</STRONG> <a href='http://edg.topbraid.solutions/maeco/term/NationalIncome'>National income</a> .  <STRONG>3.</STRONG> The return earned on an <a href='http://edg.topbraid.solutions/maeco/term/Asset'>asset</a> per unit time." ;
  skos:prefLabel "Capital"@en ;
.
maecot:IncomeElasticityOfDemand
  rdf:type maeco:Demand ;
  dcterms:source "http://www.wwnorton.com/college/econ/stec4/macroeconomics/glossary.asp"^^xsd:anyURI ;
  rdfs:isDefinedBy <http://eds.topbraidlive.org/1.0/taxonomy/maeco> ;
  rdfs:isDefinedBy <http://eds.topbraidlive.org/taxonomy/maeco> ;
  rdfs:label "income elasticity of demand" ;
  skos:definition "<STRONG>Income Elasticity Of Demand</STRONG> - the percentage change in quantity demanded of a good as the result of a 1 percent change in income (the percentage change in quantity demanded divided by the percentage change in income)" ;
  skos:prefLabel "Income Elasticity Of Demand" ;
.
maecot:IncomeRedistributionArgumentForATariff
  rdf:type maeco:Tariff ;
  rdfs:isDefinedBy <http://eds.topbraidlive.org/1.0/taxonomy/maeco> ;
  rdfs:isDefinedBy <http://eds.topbraidlive.org/taxonomy/maeco> ;
  rdfs:label "Income redistribution argument for a tariff" ;
  skos:broader maecot:Tariff ;
  skos:definition "The argument that tariffs should be used in order to redistribute income towards the poor.  In a rich country, where unskilled labor is the scarce factor, this can make sense as explained in the <a href='http://edg.topbraid.solutions/maeco/term/Ss2'>Stolper-Samuelson Theorem</a> , but it is a <a href='http://edg.topbraid.solutions/maeco/term/SecondBestArgument'>second-best argument</a> ." ;
  skos:prefLabel "Income Redistribution Argument For A Tariff" ;
.
maecot:IncreasingCost
  rdf:type maeco:Cost ;
  rdfs:isDefinedBy <http://eds.topbraidlive.org/1.0/taxonomy/maeco> ;
  rdfs:isDefinedBy <http://eds.topbraidlive.org/taxonomy/maeco> ;
  rdfs:label "Increasing cost" ;
  skos:broader maecot:ANY_Cost ;
  skos:definition "<STRONG>1.</STRONG> Referring to a single firm or industry, the rise in cost of production that occurs when output is increased by expanding variable inputs while holding some fixed input constant.  A corollary of the <a href='http://edg.topbraid.solutions/maeco/term/LawOfDiminishingReturns'>Law of Diminishing Returns</a> .  <STRONG>2.</STRONG> In general equilibrium, <a href='http://edg.topbraid.solutions/maeco/term/IncreasingOpportunityCost'>increasing opportunity cost</a> ." ;
  skos:prefLabel "Increasing Cost" ;
.
maecot:IncreasingOpportunityCost
  rdf:type maeco:Cost ;
  rdfs:isDefinedBy <http://eds.topbraidlive.org/1.0/taxonomy/maeco> ;
  rdfs:isDefinedBy <http://eds.topbraidlive.org/taxonomy/maeco> ;
  rdfs:label "Increasing opportunity cost" ;
  skos:broader maecot:IncreasingCost ;
  skos:broader maecot:OpportunityCost ;
  skos:definition "The characteristic of an economy that the <a href='http://edg.topbraid.solutions/maeco/term/OpportunityCost'>opportunity cost</a> of a good rises as more is produced, resulting in a <a href='http://edg.topbraid.solutions/maeco/term/TransformationCurve'>transformation curve</a> that is <a href='http://edg.topbraid.solutions/maeco/term/Concave'>concave</a> to the origin.  In the <a href='http://edg.topbraid.solutions/maeco/term/HOModel'>HO Model</a> , this happens in spite of <a href='http://edg.topbraid.solutions/maeco/term/Crts'>CRTS</a> if sectors have different <a href='http://edg.topbraid.solutions/maeco/term/FactorIntensity'>factor intensities</a> ." ;
  skos:prefLabel "Increasing Opportunity Cost" ;
.
maecot:IndirectExchangeRate
  rdf:type maeco:Rate ;
  rdfs:isDefinedBy <http://eds.topbraidlive.org/1.0/taxonomy/maeco> ;
  rdfs:isDefinedBy <http://eds.topbraidlive.org/taxonomy/maeco> ;
  rdfs:label "Indirect exchange rate" ;
  skos:broader maecot:ANY_Rate ;
  skos:definition "The foreign-currency price of a unit of domestic currency.  (This definition appears in several places, but it is a mystery to me why this is any less direct than its reciprocal.)" ;
  skos:prefLabel "Indirect Exchange Rate" ;
.
maecot:IndirectExportSubsidy
  rdf:type maeco:Subsidy ;
  rdfs:isDefinedBy <http://eds.topbraidlive.org/1.0/taxonomy/maeco> ;
  rdfs:isDefinedBy <http://eds.topbraidlive.org/taxonomy/maeco> ;
  rdfs:label "Indirect export subsidy" ;
  skos:broader maecot:Subsidy ;
  skos:definition "An <a href='http://edg.topbraid.solutions/maeco/term/UpstreamSubsidization'>upstream subsidy</a> ." ;
  skos:prefLabel "Indirect Export Subsidy" ;
.
maecot:InflationRate
  rdf:type maeco:Rate ;
  rdfs:isDefinedBy <http://eds.topbraidlive.org/1.0/taxonomy/maeco> ;
  rdfs:isDefinedBy <http://eds.topbraidlive.org/taxonomy/maeco> ;
  rdfs:label "Inflation rate" ;
  skos:broader maecot:ANY_Rate ;
  skos:definition "The percentage increase in the price level per year.  See <a href='http://edg.topbraid.solutions/maeco/term/Inflation'>inflation</a> ." ;
  skos:prefLabel "Inflation Rate" ;
.
maecot:InitialMargin
  rdf:type maeco:QuantityKind ;
  dcterms:source "http://www.cftc.gov/LawRegulation/DoddFrankAct/index.htm"^^xsd:anyURI ;
  rdfs:isDefinedBy <http://eds.topbraidlive.org/1.0/taxonomy/maeco> ;
  rdfs:isDefinedBy <http://eds.topbraidlive.org/taxonomy/maeco> ;
  rdfs:label "Initial Margin" ;
  skos:altLabel "IM" ;
  skos:broader maecot:ANY_QuantityKind ;
  skos:definition "Initial margin. In the new world of centrally cleared derivatives, clearing members must post margin on a daily or intraday basis in order to minimize unsecured exposures. Initial margin, which is required to be posted at the outset of a transaction, is intended to provide a buffer such that, even with market volatility, unsecured exposures are expected to be minimal."@en ;
  skos:prefLabel "Initial margin"@en ;
.
maecot:InstitutionalOwnership
  rdf:type maeco:QuantityKind ;
  rdfs:isDefinedBy <http://eds.topbraidlive.org/1.0/taxonomy/maeco> ;
  rdfs:isDefinedBy <http://eds.topbraidlive.org/taxonomy/maeco> ;
  rdfs:label "Institutional Ownership" ;
  skos:broader maecot:ANY_QuantityKind ;
  skos:definition "Institutional Ownership" ;
  skos:prefLabel "Institutional Ownership" ;
.
maecot:InterbankRate
  rdf:type maeco:Rate ;
  rdfs:isDefinedBy <http://eds.topbraidlive.org/1.0/taxonomy/maeco> ;
  rdfs:isDefinedBy <http://eds.topbraidlive.org/taxonomy/maeco> ;
  rdfs:label "Interbank rate" ;
  skos:broader maecot:ANY_Rate ;
  skos:definition "The rate of interest charged by a bank on a loan to another bank.  See <a href='http://edg.topbraid.solutions/maeco/term/Libor'>LIBOR</a> ." ;
  skos:prefLabel "Interbank Rate" ;
.
maecot:InterestOnLawyersTrustAccount
  rdf:type maeco:QuantityKind ;
  dcterms:source "http://www.cftc.gov/LawRegulation/DoddFrankAct/index.htm"^^xsd:anyURI ;
  rdfs:isDefinedBy <http://eds.topbraidlive.org/1.0/taxonomy/maeco> ;
  rdfs:isDefinedBy <http://eds.topbraidlive.org/taxonomy/maeco> ;
  rdfs:label "Interest On Lawyers Trust Account" ;
  skos:altLabel "IOLTA" ;
  skos:broader maecot:ANY_QuantityKind ;
  skos:definition "Interest on Lawyers' Trust Accounts is a method of raising money for charitable purposes, primarily the provision of civil legal services to indigent persons, through the use of interest earned on certain lawyer trust accounts."@en ;
  skos:prefLabel "Interest on Lawyers' Trust Account"@en ;
.
maecot:InterestOnTrustAccount
  rdf:type maeco:QuantityKind ;
  dcterms:source "http://www.cftc.gov/LawRegulation/DoddFrankAct/index.htm"^^xsd:anyURI ;
  rdfs:isDefinedBy <http://eds.topbraidlive.org/1.0/taxonomy/maeco> ;
  rdfs:isDefinedBy <http://eds.topbraidlive.org/taxonomy/maeco> ;
  rdfs:label "Interest On Trust Account" ;
  skos:altLabel "IOTA" ;
  skos:broader maecot:ANY_QuantityKind ;
  skos:definition "Interest on Trust Account."@en ;
  skos:prefLabel "Interest on Trust Account"@en ;
.
maecot:InterestRate
  rdf:type maeco:Rate ;
  rdfs:isDefinedBy <http://eds.topbraidlive.org/1.0/taxonomy/maeco> ;
  rdfs:isDefinedBy <http://eds.topbraidlive.org/taxonomy/maeco> ;
  rdfs:label "Interest rate" ;
  skos:broader maecot:ANY_Rate ;
  skos:definition "The rate of return on bonds, loans, or deposits.  When one speaks of \"the\" interest rate, it is usually in a model or other context in which there is only one." ;
  skos:prefLabel "Interest Rate" ;
.
maecot:InterestRateCap
  rdf:type maeco:Rate ;
  dcterms:source "http://www.isda.org/c_and_a/oper_commit-dcg-glossary.html"^^xsd:anyURI ;
  rdfs:isDefinedBy <http://eds.topbraidlive.org/1.0/taxonomy/maeco> ;
  rdfs:isDefinedBy <http://eds.topbraidlive.org/taxonomy/maeco> ;
  rdfs:label "Interest Rate Cap" ;
  skos:broader maecot:InterestRate ;
  skos:definition "An option product where the holder (buyer) is guaranteed a maximum borrowing cost over a specified term."@en ;
  skos:prefLabel "Interest rate cap"@en ;
.
maecot:InterestRateCollar
  rdf:type maeco:Rate ;
  dcterms:source "http://www.isda.org/c_and_a/oper_commit-dcg-glossary.html"^^xsd:anyURI ;
  rdfs:isDefinedBy <http://eds.topbraidlive.org/1.0/taxonomy/maeco> ;
  rdfs:isDefinedBy <http://eds.topbraidlive.org/taxonomy/maeco> ;
  rdfs:label "Interest Rate Collar" ;
  skos:broader maecot:InterestRate ;
  skos:definition "An option product where the holder (buyer) is guaranteed a maximum and minimum borrowing cost over a specified term."@us ;
  skos:prefLabel "Interest rate collar"@us ;
.
maecot:InterestRateOnExcessReserves
  rdf:type maeco:Rate ;
  rdfs:isDefinedBy <http://eds.topbraidlive.org/1.0/taxonomy/maeco> ;
  rdfs:isDefinedBy <http://eds.topbraidlive.org/taxonomy/maeco> ;
  rdfs:label "Interest Rate On Excess Reserves" ;
  skos:altLabel "IOER" ;
  skos:broader maecot:InterestRate ;
  skos:prefLabel "Interest Rate on Excess Reserves"@us ;
.
maecot:InterestRateOnRequiredReserves
  rdf:type maeco:Rate ;
  rdfs:isDefinedBy <http://eds.topbraidlive.org/1.0/taxonomy/maeco> ;
  rdfs:isDefinedBy <http://eds.topbraidlive.org/taxonomy/maeco> ;
  rdfs:label "Interest Rate On Required Reserves" ;
  skos:altLabel "IORR" ;
  skos:broader maecot:InterestRate ;
  skos:prefLabel "Interest Rate on Required Reserves"@us ;
.
maecot:InterestShortfall
  rdf:type maeco:QuantityKind ;
  dcterms:source "http://www.isda.org/c_and_a/oper_commit-dcg-glossary.html"^^xsd:anyURI ;
  rdfs:isDefinedBy <http://eds.topbraidlive.org/1.0/taxonomy/maeco> ;
  rdfs:isDefinedBy <http://eds.topbraidlive.org/taxonomy/maeco> ;
  rdfs:label "Interest Shortfall" ;
  skos:definition "The payment from the seller to buyer compensating for any reduced coupon payment on the underlying bond on a PAUG swap. If the reduced coupon is subsequently made up in future coupon payments this will result in an interest shortfall reimbursement from buyer to seller."@en ;
  skos:prefLabel "Interest shortfall"@en ;
.
maecot:InternationalPrice
  rdf:type maeco:Price ;
  rdfs:isDefinedBy <http://eds.topbraidlive.org/1.0/taxonomy/maeco> ;
  rdfs:isDefinedBy <http://eds.topbraidlive.org/taxonomy/maeco> ;
  rdfs:label "International price" ;
  skos:broader maecot:Price ;
  skos:definition "<a href='http://edg.topbraid.solutions/maeco/term/WorldPrice'>World price</a>" ;
  skos:prefLabel "International Price" ;
.
maecot:IssuePrice
  rdf:type maeco:QuantityKind ;
  dcterms:source "http://www.isda.org/c_and_a/oper_commit-dcg-glossary.html"^^xsd:anyURI ;
  rdfs:isDefinedBy <http://eds.topbraidlive.org/1.0/taxonomy/maeco> ;
  rdfs:isDefinedBy <http://eds.topbraidlive.org/taxonomy/maeco> ;
  rdfs:label "Issue Price" ;
  skos:definition "The percentage of principal value at which the price of a new issue of securities is fixed."@en ;
  skos:prefLabel "Issue price"@en ;
.
maecot:JoblessRate
  rdf:type maeco:Rate ;
  rdfs:isDefinedBy <http://eds.topbraidlive.org/1.0/taxonomy/maeco> ;
  rdfs:isDefinedBy <http://eds.topbraidlive.org/taxonomy/maeco> ;
  rdfs:label "Jobless rate" ;
  skos:broader maecot:ANY_Rate ;
  skos:definition "Same as <a href='http://edg.topbraid.solutions/maeco/term/UnemploymentRate'>unemployment rate</a> ." ;
  skos:prefLabel "Jobless Rate" ;
.
maecot:L-ShapedInterest
  rdf:type maeco:QuantityKind ;
  dcterms:source "http://www.cftc.gov/LawRegulation/DoddFrankAct/index.htm"^^xsd:anyURI ;
  rdfs:isDefinedBy <http://eds.topbraidlive.org/1.0/taxonomy/maeco> ;
  rdfs:isDefinedBy <http://eds.topbraidlive.org/taxonomy/maeco> ;
  rdfs:label "L-Shaped Interest" ;
  skos:definition "A combination of a horizontal interest and a vertical interest retained by a securitizer to satisfy risk retention rules."@en ;
  skos:prefLabel "L-Shaped Interest"@en ;
.
maecot:LaborForceParticipationRate
  rdf:type maeco:Rate ;
  dcterms:source "http://www.wwnorton.com/college/econ/stec4/macroeconomics/glossary.asp"^^xsd:anyURI ;
  rdfs:isDefinedBy <http://eds.topbraidlive.org/1.0/taxonomy/maeco> ;
  rdfs:isDefinedBy <http://eds.topbraidlive.org/taxonomy/maeco> ;
  rdfs:label "labor force participation rate" ;
  skos:broader maecot:ANY_Rate ;
  skos:definition "<STRONG>Labor Force Participation Rate</STRONG> - the fraction of the working-age population that is employed or seeking employment" ;
  skos:prefLabel "Labor Force Participation Rate" ;
.
maecot:LawOfOnePrice
  rdf:type maeco:Price ;
  rdfs:isDefinedBy <http://eds.topbraidlive.org/1.0/taxonomy/maeco> ;
  rdfs:isDefinedBy <http://eds.topbraidlive.org/taxonomy/maeco> ;
  rdfs:label "Law of One Price" ;
  skos:broader maecot:Price ;
  skos:definition "The principle that identical goods should sell for the same price throughout the world if trade were <a href='http://edg.topbraid.solutions/maeco/term/FreeTrade'>free</a> and <a href='http://edg.topbraid.solutions/maeco/term/FrictionlessTrade'>frictionless</a> ." ;
  skos:prefLabel "Law Of One Price" ;
.
maecot:LessStableDeposit
  rdf:type maeco:QuantityKind ;
  rdfs:isDefinedBy <http://eds.topbraidlive.org/1.0/taxonomy/maeco> ;
  rdfs:isDefinedBy <http://eds.topbraidlive.org/taxonomy/maeco> ;
  rdfs:label "Less Stable Deposi" ;
  skos:altLabel "Less Stable Deposi"@en ;
  skos:broader maecot:ANY_QuantityKind ;
  skos:definition "Less Stable deposits have a run-off rate = 10% and higher. Supervisory authorities are expected to develop additional buckets with higher run- off rates as necessary to apply to buckets of potentially less stable retail deposits in their jurisdictions, with a minimum run-off rate of 10%. These jurisdiction-specific run-off rates should be clearly outlined and publicly transparent. Buckets of less stable deposits could include deposits that are not fully covered by an effective deposit insurance scheme or sovereign deposit guarantee, high-value deposits, deposits from sophisticated or high net worth individuals, deposits that can be withdrawn quickly (eg internet deposits) and foreign currency deposits, as determined by each jurisdiction."@en ;
  skos:prefLabel "Less Stable Deposit"@en ;
  prov:wasInfluencedBy "<http://www.bis.org/publ/bcbs238.pdf>" ;
.
maecot:LessStableRetailDeposits
  rdf:type maeco:QuantityKind ;
  rdfs:isDefinedBy <http://eds.topbraidlive.org/1.0/taxonomy/maeco> ;
  rdfs:isDefinedBy <http://eds.topbraidlive.org/taxonomy/maeco> ;
  rdfs:label "Less Stable Retail Deposits" ;
  skos:broader maecot:LessStableDeposit ;
  skos:broader maecot:RetailDeposits ;
  skos:definition "Retail deposits are divided into stable and less stable portions of funds as described below, with minimum run-off rates listed for each category. The run-off rates for retail deposits are minimum floors, with higher run-off rates established by individual jurisdictions as appropriate to capture depositor behaviour in a period of stress in each jurisdiction."@en ;
  skos:prefLabel "Less Stable Retail Deposits"@en ;
  prov:wasInfluencedBy "<http://www.bis.org/publ/bcbs238.pdf>" ;
.
maecot:LevarageBuffer
  rdf:type maeco:Buffer ;
  dcterms:source "http://www.cftc.gov/LawRegulation/DoddFrankAct/index.htm"^^xsd:anyURI ;
  rdfs:isDefinedBy <http://eds.topbraidlive.org/1.0/taxonomy/maeco> ;
  rdfs:isDefinedBy <http://eds.topbraidlive.org/taxonomy/maeco> ;
  rdfs:label "Levarage Buffer" ;
  skos:broader maecot:ANY_Buffer ;
  skos:definition "Leverage buffer."@en ;
  skos:prefLabel "Leverage buffer"@en ;
.
maecot:LiquidityCoverageRatio
  rdf:type maeco:Ratio ;
  dcterms:source "http://www.cftc.gov/LawRegulation/DoddFrankAct/index.htm"^^xsd:anyURI ;
  rdfs:isDefinedBy <http://eds.topbraidlive.org/1.0/taxonomy/maeco> ;
  rdfs:isDefinedBy <http://eds.topbraidlive.org/taxonomy/maeco> ;
  rdfs:label "Liquidity Coverage Ratio" ;
  rdfs:seeAlso maecot:StockOfHQLA ;
  skos:altLabel "LCR" ;
  skos:altLabel "Liquidity Coverage Requirement" ;
  skos:broader maecot:ANY_Ratio ;
  skos:definition """Liquidity Coverage Ratio (or Requirement). The LCR was finalized by the BCBS in 2013. It is a new short-term liquidity requirement that is implemented by a ratio test, where a bank's modeled outflows are in the denominator, and the bank's HQLA are included in the denominator. If the ratio equals or exceeds 100%, the liquidity requirement is satisfied. 

The LCR builds on traditional liquidity coverage ratio methodologies used internally by banks to assess exposure to contingent liquidity events. The total net cash outflows for the scenario are to be calculated for 30 calendar days into the future. The standard requires that, absent a situation of financial stress, the value of the ratio be no lower than 100%4 (ie the stock of HQLA should at least equal total net cash outflows) on an ongoing basis because the stock of unencumbered HQLA is intended to serve as a defence against the potential onset of liquidity stress. During a period of financial stress, however, banks may use their stock of HQLA, thereby falling below 100%, as maintaining the LCR at 100% under such circumstances could produce undue negative effects on the bank and other market participants. Supervisors will subsequently assess this situation and will adjust their response flexibly according to the circumstances.

The objective of the LCR is to promote the short-term resilience of the liquidity risk profile of banks. It does this by ensuring that banks have an adequate stock of unencumbered high-quality liquid assets (HQLA) that can be converted easily and immediately in private markets into cash to meet their liquidity needs for a 30 calendar day liquidity stress scenario. The LCR will improve the banking sector's ability to absorb shocks arising from financial and economic stress, whatever the source, thus reducing the risk of spillover from the financial sector to the real economy.

The LCR has two components: (a)	Value of the stock of HQLA in stressed conditions; and (b) total net cash outflows.  LCR is calculate by dividing the \"Stock of HQLA\" by the total net cash outflows over the next 30 calendar days. The LCA should be greater or equal to 100%.

Under the standard, banks must hold a stock of unencumbered HQLA to cover the total net cash outflows (as defined below) over a 30-day period under the prescribed stress scenario. In order to qualify as HQLA, assets should be liquid in markets during a time of stress and, ideally, be central bank eligible."""@en ;
  skos:prefLabel "Liquidity Coverage Ratio (LCR)" ;
  prov:wasInfluencedBy "<http://www.bis.org/publ/bcbs238.pdf>" ;
.
maecot:LiquidityPremium
  rdf:type maeco:QuantityKind ;
  dcterms:source "http://www.federalreserve.gov/econresdata/ifdp/2015/files/ifdp1138.pdf"^^xsd:anyURI ;
  dcterms:source "http://www.investopedia.com/terms/l/liquiditypremium.asp#ixzz43W9eSfX8"^^xsd:anyURI ;
  rdfs:isDefinedBy <http://eds.topbraidlive.org/1.0/taxonomy/maeco> ;
  rdfs:isDefinedBy <http://eds.topbraidlive.org/taxonomy/maeco> ;
  rdfs:label "Liquidity Premium" ;
  skos:altLabel "Liquidity Premia" ;
  skos:definition "A premium that investors will demand when any given security can not be easily converted into cash, and converted at the fair market value. When the liquidity premium is high, then the asset is said to be illiquid, which will cause prices to fall, and interest rates to rise." ;
  skos:prefLabel "Liquidity Premium" ;
.
maecot:LiquidityRatio
  rdf:type maeco:Ratio ;
  rdfs:isDefinedBy <http://eds.topbraidlive.org/1.0/taxonomy/maeco> ;
  rdfs:isDefinedBy <http://eds.topbraidlive.org/taxonomy/maeco> ;
  rdfs:label "Liquidity Ratio" ;
  skos:altLabel "Reserve Requirement" ;
  skos:broader maecot:ANY_Ratio ;
  skos:definition "In the United States, a reserve requirement (or liquidity ratio) is a minimum value, set by the Board of Governors of the Federal Reserve System, of the ratio of required reserves to some category of deposits held at depository institutions (e.g., commercial bank including US branch of a foreign bank, savings and loan association, savings bank, credit union). The only deposit categories currently subject to reserve requirements are transaction accounts, mainly checking accounts. There is no reserve requirement on savings accounts, nor on time deposits owned by individuals.[5] The total amount of all net transaction accounts (total transaction accounts less amounts due from other banks and less cash items in the process of collection) held in US depository institutions, plus US currency held by the nonbank public, is called M1." ;
  skos:prefLabel "Liquidity Ratio"@us ;
  prov:wasInfluencedBy "https://en.wikipedia.org/wiki/Reserve_requirement"^^xsd:anyURI ;
.
maecot:LiquidityYieldSpread
  rdf:type maeco:QuantityKind ;
  dcterms:source "http://www.federalreserve.gov/econresdata/ifdp/2015/files/ifdp1138.pdf"^^xsd:anyURI ;
  rdfs:isDefinedBy <http://eds.topbraidlive.org/1.0/taxonomy/maeco> ;
  rdfs:isDefinedBy <http://eds.topbraidlive.org/taxonomy/maeco> ;
  rdfs:label "Liquidity Yield Spread" ;
  skos:prefLabel "Liquidity Yield Spread" ;
.
maecot:LoanSpread
  rdf:type maeco:Measure ;
  rdfs:isDefinedBy <http://eds.topbraidlive.org/1.0/taxonomy/maeco> ;
  rdfs:isDefinedBy <http://eds.topbraidlive.org/taxonomy/maeco> ;
  rdfs:label "Loan Spread" ;
  skos:broader maecot:ANY_Measure ;
  skos:definition "Loan spread is a measure defined as the spread on basis points over LIBOR." ;
  skos:prefLabel "Loan Spread" ;
.
maecot:LoanToDepositRatio
  rdf:type maeco:Ratio ;
  dcterms:source "http://www.cftc.gov/LawRegulation/DoddFrankAct/index.htm"^^xsd:anyURI ;
  rdfs:isDefinedBy <http://eds.topbraidlive.org/1.0/taxonomy/maeco> ;
  rdfs:isDefinedBy <http://eds.topbraidlive.org/taxonomy/maeco> ;
  rdfs:label "Loan To Deposit Ratio" ;
  skos:altLabel "LDR" ;
  skos:broader maecot:ANY_Ratio ;
  skos:definition "Loan to Deposit Ratio."@en ;
  skos:prefLabel "Loan to Deposit Ratio"@en ;
.
maecot:LondonInterbankOfferedRate
  rdf:type maeco:Rate ;
  dcterms:source "http://www.cftc.gov/LawRegulation/DoddFrankAct/index.htm"^^xsd:anyURI ;
  dcterms:source "http://www.isda.org/c_and_a/oper_commit-dcg-glossary.html"^^xsd:anyURI ;
  dcterms:title "London InterBank Offered Rate" ;
  rdfs:isDefinedBy <http://eds.topbraidlive.org/1.0/taxonomy/maeco> ;
  rdfs:isDefinedBy <http://eds.topbraidlive.org/taxonomy/maeco> ;
  rdfs:label "LIBOR" ;
  skos:broader maecot:InterestRate ;
  skos:definition "London InterBank Offered Rate. LIBOR refers to the rate of interest historically published by the BBA based on a survey of a panel of major banks regarding the interest rate at which each such bank believes it could borrow funds in a particular currency, for a particular maturity, in the wholesale market in London. Regulators are now investigating possible rigging of this benchmark. The London Inter-Bank Offered Rate is the rate used when one bank borrows from another bank. It is the benchmark used to price many capital market and derivative transactions."@en ;
  skos:prefLabel "LIBOR" ;
.
maecot:LowToValueRatio
  rdf:type maeco:Ratio ;
  dcterms:source "http://www.cftc.gov/LawRegulation/DoddFrankAct/index.htm"^^xsd:anyURI ;
  rdfs:isDefinedBy <http://eds.topbraidlive.org/1.0/taxonomy/maeco> ;
  rdfs:isDefinedBy <http://eds.topbraidlive.org/taxonomy/maeco> ;
  rdfs:label "Low To Value Ratio" ;
  skos:altLabel "LTV" ;
  skos:broader maecot:ANY_Ratio ;
  skos:definition "Loan-to-Value Ratio. The loan-to-value ratio is most frequently used in discussing mortgage loans, with higher LTV loans being viewed as higher risk loans. Under the capital standards, risk weights for residential mortgage loans are based on the LTV of the loan. Loans are categorized for Basel purposes as Category 1 (less risky, lower risk weight) and Category 2 (higher risk, higher risk weight) loans."@en ;
  skos:prefLabel "Loan-to-Value Ratio"@en ;
.
maecot:MFNtariff
  rdf:type maeco:Tariff ;
  rdfs:isDefinedBy <http://eds.topbraidlive.org/1.0/taxonomy/maeco> ;
  rdfs:isDefinedBy <http://eds.topbraidlive.org/taxonomy/maeco> ;
  rdfs:label "MFN tariff" ;
  skos:altLabel "MFN rate" ;
  skos:broader maecot:Tariff ;
  skos:definition "The tariff level that a member of the <a href='http://edg.topbraid.solutions/maeco/term/Gatt'>GATT</a> / <a href='http://edg.topbraid.solutions/maeco/term/Wto'>WTO</a> charges on a good to other members." ;
  skos:prefLabel "MFN tariff" ;
.
maecot:MadeToMeasureTariff
  rdf:type maeco:Tariff ;
  rdfs:isDefinedBy <http://eds.topbraidlive.org/1.0/taxonomy/maeco> ;
  rdfs:isDefinedBy <http://eds.topbraidlive.org/taxonomy/maeco> ;
  rdfs:label "Made-to-measure tariff" ;
  skos:broader maecot:Tariff ;
  skos:definition "A tariff set so as to raise the price of an imported good to the level of the domestic price, so as to leave domestic producers unaffected.  Also called a <a href='http://edg.topbraid.solutions/maeco/term/ScientificTariff'>scientific tariff</a> ." ;
  skos:prefLabel "Made-To-Measure Tariff" ;
.
maecot:Margin
  rdf:type maeco:QuantityKind ;
  dcterms:source "http://www.isda.org/c_and_a/oper_commit-dcg-glossary.html"^^xsd:anyURI ;
  rdfs:isDefinedBy <http://eds.topbraidlive.org/1.0/taxonomy/maeco> ;
  rdfs:isDefinedBy <http://eds.topbraidlive.org/taxonomy/maeco> ;
  rdfs:label "Margin" ;
  skos:broader maecot:ANY_QuantityKind ;
  skos:definition "<STRONG>1.</STRONG> The edge.  In economics it usually refers to the last (in terms of quantity, not of time) unit consumed or produced by a consumer or firm.  <STRONG>2.</STRONG> A gap between one number and another, such as a <a href='http://edg.topbraid.solutions/maeco/term/DumpingMargin'>dumping margin</a> or <a href='http://edg.topbraid.solutions/maeco/term/InjuryMargin'>injury margin</a> ." ;
  skos:definition "The sum of money which must be deposited, and maintained, in order to provide protection against default by a counterparty to a trade."@en ;
  skos:prefLabel "Margin"@en ;
.
maecot:MarginalCost
  rdf:type maeco:Cost ;
  dcterms:source "http://www.wwnorton.com/college/econ/stec4/macroeconomics/glossary.asp"^^xsd:anyURI ;
  rdfs:isDefinedBy <http://eds.topbraidlive.org/1.0/taxonomy/maeco> ;
  rdfs:isDefinedBy <http://eds.topbraidlive.org/taxonomy/maeco> ;
  rdfs:label "marginal cost" ;
  skos:broader maecot:ANY_Cost ;
  skos:definition "<STRONG>Marginal Cost</STRONG> - the additional cost corresponding to an additional unit of output produced. <STRONG>1.</STRONG> The increase in cost that accompanies a unit increase in output  <STRONG>2.</STRONG> The partial derivative of a <a href='http://edg.topbraid.solutions/maeco/term/CostFunction'>cost function</a> with respect to output." ;
  skos:prefLabel "Marginal Cost" ;
.
maecot:MarginalSocialCost
  rdf:type maeco:Cost ;
  dcterms:source "http://www.wwnorton.com/college/econ/stec4/macroeconomics/glossary.asp"^^xsd:anyURI ;
  rdfs:isDefinedBy <http://eds.topbraidlive.org/1.0/taxonomy/maeco> ;
  rdfs:isDefinedBy <http://eds.topbraidlive.org/taxonomy/maeco> ;
  rdfs:label "Marginal social cost" ;
  skos:altLabel "social marginal cost" ;
  skos:broader maecot:MarginalCost ;
  skos:definition "The <a href='http://edg.topbraid.solutions/maeco/term/MarginalCost'>marginal cost</a> of an activity, such as producing an additional unit of a good, where cost here includes all negative effects on society as a whole, such as <a href='http://edg.topbraid.solutions/maeco/term/NegativeExternality'>negative externalities</a> , not just the cost borne by the producer of the good. <a href='http://edg.topbraid.solutions/maeco/term/PositiveExternality'>Positive externalities</a> should also be deducted. <STRONG>Social Marginal Cost</STRONG> - the marginal cost of production, including the cost of any negative externality, such as air pollution, borne by individuals in the economy other than the producer" ;
  skos:prefLabel "Marginal social cost" ;
.
maecot:MarginalTaxRate
  rdf:type maeco:Rate ;
  dcterms:source "http://www.wwnorton.com/college/econ/stec4/macroeconomics/glossary.asp"^^xsd:anyURI ;
  rdfs:isDefinedBy <http://eds.topbraidlive.org/1.0/taxonomy/maeco> ;
  rdfs:isDefinedBy <http://eds.topbraidlive.org/taxonomy/maeco> ;
  rdfs:label "marginal tax rate" ;
  skos:broader maecot:ANY_Rate ;
  skos:definition "<STRONG>Marginal Tax Rate</STRONG> - the extra tax that will have to be paid as a result of an additional dollar of income. The amount that a taxpayer's total tax bill rises due to a one-unit increase in the activity being taxed.  Referring to an <a href='http://edg.topbraid.solutions/maeco/term/IncomeTax'>income tax</a> , it is the tax on an additional dollar of income.  Contrasts with <a href='http://edg.topbraid.solutions/maeco/term/AverageTaxRate'>average tax rate</a> ." ;
  skos:prefLabel "Marginal Tax Rate" ;
.
maecot:MarketCapitalization
  rdf:type maeco:QuantityKind ;
  rdfs:isDefinedBy <http://eds.topbraidlive.org/1.0/taxonomy/maeco> ;
  rdfs:isDefinedBy <http://eds.topbraidlive.org/taxonomy/maeco> ;
  rdfs:label "Market capitalization" ;
  skos:broader maecot:ANY_QuantityKind ;
  skos:definition "The stock-market value of a company, as measured by the number of shares outstanding times their market price." ;
  skos:prefLabel "Market Capitalization" ;
.
maecot:MarketClearingPrice
  rdf:type maeco:Price ;
  dcterms:source "http://www.wwnorton.com/college/econ/stec4/macroeconomics/glossary.asp"^^xsd:anyURI ;
  rdfs:isDefinedBy <http://eds.topbraidlive.org/1.0/taxonomy/maeco> ;
  rdfs:isDefinedBy <http://eds.topbraidlive.org/taxonomy/maeco> ;
  rdfs:label "market clearing price" ;
  skos:broader maecot:Price ;
  skos:definition "<STRONG>Market Clearing Price</STRONG> - the price at which supply equals demand, so there is neither excess supply nor excess demand" ;
  skos:prefLabel "Market Clearing Price" ;
.
maecot:MarketPrice
  rdf:type maeco:Price ;
  rdfs:isDefinedBy <http://eds.topbraidlive.org/1.0/taxonomy/maeco> ;
  rdfs:isDefinedBy <http://eds.topbraidlive.org/taxonomy/maeco> ;
  rdfs:label "Market price" ;
  skos:broader maecot:Price ;
  skos:definition "<STRONG>1.</STRONG> The price at which a <a href='http://edg.topbraid.solutions/maeco/term/Market'>market</a> <a href='http://edg.topbraid.solutions/maeco/term/Clear'>clears</a> .  <STRONG>2.</STRONG> Alternative to <a href='http://edg.topbraid.solutions/maeco/term/FactorCost'>factor cost</a> ." ;
  skos:prefLabel "Market Price" ;
.
maecot:MarketRate
  rdf:type maeco:Rate ;
  rdfs:isDefinedBy <http://eds.topbraidlive.org/1.0/taxonomy/maeco> ;
  rdfs:isDefinedBy <http://eds.topbraidlive.org/taxonomy/maeco> ;
  rdfs:label "Market rate" ;
  skos:broader maecot:ANY_Rate ;
  skos:definition "The <a href='http://edg.topbraid.solutions/maeco/term/InterestRate'>interest rate</a> or <a href='http://edg.topbraid.solutions/maeco/term/ExchangeRate'>exchange rate</a> at which a <a href='http://edg.topbraid.solutions/maeco/term/Market'>market</a> <a href='http://edg.topbraid.solutions/maeco/term/Clear'>clears</a> ." ;
  skos:prefLabel "Market Rate" ;
.
maecot:MarketRiskMeasures
  rdf:type maeco:RiskMeasure ;
  rdfs:isDefinedBy <http://eds.topbraidlive.org/1.0/taxonomy/maeco> ;
  rdfs:isDefinedBy <http://eds.topbraidlive.org/taxonomy/maeco> ;
  rdfs:label "Market Risk Measures" ;
  skos:prefLabel "Market risk measures"@en ;
.
maecot:MarketToBook
  rdf:type maeco:QuantityKind ;
  rdfs:isDefinedBy <http://eds.topbraidlive.org/1.0/taxonomy/maeco> ;
  rdfs:isDefinedBy <http://eds.topbraidlive.org/taxonomy/maeco> ;
  rdfs:label "Market to Book" ;
  skos:broader maecot:ANY_QuantityKind ;
  skos:definition "Market to Book is ... " ;
  skos:prefLabel "Market To Book" ;
.
maecot:MarketToMarketValue
  rdf:type maeco:QuantityKind ;
  dcterms:source "http://www.cftc.gov/LawRegulation/DoddFrankAct/index.htm"^^xsd:anyURI ;
  rdfs:isDefinedBy <http://eds.topbraidlive.org/1.0/taxonomy/maeco> ;
  rdfs:isDefinedBy <http://eds.topbraidlive.org/taxonomy/maeco> ;
  rdfs:label "Market To Market Value" ;
  skos:altLabel "MTM" ;
  skos:broader maecot:ANY_QuantityKind ;
  skos:definition "Mark-to-market. In relation to swaps, this is shorthand for the value of a transaction. Under the CFTC's regulations, an SD may be required to provide the mid-market mark of certain swaps both before execution and on a daily basis thereafter."@en ;
  skos:prefLabel "Mark-to-market"@en ;
.
maecot:MaterialRiskClasses
  rdf:type maeco:RiskMeasure ;
  rdfs:isDefinedBy <http://eds.topbraidlive.org/1.0/taxonomy/maeco> ;
  rdfs:isDefinedBy <http://eds.topbraidlive.org/taxonomy/maeco> ;
  rdfs:label "Material Risk Classes" ;
  skos:prefLabel "Material risk classes"@en ;
.
maecot:MaximumRevenueTariff
  rdf:type maeco:Tariff ;
  rdfs:isDefinedBy <http://eds.topbraidlive.org/1.0/taxonomy/maeco> ;
  rdfs:isDefinedBy <http://eds.topbraidlive.org/taxonomy/maeco> ;
  rdfs:label "Maximum revenue tariff" ;
  skos:broader maecot:Tariff ;
  skos:definition "A tariff set to collect the largest possible revenue for the government." ;
  skos:prefLabel "Maximum Revenue Tariff" ;
.
maecot:MinimumCapital
  rdf:type maeco:QuantityKind ;
  rdfs:isDefinedBy <http://eds.topbraidlive.org/1.0/taxonomy/maeco> ;
  rdfs:isDefinedBy <http://eds.topbraidlive.org/taxonomy/maeco> ;
  rdfs:label "Minimum Capital" ;
  skos:broader maecot:Capital ;
  skos:prefLabel "Minimum capital"@en ;
.
maecot:MinimumImportPrice
  rdf:type maeco:Price ;
  rdfs:isDefinedBy <http://eds.topbraidlive.org/1.0/taxonomy/maeco> ;
  rdfs:isDefinedBy <http://eds.topbraidlive.org/taxonomy/maeco> ;
  rdfs:label "Minimum import price" ;
  skos:broader maecot:Price ;
  skos:definition "See <a href='http://edg.topbraid.solutions/maeco/term/MinimumPriceSystem'>minimum price system</a> ." ;
  skos:prefLabel "Minimum Import Price" ;
.
maecot:MinimumReserveRequirement
  rdf:type maeco:Reserves ;
  rdfs:isDefinedBy <http://eds.topbraidlive.org/1.0/taxonomy/maeco> ;
  rdfs:isDefinedBy <http://eds.topbraidlive.org/taxonomy/maeco> ;
  rdfs:label "Minimum Reserve Requirement" ;
  skos:broader maecot:ReserveRequirement ;
  skos:prefLabel "Minimum Reserve Requirement"@us ;
.
maecot:MinimumRiskWeight
  rdf:type maeco:RiskMeasure ;
  rdfs:isDefinedBy <http://eds.topbraidlive.org/1.0/taxonomy/maeco> ;
  rdfs:isDefinedBy <http://eds.topbraidlive.org/taxonomy/maeco> ;
  rdfs:label "Minimum Risk Weight" ;
  skos:broader maecot:RiskWeightingFactor ;
  skos:prefLabel "Minimum risk weight"@en ;
.
maecot:MinimumTransferAmount
  rdf:type maeco:QuantityKind ;
  dcterms:source "http://www.isda.org/c_and_a/oper_commit-dcg-glossary.html"^^xsd:anyURI ;
  rdfs:isDefinedBy <http://eds.topbraidlive.org/1.0/taxonomy/maeco> ;
  rdfs:isDefinedBy <http://eds.topbraidlive.org/taxonomy/maeco> ;
  rdfs:label "Minimum Transfer Amount" ;
  skos:definition "A de minimis amount specified in a collateral agreement.  It is designed to avoid the movement of insignificant collateral balances."@en ;
  skos:prefLabel "Minimum transfer amount"@en ;
.
maecot:MixedTariff
  rdf:type maeco:Tariff ;
  rdfs:isDefinedBy <http://eds.topbraidlive.org/1.0/taxonomy/maeco> ;
  rdfs:isDefinedBy <http://eds.topbraidlive.org/taxonomy/maeco> ;
  rdfs:label "Mixed tariff" ;
  skos:broader maecot:Tariff ;
  skos:definition "<a href='http://edg.topbraid.solutions/maeco/term/CompoundTariff'>Compound tariff</a>" ;
  skos:prefLabel "Mixed Tariff" ;
.
maecot:MoneyDemand
  rdf:type maeco:Demand ;
  rdfs:isDefinedBy <http://eds.topbraidlive.org/1.0/taxonomy/maeco> ;
  rdfs:isDefinedBy <http://eds.topbraidlive.org/taxonomy/maeco> ;
  rdfs:label "Money Demand" ;
  skos:broader maecot:ANY_Demand ;
  skos:prefLabel "Money Demand" ;
.
maecot:MoneyPrice
  rdf:type maeco:Price ;
  rdfs:isDefinedBy <http://eds.topbraidlive.org/1.0/taxonomy/maeco> ;
  rdfs:isDefinedBy <http://eds.topbraidlive.org/taxonomy/maeco> ;
  rdfs:label "Money price" ;
  skos:broader maecot:Price ;
  skos:definition "The <a href='http://edg.topbraid.solutions/maeco/term/Nominal'>nominal</a> price; thus the price as it would actually be observed, in <a href='http://edg.topbraid.solutions/maeco/term/CurrentDollars'>current dollars</a> .  Contrasts with the <a href='http://edg.topbraid.solutions/maeco/term/Real'>real</a> price, which is adjusted for inflation." ;
  skos:prefLabel "Money Price" ;
.
maecot:MoneySupply
  rdf:type maeco:Supply ;
  rdfs:isDefinedBy <http://eds.topbraidlive.org/1.0/taxonomy/maeco> ;
  rdfs:isDefinedBy <http://eds.topbraidlive.org/taxonomy/maeco> ;
  rdfs:label "Money supply" ;
  skos:definition "There are several formal definitions, such as <a href='http://edg.topbraid.solutions/maeco/term/M1'>M1</a> and <a href='http://edg.topbraid.solutions/maeco/term/M2'>M2</a> , but all include the quantity of currency in circulation plus the amount of <a href='http://edg.topbraid.solutions/maeco/term/DemandDeposit'>demand deposits</a> .  The money supply, together with the amount of real economic activity in a country, is an important determinant of its price level and its <a href='http://edg.topbraid.solutions/maeco/term/ExchangeRate'>exchange rate</a> ." ;
  skos:prefLabel "Money Supply" ;
.
maecot:MonopolyPrice
  rdf:type maeco:Price ;
  rdfs:isDefinedBy <http://eds.topbraidlive.org/1.0/taxonomy/maeco> ;
  rdfs:isDefinedBy <http://eds.topbraidlive.org/taxonomy/maeco> ;
  rdfs:label "Monopoly price" ;
  skos:broader maecot:Price ;
  skos:definition "The <a href='http://edg.topbraid.solutions/maeco/term/Profit'>profit</a> -maximizing price charged by a <a href='http://edg.topbraid.solutions/maeco/term/Monopoly'>monopolist</a> .  Because a monopoly faces a <a href='http://edg.topbraid.solutions/maeco/term/DemandElasticity'>demand elasticity</a> , &eta;>0, that is finite, this price exceeds marginal cost. The optimal markup over marginal cost is ( <em>P&minus;MC</em> )/ <em>P</em> =1/&eta;." ;
  skos:prefLabel "Monopoly Price" ;
.
maecot:MortgageInsurancePremium
  rdf:type maeco:QuantityKind ;
  dcterms:source "http://www.cftc.gov/LawRegulation/DoddFrankAct/index.htm"^^xsd:anyURI ;
  rdfs:isDefinedBy <http://eds.topbraidlive.org/1.0/taxonomy/maeco> ;
  rdfs:isDefinedBy <http://eds.topbraidlive.org/taxonomy/maeco> ;
  rdfs:label "Mortgage Insurance Premium" ;
  skos:altLabel "MIP" ;
  skos:broader maecot:ANY_Premium ;
  skos:definition "Mortgage insurance premium."@en ;
  skos:prefLabel "Mortgage Insurance Premium"@en ;
.
maecot:NetAssetValue
  rdf:type maeco:QuantityKind ;
  dcterms:source "http://www.cftc.gov/LawRegulation/DoddFrankAct/index.htm"^^xsd:anyURI ;
  rdfs:isDefinedBy <http://eds.topbraidlive.org/1.0/taxonomy/maeco> ;
  rdfs:isDefinedBy <http://eds.topbraidlive.org/taxonomy/maeco> ;
  rdfs:label "Net asset value" ;
  skos:altLabel "NAV" ;
  skos:broader maecot:ANY_QuantityKind ;
  skos:definition "Net asset value. The price per share of an investment company or other pooled investment vehicle, calculated by dividing the total value of the fund's portfolio (less liabilities) by the number of shares outstanding."@en ;
  skos:definition "Value of assets minus liabilities." ;
  skos:prefLabel "Net asset value"@en ;
.
maecot:NetFinancingCost
  rdf:type maeco:QuantityKind ;
  dcterms:source "http://www.isda.org/c_and_a/oper_commit-dcg-glossary.html"^^xsd:anyURI ;
  rdfs:isDefinedBy <http://eds.topbraidlive.org/1.0/taxonomy/maeco> ;
  rdfs:isDefinedBy <http://eds.topbraidlive.org/taxonomy/maeco> ;
  rdfs:label "Net Financing Cost" ;
  skos:altLabel "Carry"@en ;
  skos:broader maecot:ANY_QuantityKind ;
  skos:definition "The difference between the cost of financing the purchase of an asset and the cash yield of the asset. Positive carry means that the yield earned is greater than the financing cost; negative carry means that the financing cost exceeds the yield earned."@en ;
  skos:prefLabel "Net financing cost"@en ;
.
maecot:NetOperatingLoss
  rdf:type maeco:QuantityKind ;
  dcterms:source "http://www.cftc.gov/LawRegulation/DoddFrankAct/index.htm"^^xsd:anyURI ;
  rdfs:isDefinedBy <http://eds.topbraidlive.org/1.0/taxonomy/maeco> ;
  rdfs:isDefinedBy <http://eds.topbraidlive.org/taxonomy/maeco> ;
  rdfs:label "Net Operating Loss" ;
  skos:altLabel "NOL" ;
  skos:broader maecot:ANY_QuantityKind ;
  skos:definition "Occurs when a company's allowable tax deductions are greater than its taxable income, resulting in a negative taxable income. This generally occurs when a company has incurred more expenses than revenues during the period. The net operating loss for the company can generally be used to recover past tax payments or reduce future tax payments. The reasoning behind this is that because corporations are required to pay taxes when they earn money, they also deserve some form of tax relief when they lose money."@en ;
  skos:prefLabel "Net operating loss"@en ;
.
maecot:NetStableFundingRatio
  rdf:type maeco:Ratio ;
  dcterms:source "http://www.cftc.gov/LawRegulation/DoddFrankAct/index.htm"^^xsd:anyURI ;
  rdfs:isDefinedBy <http://eds.topbraidlive.org/1.0/taxonomy/maeco> ;
  rdfs:isDefinedBy <http://eds.topbraidlive.org/taxonomy/maeco> ;
  rdfs:label "Net Stable Funding Ratio" ;
  skos:altLabel "NSFR" ;
  skos:broader maecot:ANY_Ratio ;
  skos:definition "Net Stable Funding Ratio (or Requirement). The NSFR is another liquidity tool introduced as part of the Basel III framework to assess medium- and long-term liquidity by ensuring that a bank has access to long-term funding sufficient to match long-term assets."@en ;
  skos:prefLabel "Net Stable Funding Ratio (or Requirement)."@en ;
.
maecot:NominalExchangeRate
  rdf:type maeco:Rate ;
  rdfs:isDefinedBy <http://eds.topbraidlive.org/1.0/taxonomy/maeco> ;
  rdfs:isDefinedBy <http://eds.topbraidlive.org/taxonomy/maeco> ;
  rdfs:label "Nominal exchange rate" ;
  skos:broader maecot:ANY_Rate ;
  skos:definition "The actual <a href='http://edg.topbraid.solutions/maeco/term/ExchangeRate'>exchange rate</a> at which currencies are exchanged on an <a href='http://edg.topbraid.solutions/maeco/term/ExchangeMarket'>exchange market</a> .  Contrasts with <a href='http://edg.topbraid.solutions/maeco/term/RealExchangeRate'>real exchange rate</a> ." ;
  skos:prefLabel "Nominal Exchange Rate" ;
.
maecot:NominalInterestRate
  rdf:type maeco:Rate ;
  rdfs:isDefinedBy <http://eds.topbraidlive.org/1.0/taxonomy/maeco> ;
  rdfs:isDefinedBy <http://eds.topbraidlive.org/taxonomy/maeco> ;
  rdfs:label "Nominal interest rate" ;
  skos:broader maecot:ANY_Rate ;
  skos:definition "The <a href='http://edg.topbraid.solutions/maeco/term/InterestRate'>interest rate</a> actually observed in the market, in contrast to the <a href='http://edg.topbraid.solutions/maeco/term/RealInterestRate'>real interest rate</a> ." ;
  skos:prefLabel "Nominal Interest Rate" ;
.
maecot:NominalPrice
  rdf:type maeco:Price ;
  rdfs:isDefinedBy <http://eds.topbraidlive.org/1.0/taxonomy/maeco> ;
  rdfs:isDefinedBy <http://eds.topbraidlive.org/taxonomy/maeco> ;
  rdfs:label "Nominal price" ;
  skos:broader maecot:Price ;
  skos:definition "The the price as it would actually be observed, in <a href='http://edg.topbraid.solutions/maeco/term/CurrentDollars'>current dollars</a> .  Contrasts with the <a href='http://edg.topbraid.solutions/maeco/term/Real'>real</a> price, which is adjusted for inflation." ;
  skos:prefLabel "Nominal Price" ;
.
maecot:NominalTariff
  rdf:type maeco:Tariff ;
  rdfs:isDefinedBy <http://eds.topbraidlive.org/1.0/taxonomy/maeco> ;
  rdfs:isDefinedBy <http://eds.topbraidlive.org/taxonomy/maeco> ;
  rdfs:label "Nominal tariff" ;
  skos:broader maecot:Tariff ;
  skos:definition "The <a href='http://edg.topbraid.solutions/maeco/term/NominalRateOfProtection'>nominal protection</a> provided by a tariff; that is, the tariff itself.  Contrasts with <a href='http://edg.topbraid.solutions/maeco/term/EffectiveTariff'>effective tariff</a> ." ;
  skos:prefLabel "Nominal Tariff" ;
.
maecot:NonActionableSubsidy
  rdf:type maeco:Subsidy ;
  rdfs:isDefinedBy <http://eds.topbraidlive.org/1.0/taxonomy/maeco> ;
  rdfs:isDefinedBy <http://eds.topbraidlive.org/taxonomy/maeco> ;
  rdfs:label "Non-actionable subsidy" ;
  skos:broader maecot:Subsidy ;
  skos:definition "A <a href='http://edg.topbraid.solutions/maeco/term/Subsidy'>subsidy</a> that is not subject to <a href='http://edg.topbraid.solutions/maeco/term/Cvd2'>countervailing duties</a> under the rules of the <a href='http://edg.topbraid.solutions/maeco/term/WTO'>WTO</a> .  These include <a href='http://edg.topbraid.solutions/maeco/term/NonspecificSubsidy'>non-specific subsidies</a> , subsidies for industrial research, <a href='http://edg.topbraid.solutions/maeco/term/RegionalAid'>regional aids</a> , and some <a href='http://edg.topbraid.solutions/maeco/term/EnvironmentalSubsidy'>environmental subsidies</a> ." ;
  skos:prefLabel "Non-Actionable Subsidy" ;
.
maecot:NonSpecificSubsidy
  rdf:type maeco:Subsidy ;
  rdfs:isDefinedBy <http://eds.topbraidlive.org/1.0/taxonomy/maeco> ;
  rdfs:isDefinedBy <http://eds.topbraidlive.org/taxonomy/maeco> ;
  rdfs:label "Non-specific subsidy" ;
  skos:broader maecot:Subsidy ;
  skos:definition "A <a href='http://edg.topbraid.solutions/maeco/term/Subsidy'>subsidy</a> that is available to more than a single specific industry and is therefore <a href='http://edg.topbraid.solutions/maeco/term/NonactionableSubsidy'>non-actionable</a> under <a href='http://edg.topbraid.solutions/maeco/term/Wto'>WTO</a> rules." ;
  skos:prefLabel "Non-Specific Subsidy" ;
.
maecot:NonprohibitiveTariff
  rdf:type maeco:Tariff ;
  rdfs:isDefinedBy <http://eds.topbraidlive.org/1.0/taxonomy/maeco> ;
  rdfs:isDefinedBy <http://eds.topbraidlive.org/taxonomy/maeco> ;
  rdfs:label "Nonprohibitive tariff" ;
  skos:broader maecot:Tariff ;
  skos:definition "A <a href='http://edg.topbraid.solutions/maeco/term/Tariff'>tariff</a> that is not <a href='http://edg.topbraid.solutions/maeco/term/ProhibitiveTariff'>prohibitive</a> ." ;
  skos:prefLabel "Nonprohibitive Tariff" ;
.
maecot:NotationalAmount
  rdf:type maeco:QuantityKind ;
  dcterms:source "http://www.isda.org/c_and_a/oper_commit-dcg-glossary.html"^^xsd:anyURI ;
  rdfs:isDefinedBy <http://eds.topbraidlive.org/1.0/taxonomy/maeco> ;
  rdfs:isDefinedBy <http://eds.topbraidlive.org/taxonomy/maeco> ;
  rdfs:label "Notational Amount" ;
  skos:broader maecot:ANY_QuantityKind ;
  skos:definition "The amount of principal underlying the derivative contract, to which interest rates are applied in order to calculate periodic payment obligations."@en ;
  skos:prefLabel "Notional amount"@en ;
.
maecot:NumberOfAnalysts
  rdf:type maeco:QuantityKind ;
  rdfs:isDefinedBy <http://eds.topbraidlive.org/1.0/taxonomy/maeco> ;
  rdfs:isDefinedBy <http://eds.topbraidlive.org/taxonomy/maeco> ;
  rdfs:label "Number of Analysts" ;
  skos:broader maecot:ANY_QuantityKind ;
  skos:prefLabel "Number Of Analysts" ;
.
maecot:OfferAskPrice
  rdf:type maeco:QuantityKind ;
  dcterms:source "http://www.isda.org/c_and_a/oper_commit-dcg-glossary.html"^^xsd:anyURI ;
  rdfs:isDefinedBy <http://eds.topbraidlive.org/1.0/taxonomy/maeco> ;
  rdfs:isDefinedBy <http://eds.topbraidlive.org/taxonomy/maeco> ;
  rdfs:label "Offer Ask Price" ;
  skos:broader maecot:ANY_QuantityKind ;
  skos:definition "The price at which a trader or market maker is willing to sell a contract."@en ;
  skos:prefLabel "Offer/ask price"@en ;
.
maecot:OfficialRate
  rdf:type maeco:Rate ;
  rdfs:isDefinedBy <http://eds.topbraidlive.org/1.0/taxonomy/maeco> ;
  rdfs:isDefinedBy <http://eds.topbraidlive.org/taxonomy/maeco> ;
  rdfs:label "Official rate" ;
  skos:broader maecot:ANY_Rate ;
  skos:definition "The <a href='http://edg.topbraid.solutions/maeco/term/ParValue'>par value</a> of a <a href='http://edg.topbraid.solutions/maeco/term/PeggedExchangeRate'>pegged exchange rate</a> ." ;
  skos:prefLabel "Official Rate" ;
.
maecot:OpportunityCost
  rdf:type maeco:Cost ;
  dcterms:source "http://www.wwnorton.com/college/econ/stec4/macroeconomics/glossary.asp"^^xsd:anyURI ;
  rdfs:isDefinedBy <http://eds.topbraidlive.org/1.0/taxonomy/maeco> ;
  rdfs:isDefinedBy <http://eds.topbraidlive.org/taxonomy/maeco> ;
  rdfs:label "opportunity cost" ;
  skos:broader maecot:ANY_Cost ;
  skos:definition "<STRONG>Opportunity Cost</STRONG> - the cost of a resource, measured by the value of the next-best, alternative use of that resource. The cost of something in terms of opportunity foregone.  The opportunity cost to a country of producing a unit more of a good, such as for export or to replace an import, is the quantity of some other good that could have been produced instead with the same resources." ;
  skos:prefLabel "Opportunity Cost" ;
.
maecot:OptimalTariff
  rdf:type maeco:Tariff ;
  rdfs:isDefinedBy <http://eds.topbraidlive.org/1.0/taxonomy/maeco> ;
  rdfs:isDefinedBy <http://eds.topbraidlive.org/taxonomy/maeco> ;
  rdfs:label "Optimal tariff" ;
  skos:broader maecot:Tariff ;
  skos:definition "The level of a <a href='http://edg.topbraid.solutions/maeco/term/Tariff'>tariff</a> that maximizes a country's <a href='http://edg.topbraid.solutions/maeco/term/Welfare'>welfare</a> .  In a <a href='http://edg.topbraid.solutions/maeco/term/Nondistorted'>nondistorted</a> <a href='http://edg.topbraid.solutions/maeco/term/Soe2'>small open economy</a> , the optimal tariff is zero.  In a <a href='http://edg.topbraid.solutions/maeco/term/LargeCountry'>large country</a> it is positive, due to its effect on the <a href='http://edg.topbraid.solutions/maeco/term/Tot2'>terms of trade</a> ." ;
  skos:prefLabel "Optimal Tariff" ;
.
maecot:OptimumTariff
  rdf:type maeco:Tariff ;
  rdfs:isDefinedBy <http://eds.topbraidlive.org/1.0/taxonomy/maeco> ;
  rdfs:isDefinedBy <http://eds.topbraidlive.org/taxonomy/maeco> ;
  rdfs:label "Optimum tariff" ;
  skos:broader maecot:Tariff ;
  skos:definition "<a href='http://edg.topbraid.solutions/maeco/term/OptimalTariff'>Optimal tariff</a>" ;
  skos:prefLabel "Optimum Tariff" ;
.
maecot:OverallAverageRiskWeight
  rdf:type maeco:RiskMeasure ;
  rdfs:isDefinedBy <http://eds.topbraidlive.org/1.0/taxonomy/maeco> ;
  rdfs:isDefinedBy <http://eds.topbraidlive.org/taxonomy/maeco> ;
  rdfs:label "Overall Average Risk Weight" ;
  skos:broader maecot:RiskWeightingFactor ;
  skos:prefLabel "Overall average risk weight"@en ;
.
maecot:OverallDensity
  rdf:type maeco:QuantityKind ;
  rdfs:isDefinedBy <http://eds.topbraidlive.org/1.0/taxonomy/maeco> ;
  rdfs:isDefinedBy <http://eds.topbraidlive.org/taxonomy/maeco> ;
  rdfs:label "Overall Density" ;
  skos:prefLabel "Overall density"@en ;
.
maecot:OverallVariation
  rdf:type maeco:QuantityKind ;
  rdfs:isDefinedBy <http://eds.topbraidlive.org/1.0/taxonomy/maeco> ;
  rdfs:isDefinedBy <http://eds.topbraidlive.org/taxonomy/maeco> ;
  rdfs:label "Overall Variation" ;
  skos:prefLabel "Overall variation"@en ;
.
maecot:OvernightReserves
  rdf:type maeco:Reserves ;
  rdfs:isDefinedBy <http://eds.topbraidlive.org/1.0/taxonomy/maeco> ;
  rdfs:isDefinedBy <http://eds.topbraidlive.org/taxonomy/maeco> ;
  rdfs:label "Overnight Reserves" ;
  skos:broader maecot:ANY_Reserves ;
  skos:prefLabel "Overnight Reserves"@us ;
.
maecot:ParValue
  rdf:type maeco:QuantityKind ;
  dcterms:source "http://www.isda.org/c_and_a/oper_commit-dcg-glossary.html"^^xsd:anyURI ;
  rdfs:isDefinedBy <http://eds.topbraidlive.org/1.0/taxonomy/maeco> ;
  rdfs:isDefinedBy <http://eds.topbraidlive.org/taxonomy/maeco> ;
  rdfs:label "Par value" ;
  skos:broader maecot:ANY_QuantityKind ;
  skos:definition "The central value of a <a href='http://edg.topbraid.solutions/maeco/term/PeggedExchangeRate'>pegged exchange rate</a> , around which the actual rate is permitted to fluctuate within set bounds." ;
  skos:definition "The principal amount of a bond. Also known as the face value."@en ;
  skos:prefLabel "Par value"@en ;
.
maecot:ParaTariff
  rdf:type maeco:Tariff ;
  rdfs:isDefinedBy <http://eds.topbraidlive.org/1.0/taxonomy/maeco> ;
  rdfs:isDefinedBy <http://eds.topbraidlive.org/taxonomy/maeco> ;
  rdfs:label "Para-tariff" ;
  skos:broader maecot:Tariff ;
  skos:definition "A charge on an imported good instead of, or in addition to, a <a href='http://edg.topbraid.solutions/maeco/term/Tariff'>tariff</a> ." ;
  skos:prefLabel "Para-Tariff" ;
.
maecot:PartialTermination
  rdf:type maeco:QuantityKind ;
  dcterms:source "http://www.isda.org/c_and_a/oper_commit-dcg-glossary.html"^^xsd:anyURI ;
  rdfs:isDefinedBy <http://eds.topbraidlive.org/1.0/taxonomy/maeco> ;
  rdfs:isDefinedBy <http://eds.topbraidlive.org/taxonomy/maeco> ;
  rdfs:label "Partial Termination" ;
  skos:definition "A reduction in the notional amount of a derivative contract."@en ;
  skos:prefLabel "Partial termination"@en ;
.
maecot:ParticipationRate
  rdf:type maeco:Rate ;
  rdfs:isDefinedBy <http://eds.topbraidlive.org/1.0/taxonomy/maeco> ;
  rdfs:isDefinedBy <http://eds.topbraidlive.org/taxonomy/maeco> ;
  rdfs:label "Participation rate" ;
  skos:broader maecot:ANY_Rate ;
  skos:definition "The fraction of a country's working-age population that is employed or seeking employment." ;
  skos:prefLabel "Participation Rate" ;
.
maecot:PeggedExchangeRate
  rdf:type maeco:Rate ;
  rdfs:isDefinedBy <http://eds.topbraidlive.org/1.0/taxonomy/maeco> ;
  rdfs:isDefinedBy <http://eds.topbraidlive.org/taxonomy/maeco> ;
  rdfs:label "Pegged exchange rate" ;
  skos:broader maecot:ANY_Rate ;
  skos:definition "A regime in which the government or central bank announces an official ( <STRONG>par) value</STRONG> of its currency and then maintains the actual market rate within a narrow band above and below that by means of <a href='http://edg.topbraid.solutions/maeco/term/ExchangeMarketIntervention'>exchange market intervention</a> ." ;
  skos:prefLabel "Pegged Exchange Rate" ;
.
maecot:PoolFactors
  rdf:type maeco:QuantityKind ;
  dcterms:source "http://www.isda.org/c_and_a/oper_commit-dcg-glossary.html"^^xsd:anyURI ;
  rdfs:isDefinedBy <http://eds.topbraidlive.org/1.0/taxonomy/maeco> ;
  rdfs:isDefinedBy <http://eds.topbraidlive.org/taxonomy/maeco> ;
  rdfs:label "Pool Factors" ;
  skos:definition "The current principal balance of a particular asset backed bond outstanding divided by the original issued balance of such bonds expressed as a percentage."@en ;
  skos:prefLabel "Pool factors"@en ;
.
maecot:PortfolioLevel
  rdf:type maeco:QuantityKind ;
  rdfs:isDefinedBy <http://eds.topbraidlive.org/1.0/taxonomy/maeco> ;
  rdfs:isDefinedBy <http://eds.topbraidlive.org/taxonomy/maeco> ;
  rdfs:label "Portfolio Level" ;
  skos:prefLabel "Portfolio level"@en ;
.
maecot:PotentialFutureExposure
  rdf:type maeco:QuantityKind ;
  dcterms:source "http://www.cftc.gov/LawRegulation/DoddFrankAct/index.htm"^^xsd:anyURI ;
  rdfs:isDefinedBy <http://eds.topbraidlive.org/1.0/taxonomy/maeco> ;
  rdfs:isDefinedBy <http://eds.topbraidlive.org/taxonomy/maeco> ;
  rdfs:label "Potential Future Exposure" ;
  skos:altLabel "PFE" ;
  skos:broader maecot:ANY_QuantityKind ;
  skos:definition "Potential future exposure. Under the Basel III Leverage Ratio, banks may be required to calculate their derivative exposures as the replacement cost of the transaction plus an additional charge for PFE. The PFE add-on is calculated by multiplying the notional principal of the transaction by a fixed percentage established by regulators."@en ;
  skos:prefLabel "Potential future exposure"@en ;
.
maecot:PreferentialTariff
  rdf:type maeco:Tariff ;
  rdfs:isDefinedBy <http://eds.topbraidlive.org/1.0/taxonomy/maeco> ;
  rdfs:isDefinedBy <http://eds.topbraidlive.org/taxonomy/maeco> ;
  rdfs:label "Preferential tariff" ;
  skos:broader maecot:Tariff ;
  skos:definition "A <a href='http://edg.topbraid.solutions/maeco/term/Tariff'>tariff</a> lower than the <a href='http://edg.topbraid.solutions/maeco/term/Mfn'>MFN</a> tariff, levied against imports from a country that is being given favored treatment, as in a <a href='http://edg.topbraid.solutions/maeco/term/Pta2'>preferential trading arrangement</a> or under the <a href='http://edg.topbraid.solutions/maeco/term/Gsp'>GSP</a> ." ;
  skos:prefLabel "Preferential Tariff" ;
.
maecot:Premium
  rdf:type maeco:QuantityKind ;
  dcterms:source "http://www.isda.org/c_and_a/oper_commit-dcg-glossary.html"^^xsd:anyURI ;
  rdfs:isDefinedBy <http://eds.topbraidlive.org/1.0/taxonomy/maeco> ;
  rdfs:isDefinedBy <http://eds.topbraidlive.org/taxonomy/maeco> ;
  rdfs:label "Premium" ;
  skos:broader maecot:ANY_QuantityKind ;
  skos:definition "<STRONG>1.</STRONG> The excess of one price over another.  <STRONG>2.</STRONG> <a href='http://edg.topbraid.solutions/maeco/term/ForwardPremium'>Forward premium</a>" ;
  skos:definition "The sum of money paid by the buyer, to the seller, for acquiring the rights inherent in an option. It is the sum of the intrinsic value and the time value of the option. "@en ;
  skos:prefLabel "Premium"@en ;
.
maecot:PresentValue
  rdf:type maeco:QuantityKind ;
  dcterms:source "http://www.isda.org/c_and_a/oper_commit-dcg-glossary.html"^^xsd:anyURI ;
  rdfs:isDefinedBy <http://eds.topbraidlive.org/1.0/taxonomy/maeco> ;
  rdfs:isDefinedBy <http://eds.topbraidlive.org/taxonomy/maeco> ;
  rdfs:label "Present value" ;
  skos:broader maecot:ANY_QuantityKind ;
  skos:definition "The current value of a sum which is to be paid (or received) on a future date. It is calculated as the amount that would have to be invested today at a specified rate for a specified period to obtain a known amount at the end of the period. In effect, it is a method of compounding in reverse. Also called fair value."@en ;
  skos:definition "The value today of a stream of payments and/or receipts over time in the future and/or the past, converted to the present using an interest rate.  If <em>X</em> is the amount in period <em>t</em> and <em>r</em> the interest rate, then present value at time <em>t</em> =0 is <em>V</em> = &Sigma; <MISSED-Sub>???</MISSED-Sub> ( <em>X</em> )/(1+ <em>r</em> ) <MISSED-Sup>???</MISSED-Sup> .  If the interest rate varies with time, it's somewhat harder." ;
  skos:prefLabel "Present value"@en ;
.
maecot:Price
  rdf:type maeco:Price ;
  rdf:type maeco:QuantityKind ;
  dcterms:source "http://www.wwnorton.com/college/econ/stec4/macroeconomics/glossary.asp"^^xsd:anyURI ;
  rdfs:isDefinedBy <http://eds.topbraidlive.org/1.0/taxonomy/maeco> ;
  rdfs:isDefinedBy <http://eds.topbraidlive.org/taxonomy/maeco> ;
  rdfs:label "Price" ;
  skos:broader maecot:ANY_QuantityKind ;
  skos:definition "<STRONG>Price</STRONG> - the price of a good or service is what must be given in exchange for the good." ;
  skos:prefLabel "Price" ;
  skos:prefLabel "Price"@en ;
.
maecot:PriceElasticityOfDemand
  rdf:type maeco:Demand ;
  dcterms:source "http://www.wwnorton.com/college/econ/stec4/macroeconomics/glossary.asp"^^xsd:anyURI ;
  rdfs:isDefinedBy <http://eds.topbraidlive.org/1.0/taxonomy/maeco> ;
  rdfs:isDefinedBy <http://eds.topbraidlive.org/taxonomy/maeco> ;
  rdfs:label "price elasticity of demand" ;
  skos:broader maecot:Price ;
  skos:definition "<STRONG>Price Elasticity Of Demand</STRONG> - the percentage change in quantity demanded of a good as the result of a 1 percent change in price (the percentage change in quantity demanded divided by the percentage change in price)" ;
  skos:prefLabel "Price Elasticity Of Demand" ;
.
maecot:PriceElasticityOfSupply
  rdf:type maeco:Supply ;
  dcterms:source "http://www.wwnorton.com/college/econ/stec4/macroeconomics/glossary.asp"^^xsd:anyURI ;
  rdfs:isDefinedBy <http://eds.topbraidlive.org/1.0/taxonomy/maeco> ;
  rdfs:isDefinedBy <http://eds.topbraidlive.org/taxonomy/maeco> ;
  rdfs:label "price elasticity of supply" ;
  skos:broader maecot:Price ;
  skos:definition "<STRONG>Price Elasticity Of Supply</STRONG> - the percentage change in quantity supplied of a good as the result of a 1 percent change in price (the percentage change in quantity supplied divided by the percentage change in price)" ;
  skos:prefLabel "Price Elasticity Of Supply" ;
.
maecot:PriceRatio
  rdf:type maeco:Ratio ;
  rdfs:isDefinedBy <http://eds.topbraidlive.org/1.0/taxonomy/maeco> ;
  rdfs:isDefinedBy <http://eds.topbraidlive.org/taxonomy/maeco> ;
  rdfs:label "Price Ratio" ;
  skos:broader maecot:ANY_Ratio ;
  skos:prefLabel "Price Ratio" ;
.
maecot:PriceToBook
  rdf:type maeco:Ratio ;
  rdfs:isDefinedBy <http://eds.topbraidlive.org/1.0/taxonomy/maeco> ;
  rdfs:isDefinedBy <http://eds.topbraidlive.org/taxonomy/maeco> ;
  rdfs:label "Price To Book" ;
  skos:altLabel "P/B" ;
  skos:broader maecot:PriceRatio ;
  skos:prefLabel "Price To Book" ;
.
maecot:PriceToCashFlow
  rdf:type maeco:Ratio ;
  rdfs:isDefinedBy <http://eds.topbraidlive.org/1.0/taxonomy/maeco> ;
  rdfs:isDefinedBy <http://eds.topbraidlive.org/taxonomy/maeco> ;
  rdfs:label "Price To Cash Flow" ;
  skos:altLabel "P/CF" ;
  skos:broader maecot:PriceRatio ;
  skos:prefLabel "Price To Cash Flow" ;
.
maecot:PriceToEarnings
  rdf:type maeco:Ratio ;
  rdfs:isDefinedBy <http://eds.topbraidlive.org/1.0/taxonomy/maeco> ;
  rdfs:isDefinedBy <http://eds.topbraidlive.org/taxonomy/maeco> ;
  rdfs:label "Price To Earnings" ;
  rdfs:seeAlso maecot:EarningsPerShare ;
  skos:altLabel "P/E" ;
  skos:broader maecot:PriceRatio ;
  skos:prefLabel "Price To Earnings" ;
.
maecot:PriceToSales
  rdf:type maeco:Ratio ;
  rdfs:isDefinedBy <http://eds.topbraidlive.org/1.0/taxonomy/maeco> ;
  rdfs:isDefinedBy <http://eds.topbraidlive.org/taxonomy/maeco> ;
  rdfs:label "Price To Sales" ;
  skos:altLabel "P/S" ;
  skos:broader maecot:PriceRatio ;
  skos:prefLabel "Price To Sales" ;
.
maecot:PrimeRate
  rdf:type maeco:Rate ;
  rdfs:isDefinedBy <http://eds.topbraidlive.org/1.0/taxonomy/maeco> ;
  rdfs:isDefinedBy <http://eds.topbraidlive.org/taxonomy/maeco> ;
  rdfs:label "Prime rate" ;
  skos:broader maecot:ANY_Rate ;
  skos:definition "The interest rate that a country's largest banks announce for loans to their best customers.  In practice, their most creditworthy customers get a rate lower than this." ;
  skos:prefLabel "Prime Rate" ;
.
maecot:PrivateCost
  rdf:type maeco:Cost ;
  rdfs:isDefinedBy <http://eds.topbraidlive.org/1.0/taxonomy/maeco> ;
  rdfs:isDefinedBy <http://eds.topbraidlive.org/taxonomy/maeco> ;
  rdfs:label "Private cost" ;
  skos:broader maecot:ANY_Cost ;
  skos:definition "The cost to an individual economic agent, such as a consumer or firm, from an event, action, or policy change.  May differ from the <a href='http://edg.topbraid.solutions/maeco/term/SocialCost'>social cost</a> if there are <a href='http://edg.topbraid.solutions/maeco/term/Externality'>externalities</a> ." ;
  skos:prefLabel "Private Cost" ;
.
maecot:PrivateMarginalCost
  rdf:type maeco:Cost ;
  dcterms:source "http://www.wwnorton.com/college/econ/stec4/macroeconomics/glossary.asp"^^xsd:anyURI ;
  rdfs:isDefinedBy <http://eds.topbraidlive.org/1.0/taxonomy/maeco> ;
  rdfs:isDefinedBy <http://eds.topbraidlive.org/taxonomy/maeco> ;
  rdfs:label "private marginal cost" ;
  skos:broader maecot:MarginalCost ;
  skos:broader maecot:PrivateCost ;
  skos:definition "<STRONG>Private Marginal Cost</STRONG> - the marginal cost of production borne by the producer of a good; when there is a negative externality, such as air pollution, private marginal cost is less than social marginal cost." ;
  skos:prefLabel "Private Marginal Cost" ;
.
maecot:ProhibitedSubsidy
  rdf:type maeco:Subsidy ;
  rdfs:isDefinedBy <http://eds.topbraidlive.org/1.0/taxonomy/maeco> ;
  rdfs:isDefinedBy <http://eds.topbraidlive.org/taxonomy/maeco> ;
  rdfs:label "Prohibited subsidy" ;
  skos:broader maecot:Subsidy ;
  skos:definition "A <a href='http://edg.topbraid.solutions/maeco/term/Subsidy'>subsidy</a> that is forbidden under the rules of the <a href='http://edg.topbraid.solutions/maeco/term/Wto'>WTO</a> .  These include subsidies that are specifically designed to distort international trade, such as <a href='http://edg.topbraid.solutions/maeco/term/ExportSubsidy'>export subsidies</a> or subsidies that require use of domestic rather than imported inputs." ;
  skos:prefLabel "Prohibited Subsidy" ;
.
maecot:ProhibitiveTariff
  rdf:type maeco:Tariff ;
  rdfs:isDefinedBy <http://eds.topbraidlive.org/1.0/taxonomy/maeco> ;
  rdfs:isDefinedBy <http://eds.topbraidlive.org/taxonomy/maeco> ;
  rdfs:label "Prohibitive tariff" ;
  skos:broader maecot:Tariff ;
  skos:definition "A <a href='http://edg.topbraid.solutions/maeco/term/Tariff'>tariff</a> that reduces imports to zero." ;
  skos:prefLabel "Prohibitive Tariff" ;
.
maecot:ProtectiveTariff
  rdf:type maeco:Tariff ;
  rdfs:isDefinedBy <http://eds.topbraidlive.org/1.0/taxonomy/maeco> ;
  rdfs:isDefinedBy <http://eds.topbraidlive.org/taxonomy/maeco> ;
  rdfs:label "Protective tariff" ;
  skos:broader maecot:Tariff ;
  skos:definition "An import <a href='http://edg.topbraid.solutions/maeco/term/Tariff'>tariff</a> with the avowed purpose of providing <a href='http://edg.topbraid.solutions/maeco/term/Protection'>protection</a> .  Since all tariffs, if they have any effect at all, do provide protection, this common expression is really a redundant tautology." ;
  skos:prefLabel "Protective Tariff" ;
.
maecot:PunitiveTariff
  rdf:type maeco:Tariff ;
  rdfs:isDefinedBy <http://eds.topbraidlive.org/1.0/taxonomy/maeco> ;
  rdfs:isDefinedBy <http://eds.topbraidlive.org/taxonomy/maeco> ;
  rdfs:label "Punitive tariff" ;
  skos:broader maecot:Tariff ;
  skos:definition "A high <a href='http://edg.topbraid.solutions/maeco/term/Tariff'>tariff</a> the purpose of which is to inflict harm on a foreign exporting country as punishment for some previous behavior." ;
  skos:prefLabel "Punitive Tariff" ;
.
maecot:PurchasingPowerParityExchangeRate
  rdf:type maeco:Rate ;
  rdfs:isDefinedBy <http://eds.topbraidlive.org/1.0/taxonomy/maeco> ;
  rdfs:isDefinedBy <http://eds.topbraidlive.org/taxonomy/maeco> ;
  rdfs:label "Purchasing power parity exchange rate" ;
  skos:altLabel "PPP exchange rate" ;
  skos:broader maecot:ANY_Rate ;
  skos:definition "An exchange rate, <em>R</em> , calculated to yield absolute <a href='http://edg.topbraid.solutions/maeco/term/Ppp2'>purchasing power parity</a> .  Useful for comparing <a href='http://edg.topbraid.solutions/maeco/term/Real'>real</a> values (wages, GDP) across countries with different currencies.  Since absolute <a href='http://edg.topbraid.solutions/maeco/term/PurchasingPowerParityTheory'>PPP</a> rarely holds, it contrasts with the <a href='http://edg.topbraid.solutions/maeco/term/NominalExchangeRate'>nominal exchange rate</a> , <em>E</em> .  Its calculation is that of the <a href='http://edg.topbraid.solutions/maeco/term/RealExchangeRate'>real exchange rate</a> but with <em>P</em> and <em>P*</em> the domestic and foreign prices of a basket of goods." ;
  skos:prefLabel "Purchasing Power Parity Exchange Rate" ;
.
maecot:QuotaFillRate
  rdf:type maeco:Rate ;
  rdfs:isDefinedBy <http://eds.topbraidlive.org/1.0/taxonomy/maeco> ;
  rdfs:isDefinedBy <http://eds.topbraidlive.org/taxonomy/maeco> ;
  rdfs:label "Quota fill rate" ;
  skos:broader maecot:ANY_Rate ;
  skos:definition "The percentage of an import <a href='http://edg.topbraid.solutions/maeco/term/Quota'>quota</a> that is used." ;
  skos:prefLabel "Quota Fill Rate" ;
.
maecot:RandD
  rdfs:isDefinedBy <http://eds.topbraidlive.org/1.0/taxonomy/maeco> ;
  rdfs:isDefinedBy <http://eds.topbraidlive.org/taxonomy/maeco> ;
  skos:definition "<a href='http://edg.topbraid.solutions/maeco/term/RAndD2'>Research and development</a> ." ;
  skos:prefLabel "R&D" ;
.
maecot:RealEffectiveExchangeRate
  rdf:type maeco:Rate ;
  rdfs:isDefinedBy <http://eds.topbraidlive.org/1.0/taxonomy/maeco> ;
  rdfs:isDefinedBy <http://eds.topbraidlive.org/taxonomy/maeco> ;
  rdfs:label "Real effective exchange rate" ;
  skos:altLabel "REER" ;
  skos:broader maecot:ANY_Rate ;
  skos:broader maecot:ExchangeRate ;
  skos:definition "The <a href='http://edg.topbraid.solutions/maeco/term/EffectiveExchangeRate'>effective exchange rate</a> adjusted for the rates of <a href='http://edg.topbraid.solutions/maeco/term/Inflation'>inflation</a> in each country." ;
  skos:prefLabel "Real effective exchange rate" ;
.
maecot:RealExchangeRate
  rdf:type maeco:Rate ;
  rdfs:isDefinedBy <http://eds.topbraidlive.org/1.0/taxonomy/maeco> ;
  rdfs:isDefinedBy <http://eds.topbraidlive.org/taxonomy/maeco> ;
  rdfs:label "Real exchange rate" ;
  skos:broader maecot:ANY_Rate ;
  skos:definition "<STRONG>1.</STRONG> The <a href='http://edg.topbraid.solutions/maeco/term/NominalExchangeRate'>nominal exchange rate</a> adjusted for inflation.  Unlike other <a href='http://edg.topbraid.solutions/maeco/term/Real'>real</a> variables, this adjustment must account for prices in two currencies.  In a model, the real exchange rate is: <em>R</em> &nbsp;=&nbsp; <em>EP*/P</em> with <em>E</em> the nominal domestic-currency price of foreign currency, <em>P</em> the price of domestic goods, and <em>P*</em> the price of foreign goods.  <STRONG>2.</STRONG> The real price of foreign goods; i.e., the quantity of domestic goods needed to purchase a unit of foreign goods.  Equals the reciprocal of the <a href='http://edg.topbraid.solutions/maeco/term/TermsOfTrade'>terms of trade</a> .  Equivalent to definition 1.  <STRONG>3.</STRONG> The relative price of <a href='http://edg.topbraid.solutions/maeco/term/TradedGood'>traded goods</a> in terms of <a href='http://edg.topbraid.solutions/maeco/term/NontradedGood'>nontraded goods</a> ." ;
  skos:prefLabel "Real Exchange Rate" ;
.
maecot:RealInterestRate
  rdf:type maeco:Rate ;
  rdfs:isDefinedBy <http://eds.topbraidlive.org/1.0/taxonomy/maeco> ;
  rdfs:isDefinedBy <http://eds.topbraidlive.org/taxonomy/maeco> ;
  rdfs:label "Real interest rate" ;
  skos:broader maecot:ANY_Rate ;
  skos:definition "The <a href='http://edg.topbraid.solutions/maeco/term/NominalInterestRate'>nominal interest rate</a> adjusted for <a href='http://edg.topbraid.solutions/maeco/term/Inflation'>inflation</a> , to get the percentage yield an asset holder receives in terms of goods and services.  Equals the nominal interest rate minus the rate of inflation." ;
  skos:prefLabel "Real Interest Rate" ;
.
maecot:RebateAmount
  rdf:type maeco:QuantityKind ;
  dcterms:source "http://www.isda.org/c_and_a/oper_commit-dcg-glossary.html"^^xsd:anyURI ;
  rdfs:isDefinedBy <http://eds.topbraidlive.org/1.0/taxonomy/maeco> ;
  rdfs:isDefinedBy <http://eds.topbraidlive.org/taxonomy/maeco> ;
  rdfs:label "Rebate Amount" ;
  skos:broader maecot:ANY_QuantityKind ;
  skos:definition "The amount paid out in the event of an automatic payment knock-out event occurring."@en ;
  skos:prefLabel "Rebate amount"@en ;
.
maecot:RedundantTariff
  rdf:type maeco:Tariff ;
  rdfs:isDefinedBy <http://eds.topbraidlive.org/1.0/taxonomy/maeco> ;
  rdfs:isDefinedBy <http://eds.topbraidlive.org/taxonomy/maeco> ;
  rdfs:label "Redundant tariff" ;
  skos:broader maecot:Tariff ;
  skos:definition "A tariff that, if changed, will not change the quantity of imports, either because the tariff is <a href='http://edg.topbraid.solutions/maeco/term/ProhibitiveTariff'>prohibitive</a> , or because some other policy such as a <a href='http://edg.topbraid.solutions/maeco/term/Quota'>quota</a> or an <a href='http://edg.topbraid.solutions/maeco/term/Embargo'>embargo</a> is limiting quantity." ;
  skos:prefLabel "Redundant Tariff" ;
.
maecot:ReferencePrice
  rdf:type maeco:Price ;
  rdfs:isDefinedBy <http://eds.topbraidlive.org/1.0/taxonomy/maeco> ;
  rdfs:isDefinedBy <http://eds.topbraidlive.org/taxonomy/maeco> ;
  rdfs:label "Reference price" ;
  skos:broader maecot:Price ;
  skos:definition "See <a href='http://edg.topbraid.solutions/maeco/term/MinimumPriceSystem'>minimum price system</a> ." ;
  skos:prefLabel "Reference Price" ;
.
maecot:RegulatoryAssetsUnderManagement
  rdf:type maeco:QuantityKind ;
  dcterms:source "http://www.cftc.gov/LawRegulation/DoddFrankAct/index.htm"^^xsd:anyURI ;
  rdfs:isDefinedBy <http://eds.topbraidlive.org/1.0/taxonomy/maeco> ;
  rdfs:isDefinedBy <http://eds.topbraidlive.org/taxonomy/maeco> ;
  rdfs:label "Regulatory Assets Under Management" ;
  skos:altLabel "RAUM" ;
  skos:broader maecot:ANY_QuantityKind ;
  skos:definition "Regulatory assets under management. RAUM are the gross assets under management, without subtraction of borrowings, short sales or other forms of leverage. Investment advisers to private funds with more than $150 million in RAUM must register with the SEC."@en ;
  skos:prefLabel "Regulatory assets under management"@en ;
.
maecot:RegulatoryRatio
  rdf:type maeco:Ratio ;
  rdfs:isDefinedBy <http://eds.topbraidlive.org/1.0/taxonomy/maeco> ;
  rdfs:isDefinedBy <http://eds.topbraidlive.org/taxonomy/maeco> ;
  rdfs:label "Regulatory Ratio" ;
  skos:broader maecot:ANY_Ratio ;
  skos:prefLabel "Regulatory ratio"@en ;
.
maecot:RelativeDefaultRisk
  rdf:type maeco:RiskMeasure ;
  rdfs:isDefinedBy <http://eds.topbraidlive.org/1.0/taxonomy/maeco> ;
  rdfs:isDefinedBy <http://eds.topbraidlive.org/taxonomy/maeco> ;
  rdfs:label "Relative Default Risk" ;
  skos:prefLabel "Relative default risk"@en ;
.
maecot:RelativeDemand
  rdf:type maeco:Demand ;
  rdfs:isDefinedBy <http://eds.topbraidlive.org/1.0/taxonomy/maeco> ;
  rdfs:isDefinedBy <http://eds.topbraidlive.org/taxonomy/maeco> ;
  rdfs:label "Relative demand" ;
  skos:definition "The ratio of the demand for one good to the demand for another, most useful in representing general equilibrium in a two-good economy, where relative price adjusts to equate relative supply and relative demand." ;
  skos:prefLabel "Relative Demand" ;
.
maecot:RelativeDeviation
  rdf:type maeco:QuantityKind ;
  rdfs:isDefinedBy <http://eds.topbraidlive.org/1.0/taxonomy/maeco> ;
  rdfs:isDefinedBy <http://eds.topbraidlive.org/taxonomy/maeco> ;
  rdfs:label "Relative Deviation" ;
  skos:broader maecot:ANY_QuantityKind ;
  skos:prefLabel "Relative deviation"@en ;
.
maecot:RelativePrice
  rdf:type maeco:Price ;
  dcterms:source "http://www.wwnorton.com/college/econ/stec4/macroeconomics/glossary.asp"^^xsd:anyURI ;
  rdfs:isDefinedBy <http://eds.topbraidlive.org/1.0/taxonomy/maeco> ;
  rdfs:isDefinedBy <http://eds.topbraidlive.org/taxonomy/maeco> ;
  rdfs:label "relative price" ;
  skos:broader maecot:Price ;
  skos:definition "<STRONG>Relative Price</STRONG> - the ratio of any two prices; the relative price of CDs and DVDs is just the ratio of their prices.. The price of one thing (usually a good) in terms of another; i.e., the ratio of two prices.  The relative price of good <em>X</em> in terms of good <em>Y</em> is <em>&nbsp;/&nbsp;p</em> ." ;
  skos:prefLabel "Relative Price" ;
.
maecot:RelativeSupply
  rdf:type maeco:Supply ;
  rdfs:isDefinedBy <http://eds.topbraidlive.org/1.0/taxonomy/maeco> ;
  rdfs:isDefinedBy <http://eds.topbraidlive.org/taxonomy/maeco> ;
  rdfs:label "Relative supply" ;
  skos:definition "The ratio of the supply of one good to the supply of another, most useful in representing general equilibrium in a two-good economy, where relative price adjusts to equate relative supply and relative demand." ;
  skos:prefLabel "Relative Supply" ;
.
maecot:RentalPrice
  rdf:type maeco:Price ;
  rdfs:isDefinedBy <http://eds.topbraidlive.org/1.0/taxonomy/maeco> ;
  rdfs:isDefinedBy <http://eds.topbraidlive.org/taxonomy/maeco> ;
  rdfs:label "Rental price" ;
  skos:broader maecot:Price ;
  skos:definition "The payment per unit time for the services of a unit of a <a href='http://edg.topbraid.solutions/maeco/term/Factor'>factor of production</a> , such as land or capital." ;
  skos:prefLabel "Rental Price" ;
.
maecot:ReplacementCost
  rdf:type maeco:QuantityKind ;
  dcterms:source "http://www.cftc.gov/LawRegulation/DoddFrankAct/index.htm"^^xsd:anyURI ;
  rdfs:isDefinedBy <http://eds.topbraidlive.org/1.0/taxonomy/maeco> ;
  rdfs:isDefinedBy <http://eds.topbraidlive.org/taxonomy/maeco> ;
  rdfs:label "Replacement Cost" ;
  skos:altLabel "RC" ;
  skos:broader maecot:ANY_QuantityKind ;
  skos:definition "Replacement cost. Usually used in the context of a derivatives exposure, the RC refers to the cost of replacing the derivatives contract."@en ;
  skos:prefLabel "Replacement cost"@en ;
.
maecot:ReserveRequirement
  rdf:type maeco:Reserves ;
  rdfs:isDefinedBy <http://eds.topbraidlive.org/1.0/taxonomy/maeco> ;
  rdfs:isDefinedBy <http://eds.topbraidlive.org/taxonomy/maeco> ;
  rdfs:label "Reserve requirement" ;
  skos:broader maecot:ANY_Reserves ;
  skos:definition "The level of the <a href='http://edg.topbraid.solutions/maeco/term/ReserveRatio'>reserve ratio</a> that a commercial bank is required by government or the central bank to maintain or exceed." ;
  skos:prefLabel "Reserve Requirement"@us ;
.
maecot:RetailDeposits
  rdf:type maeco:QuantityKind ;
  rdfs:isDefinedBy <http://eds.topbraidlive.org/1.0/taxonomy/maeco> ;
  rdfs:isDefinedBy <http://eds.topbraidlive.org/taxonomy/maeco> ;
  rdfs:label "Retail Deposits" ;
  skos:broader maecot:ANY_QuantityKind ;
  skos:definition """Retail deposits are defined as deposits placed with a bank by a natural person. Deposits from legal entities, sole proprietorships or partnerships are captured in wholesale deposit categories. Retail deposits subject to the LCR include demand deposits and term deposits, unless otherwise excluded under the criteria set out in paragraphs 82 and 83 of BCBS238.

These retail deposits are divided into stable and less stable portions of funds as described below, with minimum run-off rates listed for each category. The run-off rates for retail deposits are minimum floors, with higher run-off rates established by individual jurisdictions as appropriate to capture depositor behaviour in a period of stress in each jurisdiction."""@en ;
  skos:prefLabel "Retail Deposits"@en ;
  prov:wasInfluencedBy "<http://www.bis.org/publ/bcbs238.pdf>" ;
.
maecot:RetailRiskWeight
  rdf:type maeco:RiskMeasure ;
  rdfs:isDefinedBy <http://eds.topbraidlive.org/1.0/taxonomy/maeco> ;
  rdfs:isDefinedBy <http://eds.topbraidlive.org/taxonomy/maeco> ;
  rdfs:label "Retail Risk Weight" ;
  skos:broader maecot:RiskWeightingFactor ;
  skos:prefLabel "Retail risk weight"@en ;
.
maecot:RevenueArgumentForATariff
  rdf:type maeco:Tariff ;
  rdfs:isDefinedBy <http://eds.topbraidlive.org/1.0/taxonomy/maeco> ;
  rdfs:isDefinedBy <http://eds.topbraidlive.org/taxonomy/maeco> ;
  rdfs:label "Revenue argument for a tariff" ;
  skos:broader maecot:Tariff ;
  skos:definition "The use of a <a href='http://edg.topbraid.solutions/maeco/term/Tariff'>tariff</a> to raise revenue for the government.  Many other kinds of tax cause smaller distortions and are therefore preferable to tariffs for this purpose.  However, a tariff is one of the easiest taxes to collect, and it is therefore common in the early stages of a country's development." ;
  skos:prefLabel "Revenue Argument For A Tariff" ;
.
maecot:RevenueMaximizingTariff
  rdf:type maeco:Tariff ;
  rdfs:isDefinedBy <http://eds.topbraidlive.org/1.0/taxonomy/maeco> ;
  rdfs:isDefinedBy <http://eds.topbraidlive.org/taxonomy/maeco> ;
  rdfs:label "Revenue-maximizing tariff" ;
  skos:broader maecot:Tariff ;
  skos:definition "The level of <a href='http://edg.topbraid.solutions/maeco/term/Tariff'>tariff</a> that brings in the largest <a href='http://edg.topbraid.solutions/maeco/term/Revenue'>revenue</a> to a government, as opposed to the (usually smaller) <a href='http://edg.topbraid.solutions/maeco/term/OptimalTariff'>optimal tariff</a> ." ;
  skos:prefLabel "Revenue-Maximizing Tariff" ;
.
maecot:RiskBasedCapital
  rdf:type maeco:QuantityKind ;
  dcterms:source "http://www.cftc.gov/LawRegulation/DoddFrankAct/index.htm"^^xsd:anyURI ;
  rdfs:isDefinedBy <http://eds.topbraidlive.org/1.0/taxonomy/maeco> ;
  rdfs:isDefinedBy <http://eds.topbraidlive.org/taxonomy/maeco> ;
  rdfs:label "Risk Based Capital" ;
  skos:altLabel "RBC" ;
  skos:broader maecot:ANY_QuantityKind ;
  skos:definition "Risk-based capital (Also risk-based capital ratio)."@en ;
  skos:prefLabel "Risk-based capital"@en ;
.
maecot:RiskFreeRate
  rdf:type maeco:Rate ;
  rdfs:isDefinedBy <http://eds.topbraidlive.org/1.0/taxonomy/maeco> ;
  rdfs:isDefinedBy <http://eds.topbraidlive.org/taxonomy/maeco> ;
  rdfs:label "Risk-free rate" ;
  skos:broader maecot:ANY_Rate ;
  skos:definition "The <a href='http://edg.topbraid.solutions/maeco/term/InterestRate'>interest rate</a> on a riskless, or safe, asset, usually taken to be a short-term U.S. government security." ;
  skos:prefLabel "Risk-Free Rate" ;
.
maecot:RiskSensitivity
  rdf:type maeco:RiskMeasure ;
  rdfs:isDefinedBy <http://eds.topbraidlive.org/1.0/taxonomy/maeco> ;
  rdfs:isDefinedBy <http://eds.topbraidlive.org/taxonomy/maeco> ;
  rdfs:label "Risk Sensitivity" ;
  skos:prefLabel "Risk sensitivity"@en ;
.
maecot:RiskWeight
  rdf:type maeco:RiskMeasure ;
  rdfs:isDefinedBy <http://eds.topbraidlive.org/1.0/taxonomy/maeco> ;
  rdfs:isDefinedBy <http://eds.topbraidlive.org/taxonomy/maeco> ;
  rdfs:label "Risk Weight" ;
  skos:broader maecot:RiskWeightingFactor ;
  skos:prefLabel "Risk weight"@en ;
.
maecot:RiskWeightDensity
  rdf:type maeco:RiskMeasure ;
  rdfs:isDefinedBy <http://eds.topbraidlive.org/1.0/taxonomy/maeco> ;
  rdfs:isDefinedBy <http://eds.topbraidlive.org/taxonomy/maeco> ;
  rdfs:label "Risk Weight Density" ;
  skos:broader maecot:RiskWeightingFactor ;
  skos:prefLabel "Risk weight density"@en ;
.
maecot:RiskWeightDeviation
  rdf:type maeco:RiskMeasure ;
  rdfs:isDefinedBy <http://eds.topbraidlive.org/1.0/taxonomy/maeco> ;
  rdfs:isDefinedBy <http://eds.topbraidlive.org/taxonomy/maeco> ;
  rdfs:label "Risk Weight Deviation" ;
  skos:broader maecot:RiskWeightingFactor ;
  skos:prefLabel "Risk weight deviation"@en ;
.
maecot:RiskWeightDifferentials
  rdf:type maeco:RiskMeasure ;
  rdfs:isDefinedBy <http://eds.topbraidlive.org/1.0/taxonomy/maeco> ;
  rdfs:isDefinedBy <http://eds.topbraidlive.org/taxonomy/maeco> ;
  rdfs:label "Risk Weight Differentials" ;
  skos:broader maecot:RiskWeightingFactor ;
  skos:prefLabel "Risk weight differentials"@en ;
.
maecot:RiskWeightVariability
  rdf:type maeco:RiskMeasure ;
  rdfs:isDefinedBy <http://eds.topbraidlive.org/1.0/taxonomy/maeco> ;
  rdfs:isDefinedBy <http://eds.topbraidlive.org/taxonomy/maeco> ;
  rdfs:label "Risk Weight Variability" ;
  skos:broader maecot:RiskWeightingFactor ;
  skos:prefLabel "Risk weight variability"@en ;
.
maecot:RiskWeightVariation
  rdf:type maeco:RiskMeasure ;
  rdfs:isDefinedBy <http://eds.topbraidlive.org/1.0/taxonomy/maeco> ;
  rdfs:isDefinedBy <http://eds.topbraidlive.org/taxonomy/maeco> ;
  rdfs:label "Risk Weight Variation" ;
  skos:broader maecot:RiskWeightingFactor ;
  skos:prefLabel "Risk weight variation"@en ;
.
maecot:RiskWeighting
  rdf:type maeco:RiskMeasure ;
  rdfs:isDefinedBy <http://eds.topbraidlive.org/1.0/taxonomy/maeco> ;
  rdfs:isDefinedBy <http://eds.topbraidlive.org/taxonomy/maeco> ;
  rdfs:label "Risk Weighting" ;
  skos:broader maecot:RiskWeightingFactor ;
  skos:prefLabel "Risk weightings"@en ;
.
maecot:RiskWeightingFactor
  rdf:type maeco:QuantityKind ;
  rdfs:isDefinedBy <http://eds.topbraidlive.org/1.0/taxonomy/maeco> ;
  rdfs:isDefinedBy <http://eds.topbraidlive.org/taxonomy/maeco> ;
  rdfs:label "Risk Weighting Factor" ;
  skos:broader maecot:ANY_QuantityKind ;
  skos:prefLabel "Risk weighting factor"@en ;
.
maecot:RiskWeights
  rdf:type maeco:RiskMeasure ;
  rdfs:isDefinedBy <http://eds.topbraidlive.org/1.0/taxonomy/maeco> ;
  rdfs:isDefinedBy <http://eds.topbraidlive.org/taxonomy/maeco> ;
  rdfs:label "Risk Weights" ;
  skos:broader maecot:RiskWeightingFactor ;
  skos:prefLabel "Risk weights"@en ;
.
maecot:RunOnAcurrency
  rdf:type maeco:QuantityKind ;
  rdfs:isDefinedBy <http://eds.topbraidlive.org/1.0/taxonomy/maeco> ;
  rdfs:isDefinedBy <http://eds.topbraidlive.org/taxonomy/maeco> ;
  rdfs:label "Run on a currency" ;
  skos:broader maecot:ANY_QuantityKind ;
  skos:definition "The short-term <a href='http://edg.topbraid.solutions/maeco/term/CapitalOutflow'>capital outflows</a> that occur when a <a href='http://edg.topbraid.solutions/maeco/term/PeggedExchangeRate'>pegged exchange rate</a> regime is thought to be running out of <a href='http://edg.topbraid.solutions/maeco/term/Reserves'>reserves</a> and is thus expected (and therefore forced) to <a href='http://edg.topbraid.solutions/maeco/term/Devaluation'>devalue</a> ." ;
  skos:prefLabel "Run on a Currency" ;
.
maecot:RwaDensityVariation
  rdf:type maeco:QuantityKind ;
  rdfs:isDefinedBy <http://eds.topbraidlive.org/1.0/taxonomy/maeco> ;
  rdfs:isDefinedBy <http://eds.topbraidlive.org/taxonomy/maeco> ;
  rdfs:label "Rwa Density Variation" ;
  skos:broader maecot:ANY_QuantityKind ;
  skos:prefLabel "Rwa density variation"@en ;
.
maecot:RwaRiskWeighted
  rdf:type maeco:RiskMeasure ;
  rdfs:isDefinedBy <http://eds.topbraidlive.org/1.0/taxonomy/maeco> ;
  rdfs:isDefinedBy <http://eds.topbraidlive.org/taxonomy/maeco> ;
  rdfs:label "Rwa Risk Weighted" ;
  skos:broader maecot:RiskWeightingFactor ;
  skos:prefLabel "Rwa risk weighted"@en ;
.
maecot:SCHEME_FinancialEntity
  rdf:type skos:ConceptScheme ;
  rdfs:isDefinedBy <http://eds.topbraidlive.org/1.0/taxonomy/maeco> ;
  rdfs:isDefinedBy <http://eds.topbraidlive.org/taxonomy/maeco> ;
  skos:prefLabel "Financial Entity Scheme"@en ;
.
maecot:SCHEME_FinancialGovernance
  rdf:type skos:ConceptScheme ;
  rdfs:isDefinedBy <http://eds.topbraidlive.org/1.0/taxonomy/maeco> ;
  rdfs:isDefinedBy <http://eds.topbraidlive.org/taxonomy/maeco> ;
  skos:prefLabel "Financial Governance"@en ;
.
maecot:SCHEME_GovernmentSubject
  rdf:type skos:ConceptScheme ;
  rdfs:isDefinedBy <http://eds.topbraidlive.org/1.0/taxonomy/maeco> ;
  rdfs:isDefinedBy <http://eds.topbraidlive.org/taxonomy/maeco> ;
  skos:prefLabel "Government Subject Scheme"@en ;
.
maecot:SCHEME_IT-Subject
  rdf:type skos:ConceptScheme ;
  rdfs:isDefinedBy <http://eds.topbraidlive.org/1.0/taxonomy/maeco> ;
  rdfs:isDefinedBy <http://eds.topbraidlive.org/taxonomy/maeco> ;
  skos:prefLabel "IT Subject Scheme"@en ;
.
maecot:SCHEME_LegalSubject
  rdf:type skos:ConceptScheme ;
  rdfs:isDefinedBy <http://eds.topbraidlive.org/1.0/taxonomy/maeco> ;
  rdfs:isDefinedBy <http://eds.topbraidlive.org/taxonomy/maeco> ;
  skos:prefLabel "Legal Subject Scheme"@en ;
.
maecot:SayOnFrequency
  rdf:type maeco:QuantityKind ;
  dcterms:source "http://www.cftc.gov/LawRegulation/DoddFrankAct/index.htm"^^xsd:anyURI ;
  rdfs:isDefinedBy <http://eds.topbraidlive.org/1.0/taxonomy/maeco> ;
  rdfs:isDefinedBy <http://eds.topbraidlive.org/taxonomy/maeco> ;
  rdfs:label "Say On Frequency" ;
  skos:altLabel "Say on Frequency"@en ;
  skos:definition "Pursuant to the DFA and rules adopted by the SEC, certain public companies must include in their proxy statements a separate resolution to determine whether the required Say-on-Pay vote (discussed below) takes place every one, two or three years."@en ;
  skos:prefLabel "Say-on-Frequency"@en ;
.
maecot:ScientificTariff
  rdf:type maeco:Tariff ;
  rdfs:isDefinedBy <http://eds.topbraidlive.org/1.0/taxonomy/maeco> ;
  rdfs:isDefinedBy <http://eds.topbraidlive.org/taxonomy/maeco> ;
  rdfs:label "Scientific tariff" ;
  skos:broader maecot:Tariff ;
  skos:definition "A <a href='http://edg.topbraid.solutions/maeco/term/MadeToMeasureTariff'>made-to-measure tariff</a> ." ;
  skos:prefLabel "Scientific Tariff" ;
.
maecot:SeasonalTariff
  rdf:type maeco:Tariff ;
  rdfs:isDefinedBy <http://eds.topbraidlive.org/1.0/taxonomy/maeco> ;
  rdfs:isDefinedBy <http://eds.topbraidlive.org/taxonomy/maeco> ;
  rdfs:label "Seasonal tariff" ;
  skos:broader maecot:Tariff ;
  skos:definition "A tariff that is levied at different rates at different times of the year, usually on agricultural products, being highest at the time of the domestic harvest." ;
  skos:prefLabel "Seasonal Tariff" ;
.
maecot:SecuredFundingRunOff
  rdf:type maeco:QuantityKind ;
  rdfs:isDefinedBy <http://eds.topbraidlive.org/1.0/taxonomy/maeco> ;
  rdfs:isDefinedBy <http://eds.topbraidlive.org/taxonomy/maeco> ;
  rdfs:label "Secured Funding Run Off" ;
  skos:broader maecot:ANY_QuantityKind ;
  skos:definition "For the purposes of the Basel III standard, secured funding is defined as those liabilities and general obligations that are collateralised by legal rights to specifically designated assets owned by the borrowing institution in the case of bankruptcy, insolvency, liquidation or resolution."@en ;
  skos:prefLabel "Secured funding run-off"@en ;
  prov:wasInfluencedBy "<http://www.bis.org/publ/bcbs238.pdf>" ;
.
maecot:ShadowExchangeRate
  rdf:type maeco:Rate ;
  rdfs:isDefinedBy <http://eds.topbraidlive.org/1.0/taxonomy/maeco> ;
  rdfs:isDefinedBy <http://eds.topbraidlive.org/taxonomy/maeco> ;
  rdfs:label "Shadow exchange rate" ;
  skos:broader maecot:ANY_Rate ;
  skos:definition "<STRONG>1.</STRONG> The <a href='http://edg.topbraid.solutions/maeco/term/ShadowPrice'>shadow price</a> of <a href='http://edg.topbraid.solutions/maeco/term/ForeignExchange'>foreign exchange</a> .  <STRONG>2.</STRONG> What the market <a href='http://edg.topbraid.solutions/maeco/term/ExchangeRate'>exchange rate</a> would be in the absence of various <a href='http://edg.topbraid.solutions/maeco/term/MarketImperfection'>market imperfections</a> ." ;
  skos:prefLabel "Shadow Exchange Rate" ;
.
maecot:ShadowPrice
  rdf:type maeco:Price ;
  rdf:type maeco:QuantityKind ;
  dcterms:source "http://www.cftc.gov/LawRegulation/DoddFrankAct/index.htm"^^xsd:anyURI ;
  rdfs:isDefinedBy <http://eds.topbraidlive.org/1.0/taxonomy/maeco> ;
  rdfs:isDefinedBy <http://eds.topbraidlive.org/taxonomy/maeco> ;
  rdfs:label "Shadow price" ;
  skos:broader maecot:ANY_QuantityKind ;
  skos:broader maecot:Price ;
  skos:definition "The implicit value or cost associated with a constraint.  That is, the increased value that will be achieved by relaxing the constraint by one unit.  When <a href='http://edg.topbraid.solutions/maeco/term/ForeignExchange'>foreign exchange</a> is rationed, the shadow price of foreign exchange becomes the relevant <a href='http://edg.topbraid.solutions/maeco/term/ExchangeRate'>exchange rate</a> for making decisions." ;
  skos:definition "The market-based value of a stable NAV money market fund. Shadow prices fluctuate based on the market price of the underlying portfolio securities held in the fund."@en ;
  skos:prefLabel "Shadow Price"@en ;
.
maecot:ShortTermInterestRate
  rdf:type maeco:Rate ;
  rdfs:isDefinedBy <http://eds.topbraidlive.org/1.0/taxonomy/maeco> ;
  rdfs:isDefinedBy <http://eds.topbraidlive.org/taxonomy/maeco> ;
  rdfs:label "Short-term interest rate" ;
  skos:broader maecot:ANY_Rate ;
  skos:definition "<STRONG>1.</STRONG> The <a href='http://edg.topbraid.solutions/maeco/term/InterestRate'>interest rate</a> on any financial instrument of short maturity.  <STRONG>2.</STRONG> Denoted <STRONG>STIR</STRONG> , a particular financial instrument that is a futures contract on a short-term interest rate, often a 3-month interest rate in any of a variety of currencies." ;
  skos:prefLabel "Short-Term Interest Rate" ;
.
maecot:SingleColumnTariff
  rdf:type maeco:Tariff ;
  rdfs:isDefinedBy <http://eds.topbraidlive.org/1.0/taxonomy/maeco> ;
  rdfs:isDefinedBy <http://eds.topbraidlive.org/taxonomy/maeco> ;
  rdfs:label "Single column tariff" ;
  skos:broader maecot:Tariff ;
  skos:definition "A <a href='http://edg.topbraid.solutions/maeco/term/TariffSchedule'>tariff schedule</a> that specifies only a single tariff rate for each product.  Contrasts with schedules that have separate <a href='http://edg.topbraid.solutions/maeco/term/GeneralTariff'>general tariffs</a> and <a href='http://edg.topbraid.solutions/maeco/term/MFNTariff'>MFN tariffs</a> ." ;
  skos:prefLabel "Single Column Tariff" ;
.
maecot:SmootHawleyTariff
  rdf:type maeco:Tariff ;
  rdfs:isDefinedBy <http://eds.topbraidlive.org/1.0/taxonomy/maeco> ;
  rdfs:isDefinedBy <http://eds.topbraidlive.org/taxonomy/maeco> ;
  rdfs:label "Smoot-Hawley Tariff" ;
  skos:broader maecot:Tariff ;
  skos:definition "The <a href='http://edg.topbraid.solutions/maeco/term/TariffActOf1930'>Tariff Act of 1930</a> , which raised average U.S. tariffs on <a href='http://edg.topbraid.solutions/maeco/term/DutiableImports'>dutiable imports</a> to 53% and provoked <a href='http://edg.topbraid.solutions/maeco/term/Retaliation'>retaliation</a> by other countries." ;
  skos:prefLabel "Smoot-Hawley Tariff" ;
.
maecot:SocialCost
  rdf:type maeco:Cost ;
  rdfs:isDefinedBy <http://eds.topbraidlive.org/1.0/taxonomy/maeco> ;
  rdfs:isDefinedBy <http://eds.topbraidlive.org/taxonomy/maeco> ;
  rdfs:label "Social cost" ;
  skos:broader maecot:ANY_Cost ;
  skos:definition "The cost to society as a whole from an event, action, or policy change.  Includes negative <a href='http://edg.topbraid.solutions/maeco/term/Externality'>externalities</a> and does not count costs that are transfers to others, in contrast to <a href='http://edg.topbraid.solutions/maeco/term/PrivateCost'>private cost</a> ." ;
  skos:prefLabel "Social Cost" ;
.
maecot:SpecialCaseStableDeposits
  rdf:type maeco:QuantityKind ;
  maeco:runOffPercentRate 3 ;
  rdfs:isDefinedBy <http://eds.topbraidlive.org/1.0/taxonomy/maeco> ;
  rdfs:isDefinedBy <http://eds.topbraidlive.org/taxonomy/maeco> ;
  rdfs:label "Special Case Stable Deposits" ;
  skos:broader maecot:ANY_QuantityKind ;
  skos:definition "Special Case Stable deposits have a run-off rate = 3%. Examples are deposit insurance scheme meeting additional criteria"@en ;
  skos:prefLabel "Special Case Stable Deposits"@en ;
  prov:wasInfluencedBy "<http://www.bis.org/publ/bcbs238.pdf>" ;
.
maecot:SpecificTariff
  rdf:type maeco:Tariff ;
  rdfs:isDefinedBy <http://eds.topbraidlive.org/1.0/taxonomy/maeco> ;
  rdfs:isDefinedBy <http://eds.topbraidlive.org/taxonomy/maeco> ;
  rdfs:label "Specific tariff" ;
  skos:broader maecot:Tariff ;
  skos:definition "A <a href='http://edg.topbraid.solutions/maeco/term/Tariff'>tariff</a> specified as an amount of currency per unit of the good." ;
  skos:prefLabel "Specific Tariff" ;
.
maecot:SpotPrice
  rdf:type maeco:QuantityKind ;
  dcterms:source "http://www.isda.org/c_and_a/oper_commit-dcg-glossary.html"^^xsd:anyURI ;
  rdfs:isDefinedBy <http://eds.topbraidlive.org/1.0/taxonomy/maeco> ;
  rdfs:isDefinedBy <http://eds.topbraidlive.org/taxonomy/maeco> ;
  rdfs:label "Spot Price" ;
  skos:broader maecot:ANY_QuantityKind ;
  skos:definition "The price of a commodity, security or currency that is quoted for immediate payment and delivery.  "@en ;
  skos:prefLabel "Spot price/rate"@en ;
.
maecot:SpotRate
  rdf:type maeco:Rate ;
  rdfs:isDefinedBy <http://eds.topbraidlive.org/1.0/taxonomy/maeco> ;
  rdfs:isDefinedBy <http://eds.topbraidlive.org/taxonomy/maeco> ;
  rdfs:label "Spot rate" ;
  skos:broader maecot:ANY_Rate ;
  skos:definition "The <a href='http://edg.topbraid.solutions/maeco/term/ExchangeRate'>exchange rate</a> on the <a href='http://edg.topbraid.solutions/maeco/term/SpotMarket'>spot market</a> .  Also called the <STRONG>spot exchange rate</STRONG> ." ;
  skos:prefLabel "Spot Rate" ;
.
maecot:StableDeposits
  rdf:type maeco:QuantityKind ;
  maeco:runOffPercentRate 5 ;
  rdfs:isDefinedBy <http://eds.topbraidlive.org/1.0/taxonomy/maeco> ;
  rdfs:isDefinedBy <http://eds.topbraidlive.org/taxonomy/maeco> ;
  rdfs:label "Stable Deposits" ;
  skos:broader maecot:ANY_QuantityKind ;
  skos:definition "Stable deposits have a run-off rate = 3% and higher. They usually receive a run-off factor of 5%, are the amount of the deposits that are fully insured by an effective deposit insurance scheme or by a public guarantee that provides equivalent protection and where: (a) the depositors have other established relationships with the bank that make deposit withdrawal highly unlikely; or (b) the deposits are in transactional accounts (eg accounts where salaries are automatically deposited)."@en ;
  skos:prefLabel "Stable Deposits"@en ;
  prov:wasInfluencedBy "<http://www.bis.org/publ/bcbs238.pdf>" ;
.
maecot:StableRetailDeposits
  rdf:type maeco:QuantityKind ;
  rdfs:isDefinedBy <http://eds.topbraidlive.org/1.0/taxonomy/maeco> ;
  rdfs:isDefinedBy <http://eds.topbraidlive.org/taxonomy/maeco> ;
  rdfs:label "Stable Retail Deposits" ;
  skos:broader maecot:ANY_QuantityKind ;
  skos:definition "Retail deposits are divided into stable and less stable portions of funds as described below, with minimum run-off rates listed for each category. The run-off rates for retail deposits are minimum floors, with higher run-off rates established by individual jurisdictions as appropriate to capture depositor behaviour in a period of stress in each jurisdiction."@en ;
  skos:prefLabel "Stable Retail Deposits"@en ;
  prov:wasInfluencedBy "<http://www.bis.org/publ/bcbs238.pdf>" ;
.
maecot:StochasticVolatility
  rdf:type maeco:QuantityKind ;
  dcterms:source "http://www.isda.org/c_and_a/oper_commit-dcg-glossary.html"^^xsd:anyURI ;
  rdfs:isDefinedBy <http://eds.topbraidlive.org/1.0/taxonomy/maeco> ;
  rdfs:isDefinedBy <http://eds.topbraidlive.org/taxonomy/maeco> ;
  rdfs:label "Stochastic Volatility" ;
  skos:broader maecot:Volatility ;
  skos:prefLabel "Stochastic Volatility" ;
.
maecot:StockOfHQLA
  rdf:type maeco:QuantityKind ;
  rdfs:isDefinedBy <http://eds.topbraidlive.org/1.0/taxonomy/maeco> ;
  rdfs:isDefinedBy <http://eds.topbraidlive.org/taxonomy/maeco> ;
  rdfs:label "Stock Of HQLA" ;
  skos:broader maecot:ANY_QuantityKind ;
  skos:definition """<p>Stock of HQLA = Level 1 + Level 2A + Level 2B - Adjustment for 15% cap - Adjustment for 40% cap</p>
<p>where:</p>

<dd>Adjustment for 15% cap = Max (Adjusted Level 2B - 15/85*(Adjusted Level 1 + Adjusted Level 2A), Adjusted Level 2B - 15/60*Adjusted Level 1, 0)</dd>
<dd>Adjustment for 40% cap = Max ((Adjusted Level 2A + Adjusted Level 2B - Adjustment for 15% cap) - 2/3*Adjusted Level 1 assets, 0)</dd>
<dd>Alternatively, the formula can be expressed as:</dd>
<dd>Stock of HQLA = Level 1 + Level 2A + Level 2B - Max ((Adjusted Level 2A+Adjusted Level 2B) - 2/3*Adjusted Level 1, Adjusted Level 2B - 15/85*(Adjusted Level 1 + Adjusted Level 2A), 0)</dd>"""^^rdf:HTML ;
  skos:prefLabel "Stock of HQLA"@en ;
.
maecot:StrategicIndustryArgumentForATariff
  rdf:type maeco:Tariff ;
  rdfs:isDefinedBy <http://eds.topbraidlive.org/1.0/taxonomy/maeco> ;
  rdfs:isDefinedBy <http://eds.topbraidlive.org/taxonomy/maeco> ;
  rdfs:label "Strategic industry argument for a tariff" ;
  skos:broader maecot:Tariff ;
  skos:definition "The view that an industry serves a special \"strategic\" purpose in an economy and needs to be <a href='http://edg.topbraid.solutions/maeco/term/Protection'>protected</a> by a tariff to prevent it from disappearing.  Views of what constitutes a strategic purpose are often vague and contradictory.  The use of a tariff for this purpose is <a href='http://edg.topbraid.solutions/maeco/term/SecondBest'>second best</a> ." ;
  skos:prefLabel "Strategic Industry Argument For A Tariff" ;
.
maecot:StrategicTradePolicyArgumentForATariff
  rdf:type maeco:Tariff ;
  rdfs:isDefinedBy <http://eds.topbraidlive.org/1.0/taxonomy/maeco> ;
  rdfs:isDefinedBy <http://eds.topbraidlive.org/taxonomy/maeco> ;
  rdfs:label "Strategic trade policy argument for a tariff" ;
  skos:broader maecot:Tariff ;
  skos:definition "In an example of <a href='http://edg.topbraid.solutions/maeco/term/StrategicTradePolicy'>strategic trade policy</a> , the use of a tariff to extract monopoly profits from a foreign monopolist, or to <a href='http://edg.topbraid.solutions/maeco/term/ProfitShifting'>shift profit</a> from foreign to domestic competitors in an international oligopoly.  The monopoly case seems to have originated with <a href='http://edg.topbraid.solutions/maeco/term/Bib.html#Katrak1977'>Katrak (1977)</a> , but the classic treatment of the larger issue is <a href='http://edg.topbraid.solutions/maeco/term/Bib.html#BranderSpencer1984'>Brander and Spencer (1984)</a> ." ;
  skos:prefLabel "Strategic Trade Policy Argument For A Tariff" ;
.
maecot:StrikePrice
  rdf:type maeco:QuantityKind ;
  dcterms:source "http://www.isda.org/c_and_a/oper_commit-dcg-glossary.html"^^xsd:anyURI ;
  rdfs:isDefinedBy <http://eds.topbraidlive.org/1.0/taxonomy/maeco> ;
  rdfs:isDefinedBy <http://eds.topbraidlive.org/taxonomy/maeco> ;
  rdfs:label "Strike Price" ;
  skos:broader maecot:ANY_QuantityKind ;
  skos:definition "The price at which an option contract is executed."@en ;
  skos:prefLabel "Strike price"@en ;
.
maecot:StrikePriceDifferential
  rdf:type maeco:QuantityKind ;
  dcterms:source "http://www.isda.org/c_and_a/oper_commit-dcg-glossary.html"^^xsd:anyURI ;
  rdfs:isDefinedBy <http://eds.topbraidlive.org/1.0/taxonomy/maeco> ;
  rdfs:isDefinedBy <http://eds.topbraidlive.org/taxonomy/maeco> ;
  rdfs:label "Strike Price Differential" ;
  skos:broader maecot:ANY_QuantityKind ;
  skos:definition "The difference between the settlement price and the strike price at the point of option exercise."@en ;
  skos:prefLabel "Strike price differential"@en ;
.
maecot:Subsidy
  rdf:type maeco:Subsidy ;
  rdfs:isDefinedBy <http://eds.topbraidlive.org/1.0/taxonomy/maeco> ;
  rdfs:isDefinedBy <http://eds.topbraidlive.org/taxonomy/maeco> ;
  rdfs:label "Subsidy" ;
  skos:broader maecot:ANY_QuantityKind ;
  skos:definition "A payment by government, perhaps implicit, to the private sector in return for some activity that it wants to reward, encourage, or assist.  Under <a href='http://edg.topbraid.solutions/maeco/term/Wto'>WTO</a> rules, subsidies may be <a href='http://edg.topbraid.solutions/maeco/term/ProhibitedSubsidy'>prohibited</a> , <a href='http://edg.topbraid.solutions/maeco/term/ActionableSubsidy'>actionable</a> , or <a href='http://edg.topbraid.solutions/maeco/term/NonactionableSubsidy'>non-actionable</a> ." ;
  skos:prefLabel "Subsidy" ;
.
maecot:SunkCost
  rdf:type maeco:Cost ;
  dcterms:source "http://www.wwnorton.com/college/econ/stec4/macroeconomics/glossary.asp"^^xsd:anyURI ;
  rdfs:isDefinedBy <http://eds.topbraidlive.org/1.0/taxonomy/maeco> ;
  rdfs:isDefinedBy <http://eds.topbraidlive.org/taxonomy/maeco> ;
  rdfs:label "Sunk cost" ;
  skos:broader maecot:ANY_Cost ;
  skos:definition "A cost that has already been incurred and cannot be reversed, which therefore cannot be avoided by current or future action.  Sunk costs should therefore be irrelevant to current decisions." ;
  skos:prefLabel "Sunk Cost" ;
.
maecot:SupplementaryLeverageRatio
  rdf:type maeco:Ratio ;
  dcterms:source "http://www.cftc.gov/LawRegulation/DoddFrankAct/index.htm"^^xsd:anyURI ;
  rdfs:isDefinedBy <http://eds.topbraidlive.org/1.0/taxonomy/maeco> ;
  rdfs:isDefinedBy <http://eds.topbraidlive.org/taxonomy/maeco> ;
  rdfs:label "Supplementary Leverage Ratio" ;
  skos:broader maecot:ANY_Ratio ;
  skos:definition "Eight US banks that are G-SIBs are subject to a 5% supplementary leverage ratio minimum at the parent level and a 6% supplementary leverage ratio minimum at the bank subsidiary level, which is a surcharge over the Basel III 3% minimum leverage ratio"@en ;
  skos:prefLabel "Supplementary Leverage Ratio"@en ;
.
maecot:Supply
  rdf:type maeco:Supply ;
  dcterms:source "http://www.wwnorton.com/college/econ/stec4/macroeconomics/glossary.asp"^^xsd:anyURI ;
  rdfs:isDefinedBy <http://eds.topbraidlive.org/1.0/taxonomy/maeco> ;
  rdfs:isDefinedBy <http://eds.topbraidlive.org/taxonomy/maeco> ;
  rdfs:label "supply" ;
  skos:definition "<STRONG>Supply</STRONG> - the quantity of a good or service that a household or firm would like to sell at a particular price. <STRONG>1.</STRONG> The act of offering a product for sale.  <STRONG>2.</STRONG> The quantity offered for sale.  <STRONG>3.</STRONG> The quantities offered for sale at various prices; the <a href='http://edg.topbraid.solutions/maeco/term/SupplyCurve'>supply curve</a> ." ;
  skos:prefLabel "Supply" ;
.
maecot:SupplyPrice
  rdf:type maeco:Price ;
  rdfs:isDefinedBy <http://eds.topbraidlive.org/1.0/taxonomy/maeco> ;
  rdfs:isDefinedBy <http://eds.topbraidlive.org/taxonomy/maeco> ;
  rdfs:label "Supply price" ;
  skos:broader maecot:Price ;
  skos:definition "The price at which a given quantity is supplied; thus the <a href='http://edg.topbraid.solutions/maeco/term/SupplyCurve'>supply curve</a> viewed from the perspective of price as a function of quantity.  This is not well defined if the supply curve is <a href='http://edg.topbraid.solutions/maeco/term/BackwardBending'>backward bending</a> ." ;
  skos:prefLabel "Supply Price" ;
.
maecot:SupportPrice
  rdf:type maeco:Price ;
  rdfs:isDefinedBy <http://eds.topbraidlive.org/1.0/taxonomy/maeco> ;
  rdfs:isDefinedBy <http://eds.topbraidlive.org/taxonomy/maeco> ;
  rdfs:label "Support price" ;
  skos:broader maecot:Price ;
  skos:definition "The price guaranteed by a government <a href='http://edg.topbraid.solutions/maeco/term/PriceSupport'>price support</a> program.  Typically it requires that the government buy the product at that price.  If the <a href='http://edg.topbraid.solutions/maeco/term/MarketClearing'>market clearing</a> price is lower, this raises the price to that level and causes the government to acquire the resulting <a href='http://edg.topbraid.solutions/maeco/term/ExcessSupply'>excess supply</a> ." ;
  skos:prefLabel "Support Price" ;
.
maecot:SwapRate
  rdf:type maeco:Rate ;
  rdfs:isDefinedBy <http://eds.topbraidlive.org/1.0/taxonomy/maeco> ;
  rdfs:isDefinedBy <http://eds.topbraidlive.org/taxonomy/maeco> ;
  rdfs:label "Swap rate" ;
  skos:broader maecot:ANY_Rate ;
  skos:definition "The difference between the <a href='http://edg.topbraid.solutions/maeco/term/SpotRate'>spot</a> and <a href='http://edg.topbraid.solutions/maeco/term/ForwardRate'>forward</a> <a href='http://edg.topbraid.solutions/maeco/term/ExchangeRate'>exchange rates</a> .  Thus the price of a <a href='http://edg.topbraid.solutions/maeco/term/Swap'>swap</a> ." ;
  skos:prefLabel "Swap Rate" ;
.
maecot:Tariff
  rdf:type maeco:Tariff ;
  rdfs:isDefinedBy <http://eds.topbraidlive.org/1.0/taxonomy/maeco> ;
  rdfs:isDefinedBy <http://eds.topbraidlive.org/taxonomy/maeco> ;
  rdfs:label "Tariff" ;
  skos:broader maecot:ANY_QuantityKind ;
  skos:definition "A tax on trade, usually an <STRONG>import tariff</STRONG> but sometimes used to denote an <a href='http://edg.topbraid.solutions/maeco/term/ExportTax'>export tax</a> .  Tariffs may be <a href='http://edg.topbraid.solutions/maeco/term/AdValorem'>ad valorem</a> or <a href='http://edg.topbraid.solutions/maeco/term/SpecificTariff'>specific.</a>" ;
  skos:prefLabel "Tariff" ;
.
maecot:TaxCumSubsidy
  rdf:type maeco:Subsidy ;
  rdfs:isDefinedBy <http://eds.topbraidlive.org/1.0/taxonomy/maeco> ;
  rdfs:isDefinedBy <http://eds.topbraidlive.org/taxonomy/maeco> ;
  rdfs:label "Tax-cum-subsidy" ;
  skos:broader maecot:Subsidy ;
  skos:definition "This phrase is used to indicate a policy that may be either a tax or a subsidy, depending on which will achieve the stated objective, which is usually to alter or set a relative price.  The word \"cum\" here is Latin for \"with,\" which is slightly inappropriate, since in this context what is usually meant is \"or.\"" ;
  skos:prefLabel "Tax-Cum-Subsidy" ;
.
maecot:TermDeposits
  rdf:type maeco:QuantityKind ;
  <http://www.linkedmodel.org/schema/vaem#todo> "NEW" ;
  rdfs:isDefinedBy <http://eds.topbraidlive.org/1.0/taxonomy/maeco> ;
  rdfs:isDefinedBy <http://eds.topbraidlive.org/taxonomy/maeco> ;
  rdfs:label "Term Deposits" ;
  rdfs:label "Term deposits" ;
  skos:altLabel "TDF" ;
  skos:broader maecot:ANY_QuantityKind ;
  skos:definition "TBD"@en ;
  skos:prefLabel "Term Deposits" ;
  skos:prefLabel "Term Deposits"@en ;
  skos:prefLabel "Term deposits" ;
  prov:wasInfluencedBy "<http://www.bis.org/publ/bcbs238.pdf>" ;
.
maecot:Theta
  rdf:type maeco:QuantityKind ;
  dcterms:source "http://www.isda.org/c_and_a/oper_commit-dcg-glossary.html"^^xsd:anyURI ;
  rdfs:isDefinedBy <http://eds.topbraidlive.org/1.0/taxonomy/maeco> ;
  rdfs:isDefinedBy <http://eds.topbraidlive.org/taxonomy/maeco> ;
  rdfs:label "Theta" ;
  skos:broader maecot:ANY_QuantityKind ;
  skos:definition "A term in option theory measuring the time decay of the option value."@en ;
  skos:prefLabel "Theta"@en ;
.
maecot:Threshold
  rdf:type maeco:QuantityKind ;
  dcterms:source "http://www.isda.org/c_and_a/oper_commit-dcg-glossary.html"^^xsd:anyURI ;
  rdfs:isDefinedBy <http://eds.topbraidlive.org/1.0/taxonomy/maeco> ;
  rdfs:isDefinedBy <http://eds.topbraidlive.org/taxonomy/maeco> ;
  rdfs:label "Threshold" ;
  skos:definition "An amount of unsecured exposure a counterparty is prepared to accept before calling for collateral."@en ;
  skos:prefLabel "Threshold"@en ;
.
maecot:TimeValue
  rdf:type maeco:QuantityKind ;
  dcterms:source "http://www.isda.org/c_and_a/oper_commit-dcg-glossary.html"^^xsd:anyURI ;
  rdfs:isDefinedBy <http://eds.topbraidlive.org/1.0/taxonomy/maeco> ;
  rdfs:isDefinedBy <http://eds.topbraidlive.org/taxonomy/maeco> ;
  rdfs:label "Time Value" ;
  skos:definition "The amount by which the premium of an option exceeds its intrinsic value. Where an option has no intrinsic value the premium consists entirely of time value."@en ;
  skos:prefLabel "Time value"@en ;
.
maecot:TotalCost
  rdf:type maeco:Cost ;
  dcterms:source "http://www.wwnorton.com/college/econ/stec4/macroeconomics/glossary.asp"^^xsd:anyURI ;
  rdfs:isDefinedBy <http://eds.topbraidlive.org/1.0/taxonomy/maeco> ;
  rdfs:isDefinedBy <http://eds.topbraidlive.org/taxonomy/maeco> ;
  rdfs:label "Total Cost" ;
  skos:broader maecot:ANY_Cost ;
  skos:definition "<STRONG>Total Costs</STRONG> - the sum of all fixed costs and variable costs" ;
  skos:prefLabel "Total Cost" ;
.
maecot:TotalCreditRisk
  rdf:type maeco:RiskMeasure ;
  rdfs:isDefinedBy <http://eds.topbraidlive.org/1.0/taxonomy/maeco> ;
  rdfs:isDefinedBy <http://eds.topbraidlive.org/taxonomy/maeco> ;
  rdfs:label "Total Credit Risk" ;
  skos:broader maecot:ANY_QuantityKind ;
  skos:prefLabel "Total Credit Risk"@en ;
.
maecot:TotalNetCashOutflow
  rdf:type maeco:QuantityKind ;
  dcterms:source "http://www.cftc.gov/LawRegulation/DoddFrankAct/index.htm"^^xsd:anyURI ;
  rdfs:isDefinedBy <http://eds.topbraidlive.org/1.0/taxonomy/maeco> ;
  rdfs:isDefinedBy <http://eds.topbraidlive.org/taxonomy/maeco> ;
  rdfs:label "Total Net Cash Outflow" ;
  skos:altLabel "TNCO" ;
  skos:broader maecot:ANY_QuantityKind ;
  skos:definition "Total net cash outflow. TNCOs are measured in connection with the LCR. Net cash flows equal total expected cash outflows, minus total expected net cash inflows (with inflows capped at 75% of outflows)."@en ;
  skos:prefLabel "Total Net Cash Outflow"@en ;
.
maecot:TotalNetCashOutflows
  rdf:type maeco:QuantityKind ;
  rdfs:isDefinedBy <http://eds.topbraidlive.org/1.0/taxonomy/maeco> ;
  rdfs:isDefinedBy <http://eds.topbraidlive.org/taxonomy/maeco> ;
  rdfs:label "Total Net Cash Outflows" ;
  skos:broader maecot:ANY_QuantityKind ;
  skos:definition "The term \"total net cash outflows\" is defined as the total expected cash outflows minus total expected cash inflows in the specified stress scenario for the subsequent 30 calendar days. Total expected cash outflows are calculated by multiplying the outstanding balances of various categories or types of liabilities and off-balance sheet commitments by the rates at which they are expected to run off or be drawn down. Total expected cash inflows are calculated by multiplying the outstanding balances of various categories of contractual receivables by the rates at which they are expected to flow in under the scenario up to an aggregate cap of 75% of total expected cash outflows."@en ;
  skos:prefLabel "Total Net Cash Outflows"@en ;
  prov:wasInfluencedBy "<http://www.bis.org/publ/bcbs238.pdf>" ;
.
maecot:TradeCost
  rdf:type maeco:Cost ;
  rdfs:isDefinedBy <http://eds.topbraidlive.org/1.0/taxonomy/maeco> ;
  rdfs:isDefinedBy <http://eds.topbraidlive.org/taxonomy/maeco> ;
  rdfs:label "Trade cost" ;
  skos:broader maecot:ANY_Cost ;
  skos:definition "Any cost incurred in order to engage in international trade, including <a href='http://edg.topbraid.solutions/maeco/term/TransportCost'>transport cost</a> , insurance, etc." ;
  skos:prefLabel "Trade Cost" ;
.
maecot:TradeWeightedAverageTariff
  rdf:type maeco:Tariff ;
  rdfs:isDefinedBy <http://eds.topbraidlive.org/1.0/taxonomy/maeco> ;
  rdfs:isDefinedBy <http://eds.topbraidlive.org/taxonomy/maeco> ;
  rdfs:label "Trade-weighted average tariff" ;
  skos:broader maecot:Tariff ;
  skos:definition "The <a href='http://edg.topbraid.solutions/maeco/term/AverageTariff'>average</a> of a country's tariffs, weighted by value of imports.  This is easily calculated as the ratio of total tariff revenue to total value of imports." ;
  skos:prefLabel "Trade-Weighted Average Tariff" ;
.
maecot:TradeWeightedExchangeRate
  rdf:type maeco:Rate ;
  rdfs:isDefinedBy <http://eds.topbraidlive.org/1.0/taxonomy/maeco> ;
  rdfs:isDefinedBy <http://eds.topbraidlive.org/taxonomy/maeco> ;
  rdfs:label "Trade-weighted exchange rate" ;
  skos:broader maecot:ANY_Rate ;
  skos:definition "The weighted average of a country's <a href='http://edg.topbraid.solutions/maeco/term/BilateralExchangeRate'>bilateral exchange rates</a> using <a href='http://edg.topbraid.solutions/maeco/term/BilateralTrade'>bilateral trade</a> -- exports plus imports -- as weights.  Also called an <a href='http://edg.topbraid.solutions/maeco/term/EffectiveExchangeRate'>effective exchange rate</a> ." ;
  skos:prefLabel "Trade-Weighted Exchange Rate" ;
.
maecot:TransactionCost
  rdf:type maeco:Cost ;
  dcterms:source "http://www.wwnorton.com/college/econ/stec4/macroeconomics/glossary.asp"^^xsd:anyURI ;
  rdfs:isDefinedBy <http://eds.topbraidlive.org/1.0/taxonomy/maeco> ;
  rdfs:isDefinedBy <http://eds.topbraidlive.org/taxonomy/maeco> ;
  rdfs:label "Transaction cost" ;
  skos:broader maecot:ANY_Cost ;
  skos:definition "<STRONG>1.</STRONG> On the foreign exchange and other financial markets, this includes <a href='http://edg.topbraid.solutions/maeco/term/BrokersFee'>broker's fees</a> and/or the <a href='http://edg.topbraid.solutions/maeco/term/BidAskSpread'>bid/ask spread</a> .  <STRONG>2.</STRONG> Much more broadly, this can refer to any sort of cost associated with the exchange of goods or services, including information costs, legal fees, and other costs incurred in overcoming market imperfections. <STRONG>Transactions Costs</STRONG> - the extra costs (beyond the price of the purchase) of conducting a transaction, whether those costs are money, time, or inconvenience" ;
  skos:prefLabel "Transaction Cost" ;
.
maecot:TransferPrice
  rdf:type maeco:Price ;
  rdfs:isDefinedBy <http://eds.topbraidlive.org/1.0/taxonomy/maeco> ;
  rdfs:isDefinedBy <http://eds.topbraidlive.org/taxonomy/maeco> ;
  rdfs:label "Transfer price" ;
  skos:broader maecot:Price ;
  skos:definition "Literally this is the price charged on goods and services traded between subsidiaries of (often) a <a href='http://edg.topbraid.solutions/maeco/term/Mnc2'>multinational</a> ) corporation.  However, the term usually connotes setting prices to minimize taxes paid, in response to differences in <a href='http://edg.topbraid.solutions/maeco/term/CorporateTax'>corporate tax</a> rates.  Contrasts with <a href='http://edg.topbraid.solutions/maeco/term/ArmsLengthPrice'>arm's length price</a> ." ;
  skos:prefLabel "Transfer Price" ;
.
maecot:TransportCost
  rdf:type maeco:Cost ;
  rdfs:isDefinedBy <http://eds.topbraidlive.org/1.0/taxonomy/maeco> ;
  rdfs:isDefinedBy <http://eds.topbraidlive.org/taxonomy/maeco> ;
  rdfs:label "Transport cost" ;
  skos:broader maecot:ANY_Cost ;
  skos:definition "The cost of transporting a good, especially in international trade." ;
  skos:prefLabel "Transport Cost" ;
.
maecot:TransportationCost
  rdf:type maeco:Cost ;
  rdfs:isDefinedBy <http://eds.topbraidlive.org/1.0/taxonomy/maeco> ;
  rdfs:isDefinedBy <http://eds.topbraidlive.org/taxonomy/maeco> ;
  rdfs:label "Transportation cost" ;
  skos:broader maecot:ANY_Cost ;
  skos:definition "<a href='http://edg.topbraid.solutions/maeco/term/TransportCost'>Transport cost</a> ." ;
  skos:prefLabel "Transportation Cost" ;
.
maecot:TriggerPrice
  rdf:type maeco:Price ;
  rdfs:isDefinedBy <http://eds.topbraidlive.org/1.0/taxonomy/maeco> ;
  rdfs:isDefinedBy <http://eds.topbraidlive.org/taxonomy/maeco> ;
  rdfs:label "Trigger price" ;
  skos:broader maecot:Price ;
  skos:definition "See <a href='http://edg.topbraid.solutions/maeco/term/MinimumPriceSystem'>minimum price system</a> ." ;
  skos:prefLabel "Trigger Price" ;
.
maecot:UnemploymentRate
  rdf:type maeco:Rate ;
  dcterms:source "http://www.wwnorton.com/college/econ/stec4/macroeconomics/glossary.asp"^^xsd:anyURI ;
  rdfs:isDefinedBy <http://eds.topbraidlive.org/1.0/taxonomy/maeco> ;
  rdfs:isDefinedBy <http://eds.topbraidlive.org/taxonomy/maeco> ;
  rdfs:label "unemployment rate" ;
  skos:broader maecot:ANY_Rate ;
  skos:definition "<STRONG>Unemployment Rate</STRONG> - the ratio of the number of people seeking employment to the total labor force. The ratio of <a href='http://edg.topbraid.solutions/maeco/term/Unemployment'>unemployment</a> to the <a href='http://edg.topbraid.solutions/maeco/term/LaborForce'>labor force</a> of a country." ;
  skos:prefLabel "Unemployment Rate" ;
.
maecot:UnitLaborCost
  rdf:type maeco:Cost ;
  rdfs:isDefinedBy <http://eds.topbraidlive.org/1.0/taxonomy/maeco> ;
  rdfs:isDefinedBy <http://eds.topbraidlive.org/taxonomy/maeco> ;
  rdfs:label "Unit labor cost" ;
  skos:broader maecot:ANY_Cost ;
  skos:definition "The cost of labor per unit of real output." ;
  skos:prefLabel "Unit Labor Cost" ;
.
maecot:UnitTariff
  rdf:type maeco:Tariff ;
  rdfs:isDefinedBy <http://eds.topbraidlive.org/1.0/taxonomy/maeco> ;
  rdfs:isDefinedBy <http://eds.topbraidlive.org/taxonomy/maeco> ;
  rdfs:label "Unit tariff" ;
  skos:broader maecot:Tariff ;
  skos:definition "<a href='http://edg.topbraid.solutions/maeco/term/SpecificTariff'>Specific tariff</a> ." ;
  skos:prefLabel "Unit Tariff" ;
.
maecot:UnsecuredWholesaleFundingRunOff
  rdf:type maeco:QuantityKind ;
  rdfs:isDefinedBy <http://eds.topbraidlive.org/1.0/taxonomy/maeco> ;
  rdfs:isDefinedBy <http://eds.topbraidlive.org/taxonomy/maeco> ;
  rdfs:label "Unsecured Wholesale Funding Run Off" ;
  skos:broader maecot:ANY_QuantityKind ;
  skos:definition "Unsecured wholesale funding is defined as those liabilities and general obligations that are raised from non-natural persons (i.e. legal entities, including sole proprietorships and partnerships) and are not collateralised by legal rights to specifically designated assets owned by the borrowing institution in the case of bankruptcy, insolvency, liquidation or resolution. Obligations related to derivative contracts are explicitly excluded from this definition."@en ;
  skos:prefLabel "Unsecured Wholesale Funding Run-Off"@en ;
  prov:wasInfluencedBy "<http://www.bis.org/publ/bcbs238.pdf>" ;
.
maecot:VIX
  rdf:type maeco:IndexMeasure ;
  dcterms:source "http://www.futuresmag.com/2010/08/17/understanding-vix-futures-and-options"^^xsd:anyURI ;
  rdfs:isDefinedBy <http://eds.topbraidlive.org/1.0/taxonomy/maeco> ;
  rdfs:isDefinedBy <http://eds.topbraidlive.org/taxonomy/maeco> ;
  rdfs:label "VIX" ;
  skos:definition "The VIX, which is generally accepted as a broad measure of market volatility, is derived from prices of S&P 500 index options, it is not simply a weighted sum of underlying options (unlike other equity indexes like the S&P 500, where the index is a weighted sum of component prices). The options from which VIX is calculated sum up to the square of VIX, not VIX itself. This non-linear transformation means that you cannot just buy or sell a basket of options whose expiration price equals the index. Because of this non-linear component, there is no way to statically replicate the VIX." ;
  skos:prefLabel "VIX" ;
.
maecot:VIXfutures
  rdf:type maeco:IndexMeasure ;
  dcterms:source "http://www.futuresmag.com/2010/08/17/understanding-vix-futures-and-options"^^xsd:anyURI ;
  rdfs:isDefinedBy <http://eds.topbraidlive.org/1.0/taxonomy/maeco> ;
  rdfs:isDefinedBy <http://eds.topbraidlive.org/taxonomy/maeco> ;
  rdfs:label "VIX Futures" ;
  skos:broader maecot:VIX ;
  skos:prefLabel "VIX Futures" ;
.
maecot:VIXoptions
  rdf:type maeco:IndexMeasure ;
  dcterms:source "http://www.futuresmag.com/2010/08/17/understanding-vix-futures-and-options"^^xsd:anyURI ;
  rdfs:isDefinedBy <http://eds.topbraidlive.org/1.0/taxonomy/maeco> ;
  rdfs:isDefinedBy <http://eds.topbraidlive.org/taxonomy/maeco> ;
  rdfs:label "VIX Options" ;
  skos:broader maecot:VIX ;
  skos:prefLabel "VIX Options" ;
.
maecot:VaR
  rdf:type maeco:QuantityKind ;
  rdfs:isDefinedBy <http://eds.topbraidlive.org/1.0/taxonomy/maeco> ;
  rdfs:isDefinedBy <http://eds.topbraidlive.org/taxonomy/maeco> ;
  rdfs:label "Va R" ;
  skos:broader maecot:ANY_QuantityKind ;
  skos:prefLabel "Value-at-Risk"@en ;
.
maecot:ValuationPercentage
  rdf:type maeco:QuantityKind ;
  dcterms:source "http://www.isda.org/c_and_a/oper_commit-dcg-glossary.html"^^xsd:anyURI ;
  rdfs:isDefinedBy <http://eds.topbraidlive.org/1.0/taxonomy/maeco> ;
  rdfs:isDefinedBy <http://eds.topbraidlive.org/taxonomy/maeco> ;
  rdfs:label "Valuation percentage" ;
  skos:broader maecot:ANY_QuantityKind ;
  skos:definition "The percentage by which the market value of the collateral will be reduced to allow for price volatility and instrument liquidity in respect of the relevant collateral between collateral calls."@en ;
  skos:exactMatch maecot:Haircut ;
  skos:prefLabel "Valuation Percentage"@en ;
.
maecot:ValuationTime
  rdf:type maeco:QuantityKind ;
  dcterms:source "http://www.isda.org/c_and_a/oper_commit-dcg-glossary.html"^^xsd:anyURI ;
  rdfs:isDefinedBy <http://eds.topbraidlive.org/1.0/taxonomy/maeco> ;
  rdfs:isDefinedBy <http://eds.topbraidlive.org/taxonomy/maeco> ;
  rdfs:label "Valuation Time" ;
  skos:broader maecot:ANY_QuantityKind ;
  skos:definition "The time at which the collateral portfolio and collateral balance is valued for the purposes of a collateral call."@en ;
  skos:prefLabel "Valuation Time"@en ;
.
maecot:ValueAtRisk
  rdf:type maeco:QuantityKind ;
  dcterms:source "http://www.cftc.gov/LawRegulation/DoddFrankAct/index.htm"^^xsd:anyURI ;
  dcterms:source "http://www.isda.org/c_and_a/oper_commit-dcg-glossary.html"^^xsd:anyURI ;
  rdfs:isDefinedBy <http://eds.topbraidlive.org/1.0/taxonomy/maeco> ;
  rdfs:isDefinedBy <http://eds.topbraidlive.org/taxonomy/maeco> ;
  rdfs:label "Value at Risk (VaR)" ;
  skos:altLabel "VAR" ;
  skos:altLabel "VaR"@en ;
  skos:broader maecot:ANY_QuantityKind ;
  skos:definition "A statistical measure which calculates the maximum loss that any financial instrument may be expected to suffer over a defined period with a specified confidence level (e.g. a 95% confidence level on a 100 day VaR measure assumes that the maximum loss would not be exceeded on 95 days out of 100).  VaR is a valuable risk management tool as it allows risk across diverse asset classes to be pooled into a single measure of potential aggregate loss."@en ;
  skos:definition "Value-at-risk. A statistical technique used to measure and quantify the level of financial risk within a firm or investment portfolio over a specific time frame. Value at risk is used by risk managers in order to measure and control the level of risk which a firm undertakes. Value at Risk is measured according to three variables: the amount of potential loss, the probability of that loss, and the time frame."@en ;
  skos:prefLabel "Value at Risk"@en ;
  skos:prefLabel "Value-at-Risk"@en ;
.
maecot:ValueBasis
  rdf:type maeco:QuantityKind ;
  dcterms:source "http://www.isda.org/c_and_a/oper_commit-dcg-glossary.html"^^xsd:anyURI ;
  rdfs:isDefinedBy <http://eds.topbraidlive.org/1.0/taxonomy/maeco> ;
  rdfs:isDefinedBy <http://eds.topbraidlive.org/taxonomy/maeco> ;
  rdfs:label "Value Basis" ;
  skos:altLabel "Net Basis"@en ;
  skos:altLabel "Value Basis"@en ;
  skos:broader maecot:ANY_QuantityKind ;
  skos:definition "The difference between the gross basis and the carry."@en ;
  skos:prefLabel "Basis (Value or Net)"@en ;
.
maecot:VariableCost
  rdf:type maeco:Cost ;
  dcterms:source "http://www.wwnorton.com/college/econ/stec4/macroeconomics/glossary.asp"^^xsd:anyURI ;
  rdfs:isDefinedBy <http://eds.topbraidlive.org/1.0/taxonomy/maeco> ;
  rdfs:isDefinedBy <http://eds.topbraidlive.org/taxonomy/maeco> ;
  rdfs:label "Variable cost" ;
  skos:broader maecot:ANY_Cost ;
  skos:definition "<STRONG>Variable Costs</STRONG> - the costs resulting from variable inputs. The portion of a firm or industry's cost that changes with output, in contrast to <a href='http://edg.topbraid.solutions/maeco/term/FixedCost'>fixed cost</a> ." ;
  skos:prefLabel "Variable Cost" ;
.
maecot:VariationMargin
  rdf:type maeco:QuantityKind ;
  dcterms:source "http://www.cftc.gov/LawRegulation/DoddFrankAct/index.htm"^^xsd:anyURI ;
  rdfs:isDefinedBy <http://eds.topbraidlive.org/1.0/taxonomy/maeco> ;
  rdfs:isDefinedBy <http://eds.topbraidlive.org/taxonomy/maeco> ;
  rdfs:label "Variation Margin" ;
  skos:altLabel "VM"@en ;
  skos:broader maecot:ANY_QuantityKind ;
  skos:definition "Variation margin. In the new world of centrally cleared derivatives, clearing members must post margin on a daily or intraday basis in order to minimize unsecured exposures. VM, which is required to be posted over the life of a cleared swap transaction, is intended to account for variations over time in the MTM of the relevant transaction or transactions."@en ;
  skos:prefLabel "Variation margin"@en ;
.
maecot:VaultCash
  rdf:type maeco:Reserves ;
  rdfs:isDefinedBy <http://eds.topbraidlive.org/1.0/taxonomy/maeco> ;
  rdfs:isDefinedBy <http://eds.topbraidlive.org/taxonomy/maeco> ;
  rdfs:label "Vault Cash" ;
  skos:broader maecot:ANY_Reserves ;
  skos:prefLabel "Vault Cash"@us ;
.
maecot:Vega
  rdf:type maeco:QuantityKind ;
  dcterms:source "http://www.isda.org/c_and_a/oper_commit-dcg-glossary.html"^^xsd:anyURI ;
  rdfs:isDefinedBy <http://eds.topbraidlive.org/1.0/taxonomy/maeco> ;
  rdfs:isDefinedBy <http://eds.topbraidlive.org/taxonomy/maeco> ;
  rdfs:label "Vega" ;
  skos:definition "The measure of volatility in option theory."@en ;
  skos:prefLabel "Vega"@en ;
.
maecot:Volatility
  rdf:type maeco:QuantityKind ;
  dcterms:source "http://www.isda.org/c_and_a/oper_commit-dcg-glossary.html"^^xsd:anyURI ;
  rdfs:isDefinedBy <http://eds.topbraidlive.org/1.0/taxonomy/maeco> ;
  rdfs:isDefinedBy <http://eds.topbraidlive.org/taxonomy/maeco> ;
  rdfs:label "Volatility" ;
  skos:broader maecot:ANY_QuantityKind ;
  skos:definition "The extent to which an economic variable, such as a price or an exchange rate, moves up and down over time. The variability of movements in a security or underlying instrumen's price. It is a measure of the amount by which an asset's price is expected to fluctuate over a given period of time. It is normally measured by the annual standard deviation of daily price changes."@en ;
  skos:prefLabel "Volatility"@en ;
.
maecot:WaterInTheTariff
  rdf:type maeco:Tariff ;
  rdfs:isDefinedBy <http://eds.topbraidlive.org/1.0/taxonomy/maeco> ;
  rdfs:isDefinedBy <http://eds.topbraidlive.org/taxonomy/maeco> ;
  rdfs:label "Water in the tariff" ;
  skos:broader maecot:Tariff ;
  skos:definition "<STRONG>1.</STRONG> The extent to which a tariff is higher than necessary to be <a href='http://edg.topbraid.solutions/maeco/term/ProhibitiveTariff'>prohibitive</a> .  <STRONG>2.</STRONG> The extent to which an <a href='http://edg.topbraid.solutions/maeco/term/AppliedTariffRate'>applied tariff</a> is below the <a href='http://edg.topbraid.solutions/maeco/term/BoundTariff'>bound tariff</a> ." ;
  skos:prefLabel "Water In The Tariff" ;
.
maecot:WeightedAverageMaturity
  rdf:type maeco:QuantityKind ;
  dcterms:source "http://www.cftc.gov/LawRegulation/DoddFrankAct/index.htm"^^xsd:anyURI ;
  rdfs:isDefinedBy <http://eds.topbraidlive.org/1.0/taxonomy/maeco> ;
  rdfs:isDefinedBy <http://eds.topbraidlive.org/taxonomy/maeco> ;
  rdfs:label "Weighted Average Maturity" ;
  skos:altLabel "Average effective maturity" ;
  skos:altLabel "WAM" ;
  skos:broader maecot:ANY_QuantityKind ;
  skos:definition "The weighted average of the time until all maturities on mortgages in a mortgage-backed security (MBS). The higher the weighted average to maturity, the longer the mortgages in the security have until maturity. Also known as \"average effective maturity\"."@en ;
  skos:prefLabel "Weighted Average Maturity"@en ;
.
maecot:WeightedAveragePds
  rdf:type maeco:QuantityKind ;
  rdfs:isDefinedBy <http://eds.topbraidlive.org/1.0/taxonomy/maeco> ;
  rdfs:isDefinedBy <http://eds.topbraidlive.org/taxonomy/maeco> ;
  rdfs:label "Weighted Average Pds" ;
  skos:broader maecot:RiskWeightingFactor ;
  skos:prefLabel "Weighted Average Probability of Defaults"@en ;
.
maecot:WorldPrice
  rdf:type maeco:Price ;
  rdfs:isDefinedBy <http://eds.topbraidlive.org/1.0/taxonomy/maeco> ;
  rdfs:isDefinedBy <http://eds.topbraidlive.org/taxonomy/maeco> ;
  rdfs:label "World price" ;
  skos:broader maecot:Price ;
  skos:definition "The price of a good on the \" <STRONG>world market</STRONG> ,\" meaning the price outside of any country's borders and therefore exclusive of any trade taxes or subsidies that might apply crossing a border into a country but inclusive of any that might apply crossing out of a country." ;
  skos:prefLabel "World Price" ;
.
maecot:YieldSpreadPremium
  rdf:type maeco:QuantityKind ;
  dcterms:source "http://www.cftc.gov/LawRegulation/DoddFrankAct/index.htm"^^xsd:anyURI ;
  rdfs:isDefinedBy <http://eds.topbraidlive.org/1.0/taxonomy/maeco> ;
  rdfs:isDefinedBy <http://eds.topbraidlive.org/taxonomy/maeco> ;
  rdfs:label "Yield Spread Premium" ;
  skos:altLabel "YSP" ;
  skos:broader maecot:ANY_Premium ;
  skos:definition "Yield spread premium. A YSP is a payment from a lender to a mortgage originator when a residential mortgage loan is closed. The DFA prohibits certain types of YSPs."@en ;
  skos:prefLabel "Yield Spread Premium"@en ;
.
maecot:YieldToMaturity
  rdf:type maeco:QuantityKind ;
  dcterms:source "http://www.isda.org/c_and_a/oper_commit-dcg-glossary.html"^^xsd:anyURI ;
  rdfs:isDefinedBy <http://eds.topbraidlive.org/1.0/taxonomy/maeco> ;
  rdfs:isDefinedBy <http://eds.topbraidlive.org/taxonomy/maeco> ;
  rdfs:label "Yield To Maturity" ;
  skos:definition "The amount of interest on an annual compound basis, which a bond would pay if held until redemption or the maturity date. Also, the interest rate that, if used to discount all cash flows, would yield the current price."@en ;
  skos:prefLabel "Yield to Maturity"@en ;
.
<http://eds.topbraidlive.org/1.0/quantitykinds/maeco>
  rdf:type owl:Ontology ;
  swa:defaultNamespace "http://finance.topbraid.org/vocabulary/finance" ;
  <http://www.linkedmodel.org/schema/vaem#hasGraphMetadata> <http://eds.topbraidlive.org/quantitykinds/maeco/GMD_maeco> ;
  rdfs:isDefinedBy <http://eds.topbraidlive.org/1.0/taxonomy/maeco> ;
  rdfs:isDefinedBy <http://eds.topbraidlive.org/taxonomy/maeco> ;
  rdfs:label "Finance Vocabulary" ;
  owl:imports <http://edg.topbraid.solutions/1.0/schema/maeco> ;
  owl:imports <http://spinrdf.org/spl> ;
  owl:imports <http://www.w3.org/2004/02/skos/core> ;
.
<http://eds.topbraidlive.org/quantitykinds/maeco/GMD_maeco>
  rdf:type <http://www.linkedmodel.org/schema/vaem#GraphMetaData> ;
  dcterms:modified "2016-12-18"^^xsd:date ;
  dcterms:rights "<p>This ontology is issued under a restricted copyright license that prohibits reproduction, distribution, copying and any other form of sharing. The license agreement can be found at <a href='http://www.topquadrant.com/docs/legal/EULA.pdf'>http://www.topquadrant.com/docs/legal/EULA.pdf.</p>"^^rdf:HTML ;
  <http://www.linkedmodel.org/schema/vaem#hasGraphRole> <http://www.linkedmodel.org/schema/vaem#UnspecifiedGraphRole> ;
  <http://www.linkedmodel.org/schema/vaem#hasLicenseType> <voag:TopQuadrant_ONTOLOGY-LICENSE> ;
  <http://www.linkedmodel.org/schema/vaem#hasOwner> <http://www.linkedmodel.org/schema/vaem#TopQuadrant> ;
  <http://www.linkedmodel.org/schema/vaem#hasSteward> <http://www.linkedmodel.org/schema/vaem#TopQuadrant> ;
  <http://www.linkedmodel.org/schema/vaem#isMetadataFor> <http://eds.topbraidlive.org/1.0/quantitykinds/maeco> ;
  <http://www.linkedmodel.org/schema/vaem#name> "EDG" ;
  <http://www.linkedmodel.org/schema/vaem#namespace> "http://edg.topbraid.solutions/model/" ;
  <http://www.linkedmodel.org/schema/vaem#namespacePrefix> "edg" ;
  <http://www.linkedmodel.org/schema/vaem#owner> "TopQuadrant, Inc." ;
  <http://www.linkedmodel.org/schema/vaem#releaseDate> "2016-12-18"^^xsd:date ;
  <http://www.linkedmodel.org/schema/vaem#revision> "1.0" ;
  <http://www.linkedmodel.org/schema/vaem#usesNonImportedResource> dcterms:abstract ;
  <http://www.linkedmodel.org/schema/vaem#usesNonImportedResource> dcterms:author ;
  <http://www.linkedmodel.org/schema/vaem#usesNonImportedResource> dcterms:created ;
  <http://www.linkedmodel.org/schema/vaem#usesNonImportedResource> dcterms:modified ;
  <http://www.linkedmodel.org/schema/vaem#usesNonImportedResource> dcterms:rights ;
  <http://www.linkedmodel.org/schema/vaem#usesNonImportedResource> dcterms:title ;
  <http://www.linkedmodel.org/schema/vaem#usesNonImportedResource> <http://voag.linkedmodel.org/voag#TopQuadrant_ONTOLOGY-LICENSE> ;
  <http://www.linkedmodel.org/schema/vaem#withAttributionTo> "Any references to this ontology should give attribution to TopQuadrant, Inc." ;
.
dcterms:abstract
  rdf:type owl:AnnotationProperty ;
  rdfs:isDefinedBy <http://eds.topbraidlive.org/1.0/taxonomy/maeco> ;
  rdfs:isDefinedBy <http://eds.topbraidlive.org/taxonomy/maeco> ;
  rdfs:isDefinedBy dcterms: ;
  rdfs:label "abstract" ;
  rdfs:range xsd:string ;
.
dcterms:author
  rdf:type owl:AnnotationProperty ;
  rdfs:isDefinedBy <http://eds.topbraidlive.org/1.0/taxonomy/maeco> ;
  rdfs:isDefinedBy <http://eds.topbraidlive.org/taxonomy/maeco> ;
  rdfs:isDefinedBy dcterms: ;
  rdfs:label "author" ;
  rdfs:range xsd:string ;
.
dcterms:contributor
  rdf:type owl:AnnotationProperty ;
  rdfs:isDefinedBy <http://eds.topbraidlive.org/1.0/taxonomy/maeco> ;
  rdfs:isDefinedBy <http://eds.topbraidlive.org/taxonomy/maeco> ;
  rdfs:isDefinedBy dcterms: ;
  rdfs:label "contributor" ;
  rdfs:range xsd:string ;
.
dcterms:created
  rdf:type owl:AnnotationProperty ;
  rdfs:isDefinedBy <http://eds.topbraidlive.org/1.0/taxonomy/maeco> ;
  rdfs:isDefinedBy <http://eds.topbraidlive.org/taxonomy/maeco> ;
  rdfs:isDefinedBy dcterms: ;
  rdfs:label "created" ;
  rdfs:range xsd:date ;
.
dcterms:creator
  rdf:type owl:AnnotationProperty ;
  rdfs:isDefinedBy <http://eds.topbraidlive.org/1.0/taxonomy/maeco> ;
  rdfs:isDefinedBy <http://eds.topbraidlive.org/taxonomy/maeco> ;
  rdfs:isDefinedBy dcterms: ;
  rdfs:label "creator" ;
  rdfs:range xsd:string ;
.
dcterms:description
  rdf:type owl:AnnotationProperty ;
  rdfs:isDefinedBy <http://eds.topbraidlive.org/1.0/taxonomy/maeco> ;
  rdfs:isDefinedBy <http://eds.topbraidlive.org/taxonomy/maeco> ;
  rdfs:isDefinedBy dcterms: ;
  rdfs:label "description" ;
  rdfs:range xsd:string ;
.
dcterms:modified
  rdf:type owl:AnnotationProperty ;
  rdfs:isDefinedBy <http://eds.topbraidlive.org/1.0/taxonomy/maeco> ;
  rdfs:isDefinedBy <http://eds.topbraidlive.org/taxonomy/maeco> ;
  rdfs:isDefinedBy dcterms: ;
  rdfs:label "modified" ;
  rdfs:range xsd:date ;
.
dcterms:replaces
  rdf:type owl:AnnotationProperty ;
  rdfs:isDefinedBy <http://eds.topbraidlive.org/1.0/taxonomy/maeco> ;
  rdfs:isDefinedBy <http://eds.topbraidlive.org/taxonomy/maeco> ;
  rdfs:isDefinedBy dcterms: ;
  rdfs:label "replaces" ;
  rdfs:range rdfs:Resource ;
.
dcterms:rights
  rdf:type owl:AnnotationProperty ;
  rdfs:isDefinedBy <http://eds.topbraidlive.org/1.0/taxonomy/maeco> ;
  rdfs:isDefinedBy <http://eds.topbraidlive.org/taxonomy/maeco> ;
  rdfs:isDefinedBy dcterms: ;
  rdfs:label "rights" ;
  rdfs:range xsd:string ;
.
dcterms:source
  rdf:type owl:AnnotationProperty ;
  rdfs:isDefinedBy <http://eds.topbraidlive.org/1.0/taxonomy/maeco> ;
  rdfs:isDefinedBy <http://eds.topbraidlive.org/taxonomy/maeco> ;
  rdfs:isDefinedBy dcterms: ;
  rdfs:label "source" ;
  rdfs:range xsd:anyURI ;
.
dcterms:subject
  rdf:type owl:AnnotationProperty ;
  rdfs:isDefinedBy <http://eds.topbraidlive.org/1.0/taxonomy/maeco> ;
  rdfs:isDefinedBy <http://eds.topbraidlive.org/taxonomy/maeco> ;
  rdfs:isDefinedBy dcterms: ;
  rdfs:label "subject" ;
  rdfs:range xsd:string ;
.
dcterms:title
  rdf:type owl:AnnotationProperty ;
  rdfs:isDefinedBy <http://eds.topbraidlive.org/1.0/taxonomy/maeco> ;
  rdfs:isDefinedBy <http://eds.topbraidlive.org/taxonomy/maeco> ;
  rdfs:isDefinedBy dcterms: ;
  rdfs:label "title" ;
  rdfs:range xsd:string ;
.
prov:wasInfluencedBy
  rdf:type rdf:Property ;
  rdfs:isDefinedBy <http://eds.topbraidlive.org/1.0/taxonomy/maeco> ;
  rdfs:isDefinedBy <http://eds.topbraidlive.org/taxonomy/maeco> ;
  rdfs:range xsd:anyURI ;
  skos:prefLabel "was influenced by"@en ;
.
