# baseURI: http://www.nwcg.gov/vocabularies/fire-resource-kinds
# imports: http://www.nwcg.gov/ontologies/fire-resource

@prefix : <http://www.nwcg.gov/vocabularies/fire-resource-kinds#> .
@prefix dcterms: <http://purl.org/dc/terms/> .
@prefix nwcg-fire: <http://www.nwcg.gov/ontologies/fire-resource#> .
@prefix owl: <http://www.w3.org/2002/07/owl#> .
@prefix rdf: <http://www.w3.org/1999/02/22-rdf-syntax-ns#> .
@prefix rdfs: <http://www.w3.org/2000/01/rdf-schema#> .
@prefix skos: <http://www.w3.org/2004/02/skos/core#> .
@prefix xsd: <http://www.w3.org/2001/XMLSchema#> .

<http://www.nwcg.gov/vocabularies/fire-resource-kinds>
  a owl:Ontology ;
  dcterms:creator "Sofiane Fellah, Image Matters LLC" ;
  dcterms:creator "Stephane Fellah, Image Matters LLC" ;
  dcterms:description "The NWCG Fire Resource Kinds Codelist defines Aircraft, Crews, Equipment, and Overhead as a Fire Resource Kind " ;
  rdfs:label "National Wildfire Coordination Group (NWCG) Fire Resource Kinds Codelist" ;
  owl:imports <http://www.nwcg.gov/ontologies/fire-resource> ;
  owl:versionInfo "v1" ;
.
:Aircraft
  a nwcg-fire:ResourceKind ;
  rdfs:label "Aircraft" ;
  skos:definition "A machine, such as an airplane or helicopter, capable of sustained flight and used for wildland fire operations." ;
  skos:prefLabel "Aircraft" ;
  skos:topConceptOf :NWCG_FireResourceKindCS ;
.
:Crews
  a nwcg-fire:ResourceKind ;
  rdfs:label "Crews" ;
  skos:definition "An organized group of workers, such as firefighters under the leadership of a crew boss or other designated official, that are used for wildland fire operations." ;
  skos:prefLabel "Crews" ;
  skos:topConceptOf :NWCG_FireResourceKindCS ;
.
:Equipment
  a nwcg-fire:ResourceKind ;
  rdfs:label "Equipment" ;
  skos:definition "An apparatus, such as an engine or dozer, that is used for wildland fire operations." ;
  skos:prefLabel "Equipment" ;
  skos:topConceptOf :NWCG_FireResourceKindCS ;
.
:NWCG_FireResourceKindCS
  a skos:ConceptScheme ;
  rdfs:label "NWCG Fire Resource Kind Concept Scheme" ;
  skos:definition "This Concept Scheme defines the NWCG Codelist for Fire Resource KInd." ;
  skos:prefLabel "NWCG Fire Resource Kind Concept Scheme" ;
.
:Overhead
  a nwcg-fire:ResourceKind ;
  rdfs:label "Overhead" ;
  skos:definition "An organized group of workers, such as firefighters under the leadership of a crew boss or other designated official, that are used for wildland fire operations." ;
  skos:prefLabel "Overhead" ;
  skos:topConceptOf :NWCG_FireResourceKindCS ;
.
