# baseURI: http://datashapes.org/datagen
# imports: http://datashapes.org/dash
# prefix: datagen

@prefix datagen: <http://datashapes.org/datagen#> .
@prefix owl: <http://www.w3.org/2002/07/owl#> .
@prefix rdf: <http://www.w3.org/1999/02/22-rdf-syntax-ns#> .
@prefix rdfs: <http://www.w3.org/2000/01/rdf-schema#> .
@prefix xsd: <http://www.w3.org/2001/XMLSchema#> .

<http://datashapes.org/datagen>
  a owl:Ontology ;
  rdfs:comment "A vocabulary extending SHACL with properties to instruct a data generator on how to produce triples for a given set of shapes." ;
  rdfs:label "Data Generator Vocabulary for SHACL" ;
  owl:imports <http://datashapes.org/dash> ;
  owl:versionInfo "In TopBraid, see the SPARQLMotion sml:GenerateRandomData and the Composer help page \"Random Data Generator\"." ;
.
datagen:maxInstanceCount
  a rdf:Property ;
  rdfs:comment "The maximum number of instances that shall be created for the associated class." ;
  rdfs:domain rdfs:Class ;
  rdfs:label "max instance count" ;
  rdfs:range xsd:integer ;
.
datagen:maxValueCount
  a rdf:Property ;
  rdfs:comment "The maximum number of values that shall be created for an instance for the associated property. The system will use the minimum value of this or any applicable sh:maxCount constraint on the same property." ;
  rdfs:domain <http://www.w3.org/ns/shacl#PropertyShape> ;
  rdfs:label "max value count" ;
  rdfs:range xsd:integer ;
.
datagen:minInstanceCount
  a rdf:Property ;
  rdfs:comment "The minimum number of instances that shall be created for the associated class." ;
  rdfs:domain rdfs:Class ;
  rdfs:label "min instance count" ;
  rdfs:range xsd:integer ;
.
datagen:minValueCount
  a rdf:Property ;
  rdfs:comment "The minimum number of values that shall be created for an instance for the associated property. The system will use the maximum value of this or any applicable sh:minCount constraint on the same property." ;
  rdfs:domain <http://www.w3.org/ns/shacl#PropertyShape> ;
  rdfs:label "min value count" ;
  rdfs:range xsd:integer ;
.
