# baseURI: http://edg.topbraid.solutions/1.0/datatypes/jdbc
# imports: http://edg.topbraid.solutions/1.0/codelist/datatypes
# imports: http://edg.topbraid.solutions/1.0/schema/core
# imports: http://edg.topbraid.solutions/1.0/schema/datatypes
# imports: http://qudt.org/2.0/refdata/scalar-datatypes
# imports: http://qudt.org/2.0/schema/scalar-datatypes

@prefix dcterms: <http://purl.org/dc/terms/> .
@prefix edg: <http://edg.topbraid.solutions/model/> .
@prefix org: <http://www.w3.org/ns/org#> .
@prefix owl: <http://www.w3.org/2002/07/owl#> .
@prefix rdf: <http://www.w3.org/1999/02/22-rdf-syntax-ns#> .
@prefix rdfs: <http://www.w3.org/2000/01/rdf-schema#> .
@prefix sp: <http://spinrdf.org/sp#> .
@prefix spin: <http://spinrdf.org/spin#> .
@prefix spl: <http://spinrdf.org/spl#> .
@prefix vaem: <http://www.linkedmodel.org/schema/vaem#> .
@prefix xsd: <http://www.w3.org/2001/XMLSchema#> .

<http://edg.topbraid.solutions/1.0/datatypes/jdbc>
  a owl:Ontology ;
  vaem:hasGraphMetadata <http://edg.topbraid.solutions/datatypes/jdbc/GMD_jdbc> ;
  rdfs:label "JDBC Datatypes" ;
  owl:imports <http://edg.topbraid.solutions/1.0/codelist/datatypes> ;
  owl:imports <http://edg.topbraid.solutions/1.0/schema/core> ;
  owl:imports <http://edg.topbraid.solutions/1.0/schema/datatypes> ;
  owl:imports <http://qudt.org/2.0/refdata/scalar-datatypes> ;
  owl:imports <http://qudt.org/2.0/schema/scalar-datatypes> ;
  owl:versionInfo "Created with TopBraid Composer" ;
.
<http://edg.topbraid.solutions/datatypes/jdbc/GMD_jdbc>
  a vaem:GraphMetaData ;
  dcterms:modified "2016-12-18"^^xsd:date ;
  dcterms:rights "<p>This ontology is issued under a restricted copyright license that prohibits reproduction, distribution, copying and any other form of sharing. The license agreement can be found at <a href='http://www.topquadrant.com/docs/legal/EULA.pdf'>http://www.topquadrant.com/docs/legal/EULA.pdf.</p>"^^rdf:HTML ;
  vaem:hasGraphRole vaem:DatatypesGraph ;
  vaem:hasLicenseType <voag:TopQuadrant_ONTOLOGY-LICENSE> ;
  vaem:hasOwner vaem:TopQuadrant ;
  vaem:hasSteward vaem:TopQuadrant ;
  vaem:isMetadataFor <http://edg.topbraid.solutions/1.0/datatypes/jdbc> ;
  vaem:name "EDG" ;
  vaem:namespace "http://edg.topbraid.solutions/model/" ;
  vaem:namespacePrefix "edg" ;
  vaem:owner "TopQuadrant, Inc." ;
  vaem:releaseDate "2016-12-18"^^xsd:date ;
  vaem:revision "1.0" ;
  vaem:usesNonImportedResource dcterms:abstract ;
  vaem:usesNonImportedResource dcterms:author ;
  vaem:usesNonImportedResource dcterms:created ;
  vaem:usesNonImportedResource dcterms:modified ;
  vaem:usesNonImportedResource dcterms:rights ;
  vaem:usesNonImportedResource dcterms:title ;
  vaem:usesNonImportedResource <http://voag.linkedmodel.org/voag#TopQuadrant_ONTOLOGY-LICENSE> ;
  vaem:withAttributionTo "Any references to this ontology should give attribution to TopQuadrant, Inc." ;
.
edg:JDBC_ARRAY
  a edg:JDBCdatatype ;
  edg:belongsTo edg:DTFT_JDBC ;
  edg:name "ARRAY" ;
  edg:referenceLink "https://www.ibm.com/support/knowledgecenter/en/SS62YD_3.1.1/com.ibm.datatools.dsws.tooling.ui.doc/topics/rdswssupdattyp.html"^^xsd:anyURI ;
  rdfs:comment "A set-length and ordered collection of elements. Identifies the generic SQL type ARRAY." ;
  rdfs:isDefinedBy <http://edg.topbraid.solutions/1.0/datatypes/jdbc> ;
  rdfs:label "ARRAY (JDBC)" ;
.
edg:JDBC_BIGINT
  a edg:JDBCintegerDatatype ;
  edg:belongsTo edg:DTFT_JDBC ;
  edg:name "BIGINT" ;
  edg:normativeDatatype <http://qudt.org/schema/qudt/SIGNED-BIG-INTEGER> ;
  edg:realizes <http://qudt.org/schema/qudt/SIGNED-BIG-INTEGER> ;
  edg:referenceLink "https://www.ibm.com/support/knowledgecenter/en/SS62YD_3.1.1/com.ibm.datatools.dsws.tooling.ui.doc/topics/rdswssupdattyp.html"^^xsd:anyURI ;
  edg:xsdDataType xsd:integer ;
  rdfs:comment "Integer numerical (no decimal). Precision 19. Identifies the generic SQL type BIGINT." ;
  rdfs:isDefinedBy <http://edg.topbraid.solutions/1.0/datatypes/jdbc> ;
  rdfs:label "BIGINT (JDBC)" ;
.
edg:JDBC_BINARY
  a edg:JDBCstringDatatype ;
  edg:belongsTo edg:DTFT_JDBC ;
  edg:name "BINARY(n)" ;
  edg:normativeDatatype <http://qudt.org/schema/qudt/UTF8-STRING> ;
  edg:referenceLink "https://www.ibm.com/support/knowledgecenter/en/SS62YD_3.1.1/com.ibm.datatools.dsws.tooling.ui.doc/topics/rdswssupdattyp.html"^^xsd:anyURI ;
  edg:xsdDataType xsd:hexBinary ;
  rdfs:comment "Binary string. Fixed-length n. Identifies the generic SQL type BINARY." ;
  rdfs:isDefinedBy <http://edg.topbraid.solutions/1.0/datatypes/jdbc> ;
  rdfs:label "BINARY(n) (JDBC)" ;
.
edg:JDBC_BIT
  a edg:JDBCdatatype ;
  edg:belongsTo edg:DTFT_JDBC ;
  edg:name "BIT" ;
  edg:xsdDataType xsd:boolean ;
  rdfs:comment "Identifies the generic SQL type BIT." ;
  rdfs:isDefinedBy <http://edg.topbraid.solutions/1.0/datatypes/jdbc> ;
  rdfs:label "BIT (JDBC)" ;
.
edg:JDBC_BLOB
  a edg:JDBCdatatype ;
  edg:name "BLOB" ;
  rdfs:comment "Identifies the generic SQL type BLOB." ;
  rdfs:isDefinedBy <http://edg.topbraid.solutions/1.0/datatypes/jdbc> ;
  rdfs:label "BLOB (JDBC)" ;
.
edg:JDBC_BOOLEAN
  a edg:JDBCdatatype ;
  edg:belongsTo edg:DTFT_JDBC ;
  edg:name "BOOLEAN" ;
  edg:normativeDatatype <http://qudt.org/schema/qudt/BOOLEAN> ;
  edg:referenceLink "https://www.ibm.com/support/knowledgecenter/en/SS62YD_3.1.1/com.ibm.datatools.dsws.tooling.ui.doc/topics/rdswssupdattyp.html"^^xsd:anyURI ;
  edg:xsdDataType xsd:boolean ;
  rdfs:comment "Stores TRUE or FALSE values. Identifies the generic SQL type BOOLEAN." ;
  rdfs:isDefinedBy <http://edg.topbraid.solutions/1.0/datatypes/jdbc> ;
  rdfs:label "BOOLEAN (JDBC)" ;
.
edg:JDBC_CHAR
  a edg:JDBCdatatype ;
  edg:name "CHAR" ;
  rdfs:comment "Identifies the generic SQL type CHAR." ;
  rdfs:isDefinedBy <http://edg.topbraid.solutions/1.0/datatypes/jdbc> ;
  rdfs:label "CHAR (JDBC)" ;
.
edg:JDBC_CHARACTER
  a edg:JDBCstringDatatype ;
  edg:belongsTo edg:DTFT_JDBC ;
  edg:name "CHARACTER(n)" ;
  edg:normativeDatatype <http://qudt.org/schema/qudt/STRING> ;
  edg:referenceLink "https://www.ibm.com/support/knowledgecenter/en/SS62YD_3.1.1/com.ibm.datatools.dsws.tooling.ui.doc/topics/rdswssupdattyp.html"^^xsd:anyURI ;
  edg:xsdDataType xsd:string ;
  rdfs:comment "Character string. Fixed-length n" ;
  rdfs:isDefinedBy <http://edg.topbraid.solutions/1.0/datatypes/jdbc> ;
  rdfs:label "CHARACTER(n) (JDBC)" ;
.
edg:JDBC_CLOB
  a edg:JDBCdatatype ;
  edg:name "COB" ;
  rdfs:comment "Identifies the generic SQL type CLOB." ;
  rdfs:isDefinedBy <http://edg.topbraid.solutions/1.0/datatypes/jdbc> ;
  rdfs:label "CLOB (JDBC)" ;
.
edg:JDBC_DATALINK
  a edg:JDBCdatatype ;
  edg:belongsTo edg:DTFT_JDBC ;
  edg:name "DATALINK" ;
  rdfs:comment "Identifies the generic SQL type DATALINK." ;
  rdfs:isDefinedBy <http://edg.topbraid.solutions/1.0/datatypes/jdbc> ;
  rdfs:label "DATALINK (JDBC)" ;
.
edg:JDBC_DATE
  a edg:JDBCdateDatatype ;
  edg:belongsTo edg:DTFT_JDBC ;
  edg:name "DATE" ;
  edg:normativeDatatype <http://qudt.org/schema/qudt/DATE> ;
  edg:realizes <http://qudt.org/schema/qudt/DATE> ;
  edg:referenceLink "https://www.ibm.com/support/knowledgecenter/en/SS62YD_3.1.1/com.ibm.datatools.dsws.tooling.ui.doc/topics/rdswssupdattyp.html"^^xsd:anyURI ;
  edg:xsdDataType xsd:date ;
  rdfs:comment "Stores year, month, and day values. Identifies the generic SQL type DATE." ;
  rdfs:isDefinedBy <http://edg.topbraid.solutions/1.0/datatypes/jdbc> ;
  rdfs:label "DATE (JDBC)" ;
.
edg:JDBC_DECIMAL
  a edg:JDBCnumericDatatype ;
  edg:belongsTo edg:DTFT_JDBC ;
  edg:name "DECIMAL" ;
  edg:normativeDatatype <http://qudt.org/schema/qudt/DECIMAL> ;
  edg:realizes <http://qudt.org/schema/qudt/DECIMAL> ;
  edg:referenceLink "https://www.ibm.com/support/knowledgecenter/en/SS62YD_3.1.1/com.ibm.datatools.dsws.tooling.ui.doc/topics/rdswssupdattyp.html"^^xsd:anyURI ;
  edg:xsdDataType xsd:decimal ;
  rdfs:comment "Exact numerical, precision p, scale s, specified as DECIMAL(p,s). Example: decimal(5,2) is a number that has 3 digits before the decimal and 2 digits after the decimal. Identifies the generic SQL type DECIMAL." ;
  rdfs:isDefinedBy <http://edg.topbraid.solutions/1.0/datatypes/jdbc> ;
  rdfs:label "DECIMAL (JDBC)" ;
  rdfs:seeAlso edg:JDBC_NUMERIC ;
.
edg:JDBC_DISTINCT
  a edg:JDBCdatatype ;
  edg:belongsTo edg:DTFT_JDBC ;
  edg:name "DISTINCT" ;
  rdfs:comment "Identifies the generic SQL type DISTINCT." ;
  rdfs:isDefinedBy <http://edg.topbraid.solutions/1.0/datatypes/jdbc> ;
  rdfs:label "DISTINCT (JDBC)" ;
.
edg:JDBC_DOUBLE
  a edg:JDBCrealDatatype ;
  edg:belongsTo edg:DTFT_JDBC ;
  edg:name "DOUBLE" ;
  edg:realizes <http://qudt.org/schema/qudt/FLOAT-DP> ;
  rdfs:comment "Identifies the generic SQL type DOUBLE." ;
  rdfs:isDefinedBy <http://edg.topbraid.solutions/1.0/datatypes/jdbc> ;
  rdfs:label "DOUBLE (JDBC)" ;
.
edg:JDBC_DOUBLE-PRECISION
  a edg:JDBCrealDatatype ;
  edg:belongsTo edg:DTFT_JDBC ;
  edg:name "DOUBLE PRECISION" ;
  edg:normativeDatatype <http://qudt.org/schema/qudt/FLOAT-DP> ;
  edg:referenceLink "https://www.ibm.com/support/knowledgecenter/en/SS62YD_3.1.1/com.ibm.datatools.dsws.tooling.ui.doc/topics/rdswssupdattyp.html"^^xsd:anyURI ;
  edg:xsdDataType xsd:double ;
  rdfs:comment "Approximate numerical, mantissa precision 16" ;
  rdfs:isDefinedBy <http://edg.topbraid.solutions/1.0/datatypes/jdbc> ;
  rdfs:label "DOUBLE PRECISION" ;
.
edg:JDBC_FLOAT
  a edg:JDBCrealDatatype ;
  edg:belongsTo edg:DTFT_JDBC ;
  edg:name "FLOAT" ;
  edg:normativeDatatype <http://qudt.org/schema/qudt/FLOAT-SP> ;
  edg:realizes <http://qudt.org/schema/qudt/FLOAT-DP> ;
  edg:referenceLink "https://www.ibm.com/support/knowledgecenter/en/SS62YD_3.1.1/com.ibm.datatools.dsws.tooling.ui.doc/topics/rdswssupdattyp.html"^^xsd:anyURI ;
  edg:xsdDataType xsd:float ;
  rdfs:comment "Approximate numerical. A floating number in base 10 exponential notation. The size argument for this type consists of a single number specifying the minimum precision Identifies the generic SQL type FLOAT." ;
  rdfs:isDefinedBy <http://edg.topbraid.solutions/1.0/datatypes/jdbc> ;
  rdfs:label "FLOAT (JDBC)" ;
.
edg:JDBC_INTEGER
  a edg:JDBCintegerDatatype ;
  edg:belongsTo edg:DTFT_JDBC ;
  edg:name "INTEGER" ;
  edg:normativeDatatype <http://qudt.org/schema/qudt/SIGNED-LONG-INTEGER> ;
  edg:realizes <http://qudt.org/schema/qudt/SIGNED-LONG-INTEGER> ;
  edg:referenceLink "https://www.ibm.com/support/knowledgecenter/en/SS62YD_3.1.1/com.ibm.datatools.dsws.tooling.ui.doc/topics/rdswssupdattyp.html"^^xsd:anyURI ;
  edg:xsdDataType xsd:integer ;
  rdfs:comment "Integer numerical (no decimal). Precision 10 or given precision. Identifies the generic SQL type INTEGER." ;
  rdfs:isDefinedBy <http://edg.topbraid.solutions/1.0/datatypes/jdbc> ;
  rdfs:label "INTEGER (JDBC)" ;
.
edg:JDBC_INTERVAL
  a edg:JDBCstructuredDatatype ;
  edg:belongsTo edg:DTFT_JDBC ;
  edg:name "INTERVAL" ;
  edg:referenceLink "https://www.ibm.com/support/knowledgecenter/en/SS62YD_3.1.1/com.ibm.datatools.dsws.tooling.ui.doc/topics/rdswssupdattyp.html"^^xsd:anyURI ;
  rdfs:comment "Composed of a number of integer fields, representing a period of time, depending on the type of interval" ;
  rdfs:isDefinedBy <http://edg.topbraid.solutions/1.0/datatypes/jdbc> ;
  rdfs:label "INTERVAL (JDBC)" ;
.
edg:JDBC_JAVA_OBJECT
  a edg:JDBCstructuredDatatype ;
  edg:belongsTo edg:DTFT_JDBC ;
  edg:name "JAVA OBJECT" ;
  rdfs:comment "Indicates that the SQL type is database-specific and gets mapped to a Java object that can be accessed via the methods getObject and setObject." ;
  rdfs:isDefinedBy <http://edg.topbraid.solutions/1.0/datatypes/jdbc> ;
  rdfs:label "JAVA OBJECT (JDBC)" ;
.
edg:JDBC_LONGNVARCHAR
  a edg:JDBCstringDatatype ;
  edg:belongsTo edg:DTFT_JDBC ;
  edg:name "LONGNVARCHAR" ;
  rdfs:comment "Identifies the generic SQL type LONGNVARCHAR." ;
  rdfs:isDefinedBy <http://edg.topbraid.solutions/1.0/datatypes/jdbc> ;
  rdfs:label "LONGNVARCHAR (JDBC)" ;
.
edg:JDBC_LONGVARBINARY
  a edg:JDBCstringDatatype ;
  edg:belongsTo edg:DTFT_JDBC ;
  edg:name "LONGVARBINARY" ;
  rdfs:comment "Identifies the generic SQL type LONGVARBINARY." ;
  rdfs:isDefinedBy <http://edg.topbraid.solutions/1.0/datatypes/jdbc> ;
  rdfs:label "LONGVARBINARY (JDBC)" ;
.
edg:JDBC_LONGVARCHAR
  a edg:JDBCstringDatatype ;
  edg:belongsTo edg:DTFT_JDBC ;
  edg:name "LONGVARCHAR" ;
  rdfs:comment "Identifies the generic SQL type LONGVARCHAR." ;
  rdfs:isDefinedBy <http://edg.topbraid.solutions/1.0/datatypes/jdbc> ;
  rdfs:label "LONGVARCHAR (JDBC)" ;
.
edg:JDBC_MULTISET
  a edg:JDBCstructuredDatatype ;
  edg:belongsTo edg:DTFT_JDBC ;
  edg:name "MULTISET" ;
  edg:referenceLink "https://www.ibm.com/support/knowledgecenter/en/SS62YD_3.1.1/com.ibm.datatools.dsws.tooling.ui.doc/topics/rdswssupdattyp.html"^^xsd:anyURI ;
  rdfs:comment "A variable-length and unordered collection of elements" ;
  rdfs:isDefinedBy <http://edg.topbraid.solutions/1.0/datatypes/jdbc> ;
  rdfs:label "MULTISET (JDBC)" ;
.
edg:JDBC_NCHAR
  a edg:JDBCstringDatatype ;
  edg:belongsTo edg:DTFT_JDBC ;
  edg:name "NCHAR" ;
  rdfs:comment "Identifies the generic SQL type NCHAR." ;
  rdfs:isDefinedBy <http://edg.topbraid.solutions/1.0/datatypes/jdbc> ;
  rdfs:label "NCHAR (JDBC)" ;
.
edg:JDBC_NCLOB
  a edg:JDBCstructuredDatatype ;
  edg:belongsTo edg:DTFT_JDBC ;
  edg:name "NCLOB" ;
  rdfs:comment "Identifies the generic SQL type NCLOB." ;
  rdfs:isDefinedBy <http://edg.topbraid.solutions/1.0/datatypes/jdbc> ;
  rdfs:label "NCLOB (JDBC)" ;
.
edg:JDBC_NULL
  a edg:JDBCdatatype ;
  edg:belongsTo edg:DTFT_JDBC ;
  edg:name "NULL" ;
  rdfs:comment "Identifies the generic SQL value NULL." ;
  rdfs:isDefinedBy <http://edg.topbraid.solutions/1.0/datatypes/jdbc> ;
  rdfs:label "NULL (JDBC)" ;
.
edg:JDBC_NUMERIC
  a edg:JDBCnumericDatatype ;
  edg:belongsTo edg:DTFT_JDBC ;
  edg:name "NUMERIC" ;
  edg:realizes <http://qudt.org/schema/qudt/NUMERIC> ;
  edg:referenceLink "https://www.ibm.com/support/knowledgecenter/en/SS62YD_3.1.1/com.ibm.datatools.dsws.tooling.ui.doc/topics/rdswssupdattyp.html"^^xsd:anyURI ;
  edg:xsdDataType xsd:decimal ;
  rdfs:comment "Exact numerical, precision p, scale s. This is specifed as NUMERIC(p,s) as is  DECIMAL. Identifies the generic SQL type NUMERIC." ;
  rdfs:isDefinedBy <http://edg.topbraid.solutions/1.0/datatypes/jdbc> ;
  rdfs:label "NUMERIC (JDBC)" ;
  rdfs:seeAlso edg:JDBC_DECIMAL ;
.
edg:JDBC_NVARCHAR
  a edg:JDBCstringDatatype ;
  edg:belongsTo edg:DTFT_JDBC ;
  edg:name "NVARCHAR" ;
  rdfs:comment "Identifies the generic SQL type NVARCHAR." ;
  rdfs:isDefinedBy <http://edg.topbraid.solutions/1.0/datatypes/jdbc> ;
  rdfs:label "NVARCHAR (JDBC)" ;
.
edg:JDBC_OTHER
  a edg:JDBCdatatype ;
  edg:belongsTo edg:DTFT_JDBC ;
  edg:name "OTHER" ;
  rdfs:comment "Indicates that the SQL type is database-specific and gets mapped to a Java object that can be accessed via the methods getObject and setObject." ;
  rdfs:isDefinedBy <http://edg.topbraid.solutions/1.0/datatypes/jdbc> ;
  rdfs:label "OTHER (JDBC)" ;
.
edg:JDBC_REAL
  a edg:JDBCrealDatatype ;
  edg:belongsTo edg:DTFT_JDBC ;
  edg:name "REAL" ;
  edg:realizes <http://qudt.org/schema/qudt/FLOAT-SP> ;
  edg:referenceLink "https://www.ibm.com/support/knowledgecenter/en/SS62YD_3.1.1/com.ibm.datatools.dsws.tooling.ui.doc/topics/rdswssupdattyp.html"^^xsd:anyURI ;
  edg:xsdDataType xsd:float ;
  rdfs:comment "Approximate numerical, mantissa precision 7. Identifies the generic SQL type REAL." ;
  rdfs:isDefinedBy <http://edg.topbraid.solutions/1.0/datatypes/jdbc> ;
  rdfs:label "REAL (JDBC)" ;
.
edg:JDBC_REF
  a edg:JDBCdatatype ;
  edg:belongsTo edg:DTFT_JDBC ;
  edg:name "REF" ;
  rdfs:comment "Identifies the generic SQL type REF." ;
  rdfs:isDefinedBy <http://edg.topbraid.solutions/1.0/datatypes/jdbc> ;
  rdfs:label "REF (JDBC)" ;
.
edg:JDBC_REF_CURSOR
  a edg:JDBCdatatype ;
  edg:belongsTo edg:DTFT_JDBC ;
  edg:name "REF CURSOR" ;
  rdfs:comment "Identifies the generic SQL type REF_CURSOR." ;
  rdfs:isDefinedBy <http://edg.topbraid.solutions/1.0/datatypes/jdbc> ;
  rdfs:label "REF CURSOR (JDBC)" ;
.
edg:JDBC_ROWID
  a edg:JDBCdatatype ;
  edg:belongsTo edg:DTFT_JDBC ;
  edg:name "ROWID" ;
  rdfs:comment "Identifies the SQL type ROWID." ;
  rdfs:isDefinedBy <http://edg.topbraid.solutions/1.0/datatypes/jdbc> ;
  rdfs:label "ROWID (JDBC)" ;
.
edg:JDBC_SMALLINT
  a edg:JDBCintegerDatatype ;
  edg:belongsTo edg:DTFT_JDBC ;
  edg:name "SMALLINT" ;
  edg:normativeDatatype <http://qudt.org/schema/qudt/SIGNED-INTEGER> ;
  edg:realizes <http://qudt.org/schema/qudt/SIGNED-INTEGER> ;
  edg:referenceLink "https://www.ibm.com/support/knowledgecenter/en/SS62YD_3.1.1/com.ibm.datatools.dsws.tooling.ui.doc/topics/rdswssupdattyp.html"^^xsd:anyURI ;
  edg:xsdDataType xsd:integer ;
  rdfs:comment "Integer numerical (no decimal). Precision 5. Identifies the generic SQL type SMALLINT." ;
  rdfs:isDefinedBy <http://edg.topbraid.solutions/1.0/datatypes/jdbc> ;
  rdfs:label "SMALLINT (JDBC)" ;
.
edg:JDBC_SQLXML
  a edg:JDBCstructuredDatatype ;
  edg:belongsTo edg:DTFT_JDBC ;
  edg:name "SQLXML" ;
  rdfs:comment "Identifies the generic SQL type SQLXML." ;
  rdfs:isDefinedBy <http://edg.topbraid.solutions/1.0/datatypes/jdbc> ;
  rdfs:label "SQLXML (JDBC)" ;
.
edg:JDBC_STRUCT
  a edg:JDBCstructuredDatatype ;
  edg:belongsTo edg:DTFT_JDBC ;
  edg:name "STRUCT" ;
  rdfs:comment "Identifies the generic SQL type STRUCT." ;
  rdfs:isDefinedBy <http://edg.topbraid.solutions/1.0/datatypes/jdbc> ;
  rdfs:label "STRUCT (JDBC)" ;
.
edg:JDBC_TIME
  a edg:JDBCtimeDatatype ;
  edg:belongsTo edg:DTFT_JDBC ;
  edg:name "TIME" ;
  edg:normativeDatatype <http://qudt.org/schema/qudt/TIME> ;
  edg:realizes <http://qudt.org/schema/qudt/TIME> ;
  edg:referenceLink "https://www.ibm.com/support/knowledgecenter/en/SS62YD_3.1.1/com.ibm.datatools.dsws.tooling.ui.doc/topics/rdswssupdattyp.html"^^xsd:anyURI ;
  edg:xsdDataType xsd:time ;
  rdfs:comment "Stores hour, minute, and second values. Identifies the generic SQL type TIME." ;
  rdfs:isDefinedBy <http://edg.topbraid.solutions/1.0/datatypes/jdbc> ;
  rdfs:label "TIME (JDBC)" ;
.
edg:JDBC_TIMESTAMP
  a edg:JDBCtimeDatatype ;
  edg:belongsTo edg:DTFT_JDBC ;
  edg:name "TIMESTAMP" ;
  edg:normativeDatatype <http://qudt.org/schema/qudt/UTC-DATETIME> ;
  edg:realizes <http://qudt.org/schema/qudt/UTC-DATETIME> ;
  edg:referenceLink "https://www.ibm.com/support/knowledgecenter/en/SS62YD_3.1.1/com.ibm.datatools.dsws.tooling.ui.doc/topics/rdswssupdattyp.html"^^xsd:anyURI ;
  edg:xsdDataType xsd:dateTime ;
  rdfs:comment "Stores year, month, day, hour, minute, and second values. Identifies the generic SQL type TIMESTAMP." ;
  rdfs:isDefinedBy <http://edg.topbraid.solutions/1.0/datatypes/jdbc> ;
  rdfs:label "TIMESTAMP (JDBC)" ;
.
edg:JDBC_TIMESTAMP_WITH_TIMEZONE
  a edg:JDBCtimeDatatype ;
  edg:belongsTo edg:DTFT_JDBC ;
  edg:name "TIMESTAMP WITH TIMEZONE" ;
  edg:realizes <http://qudt.org/schema/qudt/DATETIME> ;
  rdfs:comment "Identifies the generic SQL type TIMESTAMP_WITH_TIMEZONE." ;
  rdfs:isDefinedBy <http://edg.topbraid.solutions/1.0/datatypes/jdbc> ;
  rdfs:label "TIMESTAMP WITH TIMEZONE (JDBC)" ;
.
edg:JDBC_TIME_WITH_TIMEZONE
  a edg:JDBCtimeDatatype ;
  edg:belongsTo edg:DTFT_JDBC ;
  edg:name "TIME WITH TIMEZONE " ;
  edg:realizes <http://qudt.org/schema/qudt/TIME> ;
  rdfs:comment "Identifies the generic SQL type TIME_WITH_TIMEZONE." ;
  rdfs:isDefinedBy <http://edg.topbraid.solutions/1.0/datatypes/jdbc> ;
  rdfs:label "TIME WITH TIMEZONE (JDBC)" ;
.
edg:JDBC_TINYINT
  a edg:JDBCintegerDatatype ;
  edg:belongsTo edg:DTFT_JDBC ;
  edg:name "TINYINT" ;
  edg:realizes <http://qudt.org/schema/qudt/SIGNED-SHORT-INTEGER> ;
  rdfs:comment "Identifies the generic SQL type TINYINT." ;
  rdfs:isDefinedBy <http://edg.topbraid.solutions/1.0/datatypes/jdbc> ;
  rdfs:label "TINYINT (JDBC)" ;
.
edg:JDBC_VARBINARY
  a edg:JDBCstringDatatype ;
  edg:belongsTo edg:DTFT_JDBC ;
  edg:name "VARBINARY" ;
  edg:referenceLink "https://www.ibm.com/support/knowledgecenter/en/SS62YD_3.1.1/com.ibm.datatools.dsws.tooling.ui.doc/topics/rdswssupdattyp.html"^^xsd:anyURI ;
  edg:xsdDataType xsd:base64Binary ;
  rdfs:comment "Binary string. Variable length. Maximum length n, specified as VARBINARY(n). Identifies the generic SQL type VARBINARY." ;
  rdfs:isDefinedBy <http://edg.topbraid.solutions/1.0/datatypes/jdbc> ;
  rdfs:label "VARBINARY (JDBC)" ;
.
edg:JDBC_VARCHAR
  a edg:JDBCstringDatatype ;
  edg:belongsTo edg:DTFT_JDBC ;
  edg:name "VARCHAR" ;
  edg:normativeDatatype <http://qudt.org/schema/qudt/STRING> ;
  edg:referenceLink "https://www.ibm.com/support/knowledgecenter/en/SS62YD_3.1.1/com.ibm.datatools.dsws.tooling.ui.doc/topics/rdswssupdattyp.html"^^xsd:anyURI ;
  edg:xsdDataType xsd:string ;
  rdfs:comment "Character string. Variable length. Maximum length n, specified as VARCHAR(n). Identifies the generic SQL type VARCHAR." ;
  rdfs:isDefinedBy <http://edg.topbraid.solutions/1.0/datatypes/jdbc> ;
  rdfs:label "VARCHAR(n) (JDBC)" ;
.
edg:JDBC_XML
  a edg:JDBCstructuredDatatype ;
  edg:belongsTo edg:DTFT_JDBC ;
  edg:name "XML" ;
  edg:referenceLink "https://www.ibm.com/support/knowledgecenter/en/SS62YD_3.1.1/com.ibm.datatools.dsws.tooling.ui.doc/topics/rdswssupdattyp.html"^^xsd:anyURI ;
  rdfs:comment "Stores XML data" ;
  rdfs:isDefinedBy <http://edg.topbraid.solutions/1.0/datatypes/jdbc> ;
  rdfs:label "XML (JDBC)" ;
.
edg:JDBCdatatype
  a owl:Class ;
  rdfs:subClassOf edg:PhysicalDatatype ;
.
edg:JDBCdateDatatype
  a edg:AssetClass ;
  rdfs:isDefinedBy <http://edg.topbraid.solutions/1.0/datatypes/jdbc> ;
  rdfs:label "JDBC Date Datatype" ;
  rdfs:subClassOf edg:JDBCdatatype ;
.
edg:JDBCintegerDatatype
  a edg:AssetClass ;
  rdfs:isDefinedBy <http://edg.topbraid.solutions/1.0/datatypes/jdbc> ;
  rdfs:label "JDBC Integer Datatype" ;
  rdfs:subClassOf edg:JDBCnumericDatatype ;
.
edg:JDBCnumericDatatype
  a edg:AssetClass ;
  rdfs:isDefinedBy <http://edg.topbraid.solutions/1.0/datatypes/jdbc> ;
  rdfs:label "JDBC Numeric Datatype" ;
  rdfs:subClassOf edg:JDBCdatatype ;
.
edg:JDBCrealDatatype
  a edg:AssetClass ;
  rdfs:isDefinedBy <http://edg.topbraid.solutions/1.0/datatypes/jdbc> ;
  rdfs:label "JDBC Real Datatype" ;
  rdfs:subClassOf edg:JDBCnumericDatatype ;
.
edg:JDBCstringDatatype
  a edg:AssetClass ;
  rdfs:isDefinedBy <http://edg.topbraid.solutions/1.0/datatypes/jdbc> ;
  rdfs:label "JDBC String Datatype" ;
  rdfs:subClassOf edg:JDBCdatatype ;
.
edg:JDBCstructuredDatatype
  a edg:AssetClass ;
  rdfs:isDefinedBy <http://edg.topbraid.solutions/1.0/datatypes/jdbc> ;
  rdfs:label "JDBC Structured Datatype" ;
  rdfs:subClassOf edg:JDBCdatatype ;
.
edg:JDBCtimeDatatype
  a edg:AssetClass ;
  rdfs:isDefinedBy <http://edg.topbraid.solutions/1.0/datatypes/jdbc> ;
  rdfs:label "JDBC Time Datatype" ;
  rdfs:subClassOf edg:JDBCdatatype ;
.
dcterms:description
  a rdf:Property ;
  a owl:AnnotationProperty ;
  rdfs:isDefinedBy dcterms: ;
  rdfs:label "description" ;
  rdfs:range xsd:string ;
.
dcterms:source
  a owl:AnnotationProperty ;
  rdfs:isDefinedBy dcterms: ;
  rdfs:label "source" ;
  rdfs:range xsd:anyURI ;
.
